<?xml version="1.0" encoding="UTF-8"?>
<rdf:RDF xmlns:rdf="http://www.w3.org/1999/02/22-rdf-syntax-ns#" xmlns:xlink="http://www.w3.org/1999/xlink" xmlns:skos="http://www.w3.org/2004/02/skos/core#" xmlns:dc="http://purl.org/dc/elements/1.1/" xmlns:dcterms="http://purl.org/dc/terms/" xmlns:rdfs="http://www.w3.org/2000/01/rdf-schema#" xmlns:owl="http://www.w3.org/2002/07/owl#">
   <skos:ConceptScheme rdf:about="http://resource.geosciml.org/classifierscheme/cgi/2016.01/earth-resource-shape">
      <dcterms:title xml:lang="en">Earth Resource Shape</dcterms:title>
      <dcterms:description xml:lang="en">This file contains the CGI Earth Resource Shape vocabulary, as defined by the IUGS Commission for Geoscience Information (CGI) Geoscience Terminology Working Group. The vocabulary defines concepts specifying the typical geometrical shape of an Earth Resource (e.g. lenticular, pipelike, irregular etc). By extension, this vocabulary includes all concepts in this conceptScheme, as well as concepts in any previous versions of the scheme.</dcterms:description>
      <skos:editorialNote xml:lang="en">This file contains the 2016 SKOS-RDF version of the CGI Earth Resource Shape vocabulary. Vocabulary Shepherd: Tim McCormick/Rachel Heaven. Compilation and review in Google doc spreadsheet, adopted 2014-01-09, converted to MS Excel for SKOS generation using SKOS_for_GA_from_XLS_2016.03.xslt</skos:editorialNote>
      <skos:changeNote xml:lang="en">2014-02-23 Conversion to SKOS by SM Richard.</skos:changeNote>
      <skos:changeNote xml:lang="en">2016-11-28 OLR regenerate SKOS-RDF file as part of migration to new vocabulary server. No change to previous concepts definitions.</skos:changeNote>
      <dcterms:date>2016-11-28</dcterms:date>
      <dcterms:creator>CGI Geoscience Terminology Working Group</dcterms:creator>
   </skos:ConceptScheme>
   <skos:ConceptScheme rdf:about="http://resource.geosciml.org/classifierscheme/cgi/2016.01/earth-resource-shape">
      <skos:hasTopConcept rdf:resource="http://resource.geosciml.org/classifier/cgi/earth-resource-shape/lensoidal"/>
   </skos:ConceptScheme>
   <skos:Concept rdf:about="http://resource.geosciml.org/classifier/cgi/earth-resource-shape/lensoidal">
      <skos:inScheme rdf:resource="http://resource.geosciml.org/classifierscheme/cgi/2016.01/earth-resource-shape"/>
      <skos:definition xml:lang="en">A body bounded by converging surfaces (at least one of which is curved), thick in the middle and thinning out toward the edges, resembling a convex lens.</skos:definition>
      <skos:prefLabel xml:lang="en">lensoidal</skos:prefLabel>
      <skos:notation rdf:datatype="LocalHierarchyKey">01..</skos:notation>
      <skos:altLabel xml:lang="en">lens</skos:altLabel>
      <skos:altLabel xml:lang="en">lenticular</skos:altLabel>
      <skos:topConceptOf rdf:resource="http://resource.geosciml.org/classifierscheme/cgi/2016.01/earth-resource-shape"/>
      <dcterms:source xml:lang="en">Glossary of Geology. 4th Edition, AGI + DC, adapted from</dcterms:source>
   </skos:Concept>
   <skos:ConceptScheme rdf:about="http://resource.geosciml.org/classifierscheme/cgi/2016.01/earth-resource-shape">
      <skos:hasTopConcept rdf:resource="http://resource.geosciml.org/classifier/cgi/earth-resource-shape/tabular"/>
   </skos:ConceptScheme>
   <skos:Concept rdf:about="http://resource.geosciml.org/classifier/cgi/earth-resource-shape/tabular">
      <skos:inScheme rdf:resource="http://resource.geosciml.org/classifierscheme/cgi/2016.01/earth-resource-shape"/>
      <skos:definition xml:lang="en">A body having two dimensions that are much larger or longer than the third, e.g. a dyke-hosted or bed-hosted deposit</skos:definition>
      <skos:prefLabel xml:lang="en">tabular</skos:prefLabel>
      <skos:notation rdf:datatype="LocalHierarchyKey">02..</skos:notation>
      <skos:altLabel xml:lang="en">planar</skos:altLabel>
      <skos:altLabel xml:lang="en">sheet-like</skos:altLabel>
      <skos:altLabel xml:lang="en">sheeted</skos:altLabel>
      <skos:altLabel xml:lang="en">layer</skos:altLabel>
      <skos:altLabel xml:lang="en">blanket-like</skos:altLabel>
      <skos:altLabel xml:lang="en">blanket</skos:altLabel>
      <skos:altLabel xml:lang="en">manto</skos:altLabel>
      <skos:topConceptOf rdf:resource="http://resource.geosciml.org/classifierscheme/cgi/2016.01/earth-resource-shape"/>
      <dcterms:source xml:lang="en">Dictionary of Mining 2nd ed, AGI 1997, adapted from</dcterms:source>
   </skos:Concept>
   <skos:ConceptScheme rdf:about="http://resource.geosciml.org/classifierscheme/cgi/2016.01/earth-resource-shape">
      <skos:hasTopConcept rdf:resource="http://resource.geosciml.org/classifier/cgi/earth-resource-shape/podiform"/>
   </skos:ConceptScheme>
   <skos:Concept rdf:about="http://resource.geosciml.org/classifier/cgi/earth-resource-shape/podiform">
      <skos:inScheme rdf:resource="http://resource.geosciml.org/classifierscheme/cgi/2016.01/earth-resource-shape"/>
      <skos:definition xml:lang="en">A roughly cylindrical body having a diameter that decreases to zero at both ends like a cigar or a potato.</skos:definition>
      <skos:prefLabel xml:lang="en">podiform</skos:prefLabel>
      <skos:notation rdf:datatype="LocalHierarchyKey">03..</skos:notation>
      <skos:altLabel xml:lang="en">pod</skos:altLabel>
      <skos:altLabel xml:lang="en">pod-like</skos:altLabel>
      <skos:topConceptOf rdf:resource="http://resource.geosciml.org/classifierscheme/cgi/2016.01/earth-resource-shape"/>
      <dcterms:source xml:lang="en">Dictionary of Mining 2nd ed, AGI 1997, adapted from</dcterms:source>
   </skos:Concept>
   <skos:ConceptScheme rdf:about="http://resource.geosciml.org/classifierscheme/cgi/2016.01/earth-resource-shape">
      <skos:hasTopConcept rdf:resource="http://resource.geosciml.org/classifier/cgi/earth-resource-shape/nodular"/>
   </skos:ConceptScheme>
   <skos:Concept rdf:about="http://resource.geosciml.org/classifier/cgi/earth-resource-shape/nodular">
      <skos:inScheme rdf:resource="http://resource.geosciml.org/classifierscheme/cgi/2016.01/earth-resource-shape"/>
      <skos:definition xml:lang="en">Having the shape of a nodule or occurring in the form of nodules; e.g. "nodular ore" such as a colloform mineral aggregate with a bulbed surface.</skos:definition>
      <skos:prefLabel xml:lang="en">nodular</skos:prefLabel>
      <skos:notation rdf:datatype="LocalHierarchyKey">04..</skos:notation>
      <skos:altLabel xml:lang="en">nodule</skos:altLabel>
      <skos:topConceptOf rdf:resource="http://resource.geosciml.org/classifierscheme/cgi/2016.01/earth-resource-shape"/>
      <dcterms:source xml:lang="en">Glossary of Geology. 5th Edition, AGI, definition (b)</dcterms:source>
   </skos:Concept>
   <skos:ConceptScheme rdf:about="http://resource.geosciml.org/classifierscheme/cgi/2016.01/earth-resource-shape">
      <skos:hasTopConcept rdf:resource="http://resource.geosciml.org/classifier/cgi/earth-resource-shape/cylindrical"/>
   </skos:ConceptScheme>
   <skos:Concept rdf:about="http://resource.geosciml.org/classifier/cgi/earth-resource-shape/cylindrical">
      <skos:inScheme rdf:resource="http://resource.geosciml.org/classifierscheme/cgi/2016.01/earth-resource-shape"/>
      <skos:definition xml:lang="en">A roughly cylindrical body, which may reduce in diameter at one end like a funnel</skos:definition>
      <skos:prefLabel xml:lang="en">cylindrical</skos:prefLabel>
      <skos:notation rdf:datatype="LocalHierarchyKey">05..</skos:notation>
      <skos:altLabel xml:lang="en">tube</skos:altLabel>
      <skos:altLabel xml:lang="en">tube-like</skos:altLabel>
      <skos:altLabel xml:lang="en">pipe</skos:altLabel>
      <skos:altLabel xml:lang="en">pipe-like</skos:altLabel>
      <skos:altLabel xml:lang="en">chimney</skos:altLabel>
      <skos:altLabel xml:lang="en">shoot</skos:altLabel>
      <skos:altLabel xml:lang="en">funnel</skos:altLabel>
      <skos:altLabel xml:lang="en">tubular</skos:altLabel>
      <skos:topConceptOf rdf:resource="http://resource.geosciml.org/classifierscheme/cgi/2016.01/earth-resource-shape"/>
      <dcterms:source xml:lang="en">BGS Mineral Occurrence Database</dcterms:source>
   </skos:Concept>
   <skos:ConceptScheme rdf:about="http://resource.geosciml.org/classifierscheme/cgi/2016.01/earth-resource-shape">
      <skos:hasTopConcept rdf:resource="http://resource.geosciml.org/classifier/cgi/earth-resource-shape/saddle-shaped"/>
   </skos:ConceptScheme>
   <skos:Concept rdf:about="http://resource.geosciml.org/classifier/cgi/earth-resource-shape/saddle-shaped">
      <skos:inScheme rdf:resource="http://resource.geosciml.org/classifierscheme/cgi/2016.01/earth-resource-shape"/>
      <skos:definition xml:lang="en">Having a curved form like a fold hinge</skos:definition>
      <skos:prefLabel xml:lang="en">saddle-shaped</skos:prefLabel>
      <skos:notation rdf:datatype="LocalHierarchyKey">06..</skos:notation>
      <skos:altLabel xml:lang="en">saddle reef</skos:altLabel>
      <skos:altLabel xml:lang="en">reverse saddle</skos:altLabel>
      <skos:topConceptOf rdf:resource="http://resource.geosciml.org/classifierscheme/cgi/2016.01/earth-resource-shape"/>
      <dcterms:source xml:lang="en">This vocabulary</dcterms:source>
   </skos:Concept>
   <skos:ConceptScheme rdf:about="http://resource.geosciml.org/classifierscheme/cgi/2016.01/earth-resource-shape">
      <skos:hasTopConcept rdf:resource="http://resource.geosciml.org/classifier/cgi/earth-resource-shape/irregular"/>
   </skos:ConceptScheme>
   <skos:Concept rdf:about="http://resource.geosciml.org/classifier/cgi/earth-resource-shape/irregular">
      <skos:inScheme rdf:resource="http://resource.geosciml.org/classifierscheme/cgi/2016.01/earth-resource-shape"/>
      <skos:definition xml:lang="en">Body geometry is irregular and can not be characterized using terminology.</skos:definition>
      <skos:prefLabel xml:lang="en">irregular</skos:prefLabel>
      <skos:notation rdf:datatype="LocalHierarchyKey">07..</skos:notation>
      <skos:topConceptOf rdf:resource="http://resource.geosciml.org/classifierscheme/cgi/2016.01/earth-resource-shape"/>
      <dcterms:source xml:lang="en">From CGI GeologicUnitMorphology vocabulary</dcterms:source>
   </skos:Concept>
   <skos:Collection rdf:about="http://resource.geosciml.org/classifier/cgi/earth-resource-shape">
      <dcterms:title xml:lang="en">Earth Resource Shape - All Concepts</dcterms:title>
      <skos:member><skos:Concept rdf:about="http://resource.geosciml.org/classifier/cgi/earth-resource-shape/lensoidal"/></skos:member>
      <skos:member><skos:Concept rdf:about="http://resource.geosciml.org/classifier/cgi/earth-resource-shape/tabular"/></skos:member>
      <skos:member><skos:Concept rdf:about="http://resource.geosciml.org/classifier/cgi/earth-resource-shape/podiform"/></skos:member>
      <skos:member><skos:Concept rdf:about="http://resource.geosciml.org/classifier/cgi/earth-resource-shape/nodular"/></skos:member>
      <skos:member><skos:Concept rdf:about="http://resource.geosciml.org/classifier/cgi/earth-resource-shape/cylindrical"/></skos:member>
      <skos:member><skos:Concept rdf:about="http://resource.geosciml.org/classifier/cgi/earth-resource-shape/saddle-shaped"/></skos:member>
      <skos:member><skos:Concept rdf:about="http://resource.geosciml.org/classifier/cgi/earth-resource-shape/irregular"/></skos:member>
   </skos:Collection>
   
</rdf:RDF>