<?xml version="1.0" encoding="UTF-8"?>
<rdf:RDF xmlns:rdf="http://www.w3.org/1999/02/22-rdf-syntax-ns#" xmlns:xlink="http://www.w3.org/1999/xlink" xmlns:skos="http://www.w3.org/2004/02/skos/core#" xmlns:dc="http://purl.org/dc/elements/1.1/" xmlns:dcterms="http://purl.org/dc/terms/" xmlns:rdfs="http://www.w3.org/2000/01/rdf-schema#" xmlns:owl="http://www.w3.org/2002/07/owl#">
   <skos:ConceptScheme rdf:about="http://resource.geosciml.org/classifierscheme/cgi/2016.01/exploration-result">
      <dcterms:title xml:lang="en">Exploration Result</dcterms:title>
      <dcterms:description xml:lang="en">This file contains the CGI Exploration Result vocabulary, as defined by the IUGS Commission for Geoscience Information (CGI) Geoscience Terminology Working Group. The vocabulary defines concepts for categorizing the result of the exploration activity. Note that broader-narrower relationships have not been populated for the most part. By extension, this vocabulary includes all concepts in this conceptScheme, as well as concepts in any previous versions of the scheme.</dcterms:description>
      <skos:editorialNote xml:lang="en">This file contains the 2016 SKOS-RDF version of the CGI Exploration Result vocabulary. Vocabulary Shepherd: Mark Rattenbury. Compilation and review in Google doc spreadsheet; adopted 14/01/2014; converted to MS Excel XML for SKOS generation using SKOS_for_GA_from_XLS_2016.03.xslt</skos:editorialNote>
      <skos:changeNote xml:lang="en">2014-02-23 SMR Conversion to SKOS</skos:changeNote>
      <skos:changeNote xml:lang="en">2015-01-08 OLR Edits to fix typos and remove '201401' from rdf file name.</skos:changeNote>
      <skos:changeNote xml:lang="en">2016-11-29 OLR Regenerate SKOS-RDF file as part of migration to new vocabulary server. No change to previous concepts definitions.</skos:changeNote>
      <dcterms:date>2016-11-29</dcterms:date>
      <dcterms:creator>CGI Geoscience Terminology Working Group</dcterms:creator>
   </skos:ConceptScheme>
   <skos:ConceptScheme rdf:about="http://resource.geosciml.org/classifierscheme/cgi/2016.01/exploration-result">
      <skos:hasTopConcept rdf:resource="http://resource.geosciml.org/classifier/cgi/exploration-result/favorable-geological-environment"/>
   </skos:ConceptScheme>
   <skos:Concept rdf:about="http://resource.geosciml.org/classifier/cgi/exploration-result/favorable-geological-environment">
      <skos:inScheme rdf:resource="http://resource.geosciml.org/classifierscheme/cgi/2016.01/exploration-result"/>
      <skos:definition xml:lang="en">Identification of geological units or environments that are favorable or permissive for the occurrence of mineral deposits.</skos:definition>
      <skos:prefLabel xml:lang="en">favorable geological environment</skos:prefLabel>
      <skos:notation rdf:datatype="LocalHierarchyKey">01</skos:notation>
      <skos:altLabel xml:lang="en">prospective area</skos:altLabel>
      <skos:topConceptOf rdf:resource="http://resource.geosciml.org/classifierscheme/cgi/2016.01/exploration-result"/>
      <dcterms:source xml:lang="en">This vocabulary</dcterms:source>
   </skos:Concept>
   <skos:ConceptScheme rdf:about="http://resource.geosciml.org/classifierscheme/cgi/2016.01/exploration-result">
      <skos:hasTopConcept rdf:resource="http://resource.geosciml.org/classifier/cgi/exploration-result/mineral-occurrences"/>
   </skos:ConceptScheme>
   <skos:Concept rdf:about="http://resource.geosciml.org/classifier/cgi/exploration-result/mineral-occurrences">
      <skos:inScheme rdf:resource="http://resource.geosciml.org/classifierscheme/cgi/2016.01/exploration-result"/>
      <skos:definition xml:lang="en">Identification of occurrences of the target minerals as float (stone) or outcrop.</skos:definition>
      <skos:prefLabel xml:lang="en">mineral occurrences</skos:prefLabel>
      <skos:notation rdf:datatype="LocalHierarchyKey">02</skos:notation>
      <skos:altLabel xml:lang="en">mineral showings</skos:altLabel>
      <skos:topConceptOf rdf:resource="http://resource.geosciml.org/classifierscheme/cgi/2016.01/exploration-result"/>
      <dcterms:source xml:lang="en">This vocabulary</dcterms:source>
   </skos:Concept>
   <skos:ConceptScheme rdf:about="http://resource.geosciml.org/classifierscheme/cgi/2016.01/exploration-result">
      <skos:hasTopConcept rdf:resource="http://resource.geosciml.org/classifier/cgi/exploration-result/identification-anomalous-area"/>
   </skos:ConceptScheme>
   <skos:Concept rdf:about="http://resource.geosciml.org/classifier/cgi/exploration-result/identification-anomalous-area">
      <skos:inScheme rdf:resource="http://resource.geosciml.org/classifierscheme/cgi/2016.01/exploration-result"/>
      <skos:definition xml:lang="en">Area where geological, geophysical or geochemical properties are different from areas around and which might indicate the presence of a mineralizing process in the vicinity.</skos:definition>
      <skos:prefLabel xml:lang="en">identification of an anomalous area</skos:prefLabel>
      <skos:notation rdf:datatype="LocalHierarchyKey">03</skos:notation>
      <skos:topConceptOf rdf:resource="http://resource.geosciml.org/classifierscheme/cgi/2016.01/exploration-result"/>
      <skos:narrower rdf:resource="http://resource.geosciml.org/classifier/cgi/exploration-result/key-geological-features"/>
      <skos:narrower rdf:resource="http://resource.geosciml.org/classifier/cgi/exploration-result/geophysical-anomaly"/>
      <skos:narrower rdf:resource="http://resource.geosciml.org/classifier/cgi/exploration-result/geochemical-anomaly"/>
      <dcterms:source xml:lang="en">This vocabulary</dcterms:source>
   </skos:Concept>
   <skos:Concept rdf:about="http://resource.geosciml.org/classifier/cgi/exploration-result/key-geological-features">
      <skos:inScheme rdf:resource="http://resource.geosciml.org/classifierscheme/cgi/2016.01/exploration-result"/>
      <skos:definition xml:lang="en">Identification of particular minerals or geological features which may indicate a possible mineralized area or accompany a mineralizing process</skos:definition>
      <skos:prefLabel xml:lang="en">key geological features</skos:prefLabel>
      <skos:notation rdf:datatype="LocalHierarchyKey">03.1</skos:notation>
      <skos:altLabel xml:lang="en">identification of key minerals</skos:altLabel>
      <skos:broader rdf:resource="http://resource.geosciml.org/classifier/cgi/exploration-result/identification-anomalous-area"/>
      <dcterms:source xml:lang="en">This vocabulary</dcterms:source>
   </skos:Concept>
   <skos:Concept rdf:about="http://resource.geosciml.org/classifier/cgi/exploration-result/geophysical-anomaly">
      <skos:inScheme rdf:resource="http://resource.geosciml.org/classifierscheme/cgi/2016.01/exploration-result"/>
      <skos:definition xml:lang="en">Area where geophysical properties (e.g. radiometric, magnetic, electromagnetic, gravity) differ from surrounding areas and which may be the result of mineralisation.</skos:definition>
      <skos:prefLabel xml:lang="en">geophysical anomaly</skos:prefLabel>
      <skos:notation rdf:datatype="LocalHierarchyKey">03.2</skos:notation>
      <skos:broader rdf:resource="http://resource.geosciml.org/classifier/cgi/exploration-result/identification-anomalous-area"/>
      <dcterms:source xml:lang="en">This vocabulary</dcterms:source>
   </skos:Concept>
   <skos:Concept rdf:about="http://resource.geosciml.org/classifier/cgi/exploration-result/geochemical-anomaly">
      <skos:inScheme rdf:resource="http://resource.geosciml.org/classifierscheme/cgi/2016.01/exploration-result"/>
      <skos:definition xml:lang="en">Area where geochemical properties (e.g. single or multiple element concentrations or isotope ratios) differ from surrounding areas and which may be the result of mineralisation.</skos:definition>
      <skos:prefLabel xml:lang="en">geochemical anomaly</skos:prefLabel>
      <skos:notation rdf:datatype="LocalHierarchyKey">03.3</skos:notation>
      <skos:broader rdf:resource="http://resource.geosciml.org/classifier/cgi/exploration-result/identification-anomalous-area"/>
      <dcterms:source xml:lang="en">This vocabulary</dcterms:source>
   </skos:Concept>
   <skos:ConceptScheme rdf:about="http://resource.geosciml.org/classifierscheme/cgi/2016.01/exploration-result">
      <skos:hasTopConcept rdf:resource="http://resource.geosciml.org/classifier/cgi/exploration-result/mineralized-zone-identified"/>
   </skos:ConceptScheme>
   <skos:Concept rdf:about="http://resource.geosciml.org/classifier/cgi/exploration-result/mineralized-zone-identified">
      <skos:inScheme rdf:resource="http://resource.geosciml.org/classifierscheme/cgi/2016.01/exploration-result"/>
      <skos:definition xml:lang="en">Identification by mapping and sampling of a two dimensional zone where the target minerals are found. This is done mainly by geological mapping and geochemical sampling and may include trenching and pitting.</skos:definition>
      <skos:prefLabel xml:lang="en">mineralized zone identified</skos:prefLabel>
      <skos:notation rdf:datatype="LocalHierarchyKey">04</skos:notation>
      <skos:topConceptOf rdf:resource="http://resource.geosciml.org/classifierscheme/cgi/2016.01/exploration-result"/>
      <dcterms:source xml:lang="en">This vocabulary</dcterms:source>
   </skos:Concept>
   <skos:ConceptScheme rdf:about="http://resource.geosciml.org/classifierscheme/cgi/2016.01/exploration-result">
      <skos:hasTopConcept rdf:resource="http://resource.geosciml.org/classifier/cgi/exploration-result/mineral-resource-indicated"/>
   </skos:ConceptScheme>
   <skos:Concept rdf:about="http://resource.geosciml.org/classifier/cgi/exploration-result/mineral-resource-indicated">
      <skos:inScheme rdf:resource="http://resource.geosciml.org/classifierscheme/cgi/2016.01/exploration-result"/>
      <skos:definition xml:lang="en">Identification of a three dimension zone of mineralization. This is done by augmenting surface work with a small number of drill holes. At this stage there is insufficient data to estimate tonnage and grade.</skos:definition>
      <skos:prefLabel xml:lang="en">mineral resource indicated</skos:prefLabel>
      <skos:notation rdf:datatype="LocalHierarchyKey">05</skos:notation>
      <skos:topConceptOf rdf:resource="http://resource.geosciml.org/classifierscheme/cgi/2016.01/exploration-result"/>
      <dcterms:source xml:lang="en">This vocabulary</dcterms:source>
   </skos:Concept>
   <skos:ConceptScheme rdf:about="http://resource.geosciml.org/classifierscheme/cgi/2016.01/exploration-result">
      <skos:hasTopConcept rdf:resource="http://resource.geosciml.org/classifier/cgi/exploration-result/mineral-resource-defined"/>
   </skos:ConceptScheme>
   <skos:Concept rdf:about="http://resource.geosciml.org/classifier/cgi/exploration-result/mineral-resource-defined">
      <skos:inScheme rdf:resource="http://resource.geosciml.org/classifierscheme/cgi/2016.01/exploration-result"/>
      <skos:definition xml:lang="en">Work has been completed to identify a three dimensional zone of mineralization and estimate its tonnage and grade to the standard of a "mineral resource". Result allows definition of a 'Measured Mineral Resource' as defined by CIM (2010-11-27)</skos:definition>
      <skos:prefLabel xml:lang="en">mineral resource defined</skos:prefLabel>
      <skos:notation rdf:datatype="LocalHierarchyKey">06</skos:notation>
      <skos:topConceptOf rdf:resource="http://resource.geosciml.org/classifierscheme/cgi/2016.01/exploration-result"/>
      <dcterms:source xml:lang="en">Canadian Institute of Mining (CIM) Definitions Standards, 2010-11-27, http://web.cim.org/UserFiles/File/CIM_DEFINITON_STANDARDS_Nov_2010.pdf.</dcterms:source>
   </skos:Concept>
   <skos:ConceptScheme rdf:about="http://resource.geosciml.org/classifierscheme/cgi/2016.01/exploration-result">
      <skos:hasTopConcept rdf:resource="http://resource.geosciml.org/classifier/cgi/exploration-result/mineral-reserve-defined"/>
   </skos:ConceptScheme>
   <skos:Concept rdf:about="http://resource.geosciml.org/classifier/cgi/exploration-result/mineral-reserve-defined">
      <skos:inScheme rdf:resource="http://resource.geosciml.org/classifierscheme/cgi/2016.01/exploration-result"/>
      <skos:definition xml:lang="en">Definition of a three dimensional body of mineralization in sufficient technical detail and accompanied by an economic evaluation so that the estimated tonnage and grade can be classified as a mineral reserve. A Mineral Reserve is the economically mineable part of a Measured or Indicated Mineral Resource demonstrated by at least a Preliminary Feasibility Study.</skos:definition>
      <skos:prefLabel xml:lang="en">mineral reserve defined</skos:prefLabel>
      <skos:notation rdf:datatype="LocalHierarchyKey">07</skos:notation>
      <skos:topConceptOf rdf:resource="http://resource.geosciml.org/classifierscheme/cgi/2016.01/exploration-result"/>
      <dcterms:source xml:lang="en">Canadian Institute of Mining (CIM) Definitions Standards, 2010-11-27, http://web.cim.org/UserFiles/File/CIM_DEFINITON_STANDARDS_Nov_2010.pdf.</dcterms:source>
   </skos:Concept>
   <skos:ConceptScheme rdf:about="http://resource.geosciml.org/classifierscheme/cgi/2016.01/exploration-result">
      <skos:hasTopConcept rdf:resource="http://resource.geosciml.org/classifier/cgi/exploration-result/positive-feasibility-study"/>
   </skos:ConceptScheme>
   <skos:Concept rdf:about="http://resource.geosciml.org/classifier/cgi/exploration-result/positive-feasibility-study">
      <skos:inScheme rdf:resource="http://resource.geosciml.org/classifierscheme/cgi/2016.01/exploration-result"/>
      <skos:definition xml:lang="en">Completion of an economic evaluation of the mineral project at a level sufficient for a feasibility study with a resulting determination that extraction is reaonably justfied. A Feasibility Study is a comprehensive technical and economic study of the selected development option for a mineral project that includes appropriately detailed assessments of all factors necessary to determine at the time of reporting whether extraction is reasonably justified (economically mineable).</skos:definition>
      <skos:prefLabel xml:lang="en">positive feasibility study</skos:prefLabel>
      <skos:notation rdf:datatype="LocalHierarchyKey">08</skos:notation>
      <skos:topConceptOf rdf:resource="http://resource.geosciml.org/classifierscheme/cgi/2016.01/exploration-result"/>
      <dcterms:source xml:lang="en">Canadian Institute of Mining (CIM) Definitions Standards, 2010-11-27, http://web.cim.org/UserFiles/File/CIM_DEFINITON_STANDARDS_Nov_2010.pdf.</dcterms:source>
   </skos:Concept>
   <skos:ConceptScheme rdf:about="http://resource.geosciml.org/classifierscheme/cgi/2016.01/exploration-result">
      <skos:hasTopConcept rdf:resource="http://resource.geosciml.org/classifier/cgi/exploration-result/negative-feasibility-study"/>
   </skos:ConceptScheme>
   <skos:Concept rdf:about="http://resource.geosciml.org/classifier/cgi/exploration-result/negative-feasibility-study">
      <skos:inScheme rdf:resource="http://resource.geosciml.org/classifierscheme/cgi/2016.01/exploration-result"/>
      <skos:definition xml:lang="en">Completion of an economic evaluation of the mineral project at a level sufficient for a feasbility study with a resulting determination that extraction is not reasonably justified. A Feasibility Study is a comprehensive technical and economic study of the selected development option for a mineral project that includes appropriately detailed assessments of all factors necessary to determine at the time of reporting whether extraction is reasonably justified (economically mineable).</skos:definition>
      <skos:prefLabel xml:lang="en">negative feasibility study</skos:prefLabel>
      <skos:notation rdf:datatype="LocalHierarchyKey">09</skos:notation>
      <skos:topConceptOf rdf:resource="http://resource.geosciml.org/classifierscheme/cgi/2016.01/exploration-result"/>
      <dcterms:source xml:lang="en">Canadian Institute of Mining (CIM) Definitions Standards, 2010-11-27, http://web.cim.org/UserFiles/File/CIM_DEFINITON_STANDARDS_Nov_2010.pdf.</dcterms:source>
   </skos:Concept>
   <skos:Collection rdf:about="http://resource.geosciml.org/classifier/cgi/exploration-result">
      <dcterms:title xml:lang="en">Exploration Result - All Concepts</dcterms:title>
      <skos:member><skos:Concept rdf:about="http://resource.geosciml.org/classifier/cgi/exploration-result/favorable-geological-environment"/></skos:member>
      <skos:member><skos:Concept rdf:about="http://resource.geosciml.org/classifier/cgi/exploration-result/mineral-occurrences"/></skos:member>
      <skos:member><skos:Concept rdf:about="http://resource.geosciml.org/classifier/cgi/exploration-result/identification-anomalous-area"/></skos:member>
      <skos:member><skos:Concept rdf:about="http://resource.geosciml.org/classifier/cgi/exploration-result/key-geological-features"/></skos:member>
      <skos:member><skos:Concept rdf:about="http://resource.geosciml.org/classifier/cgi/exploration-result/geophysical-anomaly"/></skos:member>
      <skos:member><skos:Concept rdf:about="http://resource.geosciml.org/classifier/cgi/exploration-result/geochemical-anomaly"/></skos:member>
      <skos:member><skos:Concept rdf:about="http://resource.geosciml.org/classifier/cgi/exploration-result/mineralized-zone-identified"/></skos:member>
      <skos:member><skos:Concept rdf:about="http://resource.geosciml.org/classifier/cgi/exploration-result/mineral-resource-indicated"/></skos:member>
      <skos:member><skos:Concept rdf:about="http://resource.geosciml.org/classifier/cgi/exploration-result/mineral-resource-defined"/></skos:member>
      <skos:member><skos:Concept rdf:about="http://resource.geosciml.org/classifier/cgi/exploration-result/mineral-reserve-defined"/></skos:member>
      <skos:member><skos:Concept rdf:about="http://resource.geosciml.org/classifier/cgi/exploration-result/positive-feasibility-study"/></skos:member>
      <skos:member><skos:Concept rdf:about="http://resource.geosciml.org/classifier/cgi/exploration-result/negative-feasibility-study"/></skos:member>
   </skos:Collection>
</rdf:RDF>