<?xml version="1.0" encoding="UTF-8"?>
<rdf:RDF xmlns:rdf="http://www.w3.org/1999/02/22-rdf-syntax-ns#" xmlns:xlink="http://www.w3.org/1999/xlink" xmlns:skos="http://www.w3.org/2004/02/skos/core#" xmlns:dc="http://purl.org/dc/elements/1.1/" xmlns:dcterms="http://purl.org/dc/terms/" xmlns:rdfs="http://www.w3.org/2000/01/rdf-schema#" xmlns:owl="http://www.w3.org/2002/07/owl#">
   <skos:ConceptScheme rdf:about="http://resource.geosciml.org/classifierscheme/cgi/2016.02/earth-resource-form">
      <dcterms:title xml:lang="en">Earth Resource Form</dcterms:title>
      <dcterms:description xml:lang="en">This file contains the CGI Earth Resource Form vocabulary, as defined by the IUGS Commission for Geoscience Information (CGI) Geoscience Terminology Working Group. This scheme describes concepts specifying an orebody's typical physical and structural relationship to wallrocks and associated rocks (e.g. strataform, stratabound, cross-cutting, vein, intrusive contact etc). The vocabulary includes two sub-schemes, one that includes categories related to the concordance or discordance to host rock structure, and the second that categorizes according to association genetic structure in the host rock. The EarthResource/form property allows multiple values, so that terms from both sub-schemes might be assigned to a given instance. By extension, this vocabulary includes all concepts in this conceptScheme, as well as concepts in any previous versions of the scheme.</dcterms:description>
      <skos:editorialNote xml:lang="en">This file contains the 2016 SKOS-RDF version of the CGI Earth Resource Form vocabulary. Compilation and review in MS Excel spreadsheet, converted to MS Excel for SKOS generation using SKOS_for_GA_from_XLS_2016.03.xslt</skos:editorialNote>
      <skos:changeNote xml:lang="en">2014-02-23 SMR - hierarchy finalized, sourceNote set to 'this vocabulary' and skos:note added by SM Richard; converted to MS Excel XML for SKOS generation using GSML_SKOS_from_XLS_2013.xslt; Conversion to SKOS by SM Richard</skos:changeNote>
      <skos:changeNote xml:lang="en">2015-01-08 OLR - Edits to fix typos and remove '201401' from rdf file name.</skos:changeNote>
      <skos:changeNote xml:lang="en">2016-07-16 Compilation and review in Google doc spreadsheet, converted to SKOS-RDF using GSML_SKOS_fromXLS_2016.02.xslt.</skos:changeNote>
      <skos:changeNote xml:lang="en">2016-11-28 OLR regenerate SKOS-RDF file as part of migration to new vocabulary server. No change to previous concepts definitions.</skos:changeNote>
      <dcterms:date>2016-11-28</dcterms:date>
      <dcterms:creator>CGI Geoscience Terminology Working Group</dcterms:creator>
   </skos:ConceptScheme>
   <skos:ConceptScheme rdf:about="http://resource.geosciml.org/classifierscheme/cgi/2016.02/earth-resource-form">
      <skos:hasTopConcept rdf:resource="http://resource.geosciml.org/classifier/cgi/earth-resource-form/concordant"/>
   </skos:ConceptScheme>
   <skos:Concept rdf:about="http://resource.geosciml.org/classifier/cgi/earth-resource-form/concordant">
      <skos:inScheme rdf:resource="http://resource.geosciml.org/classifierscheme/cgi/2016.02/earth-resource-form"/>
      <skos:definition xml:lang="en">A concordant or nearly concordant mineral deposit lies parallel or nearly parallel to wallrocks contacts or internal structures (bedding, foliation, etc.)</skos:definition>
      <skos:prefLabel xml:lang="en">concordant</skos:prefLabel>
      <skos:notation rdf:datatype="LocalHierarchyKey">01</skos:notation>
      <skos:topConceptOf rdf:resource="http://resource.geosciml.org/classifierscheme/cgi/2016.02/earth-resource-form"/>
      <skos:narrower rdf:resource="http://resource.geosciml.org/classifier/cgi/earth-resource-form/stratabound"/>
      <dcterms:source xml:lang="en">this vocabulary</dcterms:source>
   </skos:Concept>
   <skos:Concept rdf:about="http://resource.geosciml.org/classifier/cgi/earth-resource-form/stratabound">
      <skos:inScheme rdf:resource="http://resource.geosciml.org/classifierscheme/cgi/2016.02/earth-resource-form"/>
      <skos:definition xml:lang="en">A body of mineralisation confined to a single stratigraphic unit. A stratabound deposit may contain discordant internal structures (eg, brecciation)</skos:definition>
      <skos:prefLabel xml:lang="en">stratabound</skos:prefLabel>
      <skos:notation rdf:datatype="LocalHierarchyKey">01.1</skos:notation>
      <skos:broader rdf:resource="http://resource.geosciml.org/classifier/cgi/earth-resource-form/concordant"/>
      <skos:narrower rdf:resource="http://resource.geosciml.org/classifier/cgi/earth-resource-form/stratiform"/>
      <dcterms:source xml:lang="en">this vocabulary</dcterms:source>
   </skos:Concept>
   <skos:Concept rdf:about="http://resource.geosciml.org/classifier/cgi/earth-resource-form/stratiform">
      <skos:inScheme rdf:resource="http://resource.geosciml.org/classifierscheme/cgi/2016.02/earth-resource-form"/>
      <skos:definition xml:lang="en">A type of stratabound mineral deposit that is strictly coextensive with one or more sedimentary, metamorphic or igneous layers</skos:definition>
      <skos:prefLabel xml:lang="en">stratiform</skos:prefLabel>
      <skos:notation rdf:datatype="LocalHierarchyKey">01.1.1</skos:notation>
      <skos:broader rdf:resource="http://resource.geosciml.org/classifier/cgi/earth-resource-form/stratabound"/>
      <dcterms:source xml:lang="en">this vocabulary</dcterms:source>
   </skos:Concept>
   <skos:ConceptScheme rdf:about="http://resource.geosciml.org/classifierscheme/cgi/2016.02/earth-resource-form">
      <skos:hasTopConcept rdf:resource="http://resource.geosciml.org/classifier/cgi/earth-resource-form/discordant"/>
   </skos:ConceptScheme>
   <skos:Concept rdf:about="http://resource.geosciml.org/classifier/cgi/earth-resource-form/discordant">
      <skos:inScheme rdf:resource="http://resource.geosciml.org/classifierscheme/cgi/2016.02/earth-resource-form"/>
      <skos:definition xml:lang="en">A mineral deposit which crosscuts stratigraphic contacts or internal structures (eg, bedding, foliation) within its host rocks (eg, vein, reef, mass, lens, pipe, column, etc.)</skos:definition>
      <skos:prefLabel xml:lang="en">discordant</skos:prefLabel>
      <skos:notation rdf:datatype="LocalHierarchyKey">02</skos:notation>
      <skos:topConceptOf rdf:resource="http://resource.geosciml.org/classifierscheme/cgi/2016.02/earth-resource-form"/>
      <dcterms:source xml:lang="en">this vocabulary</dcterms:source>
   </skos:Concept>
   <skos:ConceptScheme rdf:about="http://resource.geosciml.org/classifierscheme/cgi/2016.02/earth-resource-form">
      <skos:hasTopConcept rdf:resource="http://resource.geosciml.org/classifier/cgi/earth-resource-form/mixed-concordant-discordant"/>
   </skos:ConceptScheme>
   <skos:Concept rdf:about="http://resource.geosciml.org/classifier/cgi/earth-resource-form/mixed-concordant-discordant">
      <skos:inScheme rdf:resource="http://resource.geosciml.org/classifierscheme/cgi/2016.02/earth-resource-form"/>
      <skos:definition xml:lang="en">A subconcordant body in some places lies parallel to, and in other places crosscuts, wallrock contacts or internal structures (eg, bedding, foliation)</skos:definition>
      <skos:prefLabel xml:lang="en">mixed concordant discordant</skos:prefLabel>
      <skos:notation rdf:datatype="LocalHierarchyKey">03</skos:notation>
      <skos:topConceptOf rdf:resource="http://resource.geosciml.org/classifierscheme/cgi/2016.02/earth-resource-form"/>
      <dcterms:source xml:lang="en">this vocabulary</dcterms:source>
   </skos:Concept>
   <skos:ConceptScheme rdf:about="http://resource.geosciml.org/classifierscheme/cgi/2016.02/earth-resource-form">
      <skos:hasTopConcept rdf:resource="http://resource.geosciml.org/classifier/cgi/earth-resource-form/intrusive-contact-related"/>
   </skos:ConceptScheme>
   <skos:Concept rdf:about="http://resource.geosciml.org/classifier/cgi/earth-resource-form/intrusive-contact-related">
      <skos:inScheme rdf:resource="http://resource.geosciml.org/classifierscheme/cgi/2016.02/earth-resource-form"/>
      <skos:definition xml:lang="en">The form of the mineral deposit is controlled by an igneous intrusive contact</skos:definition>
      <skos:prefLabel xml:lang="en">intrusive contact-related</skos:prefLabel>
      <skos:note xml:lang="en">Mineralization is concordant to the intrusive contact. If the intrusion is discordant to host rock structure, the mineral deposit is discordant to the host rock.</skos:note>
      <skos:notation rdf:datatype="LocalHierarchyKey">04</skos:notation>
      <skos:topConceptOf rdf:resource="http://resource.geosciml.org/classifierscheme/cgi/2016.02/earth-resource-form"/>
      <dcterms:source xml:lang="en">this vocabulary</dcterms:source>
   </skos:Concept>
   <skos:ConceptScheme rdf:about="http://resource.geosciml.org/classifierscheme/cgi/2016.02/earth-resource-form">
      <skos:hasTopConcept rdf:resource="http://resource.geosciml.org/classifier/cgi/earth-resource-form/fault-hosted"/>
   </skos:ConceptScheme>
   <skos:Concept rdf:about="http://resource.geosciml.org/classifier/cgi/earth-resource-form/fault-hosted">
      <skos:inScheme rdf:resource="http://resource.geosciml.org/classifierscheme/cgi/2016.02/earth-resource-form"/>
      <skos:definition xml:lang="en">The mineral deposit is hosted within a fault or shear zone.</skos:definition>
      <skos:prefLabel xml:lang="en">fault-hosted</skos:prefLabel>
      <skos:note xml:lang="en">Mineralization is concordant to the fault. If the fault is discordant to host rock structure, the mineral deposit is discordant.</skos:note>
      <skos:notation rdf:datatype="LocalHierarchyKey">05</skos:notation>
      <skos:topConceptOf rdf:resource="http://resource.geosciml.org/classifierscheme/cgi/2016.02/earth-resource-form"/>
      <dcterms:source xml:lang="en">this vocabulary</dcterms:source>
   </skos:Concept>
   <skos:ConceptScheme rdf:about="http://resource.geosciml.org/classifierscheme/cgi/2016.02/earth-resource-form">
      <skos:hasTopConcept rdf:resource="http://resource.geosciml.org/classifier/cgi/earth-resource-form/structurally-transposed"/>
   </skos:ConceptScheme>
   <skos:Concept rdf:about="http://resource.geosciml.org/classifier/cgi/earth-resource-form/structurally-transposed">
      <skos:inScheme rdf:resource="http://resource.geosciml.org/classifierscheme/cgi/2016.02/earth-resource-form"/>
      <skos:definition xml:lang="en">The form of the mineral deposit has been significantly modified by post-mineralization structural modification.</skos:definition>
      <skos:prefLabel xml:lang="en">structurally transposed</skos:prefLabel>
      <skos:note xml:lang="en">The term 'transposition' has a connotation of ductile deformation. The deformed ore body might be transposed into concordance with the fabric produced by the transposition and is concordant in that sense. At the same time the pre-deformation ore body might have orignated as a discordant body.</skos:note>
      <skos:notation rdf:datatype="LocalHierarchyKey">06</skos:notation>
      <skos:topConceptOf rdf:resource="http://resource.geosciml.org/classifierscheme/cgi/2016.02/earth-resource-form"/>
      <dcterms:source xml:lang="en">this vocabulary</dcterms:source>
   </skos:Concept>
   <skos:ConceptScheme rdf:about="http://resource.geosciml.org/classifierscheme/cgi/2016.02/earth-resource-form">
      <skos:hasTopConcept rdf:resource="http://resource.geosciml.org/classifier/cgi/earth-resource-form/unconformity-related"/>
   </skos:ConceptScheme>
   <skos:Concept rdf:about="http://resource.geosciml.org/classifier/cgi/earth-resource-form/unconformity-related">
      <skos:inScheme rdf:resource="http://resource.geosciml.org/classifierscheme/cgi/2016.02/earth-resource-form"/>
      <skos:definition xml:lang="en">A mineral deposit whose location and form are related to an unconformity between sedimentary host rocks</skos:definition>
      <skos:prefLabel xml:lang="en">unconformity-related</skos:prefLabel>
      <skos:note xml:lang="en">Mineralization is concordant to the unconformity, and thus concordant to whatever is above the unconformity, but if the unconformity is an angular unconformity, the resource body will be discordant to bedding below the unconformity</skos:note>
      <skos:notation rdf:datatype="LocalHierarchyKey">07</skos:notation>
      <skos:topConceptOf rdf:resource="http://resource.geosciml.org/classifierscheme/cgi/2016.02/earth-resource-form"/>
      <dcterms:source xml:lang="en">this vocabulary</dcterms:source>
   </skos:Concept>
   <skos:ConceptScheme rdf:about="http://resource.geosciml.org/classifierscheme/cgi/2016.02/earth-resource-form">
      <skos:hasTopConcept rdf:resource="http://resource.geosciml.org/classifier/cgi/earth-resource-form/surficial"/>
   </skos:ConceptScheme>
   <skos:Concept rdf:about="http://resource.geosciml.org/classifier/cgi/earth-resource-form/surficial">
      <skos:inScheme rdf:resource="http://resource.geosciml.org/classifierscheme/cgi/2016.02/earth-resource-form"/>
      <skos:definition xml:lang="en">A mineral deposit forming a surficial layer in or on its host rocks</skos:definition>
      <skos:prefLabel xml:lang="en">surficial</skos:prefLabel>
      <skos:note xml:lang="en">If sedimentary rocks underlying the surface are horizontal, then the surficial deposit will be concordant, and would be expected to be stratiform if preserved in the geologic record. If the Earth Surface is an erosional surface on older rocks, the deposit will also be unconformity-related.</skos:note>
      <skos:notation rdf:datatype="LocalHierarchyKey">08</skos:notation>
      <skos:topConceptOf rdf:resource="http://resource.geosciml.org/classifierscheme/cgi/2016.02/earth-resource-form"/>
      <dcterms:source xml:lang="en">this vocabulary</dcterms:source>
   </skos:Concept>
   <skos:Collection rdf:about="http://resource.geosciml.org/classifier/cgi/earth-resource-form">
      <dcterms:title xml:lang="en">Earth Resource Form - All Concepts</dcterms:title>
      <skos:member>
         <skos:Concept rdf:about="http://resource.geosciml.org/classifier/cgi/earth-resource-form/concordant"/>
      </skos:member>
      <skos:member>
         <skos:Concept rdf:about="http://resource.geosciml.org/classifier/cgi/earth-resource-form/stratabound"/>
      </skos:member>
      <skos:member>
         <skos:Concept rdf:about="http://resource.geosciml.org/classifier/cgi/earth-resource-form/stratiform"/>
      </skos:member>
      <skos:member>
         <skos:Concept rdf:about="http://resource.geosciml.org/classifier/cgi/earth-resource-form/discordant"/>
      </skos:member>
      <skos:member>
         <skos:Concept rdf:about="http://resource.geosciml.org/classifier/cgi/earth-resource-form/mixed-concordant-discordant"/>
      </skos:member>
      <skos:member>
         <skos:Concept rdf:about="http://resource.geosciml.org/classifier/cgi/earth-resource-form/intrusive-contact-related"/>
      </skos:member>
      <skos:member>
         <skos:Concept rdf:about="http://resource.geosciml.org/classifier/cgi/earth-resource-form/fault-hosted"/>
      </skos:member>
      <skos:member>
         <skos:Concept rdf:about="http://resource.geosciml.org/classifier/cgi/earth-resource-form/structurally-transposed"/>
      </skos:member>
      <skos:member>
         <skos:Concept rdf:about="http://resource.geosciml.org/classifier/cgi/earth-resource-form/unconformity-related"/>
      </skos:member>
      <skos:member>
         <skos:Concept rdf:about="http://resource.geosciml.org/classifier/cgi/earth-resource-form/surficial"/>
      </skos:member>
   </skos:Collection>
</rdf:RDF>