<?xml version="1.0"?>


<!DOCTYPE rdf:RDF [
    <!ENTITY owl "http://www.w3.org/2002/07/owl#" >
    <!ENTITY dc "http://purl.org/dc/elements/1.1/" >
    <!ENTITY xsd "http://www.w3.org/2001/XMLSchema#" >
    <!ENTITY owl2xml "http://www.w3.org/2006/12/owl2-xml#" >
    <!ENTITY skos "http://www.w3.org/2004/02/skos/core#" >
    <!ENTITY rdfs "http://www.w3.org/2000/01/rdf-schema#" >
    <!ENTITY rdf "http://www.w3.org/1999/02/22-rdf-syntax-ns#" >
    <!ENTITY cgi "http://resource.geosciml.org/classifierscheme/cgi/201012/" >
]>


<rdf:RDF xmlns="&cgi;stratigraphicrank#"
     xml:base="&cgi;stratigraphicrank"
     xmlns:dc="http://purl.org/dc/elements/1.1/"
     xmlns:rdfs="http://www.w3.org/2000/01/rdf-schema#"
     xmlns:owl2xml="http://www.w3.org/2006/12/owl2-xml#"
     xmlns:cgi="http://resource.geosciml.org/classifierscheme/cgi/201012/"
     xmlns:owl="http://www.w3.org/2002/07/owl#"
     xmlns:xsd="http://www.w3.org/2001/XMLSchema#"
     xmlns:rdf="http://www.w3.org/1999/02/22-rdf-syntax-ns#"
     xmlns:skos="http://www.w3.org/2004/02/skos/core#">
    <owl:Ontology rdf:about="">
        <skos:historyNote xml:lang="en"
            >2009-07-14. Generate SKOS encoding of vocabulary from Excel spreadsheet.</skos:historyNote>
        <skos:historyNote xml:lang="en"
            >2010-02-08. SMR Clean up namespace declarations so concept URI&#39;s follow CGI URN scheme; concepts have URN, are not document fragments.</skos:historyNote>
        <dc:language>en</dc:language>
        <dc:identifier
            >http://resource.geosciml.org/classifierscheme/cgi/201012/stratigraphicrank</dc:identifier>
        <dc:creator
            >Concept Definition Task Group of IUGS CGI Interoperability Working Group (http://www.cgi-iugs.org/tech_collaboration/interoperability_working_group.html)</dc:creator>
        <skos:historyNote xml:lang="en"
            >2010-02-08. SMR Clean up namespace declarations so concept URI\&#39;s follow CGI URN scheme; concepts have URN, are not document fragments.</skos:historyNote>
        <skos:historyNote xml:lang="en"
            >2010-11-28 SMR replace URN with http URI constructed according to CGI URI scheme (see https://www.seegrid.csiro.au/wiki/bin/view/CGIModel/PersistentIdentifiersInGeoSciMLServices)</skos:historyNote>
        <skos:historyNote xml:lang="en"
            >2011-02-16 SMR Add broader/narrower relations according to stratigraphic code. These are not meant to be formal isA or PartOf relations, rather should be read something like &#39;broader in local intention&#39; or &#39;may be part of&#39;. Add term &#39;Complex&#39; to vocabulary</skos:historyNote>
        <dc:title xml:lang="en"
            >CGI Stratigraphic rank vocabulary</dc:title>
        <dc:publisher
            >Concept Definition Task Group of IUGS CGI Interoperability Working Group (http://www.cgi-iugs.org/tech_collaboration/interoperability_working_group.html)</dc:publisher>
        <owl:versionInfo>201012</owl:versionInfo>
        <dc:format xml:lang="en"
            >application/rdf+xml</dc:format>
    </owl:Ontology>
    


    <!-- 
    ///////////////////////////////////////////////////////////////////////////////////////
    //
    // Annotation properties
    //
    ///////////////////////////////////////////////////////////////////////////////////////
     -->

    <owl:AnnotationProperty rdf:about="&dc;title"/>
    <owl:AnnotationProperty rdf:about="&dc;format"/>
    <owl:AnnotationProperty rdf:about="&dc;creator"/>
    <owl:AnnotationProperty rdf:about="&dc;source"/>
    <owl:AnnotationProperty rdf:about="&dc;publisher"/>
    <owl:AnnotationProperty rdf:about="&dc;identifier"/>
    <owl:AnnotationProperty rdf:about="&dc;language"/>
    <owl:AnnotationProperty rdf:about="&skos;historyNote"/>
    


    <!-- 
    ///////////////////////////////////////////////////////////////////////////////////////
    //
    // Object Properties
    //
    ///////////////////////////////////////////////////////////////////////////////////////
     -->

    


    <!-- http://www.w3.org/1999/02/22-rdf-syntax-ns#value -->

    <owl:ObjectProperty rdf:about="&rdf;value">
        <owl:subObjectPropertyOf rdf:resource="&owl;topDataProperty"/>
    </owl:ObjectProperty>
    


    <!-- http://www.w3.org/2002/07/owl#topDataProperty -->

    <owl:ObjectProperty rdf:about="&owl;topDataProperty"/>
    


    <!-- http://www.w3.org/2002/07/owl#topObjectProperty -->

    <owl:ObjectProperty rdf:about="&owl;topObjectProperty"/>
    


    <!-- http://www.w3.org/2004/02/skos/core#broadMatch -->

    <owl:ObjectProperty rdf:about="&skos;broadMatch">
        <rdfs:label xml:lang="en">broader match</rdfs:label>
        <rdfs:isDefinedBy rdf:datatype="&xsd;anyURI"
            >http://www.w3.org/2004/02/skos/core</rdfs:isDefinedBy>
        <rdfs:subPropertyOf rdf:resource="&skos;broader"/>
        <rdfs:subPropertyOf rdf:resource="&skos;mappingRelation"/>
    </owl:ObjectProperty>
    


    <!-- http://www.w3.org/2004/02/skos/core#broader -->

    <owl:ObjectProperty rdf:about="&skos;broader">
        <rdfs:label xml:lang="en">has broader</rdfs:label>
        <rdfs:isDefinedBy rdf:datatype="&xsd;anyURI"
            >http://www.w3.org/2004/02/skos/core</rdfs:isDefinedBy>
        <rdfs:comment xml:lang="en"
            >Broader concepts are typically rendered as parents in a concept
      hierarchy (tree).</rdfs:comment>
        <rdfs:comment xml:lang="en"
            >By convention, skos:broader is only used to assert an immediate
      (i.e. direct) hierarchical link between two conceptual resources.</rdfs:comment>
        <rdfs:subPropertyOf rdf:resource="&skos;broaderTransitive"/>
    </owl:ObjectProperty>
    


    <!-- http://www.w3.org/2004/02/skos/core#broaderTransitive -->

    <owl:ObjectProperty rdf:about="&skos;broaderTransitive">
        <rdf:type rdf:resource="&owl;TransitiveProperty"/>
        <rdfs:label xml:lang="en"
            >broader transitive</rdfs:label>
        <rdfs:isDefinedBy rdf:datatype="&xsd;anyURI"
            >http://www.w3.org/2004/02/skos/core</rdfs:isDefinedBy>
        <rdfs:comment xml:lang="en"
            >By convention, skos:broaderTransitive is not used to make
      assertions. Rather, the properties can be used to draw inferences about the transitive closure
      of the hierarchical relation, which is useful e.g. when implementing a simple query expansion
      algorithm in a search application.</rdfs:comment>
        <owl:inverseOf rdf:resource="&skos;narrowerTransitive"/>
        <rdfs:subPropertyOf rdf:resource="&skos;semanticRelation"/>
    </owl:ObjectProperty>
    


    <!-- http://www.w3.org/2004/02/skos/core#changeNote -->

    <owl:ObjectProperty rdf:about="&skos;changeNote">
        <owl:subObjectPropertyOf rdf:resource="&owl;topDataProperty"/>
    </owl:ObjectProperty>
    


    <!-- http://www.w3.org/2004/02/skos/core#closeMatch -->

    <owl:ObjectProperty rdf:about="&skos;closeMatch">
        <rdf:type rdf:resource="&owl;SymmetricProperty"/>
        <rdfs:label xml:lang="en">close match</rdfs:label>
        <rdfs:isDefinedBy rdf:datatype="&xsd;anyURI"
            >http://www.w3.org/2004/02/skos/core</rdfs:isDefinedBy>
        <owl:inverseOf rdf:resource="&skos;closeMatch"/>
        <rdfs:subPropertyOf rdf:resource="&skos;mappingRelation"/>
    </owl:ObjectProperty>
    


    <!-- http://www.w3.org/2004/02/skos/core#definition -->

    <owl:ObjectProperty rdf:about="&skos;definition">
        <owl:subObjectPropertyOf rdf:resource="&owl;topDataProperty"/>
    </owl:ObjectProperty>
    


    <!-- http://www.w3.org/2004/02/skos/core#exactMatch -->

    <owl:ObjectProperty rdf:about="&skos;exactMatch">
        <rdf:type rdf:resource="&owl;SymmetricProperty"/>
        <rdf:type rdf:resource="&owl;TransitiveProperty"/>
        <rdfs:label xml:lang="en">exact match</rdfs:label>
        <rdfs:isDefinedBy rdf:datatype="&xsd;anyURI"
            >http://www.w3.org/2004/02/skos/core</rdfs:isDefinedBy>
        <rdfs:comment xml:lang="en"
            >skos:exactMatch is disjoint with each of the properties
      skos:broadMatch and skos:relatedMatch.</rdfs:comment>
        <rdfs:subPropertyOf rdf:resource="&skos;closeMatch"/>
        <owl:inverseOf rdf:resource="&skos;exactMatch"/>
    </owl:ObjectProperty>
    


    <!-- http://www.w3.org/2004/02/skos/core#hasTopConcept -->

    <owl:ObjectProperty rdf:about="&skos;hasTopConcept">
        <rdf:type rdf:resource="&owl;AsymmetricProperty"/>
        <rdf:type rdf:resource="&owl;IrreflexiveProperty"/>
        <rdfs:label xml:lang="en">has top concept</rdfs:label>
        <rdfs:isDefinedBy rdf:datatype="&xsd;anyURI"
            >http://www.w3.org/2004/02/skos/core</rdfs:isDefinedBy>
        <rdfs:range rdf:resource="&skos;Concept"/>
        <rdfs:domain rdf:resource="&skos;ConceptScheme"/>
    </owl:ObjectProperty>
    


    <!-- http://www.w3.org/2004/02/skos/core#historyNote -->

    <owl:ObjectProperty rdf:about="&skos;historyNote">
        <rdf:type rdf:resource="&owl;AnnotationProperty"/>
        <owl:subObjectPropertyOf rdf:resource="&owl;topDataProperty"/>
    </owl:ObjectProperty>
    


    <!-- http://www.w3.org/2004/02/skos/core#inScheme -->

    <owl:ObjectProperty rdf:about="&skos;inScheme">
        <rdfs:label xml:lang="en">in scheme</rdfs:label>
        <rdfs:isDefinedBy rdf:datatype="&xsd;anyURI"
            >http://www.w3.org/2004/02/skos/core</rdfs:isDefinedBy>
        <rdfs:comment xml:lang="en"
            >A concept may be a member of more than one concept scheme.</rdfs:comment>
        <rdfs:subPropertyOf rdf:resource="&owl;topObjectProperty"/>
        <rdfs:range rdf:resource="&skos;ConceptScheme"/>
    </owl:ObjectProperty>
    


    <!-- http://www.w3.org/2004/02/skos/core#mappingRelation -->

    <owl:ObjectProperty rdf:about="&skos;mappingRelation">
        <rdfs:label xml:lang="en"
            >mapping relation</rdfs:label>
        <rdfs:isDefinedBy rdf:datatype="&xsd;anyURI"
            >http://www.w3.org/2004/02/skos/core</rdfs:isDefinedBy>
        <rdfs:comment xml:lang="en"
            >These concept mapping relations mirror semantic relations, and the
      data model defined below is similar (with the exception of skos:exactMatch) to the data model
      defined for semantic relations. A distinct vocabulary is provided for concept mapping
      relations, to provide a convenient way to differentiate links within a concept scheme from
      links between concept schemes. However, this pattern of usage is not a formal requirement of
      the SKOS data model, and relies on informal definitions of best practice.</rdfs:comment>
        <rdfs:subPropertyOf rdf:resource="&skos;semanticRelation"/>
    </owl:ObjectProperty>
    


    <!-- http://www.w3.org/2004/02/skos/core#member -->

    <owl:ObjectProperty rdf:about="&skos;member">
        <rdfs:label xml:lang="en">member</rdfs:label>
        <rdfs:isDefinedBy rdf:datatype="&xsd;anyURI"
            >http://www.w3.org/2004/02/skos/core</rdfs:isDefinedBy>
        <rdfs:subPropertyOf rdf:resource="&owl;topObjectProperty"/>
        <rdfs:domain rdf:resource="&skos;Collection"/>
        <rdfs:range>
            <owl:Class>
                <owl:unionOf rdf:parseType="Collection">
                    <rdf:Description rdf:about="&skos;Collection"/>
                    <rdf:Description rdf:about="&skos;Concept"/>
                </owl:unionOf>
            </owl:Class>
        </rdfs:range>
    </owl:ObjectProperty>
    


    <!-- http://www.w3.org/2004/02/skos/core#memberList -->

    <owl:ObjectProperty rdf:about="&skos;memberList">
        <rdf:type rdf:resource="&owl;FunctionalProperty"/>
        <rdfs:label xml:lang="en">member list</rdfs:label>
        <rdfs:isDefinedBy rdf:datatype="&xsd;anyURI"
            >http://www.w3.org/2004/02/skos/core</rdfs:isDefinedBy>
        <rdfs:comment xml:lang="en"
            >For any resource, every item in the list given as the value of the
      skos:memberList property is also a value of the skos:member property.</rdfs:comment>
        <rdfs:subPropertyOf rdf:resource="&owl;topObjectProperty"/>
        <rdfs:domain rdf:resource="&skos;OrderedCollection"/>
    </owl:ObjectProperty>
    


    <!-- http://www.w3.org/2004/02/skos/core#narrowMatch -->

    <owl:ObjectProperty rdf:about="&skos;narrowMatch">
        <rdfs:label xml:lang="en">narrower match</rdfs:label>
        <rdfs:isDefinedBy rdf:datatype="&xsd;anyURI"
            >http://www.w3.org/2004/02/skos/core</rdfs:isDefinedBy>
        <owl:inverseOf rdf:resource="&skos;broadMatch"/>
        <rdfs:subPropertyOf rdf:resource="&skos;mappingRelation"/>
        <rdfs:subPropertyOf rdf:resource="&skos;narrower"/>
    </owl:ObjectProperty>
    


    <!-- http://www.w3.org/2004/02/skos/core#narrower -->

    <owl:ObjectProperty rdf:about="&skos;narrower">
        <rdfs:label xml:lang="en">has narrower</rdfs:label>
        <rdfs:isDefinedBy rdf:datatype="&xsd;anyURI"
            >http://www.w3.org/2004/02/skos/core</rdfs:isDefinedBy>
        <rdfs:comment xml:lang="en"
            >By convention, skos:broader is only used to assert an immediate
      (i.e. direct) hierarchical link between two conceptual resources.</rdfs:comment>
        <rdfs:comment xml:lang="en"
            >Narrower concepts are typically rendered as children in a concept
      hierarchy (tree).</rdfs:comment>
        <owl:inverseOf rdf:resource="&skos;broader"/>
        <rdfs:subPropertyOf rdf:resource="&skos;narrowerTransitive"/>
    </owl:ObjectProperty>
    


    <!-- http://www.w3.org/2004/02/skos/core#narrowerTransitive -->

    <owl:ObjectProperty rdf:about="&skos;narrowerTransitive">
        <rdf:type rdf:resource="&owl;TransitiveProperty"/>
        <rdfs:label xml:lang="en"
            >narrower transitive</rdfs:label>
        <rdfs:isDefinedBy rdf:datatype="&xsd;anyURI"
            >http://www.w3.org/2004/02/skos/core</rdfs:isDefinedBy>
        <rdfs:comment xml:lang="en"
            >By convention, skos:narrowerTransitive is not used to make
      assertions. Rather, the properties can be used to draw inferences about the transitive closure
      of the hierarchical relation, which is useful e.g. when implementing a simple query expansion
      algorithm in a search application.</rdfs:comment>
        <rdfs:subPropertyOf rdf:resource="&skos;semanticRelation"/>
    </owl:ObjectProperty>
    


    <!-- http://www.w3.org/2004/02/skos/core#notation -->

    <owl:ObjectProperty rdf:about="&skos;notation">
        <owl:subObjectPropertyOf rdf:resource="&owl;topDataProperty"/>
    </owl:ObjectProperty>
    


    <!-- http://www.w3.org/2004/02/skos/core#prefLabel -->

    <owl:ObjectProperty rdf:about="&skos;prefLabel">
        <owl:subObjectPropertyOf rdf:resource="&owl;topDataProperty"/>
    </owl:ObjectProperty>
    


    <!-- http://www.w3.org/2004/02/skos/core#related -->

    <owl:ObjectProperty rdf:about="&skos;related">
        <rdf:type rdf:resource="&owl;SymmetricProperty"/>
        <rdfs:label xml:lang="en">related to</rdfs:label>
        <rdfs:isDefinedBy rdf:datatype="&xsd;anyURI"
            >http://www.w3.org/2004/02/skos/core</rdfs:isDefinedBy>
        <rdfs:comment xml:lang="en"
            >skos:related is disjoint with skos:broaderTransitive</rdfs:comment>
        <owl:inverseOf rdf:resource="&skos;related"/>
        <rdfs:subPropertyOf rdf:resource="&skos;semanticRelation"/>
    </owl:ObjectProperty>
    


    <!-- http://www.w3.org/2004/02/skos/core#relatedMatch -->

    <owl:ObjectProperty rdf:about="&skos;relatedMatch">
        <rdf:type rdf:resource="&owl;SymmetricProperty"/>
        <rdfs:label xml:lang="en">related match</rdfs:label>
        <rdfs:isDefinedBy rdf:datatype="&xsd;anyURI"
            >http://www.w3.org/2004/02/skos/core</rdfs:isDefinedBy>
        <rdfs:subPropertyOf rdf:resource="&skos;mappingRelation"/>
        <rdfs:subPropertyOf rdf:resource="&skos;related"/>
        <owl:inverseOf rdf:resource="&skos;relatedMatch"/>
    </owl:ObjectProperty>
    


    <!-- http://www.w3.org/2004/02/skos/core#semanticRelation -->

    <owl:ObjectProperty rdf:about="&skos;semanticRelation">
        <rdfs:label xml:lang="en"
            >semantic relation</rdfs:label>
        <rdfs:isDefinedBy rdf:datatype="&xsd;anyURI"
            >http://www.w3.org/2004/02/skos/core</rdfs:isDefinedBy>
        <rdfs:comment xml:lang="en"
            >This property should not be used directly, but as a super-property
      for all properties denoting a relationship of meaning between concepts.</rdfs:comment>
        <rdfs:subPropertyOf rdf:resource="&owl;topObjectProperty"/>
        <rdfs:range rdf:resource="&skos;Concept"/>
        <rdfs:domain rdf:resource="&skos;Concept"/>
    </owl:ObjectProperty>
    


    <!-- http://www.w3.org/2004/02/skos/core#topConceptOf -->

    <owl:ObjectProperty rdf:about="&skos;topConceptOf">
        <rdf:type rdf:resource="&owl;AsymmetricProperty"/>
        <rdf:type rdf:resource="&owl;IrreflexiveProperty"/>
        <rdfs:label xml:lang="en"
            >top concept in scheme</rdfs:label>
        <rdfs:isDefinedBy rdf:datatype="&xsd;anyURI"
            >http://www.w3.org/2004/02/skos/core</rdfs:isDefinedBy>
        <owl:inverseOf rdf:resource="&skos;hasTopConcept"/>
        <rdfs:subPropertyOf rdf:resource="&skos;inScheme"/>
    </owl:ObjectProperty>
    


    <!-- 
    ///////////////////////////////////////////////////////////////////////////////////////
    //
    // Data properties
    //
    ///////////////////////////////////////////////////////////////////////////////////////
     -->

    


    <!-- http://www.w3.org/1999/02/22-rdf-syntax-ns#value -->

    <owl:DatatypeProperty rdf:about="&rdf;value"/>
    


    <!-- http://www.w3.org/2002/07/owl#topDataProperty -->

    <owl:DatatypeProperty rdf:about="&owl;topDataProperty"/>
    


    <!-- http://www.w3.org/2004/02/skos/core#changeNote -->

    <owl:DatatypeProperty rdf:about="&skos;changeNote"/>
    


    <!-- http://www.w3.org/2004/02/skos/core#definition -->

    <owl:DatatypeProperty rdf:about="&skos;definition"/>
    


    <!-- http://www.w3.org/2004/02/skos/core#historyNote -->

    <owl:DatatypeProperty rdf:about="&skos;historyNote">
        <rdf:type rdf:resource="&owl;AnnotationProperty"/>
    </owl:DatatypeProperty>
    


    <!-- http://www.w3.org/2004/02/skos/core#notation -->

    <owl:DatatypeProperty rdf:about="&skos;notation"/>
    


    <!-- http://www.w3.org/2004/02/skos/core#prefLabel -->

    <owl:DatatypeProperty rdf:about="&skos;prefLabel"/>
    


    <!-- 
    ///////////////////////////////////////////////////////////////////////////////////////
    //
    // Classes
    //
    ///////////////////////////////////////////////////////////////////////////////////////
     -->

    


    <!-- http://www.w3.org/2002/07/owl#Thing -->

    <owl:Class rdf:about="&owl;Thing"/>
    


    <!-- http://www.w3.org/2004/02/skos/core#Collection -->

    <owl:Class rdf:about="&skos;Collection">
        <rdfs:label xml:lang="en">Collection</rdfs:label>
        <rdfs:subClassOf rdf:resource="&owl;Thing"/>
        <owl:disjointWith rdf:resource="&skos;Concept"/>
        <owl:disjointWith rdf:resource="&skos;ConceptScheme"/>
        <rdfs:isDefinedBy rdf:datatype="&xsd;anyURI"
            >http://www.w3.org/2004/02/skos/core</rdfs:isDefinedBy>
        <rdfs:comment xml:lang="en"
            >Labelled collections can be used with collectable semantic relation
      properties e.g. skos:narrower, where you would like a set of concepts to be displayed under a
      &#39;node label&#39; in the hierarchy.</rdfs:comment>
    </owl:Class>
    


    <!-- http://www.w3.org/2004/02/skos/core#Concept -->

    <owl:Class rdf:about="&skos;Concept">
        <rdfs:label xml:lang="en">Concept</rdfs:label>
        <rdfs:subClassOf rdf:resource="&owl;Thing"/>
        <owl:disjointWith rdf:resource="&skos;ConceptScheme"/>
        <owl:disjointWith rdf:resource="&skos;OrderedCollection"/>
        <rdfs:isDefinedBy rdf:datatype="&xsd;anyURI"
            >http://www.w3.org/2004/02/skos/core</rdfs:isDefinedBy>
    </owl:Class>
    


    <!-- http://www.w3.org/2004/02/skos/core#ConceptScheme -->

    <owl:Class rdf:about="&skos;ConceptScheme">
        <rdfs:label xml:lang="en">Concept Scheme</rdfs:label>
        <rdfs:subClassOf rdf:resource="&owl;Thing"/>
        <owl:disjointWith rdf:resource="&skos;OrderedCollection"/>
        <rdfs:isDefinedBy rdf:datatype="&xsd;anyURI"
            >http://www.w3.org/2004/02/skos/core</rdfs:isDefinedBy>
        <rdfs:comment xml:lang="en"
            >A concept scheme may be defined to include concepts from different
      sources.</rdfs:comment>
        <rdfs:comment xml:lang="en"
            >Thesauri, classification schemes, subject heading lists, taxonomies,
      &#39;folksonomies&#39;, and other types of controlled vocabulary are all examples of concept schemes.
      Concept schemes are also embedded in glossaries and terminologies.</rdfs:comment>
    </owl:Class>
    


    <!-- http://www.w3.org/2004/02/skos/core#OrderedCollection -->

    <owl:Class rdf:about="&skos;OrderedCollection">
        <rdfs:label xml:lang="en"
            >Ordered Collection</rdfs:label>
        <rdfs:subClassOf rdf:resource="&skos;Collection"/>
        <rdfs:isDefinedBy rdf:datatype="&xsd;anyURI"
            >http://www.w3.org/2004/02/skos/core</rdfs:isDefinedBy>
        <rdfs:comment xml:lang="en"
            >Ordered collections can be used where you would like a set of concepts to be displayed in a specific order, and optionally under a &#39;node label&#39;.</rdfs:comment>
    </owl:Class>
    


    <!-- 
    ///////////////////////////////////////////////////////////////////////////////////////
    //
    // Individuals
    //
    ///////////////////////////////////////////////////////////////////////////////////////
     -->

    


    <!-- http://resource.geosciml.org/classifier/cgi/stratigraphicrank/0001 -->

    <skos:Concept rdf:about="http://resource.geosciml.org/classifier/cgi/stratigraphicrank/0001">
        <rdf:type rdf:resource="&owl;Thing"/>
        <skos:definition
            >The smallest formal lithostratigraphic unit, usually a distinctive lithic entity which can be distinguished from adjacent rocks by one or more physical characteristics.</skos:definition>
        <skos:prefLabel xml:lang="en">Bed</skos:prefLabel>
        <dc:source
            >North American Commission on Stratigraphic Nomenclature, 2005; Salvador, 1994</dc:source>
        <skos:broaderTransitive rdf:resource="http://resource.geosciml.org/classifier/cgi/stratigraphicrank/0003"/>
        <skos:broader rdf:resource="http://resource.geosciml.org/classifier/cgi/stratigraphicrank/0007"/>
        <skos:inScheme rdf:resource=""/>
    </skos:Concept>
    


    <!-- http://resource.geosciml.org/classifier/cgi/stratigraphicrank/0003 -->

    <skos:Concept rdf:about="http://resource.geosciml.org/classifier/cgi/stratigraphicrank/0003">
        <rdf:type rdf:resource="&owl;Thing"/>
        <dc:source
            >North American Commission on Stratigraphic Nomenclature, 2005; Salvador, 1994</dc:source>
        <skos:definition
            >A body of rock identified by lithic characteristics and stratigraphic position; it is usually but not necessarily tabular and is mappable at the Earth&#39;s surface or traceable in the subsurface.</skos:definition>
        <skos:definition
            >A body of rock identified by lithic characteristics and stratigraphic position; it is usually but not necessarily tabular and is mappable at the Earth\&#39;s surface or traceable in the subsurface.</skos:definition>
        <skos:prefLabel xml:lang="en">Formation</skos:prefLabel>
        <skos:narrowerTransitive rdf:resource="http://resource.geosciml.org/classifier/cgi/stratigraphicrank/0001"/>
        <skos:broader rdf:resource="http://resource.geosciml.org/classifier/cgi/stratigraphicrank/0004"/>
        <skos:related rdf:resource="http://resource.geosciml.org/classifier/cgi/stratigraphicrank/0005"/>
        <skos:narrower rdf:resource="http://resource.geosciml.org/classifier/cgi/stratigraphicrank/0007"/>
        <skos:broader rdf:resource="http://resource.geosciml.org/classifier/cgi/stratigraphicrank/0010"/>
        <skos:broaderTransitive rdf:resource="http://resource.geosciml.org/classifier/cgi/stratigraphicrank/0012"/>
        <skos:inScheme rdf:resource=""/>
    </skos:Concept>
    


    <!-- http://resource.geosciml.org/classifier/cgi/stratigraphicrank/0004 -->

    <owl:Thing rdf:about="http://resource.geosciml.org/classifier/cgi/stratigraphicrank/0004">
        <rdf:type rdf:resource="&skos;Concept"/>
        <skos:definition
            >A group is the lithostratigraphic unit next higher in rank to either subgroup or formation. A groups may consist of two or more subgroups or two or more formations or a combination of both.</skos:definition>
        <skos:prefLabel xml:lang="en">Group</skos:prefLabel>
        <dc:source
            >North American Commission on Stratigraphic Nomenclature, 2005;  Salvador, 1994</dc:source>
        <skos:narrower rdf:resource="http://resource.geosciml.org/classifier/cgi/stratigraphicrank/0003"/>
        <skos:narrower rdf:resource="http://resource.geosciml.org/classifier/cgi/stratigraphicrank/0010"/>
        <skos:related rdf:resource="http://resource.geosciml.org/classifier/cgi/stratigraphicrank/0011"/>
        <skos:broader rdf:resource="http://resource.geosciml.org/classifier/cgi/stratigraphicrank/0012"/>
        <skos:inScheme rdf:resource=""/>
    </owl:Thing>
    


    <!-- http://resource.geosciml.org/classifier/cgi/stratigraphicrank/0005 -->

    <owl:Thing rdf:about="http://resource.geosciml.org/classifier/cgi/stratigraphicrank/0005">
        <rdf:type rdf:resource="&skos;Concept"/>
        <dc:source
            >North American Commission on Stratigraphic Nomenclature, 2005</dc:source>
        <skos:definition
            >A body of predominantly intrusive, highly deformed and/or highly metamorphosed rock, distinguished and delimited on the basis of rock characteristics.</skos:definition>
        <skos:prefLabel xml:lang="en">Lithodeme</skos:prefLabel>
        <skos:related rdf:resource="http://resource.geosciml.org/classifier/cgi/stratigraphicrank/0003"/>
        <skos:related rdf:resource="http://resource.geosciml.org/classifier/cgi/stratigraphicrank/0009"/>
        <skos:broader rdf:resource="http://resource.geosciml.org/classifier/cgi/stratigraphicrank/0011"/>
        <skos:broaderTransitive rdf:resource="http://resource.geosciml.org/classifier/cgi/stratigraphicrank/0014"/>
        <skos:related rdf:resource="http://resource.geosciml.org/classifier/cgi/stratigraphicrank/0015"/>
        <skos:inScheme rdf:resource=""/>
    </owl:Thing>
    


    <!-- http://resource.geosciml.org/classifier/cgi/stratigraphicrank/0006 -->

    <skos:Concept rdf:about="http://resource.geosciml.org/classifier/cgi/stratigraphicrank/0006">
        <rdf:type rdf:resource="&owl;Thing"/>
        <skos:definition xml:lang="en"
            >A succession of strata comprising two or more supersequences. A large-scale sequence-stratigraphic unit deposited during one distinct phase of basin evolution, separated by major unconformities that mark a change in fundamental basin-controlling processes.</skos:definition>
        <dc:source xml:lang="en"
            >Haq, B.U., Hardenbol, J., and Vail, P.R., 1988, Mesozoic and Cenozoic chronostratigraphy an dcycles of sea-level changes, in Wilgus, C.K., et al., eds, Sea-level Changes: an Integrated Approach: Society of Sedimentary Geology Special Publication 42, p. 71-108.
Peel, F., Cole, Gary A, Apps, Gillian M., and Moore, M. G., 2002, Implications of Megasequence Stratigraphy for the Petroleum System of the Ultra Deep Water Gulf of Mexico [abstract], Gulf Coast Association of Geological Societies Meeting October 30 - November 1, 2002, Austin, Texas, accessed at http://www.searchanddiscovery.net/documents/abstracts/gcags/images/peel01.htm, 2011-02-17</dc:source>
        <skos:prefLabel xml:lang="en">Megasequence</skos:prefLabel>
        <rdfs:seeAlso
            >http://www.sepmstrata.org/terminology/seq-strat.html; http://sepmstrata.org/terminology/second-order-cyc.html;
Heward, A.P., 1978, Alluvial fan sequence and megasequence models: With examples from Westphalian D-Stephanian B coal-fields, northern Spain, in A.D. Miall, ed., fluvial sedimentation: Canadian Society of Petroleum Geologists Memoir 5, p. 59-76.</rdfs:seeAlso>
        <skos:narrowerTransitive rdf:resource="http://resource.geosciml.org/classifier/cgi/stratigraphicrank/0009"/>
        <skos:narrower rdf:resource="http://resource.geosciml.org/classifier/cgi/stratigraphicrank/0013"/>
        <skos:related rdf:resource="http://resource.geosciml.org/classifier/cgi/stratigraphicrank/0014"/>
        <skos:inScheme rdf:resource=""/>
        <skos:topConceptOf rdf:resource=""/>
    </skos:Concept>
    


    <!-- http://resource.geosciml.org/classifier/cgi/stratigraphicrank/0007 -->

    <owl:Thing rdf:about="http://resource.geosciml.org/classifier/cgi/stratigraphicrank/0007">
        <rdf:type rdf:resource="&skos;Concept"/>
        <skos:definition
            >A formal lithostratigraphic unit next in rank below a formation, and always part of a formation. It is a named entity within a formation because it possesses characteristics distinguishing it from adjacent parts of the formation.</skos:definition>
        <skos:prefLabel xml:lang="en">Member</skos:prefLabel>
        <dc:source
            >North American Commission on Stratigraphic Nomenclature, 2005; Salvador, 1994</dc:source>
        <skos:narrower rdf:resource="http://resource.geosciml.org/classifier/cgi/stratigraphicrank/0001"/>
        <skos:broader rdf:resource="http://resource.geosciml.org/classifier/cgi/stratigraphicrank/0003"/>
        <skos:inScheme rdf:resource=""/>
    </owl:Thing>
    


    <!-- http://resource.geosciml.org/classifier/cgi/stratigraphicrank/0008 -->

    <owl:Thing rdf:about="http://resource.geosciml.org/classifier/cgi/stratigraphicrank/0008">
        <rdf:type rdf:resource="&skos;Concept"/>
        <skos:prefLabel xml:lang="en">Not specified</skos:prefLabel>
        <dc:source xml:lang="en">this vocabulary</dc:source>
        <skos:definition
            >unit is not part of a defined stratigraphic hierarchy.</skos:definition>
        <skos:inScheme rdf:resource=""/>
        <skos:topConceptOf rdf:resource=""/>
    </owl:Thing>
    


    <!-- http://resource.geosciml.org/classifier/cgi/stratigraphicrank/0009 -->

    <owl:Thing rdf:about="http://resource.geosciml.org/classifier/cgi/stratigraphicrank/0009">
        <rdf:type rdf:resource="&skos;Concept"/>
        <skos:notation rdf:datatype="&cgi;stratigraphicrank">sequence</skos:notation>
        <skos:definition xml:lang="en"
            >A genetically related succession of strata bounded by unconformites or their correlative conformable contacts, and typically having a thickness of 10-100 metres.</skos:definition>
        <skos:prefLabel xml:lang="en">Sequence</skos:prefLabel>
        <dc:source xml:lang="en"
            >Van Wagoner, J.C., Posamentier, H.W., Mitchum, R.M., Vail, P.R., Sarg, J.F., Loutit, T.S., Hardenbol, J., 1988, An overview of sequence stratigraphy and key definitions. In: Wilgus, C.K., Hastings, B.S., Kendall, C.G.St.C., Posamentier, H.W., Ross, C.A., Van Wagoner, J.C. (Eds.), Sea Level Changes&#8211;&#8211;An Integrated Approach, vol. 42. SEPM Special Publication, pp. 39&#8211;45.</dc:source>
        <rdfs:seeAlso
            >http://www.sepmstrata.org/terminology/seq-strat.html</rdfs:seeAlso>
        <skos:related rdf:resource="http://resource.geosciml.org/classifier/cgi/stratigraphicrank/0005"/>
        <skos:broaderTransitive rdf:resource="http://resource.geosciml.org/classifier/cgi/stratigraphicrank/0006"/>
        <skos:broader rdf:resource="http://resource.geosciml.org/classifier/cgi/stratigraphicrank/0013"/>
        <skos:inScheme rdf:resource=""/>
    </owl:Thing>
    


    <!-- http://resource.geosciml.org/classifier/cgi/stratigraphicrank/0010 -->

    <skos:Concept rdf:about="http://resource.geosciml.org/classifier/cgi/stratigraphicrank/0010">
        <rdf:type rdf:resource="&owl;Thing"/>
        <skos:definition
            >A subgroup is the lithostratigraphic unit next higher in rank to formation. A subgroup usually consists of several formations.</skos:definition>
        <dc:source xml:lang="en">Salvador, 1994</dc:source>
        <skos:prefLabel xml:lang="en">Subgroup</skos:prefLabel>
        <skos:narrower rdf:resource="http://resource.geosciml.org/classifier/cgi/stratigraphicrank/0003"/>
        <skos:broader rdf:resource="http://resource.geosciml.org/classifier/cgi/stratigraphicrank/0004"/>
        <skos:broaderTransitive rdf:resource="http://resource.geosciml.org/classifier/cgi/stratigraphicrank/0012"/>
        <skos:inScheme rdf:resource=""/>
    </skos:Concept>
    


    <!-- http://resource.geosciml.org/classifier/cgi/stratigraphicrank/0011 -->

    <owl:Thing rdf:about="http://resource.geosciml.org/classifier/cgi/stratigraphicrank/0011">
        <rdf:type rdf:resource="&skos;Concept"/>
        <dc:source
            >North American Commission on Stratigraphic Nomenclature, 2005</dc:source>
        <skos:definition
            >A formal lithodemic unit next higher in rank to lithodeme. It comprises two or more associated lithodemes of the same class (e.g., plutonic, metamorphic).</skos:definition>
        <skos:prefLabel xml:lang="en">Suite</skos:prefLabel>
        <skos:related rdf:resource="http://resource.geosciml.org/classifier/cgi/stratigraphicrank/0004"/>
        <skos:narrower rdf:resource="http://resource.geosciml.org/classifier/cgi/stratigraphicrank/0005"/>
        <skos:related rdf:resource="http://resource.geosciml.org/classifier/cgi/stratigraphicrank/0013"/>
        <skos:broader rdf:resource="http://resource.geosciml.org/classifier/cgi/stratigraphicrank/0014"/>
        <skos:inScheme rdf:resource=""/>
    </owl:Thing>
    


    <!-- http://resource.geosciml.org/classifier/cgi/stratigraphicrank/0012 -->

    <owl:Thing rdf:about="http://resource.geosciml.org/classifier/cgi/stratigraphicrank/0012">
        <rdf:type rdf:resource="&skos;Concept"/>
        <dc:source
            >North American Commission on Stratigraphic Nomenclature, 2005; Salvador, 1994</dc:source>
        <skos:definition
            >A supergroup is a formal assemblage of related or superposed groups or of groups and formations</skos:definition>
        <skos:prefLabel xml:lang="en">Supergroup</skos:prefLabel>
        <skos:narrowerTransitive rdf:resource="http://resource.geosciml.org/classifier/cgi/stratigraphicrank/0003"/>
        <skos:narrower rdf:resource="http://resource.geosciml.org/classifier/cgi/stratigraphicrank/0004"/>
        <skos:narrowerTransitive rdf:resource="http://resource.geosciml.org/classifier/cgi/stratigraphicrank/0010"/>
        <skos:related rdf:resource="http://resource.geosciml.org/classifier/cgi/stratigraphicrank/0014"/>
        <skos:topConceptOf rdf:resource=""/>
        <skos:inScheme rdf:resource=""/>
    </owl:Thing>
    


    <!-- http://resource.geosciml.org/classifier/cgi/stratigraphicrank/0013 -->

    <owl:Thing rdf:about="http://resource.geosciml.org/classifier/cgi/stratigraphicrank/0013">
        <rdf:type rdf:resource="&skos;Concept"/>
        <skos:definition
            >A succession of strata comprising two or more sequences</skos:definition>
        <dc:source
            >Haq, B.U., Hardenbol, J., and Vail, P.R., 1988, Mesozoic and Cenozoic chronostratigraphy an dcycles of sea-level changes, in Wilgus, C.K., et al., eds, Sea-level Changes: an Integrated Approach: Society of Sedimentary Geology Special Publication 42, p. 71-108.</dc:source>
        <skos:prefLabel xml:lang="en">Supersequence</skos:prefLabel>
        <rdfs:seeAlso
            >http://www.sepmstrata.org/terminology/seq-strat.html</rdfs:seeAlso>
        <skos:broader rdf:resource="http://resource.geosciml.org/classifier/cgi/stratigraphicrank/0006"/>
        <skos:narrower rdf:resource="http://resource.geosciml.org/classifier/cgi/stratigraphicrank/0009"/>
        <skos:related rdf:resource="http://resource.geosciml.org/classifier/cgi/stratigraphicrank/0011"/>
        <skos:inScheme rdf:resource=""/>
    </owl:Thing>
    


    <!-- http://resource.geosciml.org/classifier/cgi/stratigraphicrank/0014 -->

    <skos:Concept rdf:about="http://resource.geosciml.org/classifier/cgi/stratigraphicrank/0014">
        <rdf:type rdf:resource="&owl;Thing"/>
        <skos:definition
            >A formal lithodemic unit next higher in rank to suite. It comprises two or more suites having a degree of natural relationship to one another</skos:definition>
        <dc:source
            >North American Commission on Stratigraphic Nomenclature, 2005</dc:source>
        <skos:prefLabel xml:lang="en">Supersuite</skos:prefLabel>
        <skos:narrowerTransitive rdf:resource="http://resource.geosciml.org/classifier/cgi/stratigraphicrank/0005"/>
        <skos:related rdf:resource="http://resource.geosciml.org/classifier/cgi/stratigraphicrank/0006"/>
        <skos:narrower rdf:resource="http://resource.geosciml.org/classifier/cgi/stratigraphicrank/0011"/>
        <skos:related rdf:resource="http://resource.geosciml.org/classifier/cgi/stratigraphicrank/0012"/>
        <skos:topConceptOf rdf:resource=""/>
        <skos:inScheme rdf:resource=""/>
    </skos:Concept>
    


    <!-- http://resource.geosciml.org/classifier/cgi/stratigraphicrank/0015 -->

    <skos:Concept rdf:about="http://resource.geosciml.org/classifier/cgi/stratigraphicrank/0015">
        <rdf:type rdf:resource="&owl;Thing"/>
        <dc:source
            >Salvador, A., ed. 1994. International Stratigraphic Guide: International Union of Geological Sciences, Trondheim, NO, 214 p.</dc:source>
        <skos:definition xml:lang="en"
            >A lithostratigraphic unit composed of diverse types of any class or classes of rock (sedimentary, igneous, metamorphic), and characterized by irregularly mixed lithology or by hightly complicated structure relations to the extent that the original sequence of the component rocks may be obscured and the individual rocks or rock sequence cannot be readily mapped.</skos:definition>
        <skos:prefLabel xml:lang="en">Complex</skos:prefLabel>
        <skos:related rdf:resource="http://resource.geosciml.org/classifier/cgi/stratigraphicrank/0005"/>
        <skos:inScheme rdf:resource=""/>
        <skos:topConceptOf rdf:resource=""/>
    </skos:Concept>
    


    <!-- http://resource.geosciml.org/classifierscheme/cgi/201012/stratigraphicrank -->

    <owl:Thing rdf:about="">
        <rdf:type rdf:resource="&skos;ConceptScheme"/>
        <skos:changeNote xml:lang="en"
            >2009-12-07 SMR Update metadata properties for version, creator, title, and format.  Change skos:HistoryNote to dc:source for information on origin of terms and definitions.</skos:changeNote>
        <skos:prefLabel xml:lang="en"
            >CGI Stratigraphic rank vocabulary</skos:prefLabel>
        <skos:definition xml:lang="en"
            >This file contains the CGI StratigraphicRank vocabulary. This vocabulary contains categories used to classify geologic units in a generalization hierarchy from most local/smallest volume to most regional. Examples: group, subgroup, formation, member. No parent links because relation between e.g. formation and group is not &#39;is a&#39; it is &#39;part of&#39;. All formations are not groups, and a formation is not necessarily part of a group, therefore group is not a broader term than formation.</skos:definition>
        <skos:hasTopConcept rdf:resource="http://resource.geosciml.org/classifier/cgi/stratigraphicrank/0006"/>
        <skos:hasTopConcept rdf:resource="http://resource.geosciml.org/classifier/cgi/stratigraphicrank/0008"/>
        <skos:hasTopConcept rdf:resource="http://resource.geosciml.org/classifier/cgi/stratigraphicrank/0012"/>
        <skos:hasTopConcept rdf:resource="http://resource.geosciml.org/classifier/cgi/stratigraphicrank/0014"/>
        <skos:hasTopConcept rdf:resource="http://resource.geosciml.org/classifier/cgi/stratigraphicrank/0015"/>
    </owl:Thing>
    


    <!-- http://www.w3.org/2004/02/skos/core#Collection -->

    <owl:Thing rdf:about="&skos;Collection">
        <skos:definition xml:lang="en"
            >A meaningful collection of concepts.</skos:definition>
    </owl:Thing>
    


    <!-- http://www.w3.org/2004/02/skos/core#Concept -->

    <owl:Thing rdf:about="&skos;Concept">
        <skos:definition xml:lang="en"
            >An abstract idea or notion; a unit of thought.</skos:definition>
    </owl:Thing>
    


    <!-- http://www.w3.org/2004/02/skos/core#ConceptScheme -->

    <owl:Thing rdf:about="&skos;ConceptScheme">
        <skos:definition xml:lang="en"
            >A set of concepts, optionally including statements about semantic
      relationships between those concepts.</skos:definition>
        <skos:definition xml:lang="en"
            >A set of concepts, optionally including statements about semantic\n      relationships between those concepts.</skos:definition>
    </owl:Thing>
    


    <!-- http://www.w3.org/2004/02/skos/core#OrderedCollection -->

    <owl:Thing rdf:about="&skos;OrderedCollection">
        <skos:definition xml:lang="en"
            >An ordered collection of concepts, where both the grouping and
      the ordering are meaningful.</skos:definition>
        <skos:definition xml:lang="en"
            >An ordered collection of concepts, where both the grouping and\n      the ordering are meaningful.</skos:definition>
    </owl:Thing>
    


    <!-- http://www.w3.org/2004/02/skos/core#altLabel -->

    <owl:Thing rdf:about="&skos;altLabel">
        <skos:definition xml:lang="en"
            >An alternative lexical label for a resource.</skos:definition>
    </owl:Thing>
    


    <!-- http://www.w3.org/2004/02/skos/core#broadMatch -->

    <owl:Thing rdf:about="&skos;broadMatch">
        <skos:definition xml:lang="en"
            >skos:broadMatch is used to state a hierarchical mapping link
      between two conceptual resources in different concept schemes.</skos:definition>
        <skos:definition xml:lang="en"
            >skos:broadMatch is used to state a hierarchical mapping link\n      between two conceptual resources in different concept schemes.</skos:definition>
    </owl:Thing>
    


    <!-- http://www.w3.org/2004/02/skos/core#broader -->

    <owl:Thing rdf:about="&skos;broader">
        <skos:definition xml:lang="en"
            >A concept that is more general in meaning.</skos:definition>
    </owl:Thing>
    


    <!-- http://www.w3.org/2004/02/skos/core#broaderTransitive -->

    <owl:Thing rdf:about="&skos;broaderTransitive">
        <skos:definition
            >skos:broaderTransitive is a transitive superproperty of skos:broader.</skos:definition>
    </owl:Thing>
    


    <!-- http://www.w3.org/2004/02/skos/core#changeNote -->

    <owl:Thing rdf:about="&skos;changeNote">
        <skos:definition xml:lang="en"
            >A note about a modification to a concept.</skos:definition>
    </owl:Thing>
    


    <!-- http://www.w3.org/2004/02/skos/core#closeMatch -->

    <owl:Thing rdf:about="&skos;closeMatch">
        <skos:definition xml:lang="en"
            >skos:closeMatch is used to link two concepts that are
      sufficiently similar that they can be used interchangeably in some information retrieval
      applications. In order to avoid the possibility of &quot;compound errors&quot; when combining mappings
      across more than two concept schemes, skos:closeMatch is not declared to be a transitive
      property.</skos:definition>
        <skos:definition xml:lang="en"
            >skos:closeMatch is used to link two concepts that are\n      sufficiently similar that they can be used interchangeably in some information retrieval\n      applications. In order to avoid the possibility of \&quot;compound errors\&quot; when combining mappings\n      across more than two concept schemes, skos:closeMatch is not declared to be a transitive\n      property.</skos:definition>
    </owl:Thing>
    


    <!-- http://www.w3.org/2004/02/skos/core#definition -->

    <owl:Thing rdf:about="&skos;definition">
        <rdf:type rdf:resource="&owl;DatatypeProperty"/>
        <rdfs:label xml:lang="en">definition</rdfs:label>
        <rdfs:isDefinedBy rdf:datatype="&xsd;anyURI"
            >http://www.w3.org/2004/02/skos/core</rdfs:isDefinedBy>
        <skos:definition xml:lang="en"
            >A statement or formal explanation of the meaning of a concept.</skos:definition>
    </owl:Thing>
    


    <!-- http://www.w3.org/2004/02/skos/core#editorialNote -->

    <owl:Thing rdf:about="&skos;editorialNote">
        <skos:definition xml:lang="en"
            >A note for an editor, translator or maintainer of the vocabulary.</skos:definition>
    </owl:Thing>
    


    <!-- http://www.w3.org/2004/02/skos/core#exactMatch -->

    <owl:Thing rdf:about="&skos;exactMatch">
        <skos:definition xml:lang="en"
            >skos:exactMatch is used to link two concepts, indicating a high
      degree of confidence that the concepts can be used interchangeably across a wide range of
      information retrieval applications. skos:exactMatch is a transitive property, and is a
      sub-property of skos:closeMatch.</skos:definition>
        <skos:definition xml:lang="en"
            >skos:exactMatch is used to link two concepts, indicating a high\n      degree of confidence that the concepts can be used interchangeably across a wide range of\n      information retrieval applications. skos:exactMatch is a transitive property, and is a\n      sub-property of skos:closeMatch.</skos:definition>
    </owl:Thing>
    


    <!-- http://www.w3.org/2004/02/skos/core#example -->

    <owl:Thing rdf:about="&skos;example">
        <skos:definition xml:lang="en"
            >An example of the use of a concept.</skos:definition>
    </owl:Thing>
    


    <!-- http://www.w3.org/2004/02/skos/core#hasTopConcept -->

    <owl:Thing rdf:about="&skos;hasTopConcept">
        <skos:definition xml:lang="en"
            >A top level concept in the concept scheme.</skos:definition>
    </owl:Thing>
    


    <!-- http://www.w3.org/2004/02/skos/core#hiddenLabel -->

    <owl:Thing rdf:about="&skos;hiddenLabel">
        <skos:definition xml:lang="en"
            >A lexical label for a resource that should be hidden when
      generating visual displays of the resource, but should still be accessible to free text search
      operations.</skos:definition>
        <skos:definition xml:lang="en"
            >A lexical label for a resource that should be hidden when\n      generating visual displays of the resource, but should still be accessible to free text search\n      operations.</skos:definition>
    </owl:Thing>
    


    <!-- http://www.w3.org/2004/02/skos/core#historyNote -->

    <owl:Thing rdf:about="&skos;historyNote">
        <skos:definition xml:lang="en"
            >A note about the past state/use/meaning of a concept.</skos:definition>
    </owl:Thing>
    


    <!-- http://www.w3.org/2004/02/skos/core#inScheme -->

    <owl:Thing rdf:about="&skos;inScheme">
        <skos:definition xml:lang="en"
            >A concept scheme in which the concept is included.</skos:definition>
    </owl:Thing>
    


    <!-- http://www.w3.org/2004/02/skos/core#mappingRelation -->

    <owl:Thing rdf:about="&skos;mappingRelation">
        <skos:definition xml:lang="en">Definition</skos:definition>
    </owl:Thing>
    


    <!-- http://www.w3.org/2004/02/skos/core#member -->

    <owl:Thing rdf:about="&skos;member">
        <skos:definition xml:lang="en"
            >A member of a collection.</skos:definition>
    </owl:Thing>
    


    <!-- http://www.w3.org/2004/02/skos/core#memberList -->

    <owl:Thing rdf:about="&skos;memberList">
        <skos:definition xml:lang="en"
            >An RDF list containing the members of an ordered collection.</skos:definition>
    </owl:Thing>
    


    <!-- http://www.w3.org/2004/02/skos/core#narrowMatch -->

    <owl:Thing rdf:about="&skos;narrowMatch">
        <skos:definition xml:lang="en"
            >skos:narrowMatch is used to state a hierarchical mapping link
      between two conceptual resources in different concept schemes.</skos:definition>
        <skos:definition xml:lang="en"
            >skos:narrowMatch is used to state a hierarchical mapping link\n      between two conceptual resources in different concept schemes.</skos:definition>
    </owl:Thing>
    


    <!-- http://www.w3.org/2004/02/skos/core#narrower -->

    <owl:Thing rdf:about="&skos;narrower">
        <skos:definition xml:lang="en"
            >A concept that is more specific in meaning.</skos:definition>
    </owl:Thing>
    


    <!-- http://www.w3.org/2004/02/skos/core#narrowerTransitive -->

    <owl:Thing rdf:about="&skos;narrowerTransitive">
        <skos:definition
            >skos:narrowerTransitive is a transitive superproperty of skos:broader. By\n      convention, skos:narrowerTransitive is not intended to be used in assertions, but provides a\n      mechanism whereby the transitive closure of skos:narrower can be queried.</skos:definition>
        <skos:definition
            >skos:narrowerTransitive is a transitive superproperty of skos:broader. By
      convention, skos:narrowerTransitive is not intended to be used in assertions, but provides a
      mechanism whereby the transitive closure of skos:narrower can be queried.</skos:definition>
    </owl:Thing>
    


    <!-- http://www.w3.org/2004/02/skos/core#notation -->

    <owl:Thing rdf:about="&skos;notation">
        <rdfs:label xml:lang="en">notation</rdfs:label>
        <rdfs:isDefinedBy rdf:datatype="&xsd;anyURI"
            >http://www.w3.org/2004/02/skos/core</rdfs:isDefinedBy>
        <skos:definition xml:lang="en"
            >A notation, also known as classification code, is a string of
      characters such as &quot;T58.5&quot; or &quot;303.4833&quot; used to uniquely identify a concept within the scope
      of a given concept scheme.</skos:definition>
        <skos:definition xml:lang="en"
            >A notation, also known as classification code, is a string of\n      characters such as \&quot;T58.5\&quot; or \&quot;303.4833\&quot; used to uniquely identify a concept within the scope\n      of a given concept scheme.</skos:definition>
        <rdfs:comment xml:lang="en"
            >By convention, skos:notation is used with a typed literal in the
      object position of the triple.</rdfs:comment>
    </owl:Thing>
    


    <!-- http://www.w3.org/2004/02/skos/core#note -->

    <owl:Thing rdf:about="&skos;note">
        <skos:definition xml:lang="en"
            >A general note, for any purpose.</skos:definition>
    </owl:Thing>
    


    <!-- http://www.w3.org/2004/02/skos/core#prefLabel -->

    <owl:Thing rdf:about="&skos;prefLabel">
        <skos:definition xml:lang="en"
            >The preferred lexical label for a resource, in a given language.</skos:definition>
    </owl:Thing>
    


    <!-- http://www.w3.org/2004/02/skos/core#related -->

    <owl:Thing rdf:about="&skos;related">
        <skos:definition xml:lang="en"
            >A concept with which there is an associative semantic
      relationship.</skos:definition>
        <skos:definition xml:lang="en"
            >A concept with which there is an associative semantic\n      relationship.</skos:definition>
    </owl:Thing>
    


    <!-- http://www.w3.org/2004/02/skos/core#relatedMatch -->

    <owl:Thing rdf:about="&skos;relatedMatch">
        <skos:definition xml:lang="en"
            >skos:relatedMatch is used to state an associative mapping link
      between two conceptual resources in different concept schemes.</skos:definition>
        <skos:definition xml:lang="en"
            >skos:relatedMatch is used to state an associative mapping link\n      between two conceptual resources in different concept schemes.</skos:definition>
    </owl:Thing>
    


    <!-- http://www.w3.org/2004/02/skos/core#scopeNote -->

    <owl:Thing rdf:about="&skos;scopeNote">
        <skos:definition xml:lang="en"
            >A note that helps to clarify the meaning of a concept.</skos:definition>
    </owl:Thing>
    


    <!-- http://www.w3.org/2004/02/skos/core#semanticRelation -->

    <owl:Thing rdf:about="&skos;semanticRelation">
        <skos:definition xml:lang="en"
            >A concept related by meaning.</skos:definition>
    </owl:Thing>
    


    <!-- http://www.w3.org/2004/02/skos/core#topConceptOf -->

    <owl:Thing rdf:about="&skos;topConceptOf">
        <skos:definition xml:lang="en"
            >Relates a concept to the concept scheme in which it is a top level concept.</skos:definition>
    </owl:Thing>
</rdf:RDF>



<!-- Generated by the OWL API (version 2.2.1.1138) http://owlapi.sourceforge.net -->

