<?xml version="1.0" encoding="UTF-8"?>
<rdf:RDF xmlns:rdf="http://www.w3.org/1999/02/22-rdf-syntax-ns#" xmlns:xlink="http://www.w3.org/1999/xlink" xmlns:skos="http://www.w3.org/2004/02/skos/core#" xmlns:dc="http://purl.org/dc/elements/1.1/" xmlns:dcterms="http://purl.org/dc/terms/" xmlns:rdfs="http://www.w3.org/2000/01/rdf-schema#" xmlns:owl="http://www.w3.org/2002/07/owl#">
   <skos:ConceptScheme rdf:about="http://resource.geosciml.org/classifierscheme/cgi/2016.01/deformationstyle">
      <dcterms:title xml:lang="en">Deformation Style</dcterms:title>
      <dcterms:description xml:lang="en">This scheme specifies concepts used to describe the Deformation Style of a fault or shear, as defined by the IUGS Commission for Geoscience Information (CGI) Geoscience Terminology Working Group. By extension, it includes all concepts in this conceptScheme, as well as concepts in any previous versions of the scheme. Designed for use in the deformationStyle property in GeoSciML ShearDisplacementStructureDescription elements.</dcterms:description>
      <skos:editorialNote xml:lang="en">This file contains the 2016 SKOS-RDF version of the CGI Deformation Style vocabulary. Compilation and review in MS Excel spreadsheet, converted to MS Excel for SKOS generation using GSML_SKOS_fromXLS_2016.01.xslt.</skos:editorialNote>
      <skos:changeNote xml:lang="en">Created 2012-04 by S.M. Richard</skos:changeNote>
      <skos:changeNote xml:lang="en">2012-11-24 SMR Update to 201211 version; add collection entity, check all pref labels are lower case, remove owl:NamedIndividual and Owl:Thing rdf:types.</skos:changeNote>
      <skos:changeNote xml:lang="en">2016-06-15 OLR - reformat Excel spreadsheet to work with XSLT, to make consistent SKOS-RDF with all CGI vocabularies. No change to 2012-11 concepts. Generate new SKOS-RDF file.</skos:changeNote>
      <dcterms:date>2016-06-22</dcterms:date>
      <dcterms:creator>CGI Geoscience Terminology Working Group</dcterms:creator>
   </skos:ConceptScheme>
   <skos:ConceptScheme rdf:about="http://resource.geosciml.org/classifierscheme/cgi/2016.01/deformationstyle">
      <skos:hasTopConcept rdf:resource="http://resource.geosciml.org/classifier/cgi/deformationstyle/mixed_brittle_ductile"/>
   </skos:ConceptScheme>
   <skos:Concept rdf:about="http://resource.geosciml.org/classifier/cgi/deformationstyle/mixed_brittle_ductile">
      <skos:inScheme rdf:resource="http://resource.geosciml.org/classifierscheme/cgi/2016.01/deformationstyle"/>
      <skos:definition xml:lang="en">Deformation in fault zone has been accommodated by both fracturing and plastic shape change in rock bodies.</skos:definition>
      <skos:prefLabel xml:lang="en">mixed brittle and ductile</skos:prefLabel>
      <skos:topConceptOf rdf:resource="http://resource.geosciml.org/classifierscheme/cgi/2016.01/deformationstyle"/>
      <dcterms:source xml:lang="en">this vocabulary</dcterms:source>
   </skos:Concept>
   <skos:ConceptScheme rdf:about="http://resource.geosciml.org/classifierscheme/cgi/2016.01/deformationstyle">
      <skos:hasTopConcept rdf:resource="http://resource.geosciml.org/classifier/cgi/deformationstyle/brittle"/>
   </skos:ConceptScheme>
   <skos:Concept rdf:about="http://resource.geosciml.org/classifier/cgi/deformationstyle/brittle">
      <skos:inScheme rdf:resource="http://resource.geosciml.org/classifierscheme/cgi/2016.01/deformationstyle"/>
      <skos:definition xml:lang="en">Deformation in fault zone has been accommodated primarily through fracturing and loss of continuity between adjacent rock bodies.</skos:definition>
      <skos:prefLabel xml:lang="en">brittle deformation</skos:prefLabel>
      <skos:topConceptOf rdf:resource="http://resource.geosciml.org/classifierscheme/cgi/2016.01/deformationstyle"/>
      <dcterms:source xml:lang="en">this vocabulary</dcterms:source>
   </skos:Concept>
   <skos:ConceptScheme rdf:about="http://resource.geosciml.org/classifierscheme/cgi/2016.01/deformationstyle">
      <skos:hasTopConcept rdf:resource="http://resource.geosciml.org/classifier/cgi/deformationstyle/ductile"/>
   </skos:ConceptScheme>
   <skos:Concept rdf:about="http://resource.geosciml.org/classifier/cgi/deformationstyle/ductile">
      <skos:inScheme rdf:resource="http://resource.geosciml.org/classifierscheme/cgi/2016.01/deformationstyle"/>
      <skos:definition xml:lang="en">Displacement across shear displacement structure largely accommodated by plastic deformation of the rock body without loss of macroscopic continuity.</skos:definition>
      <skos:prefLabel xml:lang="en">ductile deformation</skos:prefLabel>
      <skos:topConceptOf rdf:resource="http://resource.geosciml.org/classifierscheme/cgi/2016.01/deformationstyle"/>
      <dcterms:source xml:lang="en">this vocabulary</dcterms:source>
   </skos:Concept>
   <skos:Collection rdf:about="http://resource.geosciml.org/classifier/cgi/deformationstyle">
      <dcterms:title xml:lang="en">Deformation Style - All Concepts</dcterms:title>
      <skos:member><skos:Concept rdf:about="http://resource.geosciml.org/classifier/cgi/deformationstyle/mixed_brittle_ductile"/></skos:member>
      <skos:member><skos:Concept rdf:about="http://resource.geosciml.org/classifier/cgi/deformationstyle/brittle"/></skos:member>
      <skos:member><skos:Concept rdf:about="http://resource.geosciml.org/classifier/cgi/deformationstyle/ductile"/></skos:member>
   </skos:Collection>
   
</rdf:RDF>