<?xml version="1.0"?>
<rdf:RDF
    xmlns:rdf="http://www.w3.org/1999/02/22-rdf-syntax-ns#"
    xmlns:skos="http://www.w3.org/2004/02/skos/core#"
    xmlns:owl="http://www.w3.org/2002/07/owl#"
    xmlns:dc="http://purl.org/dc/elements/1.1/"
    xmlns:xsd="http://www.w3.org/2001/XMLSchema#"
    xmlns:rdfs="http://www.w3.org/2000/01/rdf-schema#"
  xml:base="http://resource.geosciml.org/classifierscheme/cgi/201401/earth-resource-expression">
  <owl:Ontology rdf:about="http://resource.geosciml.org/static/vocabulary/earthresourceml/2014/EarthResourceExpression.rdf">
    <owl:imports rdf:resource="http://www.w3.org/2004/02/skos/core"/>
    <owl:imports rdf:resource="http://purl.org/dc/elements/1.1/"/>
    <skos:editorialNote>This file contains the 201401 version of CGI Earth Resource Expression Value Vocabulary, which defines concepts for specifying the kinds of surface expression associated with an EarthResource. </skos:editorialNote>
    <skos:changeNote>Vocabulary Shepherd: Rachel Heaven/Tim McCormick. Compilation and review in Google doc spreadsheet, converted to MS Excel XML for SKOS generation using GSML_SKOS_from_XLS_2013.xslt; Conversion to SKOS by SM Richard. 2014-02-23 </skos:changeNote>
    <skos:changeNote>Edits to fix typos and remove '201401' from rdf file name. Ollie Raymond 8-Jan-2015</skos:changeNote>
    <dc:creator>CGI Geoscience Terminology Working Group</dc:creator>
    <dc:date>2014-01-09T00:00:00.000</dc:date>
  </owl:Ontology>
  <skos:ConceptScheme rdf:about="http://resource.geosciml.org/classifierscheme/cgi/201401/earth-resource-expression">
    <skos:definition xml:lang="en">This resource defines the concept space for EarthResource Expression vocabulary concepts by extension; it includes all concepts in this conceptScheme, as well as concepts in previous versions of the scheme.</skos:definition>  
    <skos:prefLabel xml:lang="en">EarthResource Expression vocabulary</skos:prefLabel>
    <dc:creator xml:lang="en">CGI Geoscience Terminology Working Group</dc:creator>
  </skos:ConceptScheme>
  <skos:Collection rdf:about="http://resource.geosciml.org/classifier/cgi/earth-resource-expression/">
    <skos:member>
      <skos:Concept rdf:about="http://resource.geosciml.org/classifier/cgi/earth-resource-expression/geophysical-anomaly">
        <dc:source xml:lang="en">Government Geoscience Information Committee (GGIC), Geoscience Australia</dc:source>
        <skos:notation rdf:datatype="gtwg:LocalHierarchyKey">04..</skos:notation>
        <skos:topConceptOf rdf:resource="http://resource.geosciml.org/classifierscheme/cgi/201401/earth-resource-expression"/>
        <skos:prefLabel xml:lang="en">geophysical anomaly</skos:prefLabel>
        <skos:inScheme rdf:resource="http://resource.geosciml.org/classifierscheme/cgi/201401/earth-resource-expression"/>
        <skos:definition xml:lang="en">The Earth resource, concealed or exposed, has an anomalous geophysical signature.</skos:definition>
      </skos:Concept>
    </skos:member>
    <skos:member>
      <skos:Concept rdf:about="http://resource.geosciml.org/classifier/cgi/earth-resource-expression/botanical-anomaly">
        <dc:source xml:lang="en">Government Geoscience Information Committee (GGIC), Geoscience Australia</dc:source>
        <skos:notation rdf:datatype="gtwg:LocalHierarchyKey">06..</skos:notation>
        <skos:topConceptOf rdf:resource="http://resource.geosciml.org/classifierscheme/cgi/201401/earth-resource-expression"/>
        <skos:altLabel xml:lang="en">vegetation anomaly</skos:altLabel>
        <skos:prefLabel xml:lang="en">botanical anomaly</skos:prefLabel>
        <skos:inScheme rdf:resource="http://resource.geosciml.org/classifierscheme/cgi/201401/earth-resource-expression"/>
        <skos:definition xml:lang="en">The Earth resource, concealed or exposed, has an anomalous botanical signature (eg, particular plant growth or absence of plants).</skos:definition>
      </skos:Concept>
    </skos:member>
    <rdfs:label xml:lang="en">EarthResource Expression vocabulary</rdfs:label>
    <skos:member>
      <skos:Concept rdf:about="http://resource.geosciml.org/classifier/cgi/earth-resource-expression/gossan">
        <skos:definition xml:lang="en">The surface expression of the Earth Resource is as highly weathered (oxidized) outcrop.</skos:definition>
        <skos:notation rdf:datatype="gtwg:LocalHierarchyKey">01.1..</skos:notation>
        <skos:broader>
          <skos:Concept rdf:about="http://resource.geosciml.org/classifier/cgi/earth-resource-expression/exposed">
            <dc:source xml:lang="en">Government Geoscience Information Committee (GGIC), Geoscience Australia</dc:source>
            <skos:notation rdf:datatype="gtwg:LocalHierarchyKey"
            >01..</skos:notation>
            <skos:prefLabel xml:lang="en">exposed</skos:prefLabel>
            <skos:inScheme rdf:resource="http://resource.geosciml.org/classifierscheme/cgi/201401/earth-resource-expression"/>
            <skos:definition xml:lang="en">The Earth resource is exposed at the Earth's surface.</skos:definition>
          </skos:Concept>
        </skos:broader>
        <skos:prefLabel xml:lang="en">gossan</skos:prefLabel>
        <skos:inScheme rdf:resource="http://resource.geosciml.org/classifierscheme/cgi/201401/earth-resource-expression"/>
        <dc:source xml:lang="en">Government Geoscience Information Committee (GGIC), Geoscience Australia</dc:source>
      </skos:Concept>
    </skos:member>
    <skos:member>
      <skos:Concept rdf:about="http://resource.geosciml.org/classifier/cgi/earth-resource-expression/alteration-halo">
        <dc:source xml:lang="en">Government Geoscience Information Committee (GGIC), Geoscience Australia</dc:source>
        <skos:notation rdf:datatype="gtwg:LocalHierarchyKey">03..</skos:notation>
        <skos:prefLabel xml:lang="en">alteration halo</skos:prefLabel>
        <skos:topConceptOf rdf:resource="http://resource.geosciml.org/classifierscheme/cgi/201401/earth-resource-expression"/>
        <skos:inScheme rdf:resource="http://resource.geosciml.org/classifierscheme/cgi/201401/earth-resource-expression"/>
        <skos:definition xml:lang="en">The Earth resource, concealed or exposed, has an anomalous rock alteration halo.</skos:definition>
      </skos:Concept>
    </skos:member>
    <skos:member>
      <skos:Concept rdf:about="http://resource.geosciml.org/classifier/cgi/earth-resource-expression/geochemical-anomaly">
        <dc:source xml:lang="en">Government Geoscience Information Committee (GGIC), Geoscience Australia</dc:source>
        <skos:notation rdf:datatype="gtwg:LocalHierarchyKey">05..</skos:notation>
        <skos:prefLabel xml:lang="en">geochemical anomaly</skos:prefLabel>
        <skos:topConceptOf rdf:resource="http://resource.geosciml.org/classifierscheme/cgi/201401/earth-resource-expression"/>
        <skos:inScheme rdf:resource="http://resource.geosciml.org/classifierscheme/cgi/201401/earth-resource-expression"/>
        <skos:definition xml:lang="en">The Earth resource, concealed or exposed, has an anomalous geochemical signature.</skos:definition>
      </skos:Concept>
    </skos:member>
    <skos:member>
      <skos:Concept rdf:about="http://resource.geosciml.org/classifier/cgi/earth-resource-expression/concealed">
        <dc:source xml:lang="en">Government Geoscience Information Committee (GGIC), Geoscience Australia</dc:source>
        <skos:notation rdf:datatype="gtwg:LocalHierarchyKey">02..</skos:notation>
        <skos:topConceptOf rdf:resource="http://resource.geosciml.org/classifierscheme/cgi/201401/earth-resource-expression"/>
        <skos:prefLabel xml:lang="en">concealed</skos:prefLabel>
        <skos:inScheme rdf:resource="http://resource.geosciml.org/classifierscheme/cgi/201401/earth-resource-expression"/>
        <skos:definition xml:lang="en">The Earth resource is not exposed at the Earth's surface.</skos:definition>
      </skos:Concept>
    </skos:member>
    <skos:member rdf:resource="http://resource.geosciml.org/classifier/cgi/earth-resource-expression/exposed"/>
  </skos:Collection>
</rdf:RDF>