<?xml version="1.0"?>
<rdf:RDF
    xmlns:rdf="http://www.w3.org/1999/02/22-rdf-syntax-ns#"
    xmlns:skos="http://www.w3.org/2004/02/skos/core#"
    xmlns:owl="http://www.w3.org/2002/07/owl#"
    xmlns:dc="http://purl.org/dc/elements/1.1/"
    xmlns:xsd="http://www.w3.org/2001/XMLSchema#"
	xmlns:gtwg="http://resource.geosciml.org/authority/cgi/gtwg"
    xmlns:rdfs="http://www.w3.org/2000/01/rdf-schema#"
  xml:base="http://resource.geosciml.org/classifierscheme/cgi/201401/mining-activity">
  <owl:Ontology rdf:about="">
    <owl:imports rdf:resource="http://www.w3.org/2004/02/skos/core"/>
    <owl:imports rdf:resource="http://purl.org/dc/elements/1.1/"/>
    <dc:creator>CGI Geoscience Terminology Working Group</dc:creator>
    <dc:date>2014-01-09T00:00:00.000</dc:date>
    <skos:editorialNote>This file contains the 201401 version of CGI Mining Activity Type Vocabulary, which defines concepts to categorize the type of mining activity (eg Open Cut, Underground Mine, multiple, unspecified) or processing activity (eg Ore Processing) or production. Using activity to distinguish between the extraction, processing and production activities allows distinguishing between ore mined/grade/recovery, ore treated/grade/recovery and produced payable/plant recovery. </skos:editorialNote>
    <skos:changeNote>Vocabulary Shepherd: Rachel Heaven/Tim McCormick. Compilation and review in Google doc spreadsheet, converted to MS Excel for SKOS generation using GSML_SKOS_from_XLS_2013.xslt; Conversion to SKOS by SM Richard 2014-02-23. </skos:changeNote>
    <skos:changeNote>Edits to fix typos and remove '201401' from rdf file name. Ollie Raymond 8-Jan-2015</skos:changeNote>
  </owl:Ontology>
  <skos:ConceptScheme rdf:about="http://resource.geosciml.org/classifierscheme/cgi/201401/mining-activity">
    <skos:definition xml:lang="en">This resource defines the concept space for Mining Activity Type vocabulary concepts by extension; it includes all concepts in this conceptScheme, as well as concepts in previous versions of the scheme.</skos:definition>
    <skos:prefLabel xml:lang="en">Mining Activity Type vocabulary</skos:prefLabel>
    <dc:creator xml:lang="en">CGI Geoscience Terminology Working Group</dc:creator>
  </skos:ConceptScheme>
  <skos:Collection rdf:about="http://resource.geosciml.org/classifier/cgi/mining-activity/">
    <skos:member>
      <skos:Concept rdf:about="http://resource.geosciml.org/classifier/cgi/mining-activity/dredge-mining">
        <skos:definition xml:lang="en">Excavation of underwater mineral resources by floating equipment. Dredging systems are classified as mechanical or hydraulic, depending on the method of material transport.</skos:definition>
        <skos:notation rdf:datatype="gtwg:LocalHierarchyKey">03.03..</skos:notation>
        <skos:broader>
          <skos:Concept rdf:about="http://resource.geosciml.org/classifier/cgi/mining-activity/underwater-mining">
            <skos:notation rdf:datatype="gtwg:LocalHierarchyKey">03..</skos:notation>
            <skos:topConceptOf rdf:resource="http://resource.geosciml.org/classifierscheme/cgi/201401/mining-activity"/>
            <skos:prefLabel xml:lang="en">underwater mining</skos:prefLabel>
            <skos:definition>Mining of underwater mineral deposits at or close to the sea, lake or river bed. May be from floating or land-based platforms involving dredging or vaccuum pumping or may use remote operated vehicle (submersible).</skos:definition>
            <skos:inScheme rdf:resource="http://resource.geosciml.org/classifierscheme/cgi/201401/mining-activity"/>
          </skos:Concept>
        </skos:broader>
        <skos:notation rdf:datatype="http://resource.geosciml.org/classifierscheme/cgi/201401/mining-activity">dredge-mining</skos:notation>
        <skos:prefLabel xml:lang="en">dredge mining</skos:prefLabel>
        <dc:source xml:lang="en">http://www.britannica.com/EBchecked/topic/171297/dredgin; adapted to include all types of mineral resources, not just placer deposits (e.g. could include sulfide deposits, manganese nodules on sea floor)</dc:source>
        <skos:inScheme rdf:resource="http://resource.geosciml.org/classifierscheme/cgi/201401/mining-activity"/>
      </skos:Concept>
    </skos:member>
    <skos:member>
      <skos:Concept rdf:about="http://resource.geosciml.org/classifier/cgi/mining-activity/surface-placer-mining">
        <dc:source xml:lang="en">Dictionary of Mining, Mineral and Related Terms, 2nd ed, AGI 1997</dc:source>
        <skos:notation rdf:datatype="gtwg:LocalHierarchyKey">01.01.</skos:notation>
        <skos:broader>
          <skos:Concept rdf:about="http://resource.geosciml.org/classifier/cgi/mining-activity/surface-mining">
            <dc:source xml:lang="en">Dictionary of Mining, Mineral and Related Terms, 2nd ed, AGI 1997</dc:source>
            <skos:notation rdf:datatype="gtwg:LocalHierarchyKey">01..</skos:notation>
            <skos:topConceptOf rdf:resource="http://resource.geosciml.org/classifierscheme/cgi/201401/mining-activity"/>
            <skos:prefLabel xml:lang="en">surface mining</skos:prefLabel>
            <skos:definition>Mining via surface excavations.</skos:definition>
            <skos:inScheme rdf:resource="http://resource.geosciml.org/classifierscheme/cgi/201401/mining-activity"/>
          </skos:Concept>
        </skos:broader>
        <skos:notation rdf:datatype="http://resource.geosciml.org/classifierscheme/cgi/201401/mining-activity">surface-placer-mining</skos:notation>
        <skos:altLabel xml:lang="en">alluvial mining</skos:altLabel>
        <skos:prefLabel xml:lang="en">surface placer mining</skos:prefLabel>
        <skos:definition>The extraction of heavy mineral from beach or sand-bank deposits by concentration in running water. It includes ground sluicing, panning, shoveling gravel into a sluice, scraping by power scraper and excavation by dragline, dredge or other mechanized equipment.</skos:definition>
        <skos:inScheme rdf:resource="http://resource.geosciml.org/classifierscheme/cgi/201401/mining-activity"/>
      </skos:Concept>
    </skos:member>
    <skos:member>
      <skos:Concept rdf:about="http://resource.geosciml.org/classifier/cgi/mining-activity/borehole-mining">
        <dc:source xml:lang="en">Dictionary of Mining, Mineral and Related Terms, 2nd ed, AGI 1997</dc:source>
        <skos:notation rdf:datatype="gtwg:LocalHierarchyKey">02.02.</skos:notation>
        <skos:broader>
          <skos:Concept rdf:about="http://resource.geosciml.org/classifier/cgi/mining-activity/subsurface-mining">
            <dc:source xml:lang="en">Dictionary of Mining, Mineral and Related Terms, 2nd ed, AGI 1997</dc:source>
            <skos:notation rdf:datatype="gtwg:LocalHierarchyKey">02..</skos:notation>
            <skos:topConceptOf rdf:resource="http://resource.geosciml.org/classifierscheme/cgi/201401/mining-activity"/>
            <skos:prefLabel xml:lang="en">subsurface mining</skos:prefLabel>
            <skos:definition>Mining beneath the surface of the earth.</skos:definition>
            <skos:inScheme rdf:resource="http://resource.geosciml.org/classifierscheme/cgi/201401/mining-activity"/>
          </skos:Concept>
        </skos:broader>
        <skos:notation rdf:datatype="http://resource.geosciml.org/classifierscheme/cgi/201401/mining-activity">borehole-mining</skos:notation>
        <skos:prefLabel xml:lang="en">borehole mining</skos:prefLabel>
        <skos:definition>Extraction of a mineral product in the liquid or gaseous state from the Earth's crust by means of boreholes. Boreholes are used for mining petroleum, and for the extraction of liquid solutions of salt, sulfur, etc.</skos:definition>
        <skos:inScheme rdf:resource="http://resource.geosciml.org/classifierscheme/cgi/201401/mining-activity"/>
      </skos:Concept>
    </skos:member>
    <skos:member rdf:resource="http://resource.geosciml.org/classifier/cgi/mining-activity/subsurface-mining"/>
    <skos:member>
      <skos:Concept rdf:about="http://resource.geosciml.org/classifier/cgi/mining-activity/open-pit-mining">
        <skos:notation rdf:datatype="http://resource.geosciml.org/classifierscheme/cgi/201401/mining-activity">open-pit-mining</skos:notation>
        <dc:source xml:lang="en">CGI/ERML 2.0</dc:source>
        <skos:notation rdf:datatype="gtwg:LocalHierarchyKey">01.03.</skos:notation>
        <skos:altLabel xml:lang="en">strip mining</skos:altLabel>
        <skos:altLabel xml:lang="en">open sky mining</skos:altLabel>
        <skos:definition>An open-sky excavation for the extraction of mineral resources (eg, open cut, open cast, strip mining)</skos:definition>
        <skos:altLabel xml:lang="en">open cut mining</skos:altLabel>
        <skos:inScheme rdf:resource="http://resource.geosciml.org/classifierscheme/cgi/201401/mining-activity"/>
        <skos:prefLabel xml:lang="en">open-pit mining</skos:prefLabel>
        <skos:altLabel xml:lang="en">open-cast mining</skos:altLabel>
        <skos:broader rdf:resource="http://resource.geosciml.org/classifier/cgi/mining-activity/surface-mining"/>
      </skos:Concept>
    </skos:member>
    <skos:member rdf:resource="http://resource.geosciml.org/classifier/cgi/mining-activity/surface-mining"/>
    <skos:member>
      <skos:Concept rdf:about="http://resource.geosciml.org/classifier/cgi/mining-activity/quarrying">
        <dc:source xml:lang="en">Glossary of Geology. 5th Edition, AGI - online</dc:source>
        <skos:notation rdf:datatype="gtwg:LocalHierarchyKey">01.03.01.</skos:notation>
        <skos:broader rdf:resource="http://resource.geosciml.org/classifier/cgi/mining-activity/open-pit-mining"/>
        <skos:notation rdf:datatype="http://resource.geosciml.org/classifierscheme/cgi/201401/mining-activity">quarrying</skos:notation>
        <skos:prefLabel xml:lang="en">quarrying</skos:prefLabel>
        <skos:definition>The extraction of building stone or other valuable nonmetallic constituent from an open or surface mineral working. It is distinguished from a mine because a quarry usually is open at the top and front, and, in ordinary use of the term, by the character of the material extracted.</skos:definition>
        <skos:inScheme rdf:resource="http://resource.geosciml.org/classifierscheme/cgi/201401/mining-activity"/>
      </skos:Concept>
    </skos:member>
    <skos:member>
      <skos:Concept rdf:about="http://resource.geosciml.org/classifier/cgi/mining-activity/subaqueous-vacuum-pumping">
        <dc:source xml:lang="en">this vocabulary</dc:source>
        <skos:notation rdf:datatype="gtwg:LocalHierarchyKey">03.01..</skos:notation>
        <skos:broader rdf:resource="http://resource.geosciml.org/classifier/cgi/mining-activity/underwater-mining"/>
        <skos:notation rdf:datatype="http://resource.geosciml.org/classifierscheme/cgi/201401/mining-activity">subaqueous-vacuum-pumping</skos:notation>
        <skos:prefLabel xml:lang="en">Subaqueous vacuum pumping</skos:prefLabel>
        <skos:definition></skos:definition>
        <skos:inScheme rdf:resource="http://resource.geosciml.org/classifierscheme/cgi/201401/mining-activity"/>
      </skos:Concept>
    </skos:member>
    <skos:member>
      <skos:Concept rdf:about="http://resource.geosciml.org/classifier/cgi/mining-activity/subaqueous-remote-operated-vehicle">
        <dc:source xml:lang="en">this vocabulary</dc:source>
        <skos:notation rdf:datatype="gtwg:LocalHierarchyKey">03.02..</skos:notation>
        <skos:broader rdf:resource="http://resource.geosciml.org/classifier/cgi/mining-activity/underwater-mining"/>
        <skos:notation rdf:datatype="http://resource.geosciml.org/classifierscheme/cgi/201401/mining-activity">subaqueous-remote-operated-vehicle</skos:notation>
        <skos:prefLabel xml:lang="en">subaqueous remote operated vehicle</skos:prefLabel>
        <skos:definition></skos:definition>
        <skos:inScheme rdf:resource="http://resource.geosciml.org/classifierscheme/cgi/201401/mining-activity"/>
      </skos:Concept>
    </skos:member>
    <skos:member>
      <skos:Concept rdf:about="http://resource.geosciml.org/classifier/cgi/mining-activity/underground-mining">
        <dc:source xml:lang="en">Dictionary of Mining, Mineral and Related Terms, 1st edition</dc:source>
        <skos:notation rdf:datatype="gtwg:LocalHierarchyKey">02.01.</skos:notation>
        <skos:broader rdf:resource="http://resource.geosciml.org/classifier/cgi/mining-activity/subsurface-mining"/>
        <skos:notation rdf:datatype="http://resource.geosciml.org/classifierscheme/cgi/201401/mining-activity">underground-mining</skos:notation>
        <skos:prefLabel xml:lang="en">underground mining</skos:prefLabel>
        <skos:definition>A mineral extraction activity in which ore is extracted from the subsurface via underground mine workings (adits, shafts, drifts, stopes, etc.).</skos:definition>
        <skos:inScheme rdf:resource="http://resource.geosciml.org/classifierscheme/cgi/201401/mining-activity"/>
      </skos:Concept>
    </skos:member>
    <skos:member>
      <skos:Concept rdf:about="http://resource.geosciml.org/classifier/cgi/mining-activity/in-situ-recovery">
        <skos:altLabel xml:lang="en">chemical mining</skos:altLabel>
        <skos:definition>The extraction of valuable constituents of an orebody in place from boreholes using thermal, miscible, and chemical methods e.g. by dissolution, leaching, underground gasification</skos:definition>
        <skos:prefLabel xml:lang="en">in-situ recovery</skos:prefLabel>
        <skos:broader rdf:resource="http://resource.geosciml.org/classifier/cgi/mining-activity/borehole-mining"/>
        <skos:altLabel xml:lang="en">solution mining</skos:altLabel>
        <skos:altLabel xml:lang="en">underground gasification</skos:altLabel>
        <skos:inScheme rdf:resource="http://resource.geosciml.org/classifierscheme/cgi/201401/mining-activity"/>
        <skos:notation rdf:datatype="http://resource.geosciml.org/classifierscheme/cgi/201401/mining-activity">in-situ-recovery</skos:notation>
        <dc:source xml:lang="en">Glossary of Geology. 5th Edition, AGI - online, adapted from chemical mining and enhanced oil recovery</dc:source>
        <skos:notation rdf:datatype="gtwg:LocalHierarchyKey">02.02.01.</skos:notation>
      </skos:Concept>
    </skos:member>
    <rdfs:label xml:lang="en">Mining Activity Type vocabulary</rdfs:label>
    <skos:member>
      <skos:Concept rdf:about="http://resource.geosciml.org/classifier/cgi/mining-activity/hydraulic-mining">
        <dc:source xml:lang="en">Glossary of Geology. 5th Edition, AGI - online</dc:source>
        <skos:notation rdf:datatype="gtwg:LocalHierarchyKey">01.20.</skos:notation>
        <skos:broader rdf:resource="http://resource.geosciml.org/classifier/cgi/mining-activity/surface-mining"/>
        <skos:notation rdf:datatype="http://resource.geosciml.org/classifierscheme/cgi/201401/mining-activity">hydraulic-mining</skos:notation>
        <skos:prefLabel xml:lang="en">hydraulic mining</skos:prefLabel>
        <skos:definition>The recovery of desired material, generally in open pits, by means of strong jets of water</skos:definition>
        <skos:inScheme rdf:resource="http://resource.geosciml.org/classifierscheme/cgi/201401/mining-activity"/>
      </skos:Concept>
    </skos:member>
    <skos:member rdf:resource="http://resource.geosciml.org/classifier/cgi/mining-activity/underwater-mining"/>
    <skos:member>
      <skos:Concept rdf:about="http://resource.geosciml.org/classifier/cgi/mining-activity/placer-dredging">
        <dc:source xml:lang="en">this vocabulary</dc:source>
        <skos:notation rdf:datatype="gtwg:LocalHierarchyKey">01.01.01.</skos:notation>
        <skos:broader rdf:resource="http://resource.geosciml.org/classifier/cgi/mining-activity/dredge-mining"/>
        <skos:broader rdf:resource="http://resource.geosciml.org/classifier/cgi/mining-activity/surface-placer-mining"/>
        <skos:notation rdf:datatype="http://resource.geosciml.org/classifierscheme/cgi/201401/mining-activity">placer-dredging</skos:notation>
        <skos:prefLabel xml:lang="en">placer dredging</skos:prefLabel>
        <skos:definition>The extraction of minerals from an underwater placer deposit by the use of floating equipment for scooping or suction</skos:definition>
        <skos:inScheme rdf:resource="http://resource.geosciml.org/classifierscheme/cgi/201401/mining-activity"/>
      </skos:Concept>
    </skos:member>
  </skos:Collection>
</rdf:RDF>

<!-- Created with TopBraid -->
