<?xml version="1.0"?>
<rdf:RDF
    xmlns:rdf="http://www.w3.org/1999/02/22-rdf-syntax-ns#"
    xmlns:skos="http://www.w3.org/2004/02/skos/core#"
    xmlns="http://resource.geosciml.org/classifierscheme/cgi/201403/raw-material-role#"
    xmlns:owl="http://www.w3.org/2002/07/owl#"
    xmlns:dc="http://purl.org/dc/elements/1.1/"
    xmlns:xsd="http://www.w3.org/2001/XMLSchema#"
	xmlns:gtwg="http://resource.geosciml.org/authority/cgi/gtwg"
    xmlns:rdfs="http://www.w3.org/2000/01/rdf-schema#"
  xml:base="http://resource.geosciml.org/classifierscheme/cgi/201403/raw-material-role">
  <owl:Ontology rdf:about="http://resource.geosciml.org/static/vocabulary/earthresourceml/2014/RawMaterialRole.rdf">
    <owl:imports rdf:resource="http://purl.org/dc/elements/1.1/"/>
    <owl:imports rdf:resource="http://www.w3.org/2004/02/skos/core"/>
    <dc:creator>SKOS generated from Excel workbook using GSML_SKOS_from_XLS_2014.xslt; SM Richard</dc:creator>
    <dc:date>2014-03-19T00:00:00.000</dc:date>
    <skos:editorialNote>This file contains the 201403 version of CGI Raw material role value vocabulary for categorizing raw material relationships with Earth Resource occurrences.</skos:editorialNote>
    <skos:changeNote>Original SKOS implementation, based on 2013-06 approved vocabulary from GTWG face to face in St. Petersburg, Russia</skos:changeNote>
    <skos:changeNote>Edits to fix typos and remove '201403' from rdf file name. Ollie Raymond 8-Jan-2015</skos:changeNote>
  </owl:Ontology>
  <skos:ConceptScheme rdf:about="http://resource.geosciml.org/classifierscheme/cgi/201403/raw-material-role">
    <skos:definition xml:lang="en">This resource defines the concept space for Raw material role values concepts by extension; it includes all concepts in this conceptScheme, as well as concepts in previous versions of the scheme.</skos:definition>
    <skos:prefLabel xml:lang="en">Raw Material Role vocabulary</skos:prefLabel>
    <dc:creator xml:lang="en">CGI Geoscience Terminology Working Group</dc:creator>
  </skos:ConceptScheme>
  <skos:Collection rdf:about="http://resource.geosciml.org/classifier/cgi/raw-material-role/">
    <skos:member>
      <skos:Concept rdf:about="http://resource.geosciml.org/classifier/cgi/raw-material-role/waste">
        <skos:definition xml:lang="en">Any solid or liquid generated by human activity that has little or no economic value, usually the result of the manufacture, mining, or processing of a material to produce an economic product. (this is material that has not been processed to remove a product, either in place or in holding heaps)</skos:definition>
        <skos:notation rdf:datatype="gtwg:LocalHierarchyKey">03..</skos:notation>
        <skos:topConceptOf rdf:resource="http://resource.geosciml.org/classifierscheme/cgi/201403/raw-material-role"/>
        <skos:prefLabel xml:lang="en">waste</skos:prefLabel>
        <dc:source xml:lang="en">Glossary of Geology. 5th Edition, AGI - online</dc:source>
        <skos:inScheme rdf:resource="http://resource.geosciml.org/classifierscheme/cgi/201403/raw-material-role"/>
      </skos:Concept>
    </skos:member>
    <skos:member>
      <skos:Concept rdf:about="http://resource.geosciml.org/classifier/cgi/raw-material-role/ore">
        <skos:definition xml:lang="en">The naturally occurring material from which a mineral or minerals of economic value can be extracted at a reasonable profit. Also, the mineral(s) thus extracted. The term is generally but not always used to refer to metalliferous material, and is often modified by the name of the valuable constituent, e.g., "iron ore".</skos:definition>
        <skos:notation rdf:datatype="gtwg:LocalHierarchyKey">02..</skos:notation>
        <skos:topConceptOf rdf:resource="http://resource.geosciml.org/classifierscheme/cgi/201403/raw-material-role"/>
        <skos:prefLabel xml:lang="en">ore</skos:prefLabel>
        <dc:source xml:lang="en">Glossary of Geology. 5th Edition, AGI - online</dc:source>
        <skos:inScheme rdf:resource="http://resource.geosciml.org/classifierscheme/cgi/201403/raw-material-role"/>
      </skos:Concept>
    </skos:member>
    <skos:member>
      <skos:Concept rdf:about="http://resource.geosciml.org/classifier/cgi/raw-material-role/gangue">
        <skos:definition xml:lang="en">The valueless rock or mineral aggregates in an ore; that part of an ore that is not economically desirable but cannot be avoided in mining. It is separated from the ore minerals during concentration. (this is material that has been processed to remove some economic product)</skos:definition>
        <skos:notation rdf:datatype="gtwg:LocalHierarchyKey">01..</skos:notation>
        <skos:topConceptOf rdf:resource="http://resource.geosciml.org/classifierscheme/cgi/201403/raw-material-role"/>
        <skos:prefLabel xml:lang="en">gangue</skos:prefLabel>
        <dc:source xml:lang="en">Glossary of Geology. 5th Edition, AGI - online</dc:source>
        <skos:inScheme rdf:resource="http://resource.geosciml.org/classifierscheme/cgi/201403/raw-material-role"/>
      </skos:Concept>
    </skos:member>
    <rdfs:label xml:lang="en">Raw Material Role vocabulary</rdfs:label>
  </skos:Collection>
</rdf:RDF>

