<?xml version="1.0"?>
<rdf:RDF
    xmlns:rdf="http://www.w3.org/1999/02/22-rdf-syntax-ns#"
    xmlns:skos="http://www.w3.org/2004/02/skos/core#"
    xmlns:owl="http://www.w3.org/2002/07/owl#"
    xmlns:dc="http://purl.org/dc/elements/1.1/"
    xmlns:xsd="http://www.w3.org/2001/XMLSchema#"
	xmlns:gtwg="http://resource.geosciml.org/authority/cgi/gtwg"
    xmlns:rdfs="http://www.w3.org/2000/01/rdf-schema#"
  xml:base="http://resource.geosciml.org/classifierscheme/cgi/201403/reserve-assessment-category">
  <owl:Ontology rdf:about="">
    <owl:imports rdf:resource="http://purl.org/dc/elements/1.1/"/>
    <owl:imports rdf:resource="http://www.w3.org/2004/02/skos/core"/>
    <dc:date>2014-03-19T00:00:00.000</dc:date>
    <dc:creator xml:lang="en">SKOS generated from Excel workbook using GSML_SKOS_from_XLS_2014.xslt; SM Richard</dc:creator>
    <skos:editorialNote xml:lang="en">This file contains the 201403 version of CGI Earth resource reserve category vocabulary, for classifying reserve types associated with Earth resource occurrences.</skos:editorialNote>
    <skos:changeNote xml:lang="en">Original SKOS implementation, based on 2013-06 approved vocabulary from GTWG face to face in St. Petersburg, Russia</skos:changeNote>
    <skos:changeNote>Edits to fix typos and remove '201403' from rdf file name. Ollie Raymond 8-Jan-2015</skos:changeNote>
  </owl:Ontology>
  <skos:ConceptScheme rdf:about="http://resource.geosciml.org/classifierscheme/cgi/201403/reserve-assessment-category">
    <skos:prefLabel xml:lang="en">EarthResource reserve category vocabulary</skos:prefLabel>
    <dc:creator xml:lang="en">CGI Geoscience Terminology Working Group</dc:creator>
    <skos:definition xml:lang="en">This resource defines the concept space for Earth resource reserve category vocabulary concepts by extension; it includes all concepts in this conceptScheme, as well as concepts in previous versions of the scheme.</skos:definition>
  </skos:ConceptScheme>
  <skos:Collection rdf:about="http://resource.geosciml.org/classifier/cgi/reserve-assessment-category/">
    <rdfs:label xml:lang="en">EarthResource reserve category vocabulary</rdfs:label>
    <skos:member>
      <skos:Concept rdf:about="http://resource.geosciml.org/classifier/cgi/reserve-assessment-category/proved-ore-reserves">
        <skos:inScheme rdf:resource="http://resource.geosciml.org/classifierscheme/cgi/201403/reserve-assessment-category"/>
        <skos:definition>A ‘Proved Ore Reserve’ is the economically mineable part of a Measured Mineral Resource. It includes diluting materials and allowances for losses which may occur when the material is mined. Appropriate assessments and studies have been carried out, and include consideration of and modification by realistically assumed mining, metallurgical, economic, marketing, legal, environmental, social and governmental factors. These assessments demonstrate at the time of reporting that extraction could reasonably be justified</skos:definition>
        <skos:prefLabel xml:lang="en">proved ore reserves</skos:prefLabel>
        <skos:topConceptOf rdf:resource="http://resource.geosciml.org/classifierscheme/cgi/201403/reserve-assessment-category"/>
        <skos:notation rdf:datatype="gtwg:LocalHierarchyKey">01..</skos:notation>
        <dc:source xml:lang="en">CRIRSCO Code; JORC 2004</dc:source>
      </skos:Concept>
    </skos:member>
    <skos:member>
      <skos:Concept rdf:about="http://resource.geosciml.org/classifier/cgi/reserve-assessment-category/probable-ore-reserves">
        <skos:inScheme rdf:resource="http://resource.geosciml.org/classifierscheme/cgi/201403/reserve-assessment-category"/>
        <skos:definition>A ‘Probable Ore Reserve’ is the economically mineable part of an Indicated, and in some circumstances, a Measured Mineral Resource. It includes diluting materials and allowances for losses which may occur when the material is mined. Appropriate assessments and studies have been carried out, and include consideration of and modification by realistically assumed mining, metallurgical, economic, marketing, legal, environmental, social and governmental factors These assessments demonstrate at the time of reporting that extraction could reasonably be justified.</skos:definition>
        <skos:prefLabel xml:lang="en">probable ore reserves</skos:prefLabel>
        <skos:topConceptOf rdf:resource="http://resource.geosciml.org/classifierscheme/cgi/201403/reserve-assessment-category"/>
        <skos:notation rdf:datatype="gtwg:LocalHierarchyKey">02..</skos:notation>
        <dc:source xml:lang="en">CRIRSCO Code; JORC 2004</dc:source>
      </skos:Concept>
    </skos:member>
    <skos:member>
      <skos:Concept rdf:about="http://resource.geosciml.org/classifier/cgi/reserve-assessment-category/proved-and-probable-ore-reserves">
        <skos:inScheme rdf:resource="http://resource.geosciml.org/classifierscheme/cgi/201403/reserve-assessment-category"/>
        <skos:definition>A mixture of the economically mineable part of an Indicated, and a Measured Mineral Resource. It includes diluting materials and allowances for losses which may occur when the material is mined. Appropriate assessments and studies have been carried out, and include consideration of and modification by realistically assumed mining, metallurgical, economic, marketing, legal, environmental, social and governmental factors These assessments demonstrate at the time of reporting that extraction could reasonably be justified.</skos:definition>
        <skos:prefLabel xml:lang="en">proved and probable ore reserves</skos:prefLabel>
        <skos:topConceptOf rdf:resource="http://resource.geosciml.org/classifierscheme/cgi/201403/reserve-assessment-category"/>
        <skos:notation rdf:datatype="gtwg:LocalHierarchyKey">03..</skos:notation>
        <dc:source xml:lang="en">CRIRSCO Code; JORC 2004</dc:source>
      </skos:Concept>
    </skos:member>
  </skos:Collection>
</rdf:RDF>

