<?xml version="1.0" encoding="UTF-8"?>
<rdf:RDF
	xmlns:cgi="http://resource.geosciml.org/classifierscheme/cgi/201211/"
	xmlns:cmpartrole="http://resource.geosciml.org/classifier/cgi/compoundmaterialconstituentpartrole/"
	xmlns:dc="http://purl.org/dc/elements/1.1/"
	xmlns:owl="http://www.w3.org/2002/07/owl#"
	xmlns:owl2xml="http://www.w3.org/2006/12/owl2-xml#"
	xmlns:rdf="http://www.w3.org/1999/02/22-rdf-syntax-ns#"
	xmlns:rdfs="http://www.w3.org/2000/01/rdf-schema#"
	xmlns:skos="http://www.w3.org/2004/02/skos/core#"
	xmlns:void="http://rdfs.org/ns/void#"
	xmlns:xsd="http://www.w3.org/2001/XMLSchema#">

<rdf:Description rdf:about="http://resource.geosciml.org/classifier/cgi/compoundmaterialconstituentpartrole/">
	<rdf:type rdf:resource="http://www.w3.org/2004/02/skos/core#Collection"/>
	<rdfs:label xml:lang="en">compound material constitutent part role concepts</rdfs:label>
	<skos:definition xml:lang="en">This resource defines the concept space for compound Material Constitutent Part Role by extension; it includes all concepts in this conceptScheme, as well as concepts in previous versions of the scheme.</skos:definition>
	<skos:historyNote xml:lang="en">Updated to 201211 version by SMR; add collection entity, check all pref labels are lower case, remove owl:NamedIndividual and Owl:Thing rdf:types.</skos:historyNote>
	<skos:member rdf:resource="http://resource.geosciml.org/classifier/cgi/compoundmaterialconstituentpartrole/small_concretion"/>
	<skos:member rdf:resource="http://resource.geosciml.org/classifier/cgi/compoundmaterialconstituentpartrole/armoured_relict_inclusion"/>
	<skos:member rdf:resource="http://resource.geosciml.org/classifier/cgi/compoundmaterialconstituentpartrole/matrix"/>
	<skos:member rdf:resource="http://resource.geosciml.org/classifier/cgi/compoundmaterialconstituentpartrole/constituent_role_not_specified"/>
	<skos:member rdf:resource="http://resource.geosciml.org/classifier/cgi/compoundmaterialconstituentpartrole/porphyroblast"/>
	<skos:member rdf:resource="http://resource.geosciml.org/classifier/cgi/compoundmaterialconstituentpartrole/corrosion_rim"/>
	<skos:member rdf:resource="http://resource.geosciml.org/classifier/cgi/compoundmaterialconstituentpartrole/granular_framework_constituent"/>
	<skos:member rdf:resource="http://resource.geosciml.org/classifier/cgi/compoundmaterialconstituentpartrole/epimatrix"/>
	<skos:member rdf:resource="http://resource.geosciml.org/classifier/cgi/compoundmaterialconstituentpartrole/groundmass_constituent"/>
	<skos:member rdf:resource="http://resource.geosciml.org/classifier/cgi/compoundmaterialconstituentpartrole/vein"/>
	<skos:member rdf:resource="http://resource.geosciml.org/classifier/cgi/compoundmaterialconstituentpartrole/interstitial_constituent"/>
	<skos:member rdf:resource="http://resource.geosciml.org/classifier/cgi/compoundmaterialconstituentpartrole/particulate_constituent"/>
	<skos:member rdf:resource="http://resource.geosciml.org/classifier/cgi/compoundmaterialconstituentpartrole/layer"/>
	<skos:member rdf:resource="http://resource.geosciml.org/classifier/cgi/compoundmaterialconstituentpartrole/protomatrix"/>
	<skos:member rdf:resource="http://resource.geosciml.org/classifier/cgi/compoundmaterialconstituentpartrole/armoured_relict_crystal"/>
	<skos:member rdf:resource="http://resource.geosciml.org/classifier/cgi/compoundmaterialconstituentpartrole/sedimentary_rock_cement"/>
	<skos:member rdf:resource="http://resource.geosciml.org/classifier/cgi/compoundmaterialconstituentpartrole/megacryst"/>
	<skos:member rdf:resource="http://resource.geosciml.org/classifier/cgi/compoundmaterialconstituentpartrole/structural_part"/>
	<skos:member rdf:resource="http://resource.geosciml.org/classifier/cgi/compoundmaterialconstituentpartrole/crystalline_framework_constituent"/>
	<skos:member rdf:resource="http://resource.geosciml.org/classifier/cgi/compoundmaterialconstituentpartrole/chadacryst"/>
	<skos:member rdf:resource="http://resource.geosciml.org/classifier/cgi/compoundmaterialconstituentpartrole/kelyphitic_rim"/>
	<skos:member rdf:resource="http://resource.geosciml.org/classifier/cgi/compoundmaterialconstituentpartrole/pseudomatrix"/>
	<skos:member rdf:resource="http://resource.geosciml.org/classifier/cgi/compoundmaterialconstituentpartrole/porphyroclast"/>
	<skos:member rdf:resource="http://resource.geosciml.org/classifier/cgi/compoundmaterialconstituentpartrole/irregular_part"/>
	<skos:member rdf:resource="http://resource.geosciml.org/classifier/cgi/compoundmaterialconstituentpartrole/phenoclast"/>
	<skos:member rdf:resource="http://resource.geosciml.org/classifier/cgi/compoundmaterialconstituentpartrole/dropstone"/>
	<skos:member rdf:resource="http://resource.geosciml.org/classifier/cgi/compoundmaterialconstituentpartrole/floating_clast"/>
	<skos:member rdf:resource="http://resource.geosciml.org/classifier/cgi/compoundmaterialconstituentpartrole/orthomatrix"/>
	<skos:member rdf:resource="http://resource.geosciml.org/classifier/cgi/compoundmaterialconstituentpartrole/inclusion"/>
	<skos:member rdf:resource="http://resource.geosciml.org/classifier/cgi/compoundmaterialconstituentpartrole/phenocryst"/>
	<skos:member rdf:resource="http://resource.geosciml.org/classifier/cgi/compoundmaterialconstituentpartrole/clot"/>
	<skos:member rdf:resource="http://resource.geosciml.org/classifier/cgi/compoundmaterialconstituentpartrole/corona"/>
	<skos:member rdf:resource="http://resource.geosciml.org/classifier/cgi/compoundmaterialconstituentpartrole/overgrowth"/>
	<skos:member rdf:resource="http://resource.geosciml.org/classifier/cgi/compoundmaterialconstituentpartrole/oikocryst"/>
	<skos:member rdf:resource="http://resource.geosciml.org/classifier/cgi/compoundmaterialconstituentpartrole/clast_supporting_orthomatrix"/>
	<skos:prefLabel xml:lang="en">CGI Compound Material Constituent Part Role</skos:prefLabel>
</rdf:Description>

<rdf:Description rdf:about="http://resource.geosciml.org/classifier/cgi/compoundmaterialconstituentpartrole/armoured_relict_crystal">
	<rdf:type rdf:resource="http://www.w3.org/2004/02/skos/core#Concept"/>
	<dc:source>base on Neuendorf et al 2005</dc:source>
	<skos:broader rdf:resource="http://resource.geosciml.org/classifier/cgi/compoundmaterialconstituentpartrole/particulate_constituent"/>
	<skos:definition>a crystal of an earlier rock that is prevented from further reaction in a later rock by a rim of reaction products</skos:definition>
	<skos:exactMatch rdf:resource="http://resource.geosciml.org/classifier/cgi/compoundmaterialconstituentpartrole/0001"/>
	<skos:inScheme rdf:resource="http://resource.geosciml.org/classifierscheme/cgi/201211/compoundmaterialconstituentpartrole"/>
	<skos:prefLabel xml:lang="en">armoured relict crystal</skos:prefLabel>
</rdf:Description>

<rdf:Description rdf:about="http://resource.geosciml.org/classifier/cgi/compoundmaterialconstituentpartrole/armoured_relict_inclusion">
	<rdf:type rdf:resource="http://www.w3.org/2004/02/skos/core#Concept"/>
	<dc:source>base on Neuendorf et al 2005</dc:source>
	<skos:broader rdf:resource="http://resource.geosciml.org/classifier/cgi/compoundmaterialconstituentpartrole/inclusion"/>
	<skos:definition>an inclusion of an earlier rock that is prevented from further reaction in a later rock by a rim of reaction products</skos:definition>
	<skos:exactMatch rdf:resource="http://resource.geosciml.org/classifier/cgi/compoundmaterialconstituentpartrole/0002"/>
	<skos:inScheme rdf:resource="http://resource.geosciml.org/classifierscheme/cgi/201211/compoundmaterialconstituentpartrole"/>
	<skos:prefLabel xml:lang="en">armoured relict inclusion</skos:prefLabel>
</rdf:Description>

<rdf:Description rdf:about="http://resource.geosciml.org/classifier/cgi/compoundmaterialconstituentpartrole/chadacryst">
	<rdf:type rdf:resource="http://www.w3.org/2004/02/skos/core#Concept"/>
	<dc:source>Neuendorf et al., 2005</dc:source>
	<skos:broader rdf:resource="http://resource.geosciml.org/classifier/cgi/compoundmaterialconstituentpartrole/particulate_constituent"/>
	<skos:definition>the enclosed crystal in a poikolitic texture</skos:definition>
	<skos:exactMatch rdf:resource="http://resource.geosciml.org/classifier/cgi/compoundmaterialconstituentpartrole/0003"/>
	<skos:inScheme rdf:resource="http://resource.geosciml.org/classifierscheme/cgi/201211/compoundmaterialconstituentpartrole"/>
	<skos:prefLabel xml:lang="en">chadacryst</skos:prefLabel>
</rdf:Description>

<rdf:Description rdf:about="http://resource.geosciml.org/classifier/cgi/compoundmaterialconstituentpartrole/clast_supporting_orthomatrix">
	<rdf:type rdf:resource="http://www.w3.org/2004/02/skos/core#Concept"/>
	<dc:source xml:lang="en">This vocabulary</dc:source>
	<skos:broader rdf:resource="http://resource.geosciml.org/classifier/cgi/compoundmaterialconstituentpartrole/orthomatrix"/>
	<skos:definition>Orthomatrix in matrix supported sedimentary rock.</skos:definition>
	<skos:exactMatch rdf:resource="http://resource.geosciml.org/classifier/cgi/compoundmaterialconstituentpartrole/0004"/>
	<skos:inScheme rdf:resource="http://resource.geosciml.org/classifierscheme/cgi/201211/compoundmaterialconstituentpartrole"/>
	<skos:prefLabel xml:lang="en">clast supporting orthomatrix</skos:prefLabel>
</rdf:Description>

<rdf:Description rdf:about="http://resource.geosciml.org/classifier/cgi/compoundmaterialconstituentpartrole/clot">
	<rdf:type rdf:resource="http://www.w3.org/2004/02/skos/core#Concept"/>
	<dc:source>Neuendorf et al, 2005</dc:source>
	<skos:broader rdf:resource="http://resource.geosciml.org/classifier/cgi/compoundmaterialconstituentpartrole/structural_part"/>
	<skos:definition>A cluster of ferromagnesian minerals in an igneous rock, from several centimeters to decimeters in diameter, that may be a segregation or an altered xenolith.</skos:definition>
	<skos:exactMatch rdf:resource="http://resource.geosciml.org/classifier/cgi/compoundmaterialconstituentpartrole/0005"/>
	<skos:inScheme rdf:resource="http://resource.geosciml.org/classifierscheme/cgi/201211/compoundmaterialconstituentpartrole"/>
	<skos:prefLabel xml:lang="en">clot</skos:prefLabel>
</rdf:Description>

<rdf:Description rdf:about="http://resource.geosciml.org/classifier/cgi/compoundmaterialconstituentpartrole/constituent_role_not_specified">
	<rdf:type rdf:resource="http://www.w3.org/2004/02/skos/core#Concept"/>
	<dc:source xml:lang="en">This vocabulary</dc:source>
	<skos:definition>For descriptions in which role of constituent in compound material is not specified.</skos:definition>
	<skos:exactMatch rdf:resource="http://resource.geosciml.org/classifier/cgi/compoundmaterialconstituentpartrole/0006"/>
	<skos:inScheme rdf:resource="http://resource.geosciml.org/classifierscheme/cgi/201211/compoundmaterialconstituentpartrole"/>
	<skos:prefLabel xml:lang="en">constituent role not specified</skos:prefLabel>
	<skos:topConceptOf rdf:resource="http://resource.geosciml.org/classifierscheme/cgi/201211/compoundmaterialconstituentpartrole"/>
</rdf:Description>

<rdf:Description rdf:about="http://resource.geosciml.org/classifier/cgi/compoundmaterialconstituentpartrole/corona">
	<rdf:type rdf:resource="http://www.w3.org/2004/02/skos/core#Concept"/>
	<dc:source>Williams, Turner and Gilbert, 1954; Spry, 1969; Fettes and Desmons, 2007</dc:source>
	<skos:broader rdf:resource="http://resource.geosciml.org/classifier/cgi/compoundmaterialconstituentpartrole/structural_part"/>
	<skos:definition>Constituent occurs as a concentric envelope enclosing another constituent. Corona is a non-genetic term.</skos:definition>
	<skos:exactMatch rdf:resource="http://resource.geosciml.org/classifier/cgi/compoundmaterialconstituentpartrole/0007"/>
	<skos:inScheme rdf:resource="http://resource.geosciml.org/classifierscheme/cgi/201211/compoundmaterialconstituentpartrole"/>
	<skos:narrower rdf:resource="http://resource.geosciml.org/classifier/cgi/compoundmaterialconstituentpartrole/kelyphitic_rim"/>
	<skos:narrower rdf:resource="http://resource.geosciml.org/classifier/cgi/compoundmaterialconstituentpartrole/corrosion_rim"/>
	<skos:prefLabel xml:lang="en">corona</skos:prefLabel>
</rdf:Description>

<rdf:Description rdf:about="http://resource.geosciml.org/classifier/cgi/compoundmaterialconstituentpartrole/corrosion_rim">
	<rdf:type rdf:resource="http://www.w3.org/2004/02/skos/core#Concept"/>
	<dc:source>Neuendorf et al., 2005</dc:source>
	<skos:broader rdf:resource="http://resource.geosciml.org/classifier/cgi/compoundmaterialconstituentpartrole/corona"/>
	<skos:definition>A corona formed by a secondary mineral around an orginal igneous crystal, formed by modification of the crystal by the corrosive action of its parent magma</skos:definition>
	<skos:exactMatch rdf:resource="http://resource.geosciml.org/classifier/cgi/compoundmaterialconstituentpartrole/0008"/>
	<skos:inScheme rdf:resource="http://resource.geosciml.org/classifierscheme/cgi/201211/compoundmaterialconstituentpartrole"/>
	<skos:prefLabel xml:lang="en">corrosion rim</skos:prefLabel>
</rdf:Description>

<rdf:Description rdf:about="http://resource.geosciml.org/classifier/cgi/compoundmaterialconstituentpartrole/crystalline_framework_constituent">
	<rdf:type rdf:resource="http://www.w3.org/2004/02/skos/core#Concept"/>
	<dc:source xml:lang="en">This vocabulary</dc:source>
	<skos:broader rdf:resource="http://resource.geosciml.org/classifier/cgi/compoundmaterialconstituentpartrole/particulate_constituent"/>
	<skos:definition>Constituent forms an interconnected network of discernible crystals.</skos:definition>
	<skos:exactMatch rdf:resource="http://resource.geosciml.org/classifier/cgi/compoundmaterialconstituentpartrole/0009"/>
	<skos:inScheme rdf:resource="http://resource.geosciml.org/classifierscheme/cgi/201211/compoundmaterialconstituentpartrole"/>
	<skos:prefLabel xml:lang="en">crystalline framework constituent</skos:prefLabel>
</rdf:Description>

<rdf:Description rdf:about="http://resource.geosciml.org/classifier/cgi/compoundmaterialconstituentpartrole/dropstone">
	<rdf:type rdf:resource="http://www.w3.org/2004/02/skos/core#Concept"/>
	<dc:source>NADM SLTTs 2004; Jackson, 1997, p 193</dc:source>
	<skos:broader rdf:resource="http://resource.geosciml.org/classifier/cgi/compoundmaterialconstituentpartrole/structural_part"/>
	<skos:definition>"An oversized stone in laminated sediment that depresses the underlying laminae and may be covered by -draped laminae. Most dropstones originate through ice-rafting; other sources are floating tree roots and kelp holdfasts...."</skos:definition>
	<skos:exactMatch rdf:resource="http://resource.geosciml.org/classifier/cgi/compoundmaterialconstituentpartrole/0010"/>
	<skos:inScheme rdf:resource="http://resource.geosciml.org/classifierscheme/cgi/201211/compoundmaterialconstituentpartrole"/>
	<skos:prefLabel xml:lang="en">dropstone</skos:prefLabel>
</rdf:Description>

<rdf:Description rdf:about="http://resource.geosciml.org/classifier/cgi/compoundmaterialconstituentpartrole/epimatrix">
	<rdf:type rdf:resource="http://www.w3.org/2004/02/skos/core#Concept"/>
	<dc:source>NADM SLTTs 2004; Dickinson, 1970</dc:source>
	<skos:broader rdf:resource="http://resource.geosciml.org/classifier/cgi/compoundmaterialconstituentpartrole/matrix"/>
	<skos:definition>A type of matrix consisting of inhomogeneous interstitial materials grown in originally open interstices during diagenesis, but lacking the homogeneity and clear textural evidence of pore-filling needed to classify as phyllosilicate cement.</skos:definition>
	<skos:exactMatch rdf:resource="http://resource.geosciml.org/classifier/cgi/compoundmaterialconstituentpartrole/0011"/>
	<skos:inScheme rdf:resource="http://resource.geosciml.org/classifierscheme/cgi/201211/compoundmaterialconstituentpartrole"/>
	<skos:prefLabel xml:lang="en">epimatrix</skos:prefLabel>
</rdf:Description>

<rdf:Description rdf:about="http://resource.geosciml.org/classifier/cgi/compoundmaterialconstituentpartrole/floating_clast">
	<rdf:type rdf:resource="http://www.w3.org/2004/02/skos/core#Concept"/>
	<dc:source>Pettijohn et al., 1972, p. 90; SMR</dc:source>
	<skos:broader rdf:resource="http://resource.geosciml.org/classifier/cgi/compoundmaterialconstituentpartrole/structural_part"/>
	<skos:definition>Constituent is a clast that has no visible contacts with other clasts. Interpreted to be largely or completly immersed in matrix or cement.</skos:definition>
	<skos:exactMatch rdf:resource="http://resource.geosciml.org/classifier/cgi/compoundmaterialconstituentpartrole/0012"/>
	<skos:inScheme rdf:resource="http://resource.geosciml.org/classifierscheme/cgi/201211/compoundmaterialconstituentpartrole"/>
	<skos:prefLabel xml:lang="en">floating clast</skos:prefLabel>
</rdf:Description>

<rdf:Description rdf:about="http://resource.geosciml.org/classifier/cgi/compoundmaterialconstituentpartrole/granular_framework_constituent">
	<rdf:type rdf:resource="http://www.w3.org/2004/02/skos/core#Concept"/>
	<dc:source>Jackson, 1997, p. 250</dc:source>
	<skos:broader rdf:resource="http://resource.geosciml.org/classifier/cgi/compoundmaterialconstituentpartrole/particulate_constituent"/>
	<skos:definition>"Constituent forms a rigid arrangement of particles that support one another at their points of contact...constituting a mechanically firm structure capable of supporting open pore spaces, although interstices may be occupied by cement or matrix"</skos:definition>
	<skos:exactMatch rdf:resource="http://resource.geosciml.org/classifier/cgi/compoundmaterialconstituentpartrole/0013"/>
	<skos:inScheme rdf:resource="http://resource.geosciml.org/classifierscheme/cgi/201211/compoundmaterialconstituentpartrole"/>
	<skos:prefLabel xml:lang="en">granular framework constituent</skos:prefLabel>
</rdf:Description>

<rdf:Description rdf:about="http://resource.geosciml.org/classifier/cgi/compoundmaterialconstituentpartrole/groundmass_constituent">
	<rdf:type rdf:resource="http://www.w3.org/2004/02/skos/core#Concept"/>
	<dc:source xml:lang="en">This vocabulary</dc:source>
	<skos:broader rdf:resource="http://resource.geosciml.org/classifier/cgi/compoundmaterialconstituentpartrole/interstitial_constituent"/>
	<skos:definition>Constituent forms an interconnected network of material enclosing other constituents that are disguished by larger grain size.</skos:definition>
	<skos:exactMatch rdf:resource="http://resource.geosciml.org/classifier/cgi/compoundmaterialconstituentpartrole/0014"/>
	<skos:inScheme rdf:resource="http://resource.geosciml.org/classifierscheme/cgi/201211/compoundmaterialconstituentpartrole"/>
	<skos:prefLabel xml:lang="en">groundmass constituent</skos:prefLabel>
</rdf:Description>

<rdf:Description rdf:about="http://resource.geosciml.org/classifier/cgi/compoundmaterialconstituentpartrole/inclusion">
	<rdf:type rdf:resource="http://www.w3.org/2004/02/skos/core#Concept"/>
	<dc:source>Neuendorf et al, 2005</dc:source>
	<skos:broader rdf:resource="http://resource.geosciml.org/classifier/cgi/compoundmaterialconstituentpartrole/structural_part"/>
	<skos:definition>a fragment of older material within an igneous rock to which it may or may not be genetically related</skos:definition>
	<skos:exactMatch rdf:resource="http://resource.geosciml.org/classifier/cgi/compoundmaterialconstituentpartrole/0015"/>
	<skos:inScheme rdf:resource="http://resource.geosciml.org/classifierscheme/cgi/201211/compoundmaterialconstituentpartrole"/>
	<skos:narrower rdf:resource="http://resource.geosciml.org/classifier/cgi/compoundmaterialconstituentpartrole/armoured_relict_inclusion"/>
	<skos:prefLabel xml:lang="en">inclusion</skos:prefLabel>
</rdf:Description>

<rdf:Description rdf:about="http://resource.geosciml.org/classifier/cgi/compoundmaterialconstituentpartrole/interstitial_constituent">
	<rdf:type rdf:resource="http://www.w3.org/2004/02/skos/core#Concept"/>
	<dc:source xml:lang="en">This vocabulary</dc:source>
	<skos:definition>Constituent is distributed through the material between other constituent particles</skos:definition>
	<skos:exactMatch rdf:resource="http://resource.geosciml.org/classifier/cgi/compoundmaterialconstituentpartrole/0016"/>
	<skos:inScheme rdf:resource="http://resource.geosciml.org/classifierscheme/cgi/201211/compoundmaterialconstituentpartrole"/>
	<skos:narrower rdf:resource="http://resource.geosciml.org/classifier/cgi/compoundmaterialconstituentpartrole/groundmass_constituent"/>
	<skos:narrower rdf:resource="http://resource.geosciml.org/classifier/cgi/compoundmaterialconstituentpartrole/matrix"/>
	<skos:narrower rdf:resource="http://resource.geosciml.org/classifier/cgi/compoundmaterialconstituentpartrole/sedimentary_rock_cement"/>
	<skos:prefLabel xml:lang="en">interstitial constituent</skos:prefLabel>
	<skos:topConceptOf rdf:resource="http://resource.geosciml.org/classifierscheme/cgi/201211/compoundmaterialconstituentpartrole"/>
</rdf:Description>

<rdf:Description rdf:about="http://resource.geosciml.org/classifier/cgi/compoundmaterialconstituentpartrole/irregular_part">
	<rdf:type rdf:resource="http://www.w3.org/2004/02/skos/core#Concept"/>
	<dc:source xml:lang="en">This vocabulary</dc:source>
	<skos:broader rdf:resource="http://resource.geosciml.org/classifier/cgi/compoundmaterialconstituentpartrole/structural_part"/>
	<skos:definition>A constituent with irregular distribution and geometry, as in pseudobreccia or patch migmatite.</skos:definition>
	<skos:exactMatch rdf:resource="http://resource.geosciml.org/classifier/cgi/compoundmaterialconstituentpartrole/0017"/>
	<skos:inScheme rdf:resource="http://resource.geosciml.org/classifierscheme/cgi/201211/compoundmaterialconstituentpartrole"/>
	<skos:prefLabel xml:lang="en">irregular part</skos:prefLabel>
</rdf:Description>

<rdf:Description rdf:about="http://resource.geosciml.org/classifier/cgi/compoundmaterialconstituentpartrole/kelyphitic_rim">
	<rdf:type rdf:resource="http://www.w3.org/2004/02/skos/core#Concept"/>
	<dc:source>Williams, Turner and Gilbert, 1954; Fettes and Desmons, 2007</dc:source>
	<skos:broader rdf:resource="http://resource.geosciml.org/classifier/cgi/compoundmaterialconstituentpartrole/corona"/>
	<skos:definition>Corona that consists of concentric bands with radial fibrous texture.</skos:definition>
	<skos:exactMatch rdf:resource="http://resource.geosciml.org/classifier/cgi/compoundmaterialconstituentpartrole/0018"/>
	<skos:inScheme rdf:resource="http://resource.geosciml.org/classifierscheme/cgi/201211/compoundmaterialconstituentpartrole"/>
	<skos:prefLabel xml:lang="en">kelyphitic rim</skos:prefLabel>
</rdf:Description>

<rdf:Description rdf:about="http://resource.geosciml.org/classifier/cgi/compoundmaterialconstituentpartrole/layer">
	<rdf:type rdf:resource="http://www.w3.org/2004/02/skos/core#Concept"/>
	<dc:source xml:lang="en">This vocabulary</dc:source>
	<skos:broader rdf:resource="http://resource.geosciml.org/classifier/cgi/compoundmaterialconstituentpartrole/structural_part"/>
	<skos:definition>A thin sheet compositionally distinct from the surrounding material, related to primary genesis of rock, e.g. sedimentary layers, metamorphic segregation</skos:definition>
	<skos:exactMatch rdf:resource="http://resource.geosciml.org/classifier/cgi/compoundmaterialconstituentpartrole/0019"/>
	<skos:inScheme rdf:resource="http://resource.geosciml.org/classifierscheme/cgi/201211/compoundmaterialconstituentpartrole"/>
	<skos:prefLabel xml:lang="en">layer</skos:prefLabel>
</rdf:Description>

<rdf:Description rdf:about="http://resource.geosciml.org/classifier/cgi/compoundmaterialconstituentpartrole/matrix">
	<rdf:type rdf:resource="http://www.w3.org/2004/02/skos/core#Concept"/>
	<dc:source>NADM SLTTs 2004; Jackson, 1997</dc:source>
	<skos:broader rdf:resource="http://resource.geosciml.org/classifier/cgi/compoundmaterialconstituentpartrole/interstitial_constituent"/>
	<skos:definition>Constituent forms finer-grained material interstitial to a framework constituent. "The finer-grained material enclosing, or filling the interstices between, the larger grains or particles of a sediment or sedimentary rock....The term refers to the relative size and disposition of the particles, and no particular particle size is implied" (Jackson, 1997, p. 393). May be classifiable into orthomatrix, protomatrix, epimatrix, pseudomatrix, and unclassified matrix.</skos:definition>
	<skos:exactMatch rdf:resource="http://resource.geosciml.org/classifier/cgi/compoundmaterialconstituentpartrole/0020"/>
	<skos:inScheme rdf:resource="http://resource.geosciml.org/classifierscheme/cgi/201211/compoundmaterialconstituentpartrole"/>
	<skos:narrower rdf:resource="http://resource.geosciml.org/classifier/cgi/compoundmaterialconstituentpartrole/orthomatrix"/>
	<skos:narrower rdf:resource="http://resource.geosciml.org/classifier/cgi/compoundmaterialconstituentpartrole/epimatrix"/>
	<skos:narrower rdf:resource="http://resource.geosciml.org/classifier/cgi/compoundmaterialconstituentpartrole/protomatrix"/>
	<skos:narrower rdf:resource="http://resource.geosciml.org/classifier/cgi/compoundmaterialconstituentpartrole/pseudomatrix"/>
	<skos:prefLabel xml:lang="en">matrix</skos:prefLabel>
</rdf:Description>

<rdf:Description rdf:about="http://resource.geosciml.org/classifier/cgi/compoundmaterialconstituentpartrole/megacryst">
	<rdf:type rdf:resource="http://www.w3.org/2004/02/skos/core#Concept"/>
	<dc:source>Neuendorf et al 2005</dc:source>
	<skos:broader rdf:resource="http://resource.geosciml.org/classifier/cgi/compoundmaterialconstituentpartrole/particulate_constituent"/>
	<skos:definition>any crystal in an igneous or metamorphic rock that is sgnificantly larger than the surounding groundmass. May be a phenocryst, xenocryst, porphyroblast or porphyroclast</skos:definition>
	<skos:exactMatch rdf:resource="http://resource.geosciml.org/classifier/cgi/compoundmaterialconstituentpartrole/0021"/>
	<skos:inScheme rdf:resource="http://resource.geosciml.org/classifierscheme/cgi/201211/compoundmaterialconstituentpartrole"/>
	<skos:narrower rdf:resource="http://resource.geosciml.org/classifier/cgi/compoundmaterialconstituentpartrole/phenocryst"/>
	<skos:narrower rdf:resource="http://resource.geosciml.org/classifier/cgi/compoundmaterialconstituentpartrole/porphyroblast"/>
	<skos:narrower rdf:resource="http://resource.geosciml.org/classifier/cgi/compoundmaterialconstituentpartrole/porphyroclast"/>
	<skos:prefLabel xml:lang="en">megacryst</skos:prefLabel>
</rdf:Description>

<rdf:Description rdf:about="http://resource.geosciml.org/classifier/cgi/compoundmaterialconstituentpartrole/oikocryst">
	<rdf:type rdf:resource="http://www.w3.org/2004/02/skos/core#Concept"/>
	<dc:source>Neuendorf et al., 2005</dc:source>
	<skos:broader rdf:resource="http://resource.geosciml.org/classifier/cgi/compoundmaterialconstituentpartrole/particulate_constituent"/>
	<skos:definition>Constituent occurs as crystals that poikilitically enclose crystals of other phases in an igneous rock.</skos:definition>
	<skos:exactMatch rdf:resource="http://resource.geosciml.org/classifier/cgi/compoundmaterialconstituentpartrole/0022"/>
	<skos:inScheme rdf:resource="http://resource.geosciml.org/classifierscheme/cgi/201211/compoundmaterialconstituentpartrole"/>
	<skos:prefLabel xml:lang="en">oikocryst</skos:prefLabel>
</rdf:Description>

<rdf:Description rdf:about="http://resource.geosciml.org/classifier/cgi/compoundmaterialconstituentpartrole/orthomatrix">
	<rdf:type rdf:resource="http://www.w3.org/2004/02/skos/core#Concept"/>
	<dc:source>NADM SLTTs 2004; Dickinson, 1970</dc:source>
	<skos:broader rdf:resource="http://resource.geosciml.org/classifier/cgi/compoundmaterialconstituentpartrole/matrix"/>
	<skos:definition>A type of matrix consisting of recrystallized detrital lutum (clay fraction, less than 2 micron) or protomatrix.</skos:definition>
	<skos:exactMatch rdf:resource="http://resource.geosciml.org/classifier/cgi/compoundmaterialconstituentpartrole/0023"/>
	<skos:inScheme rdf:resource="http://resource.geosciml.org/classifierscheme/cgi/201211/compoundmaterialconstituentpartrole"/>
	<skos:narrower rdf:resource="http://resource.geosciml.org/classifier/cgi/compoundmaterialconstituentpartrole/clast_supporting_orthomatrix"/>
	<skos:prefLabel xml:lang="en">orthomatrix</skos:prefLabel>
</rdf:Description>

<rdf:Description rdf:about="http://resource.geosciml.org/classifier/cgi/compoundmaterialconstituentpartrole/overgrowth">
	<rdf:type rdf:resource="http://www.w3.org/2004/02/skos/core#Concept"/>
	<dc:source>NADM SLTTs 2004; Neuendorf et al. 2005</dc:source>
	<skos:broader rdf:resource="http://resource.geosciml.org/classifier/cgi/compoundmaterialconstituentpartrole/structural_part"/>
	<skos:definition>Constituent crystallized in crystallographic continuity with some other mineral constituent, typically quartz or calcite. In a clastic rock, commonly forms cement as well, but this should be represented using two role attribute links, 'overgrowth' and cement, because overgrowth does not necessarily imply cement.</skos:definition>
	<skos:exactMatch rdf:resource="http://resource.geosciml.org/classifier/cgi/compoundmaterialconstituentpartrole/0024"/>
	<skos:inScheme rdf:resource="http://resource.geosciml.org/classifierscheme/cgi/201211/compoundmaterialconstituentpartrole"/>
	<skos:prefLabel xml:lang="en">overgrowth</skos:prefLabel>
</rdf:Description>

<rdf:Description rdf:about="http://resource.geosciml.org/classifier/cgi/compoundmaterialconstituentpartrole/particulate_constituent">
	<rdf:type rdf:resource="http://www.w3.org/2004/02/skos/core#Concept"/>
	<dc:source xml:lang="en">This vocabulary</dc:source>
	<skos:definition>constituent occurs as a collection of particles that are characterized by average properties of the individual particles</skos:definition>
	<skos:exactMatch rdf:resource="http://resource.geosciml.org/classifier/cgi/compoundmaterialconstituentpartrole/0025"/>
	<skos:inScheme rdf:resource="http://resource.geosciml.org/classifierscheme/cgi/201211/compoundmaterialconstituentpartrole"/>
	<skos:narrower rdf:resource="http://resource.geosciml.org/classifier/cgi/compoundmaterialconstituentpartrole/megacryst"/>
	<skos:narrower rdf:resource="http://resource.geosciml.org/classifier/cgi/compoundmaterialconstituentpartrole/chadacryst"/>
	<skos:narrower rdf:resource="http://resource.geosciml.org/classifier/cgi/compoundmaterialconstituentpartrole/phenoclast"/>
	<skos:narrower rdf:resource="http://resource.geosciml.org/classifier/cgi/compoundmaterialconstituentpartrole/oikocryst"/>
	<skos:narrower rdf:resource="http://resource.geosciml.org/classifier/cgi/compoundmaterialconstituentpartrole/crystalline_framework_constituent"/>
	<skos:narrower rdf:resource="http://resource.geosciml.org/classifier/cgi/compoundmaterialconstituentpartrole/armoured_relict_crystal"/>
	<skos:narrower rdf:resource="http://resource.geosciml.org/classifier/cgi/compoundmaterialconstituentpartrole/granular_framework_constituent"/>
	<skos:prefLabel xml:lang="en">particulate constituent</skos:prefLabel>
	<skos:topConceptOf rdf:resource="http://resource.geosciml.org/classifierscheme/cgi/201211/compoundmaterialconstituentpartrole"/>
</rdf:Description>

<rdf:Description rdf:about="http://resource.geosciml.org/classifier/cgi/compoundmaterialconstituentpartrole/phenoclast">
	<rdf:type rdf:resource="http://www.w3.org/2004/02/skos/core#Concept"/>
	<dc:source>Neuendorf et al., 2005</dc:source>
	<skos:broader rdf:resource="http://resource.geosciml.org/classifier/cgi/compoundmaterialconstituentpartrole/particulate_constituent"/>
	<skos:definition>a relatively large and conspicuous fragment in a sediment or sedimentary rock</skos:definition>
	<skos:exactMatch rdf:resource="http://resource.geosciml.org/classifier/cgi/compoundmaterialconstituentpartrole/0026"/>
	<skos:inScheme rdf:resource="http://resource.geosciml.org/classifierscheme/cgi/201211/compoundmaterialconstituentpartrole"/>
	<skos:prefLabel xml:lang="en">phenoclast</skos:prefLabel>
</rdf:Description>

<rdf:Description rdf:about="http://resource.geosciml.org/classifier/cgi/compoundmaterialconstituentpartrole/phenocryst">
	<rdf:type rdf:resource="http://www.w3.org/2004/02/skos/core#Concept"/>
	<dc:source>Neuendorf et al. 2005</dc:source>
	<skos:broader rdf:resource="http://resource.geosciml.org/classifier/cgi/compoundmaterialconstituentpartrole/megacryst"/>
	<skos:definition>Constituent occurs as crystals that are distinctly larger than a groundmass of enclosing crystals. Used only in igneous rocks.</skos:definition>
	<skos:exactMatch rdf:resource="http://resource.geosciml.org/classifier/cgi/compoundmaterialconstituentpartrole/0027"/>
	<skos:inScheme rdf:resource="http://resource.geosciml.org/classifierscheme/cgi/201211/compoundmaterialconstituentpartrole"/>
	<skos:prefLabel xml:lang="en">phenocryst</skos:prefLabel>
</rdf:Description>

<rdf:Description rdf:about="http://resource.geosciml.org/classifier/cgi/compoundmaterialconstituentpartrole/porphyroblast">
	<rdf:type rdf:resource="http://www.w3.org/2004/02/skos/core#Concept"/>
	<dc:source>Fettes and Desmons, 2007</dc:source>
	<skos:broader rdf:resource="http://resource.geosciml.org/classifier/cgi/compoundmaterialconstituentpartrole/megacryst"/>
	<skos:definition>Constituent occurs as crystals formed by metamorphic crystallization, set in a finer-grained groundmass.</skos:definition>
	<skos:exactMatch rdf:resource="http://resource.geosciml.org/classifier/cgi/compoundmaterialconstituentpartrole/0028"/>
	<skos:inScheme rdf:resource="http://resource.geosciml.org/classifierscheme/cgi/201211/compoundmaterialconstituentpartrole"/>
	<skos:prefLabel xml:lang="en">porphyroblast</skos:prefLabel>
</rdf:Description>

<rdf:Description rdf:about="http://resource.geosciml.org/classifier/cgi/compoundmaterialconstituentpartrole/porphyroclast">
	<rdf:type rdf:resource="http://www.w3.org/2004/02/skos/core#Concept"/>
	<dc:source xml:lang="en">Spry, 1969</dc:source>
	<skos:broader rdf:resource="http://resource.geosciml.org/classifier/cgi/compoundmaterialconstituentpartrole/megacryst"/>
	<skos:definition>Relict crystal in metamorphic rock, in groundmass of relatively finer-grained material. Connotes that groundmass is result of tectonic reduction in grain size.</skos:definition>
	<skos:exactMatch rdf:resource="http://resource.geosciml.org/classifier/cgi/compoundmaterialconstituentpartrole/0029"/>
	<skos:inScheme rdf:resource="http://resource.geosciml.org/classifierscheme/cgi/201211/compoundmaterialconstituentpartrole"/>
	<skos:prefLabel xml:lang="en">porphyroclast</skos:prefLabel>
</rdf:Description>

<rdf:Description rdf:about="http://resource.geosciml.org/classifier/cgi/compoundmaterialconstituentpartrole/protomatrix">
	<rdf:type rdf:resource="http://www.w3.org/2004/02/skos/core#Concept"/>
	<dc:source>NADM SLTTs 2004; Dickinson, 1970</dc:source>
	<skos:broader rdf:resource="http://resource.geosciml.org/classifier/cgi/compoundmaterialconstituentpartrole/matrix"/>
	<skos:definition>A type of matrix consisting of un-recrystallized detrital clayey lutum (clay fraction, less than 2 micron) in weakly consolidated rocks.</skos:definition>
	<skos:exactMatch rdf:resource="http://resource.geosciml.org/classifier/cgi/compoundmaterialconstituentpartrole/0030"/>
	<skos:inScheme rdf:resource="http://resource.geosciml.org/classifierscheme/cgi/201211/compoundmaterialconstituentpartrole"/>
	<skos:prefLabel xml:lang="en">protomatrix</skos:prefLabel>
</rdf:Description>

<rdf:Description rdf:about="http://resource.geosciml.org/classifier/cgi/compoundmaterialconstituentpartrole/pseudomatrix">
	<rdf:type rdf:resource="http://www.w3.org/2004/02/skos/core#Concept"/>
	<dc:source>NADM SLTTs 2004; Dickinson, 1970</dc:source>
	<skos:broader rdf:resource="http://resource.geosciml.org/classifier/cgi/compoundmaterialconstituentpartrole/matrix"/>
	<skos:definition>A type of matrix consisting of soft deformable framework grains that are squeezed and flattened between stronger framework grains.</skos:definition>
	<skos:exactMatch rdf:resource="http://resource.geosciml.org/classifier/cgi/compoundmaterialconstituentpartrole/0031"/>
	<skos:inScheme rdf:resource="http://resource.geosciml.org/classifierscheme/cgi/201211/compoundmaterialconstituentpartrole"/>
	<skos:prefLabel xml:lang="en">pseudomatrix</skos:prefLabel>
</rdf:Description>

<rdf:Description rdf:about="http://resource.geosciml.org/classifier/cgi/compoundmaterialconstituentpartrole/sedimentary_rock_cement">
	<rdf:type rdf:resource="http://www.w3.org/2004/02/skos/core#Concept"/>
	<dc:source>NADM SLTTs 2004; Jackson, 1997</dc:source>
	<skos:broader rdf:resource="http://resource.geosciml.org/classifier/cgi/compoundmaterialconstituentpartrole/interstitial_constituent"/>
	<skos:definition>A constituent that occupies space between individual grains of a consolidated sedimentary rock, and binds the grains together as a rigid, coherent mass; it may be derived from the sediment or its entrapped waters, or it may be brought in by solution from outside sources. Material is usually chemically precipitated (Jackson, 1997, p. 103). Distinguished from matrix by clearly secondary origin and generally monomineralic character.</skos:definition>
	<skos:exactMatch rdf:resource="http://resource.geosciml.org/classifier/cgi/compoundmaterialconstituentpartrole/0032"/>
	<skos:inScheme rdf:resource="http://resource.geosciml.org/classifierscheme/cgi/201211/compoundmaterialconstituentpartrole"/>
	<skos:prefLabel xml:lang="en">sedimentary rock cement</skos:prefLabel>
</rdf:Description>

<rdf:Description rdf:about="http://resource.geosciml.org/classifier/cgi/compoundmaterialconstituentpartrole/small_concretion">
	<rdf:type rdf:resource="http://www.w3.org/2004/02/skos/core#Concept"/>
	<dc:source>Neuendorf et al, 2005</dc:source>
	<skos:broader rdf:resource="http://resource.geosciml.org/classifier/cgi/compoundmaterialconstituentpartrole/structural_part"/>
	<skos:definition>A hard, compact mass or aggregate of mineral matter, normally subsperical but commonly oblate, disc-shaped or irregular. Formed by precipitation of mineral from solution in the pores of a granular rock, localized around a nucleus or center, to define a discrete, sharply separated object. Size ranges from cm to decimeter for application as a compoundMaterialConstituentPart; larger concretions should be considered GeologicUnit parts.</skos:definition>
	<skos:exactMatch rdf:resource="http://resource.geosciml.org/classifier/cgi/compoundmaterialconstituentpartrole/0033"/>
	<skos:inScheme rdf:resource="http://resource.geosciml.org/classifierscheme/cgi/201211/compoundmaterialconstituentpartrole"/>
	<skos:prefLabel xml:lang="en">small concretion</skos:prefLabel>
</rdf:Description>

<rdf:Description rdf:about="http://resource.geosciml.org/classifier/cgi/compoundmaterialconstituentpartrole/structural_part">
	<rdf:type rdf:resource="http://www.w3.org/2004/02/skos/core#Concept"/>
	<dc:source xml:lang="en">This vocabulary</dc:source>
	<skos:definition>Constituent occurs in a structural configuration integral to the rock, such as layering, veinlets, overgrowths. The 'material' composition of these parts will often be other rock materials, not minerals, and 'ParticleGeometryDescription' associated with these describes the geometry of the constituent, not the particles the it is made of. These roles are mostly useful for RockMaterial descriptions that apply to individual samples, because their distribution is unlikely to be pervasive enought to be considered characteristic of a large mass of material.</skos:definition>
	<skos:exactMatch rdf:resource="http://resource.geosciml.org/classifier/cgi/compoundmaterialconstituentpartrole/0034"/>
	<skos:historyNote xml:lang="en">2010-02-12 Add narrower relationship links by adding skos:narrower link in Protege, defining skos:narrower as inverse of skos:broader, calculating with Pellet reasoner to add inferred axioms, and using 'file/Export inferred axioms as ontology' in Protege.</skos:historyNote>
	<skos:inScheme rdf:resource="http://resource.geosciml.org/classifierscheme/cgi/201211/compoundmaterialconstituentpartrole"/>
	<skos:narrower rdf:resource="http://resource.geosciml.org/classifier/cgi/compoundmaterialconstituentpartrole/irregular_part"/>
	<skos:narrower rdf:resource="http://resource.geosciml.org/classifier/cgi/compoundmaterialconstituentpartrole/dropstone"/>
	<skos:narrower rdf:resource="http://resource.geosciml.org/classifier/cgi/compoundmaterialconstituentpartrole/overgrowth"/>
	<skos:narrower rdf:resource="http://resource.geosciml.org/classifier/cgi/compoundmaterialconstituentpartrole/clot"/>
	<skos:narrower rdf:resource="http://resource.geosciml.org/classifier/cgi/compoundmaterialconstituentpartrole/small_concretion"/>
	<skos:narrower rdf:resource="http://resource.geosciml.org/classifier/cgi/compoundmaterialconstituentpartrole/corona"/>
	<skos:narrower rdf:resource="http://resource.geosciml.org/classifier/cgi/compoundmaterialconstituentpartrole/layer"/>
	<skos:narrower rdf:resource="http://resource.geosciml.org/classifier/cgi/compoundmaterialconstituentpartrole/floating_clast"/>
	<skos:narrower rdf:resource="http://resource.geosciml.org/classifier/cgi/compoundmaterialconstituentpartrole/vein"/>
	<skos:narrower rdf:resource="http://resource.geosciml.org/classifier/cgi/compoundmaterialconstituentpartrole/inclusion"/>
	<skos:prefLabel xml:lang="en">structural part</skos:prefLabel>
	<skos:topConceptOf rdf:resource="http://resource.geosciml.org/classifierscheme/cgi/201211/compoundmaterialconstituentpartrole"/>
</rdf:Description>

<rdf:Description rdf:about="http://resource.geosciml.org/classifier/cgi/compoundmaterialconstituentpartrole/vein">
	<rdf:type rdf:resource="http://www.w3.org/2004/02/skos/core#Concept"/>
	<dc:source xml:lang="en">This vocabulary</dc:source>
	<skos:broader rdf:resource="http://resource.geosciml.org/classifier/cgi/compoundmaterialconstituentpartrole/structural_part"/>
	<skos:definition>Thin sheet of material intruded into the rock. May be hydrothermal, magmatic, or sedimentary.</skos:definition>
	<skos:exactMatch rdf:resource="http://resource.geosciml.org/classifier/cgi/compoundmaterialconstituentpartrole/0035"/>
	<skos:inScheme rdf:resource="http://resource.geosciml.org/classifierscheme/cgi/201211/compoundmaterialconstituentpartrole"/>
	<skos:prefLabel xml:lang="en">vein</skos:prefLabel>
</rdf:Description>

<rdf:Description rdf:about="http://resource.geosciml.org/classifierscheme/cgi/201211/compoundmaterialconstituentpartrole">
	<rdf:type rdf:resource="http://www.w3.org/2002/07/owl#Ontology"/>
	<rdf:type rdf:resource="http://www.w3.org/2004/02/skos/core#ConceptScheme"/>
	<dc:creator>Concept Definition Task Group of IUGS CGI Interoperability Working Group (http://www.cgi-iugs.org/tech_collaboration/interoperability_working_group.html)</dc:creator>
	<dc:format>application/rdf+xml</dc:format>
	<dc:identifier rdf:datatype="http://www.w3.org/2001/XMLSchema#string">http://resource.geosciml.org/classifierscheme/cgi/201211/compoundmaterialconstituentpartrole</dc:identifier>
	<dc:language>en</dc:language>
	<dc:publisher>Concept Definition Task Group of IUGS CGI Interoperability Working Group (http://www.cgi-iugs.org/tech_collaboration/interoperability_working_group.html).</dc:publisher>
	<dc:title xml:lang="en">CGI compound Material Constituent Part Role vocabulary</dc:title>
	<owl:imports rdf:resource="http://www.w3.org/2004/02/skos/core"/>
	<owl:imports rdf:resource="http://rdfs.org/ns/void"/>
	<owl:versionInfo>201202</owl:versionInfo>
	<skos:changeNote xml:lang="en">2009-12-07 SMR Update metadata properties for version, creator, title, and format.  Change skos:HistoryNote to dc:source for information on origin of terms and definitions.</skos:changeNote>
	<skos:definition xml:lang="en">This file contains the 200811 version of CGI compound material constituent part vocabulary. Use to categorize kinds of particles that are the constituents of a compound material.</skos:definition>
	<skos:historyNote xml:lang="en">2010-02-08. SMR Clean up namespace declarations so concept URI's follow CGI URN scheme; concepts have URN, are not document fragments.</skos:historyNote>
	<skos:historyNote xml:lang="en">2009-07-14. create rdf/skos from excel spreadsheet.</skos:historyNote>
	<skos:historyNote xml:lang="en">2010-02-08 add top property assertions for root elements</skos:historyNote>
	<skos:historyNote xml:lang="en">2012-11-24 SMR Update to 201211 version; add collection entity, check all pref labels are lower case, remove owl:NamedIndividual and Owl:Thing rdf:types.</skos:historyNote>
	<skos:historyNote xml:lang="en">2012-02-07 SMR update URI to replace numeric final token with English-language string as in original URN scheme.</skos:historyNote>
	<skos:prefLabel xml:lang="en">CGI compound Material Constituent Part Role vocabulary</skos:prefLabel>
</rdf:Description>

<rdf:Description rdf:about="http://resource.geosciml.org/vocabulary/cgi/201211/compoundmaterialconstituentpartrole">
	<rdf:type rdf:resource="http://rdfs.org/ns/void#Dataset"/>
	<rdfs:label rdf:datatype="http://www.w3.org/2001/XMLSchema#string">Compound material constituent part role vocabulary</rdfs:label>
</rdf:Description>

<rdf:Description rdf:about="http://www.w3.org/2004/02/skos/core#ConceptScheme">
	<rdf:type rdf:resource="http://www.w3.org/2002/07/owl#Class"/>
</rdf:Description>

</rdf:RDF>