# baseURI: http://resource.geosciml.org/classifierscheme/cgi/201211/deformationstyle
# imports: http://rdfs.org/ns/void
# imports: http://www.w3.org/2004/02/skos/core

@prefix cgi:     <http://resource.geosciml.org/classifierscheme/cgi/201211/> .
@prefix dc:      <http://purl.org/dc/elements/1.1/> .
@prefix defstyle:  <http://resource.geosciml.org/classifier/cgi/deformationstyle/> .
@prefix owl:     <http://www.w3.org/2002/07/owl#> .
@prefix owl2xml:  <http://www.w3.org/2006/12/owl2-xml#> .
@prefix rdf:     <http://www.w3.org/1999/02/22-rdf-syntax-ns#> .
@prefix rdfs:    <http://www.w3.org/2000/01/rdf-schema#> .
@prefix skos:    <http://www.w3.org/2004/02/skos/core#> .
@prefix cgivoc:	<http://resource.geosciml.org/vocabulary/cgi/201211/> .
@prefix void:    <http://rdfs.org/ns/void#> .
@prefix xsd:     <http://www.w3.org/2001/XMLSchema#> .

defstyle:
      rdf:type skos:Collection ;
      rdfs:label "fault deformation style concepts"@en ;
      skos:definition "This resource defines the concept space for fault deformation styles by extension; it includes all concepts in this conceptScheme, as well as concepts in previous versions of the scheme."@en ;
      skos:member defstyle:mixed_brittle_ductile , defstyle:brittle , defstyle:ductile ;
      skos:prefLabel "CGI Fault Deformation Style"@en .

defstyle:brittle
      rdf:type skos:Concept ;
      dc:source "this vocabulary"@en ;
      skos:definition "Deformation in fault zone has been accommodated primarily through fracturing and loss of continuity between adjacent rock bodies."@en ;
      skos:inScheme cgi:deformationstyle ;
      skos:prefLabel "brittle deformation"@en ;
      skos:topConceptOf cgi:deformationstyle .

defstyle:ductile
      rdf:type skos:Concept ;
      dc:source "this vocabulary"@en ;
      skos:definition "Displacement across shear displacement structure largely accommodated by plastic deformation of the rock body without loss of macroscopic continuity."@en ;
      skos:inScheme cgi:deformationstyle ;
      skos:prefLabel "ductile deformation style"@en ;
      skos:topConceptOf cgi:deformationstyle .

defstyle:mixed_brittle_ductile
      rdf:type skos:Concept ;
      dc:source "this vocabulary"@en ;
      skos:definition "deformation in fault zone has been accommodated by both fracturing and plastic shape change in rock bodies."@en ;
      skos:inScheme cgi:deformationstyle ;
      skos:prefLabel "mixed brittle and ductile"@en ;
      skos:topConceptOf cgi:deformationstyle .

cgi:deformationstyle
      rdf:type skos:ConceptScheme , owl:Ontology ;
      dc:creator "Concept Definition Task Group of IUGS CGI Interoperability Working Group (http://www.cgi-iugs.org/tech_collaboration/interoperability_working_group.html)" ;
      dc:format "application/rdf+xml" ;
      dc:identifier "http://resource.geosciml.org/classifierscheme/cgi/201211/deformationstyle" ;
      dc:language "en" ;
      dc:publisher "Concept Definition Task Group of IUGS CGI Interoperability Working Group (http://www.cgi-iugs.org/tech_collaboration/interoperability_working_group.html)" ;
      dc:title "CGI deformation style vocabulary"@en ;
      owl:imports <http://www.w3.org/2004/02/skos/core> , <http://rdfs.org/ns/void> ;
      owl:versionInfo "201204" ;
      skos:historyNote "Created 2012-04 by S.M. Richard"@en , "2012-11-24 SMR Update to 201211 version; add collection entity, check all pref labels are lower case, remove owl:NamedIndividual and Owl:Thing rdf:types."@en .

<http://resource.geosciml.org/vocabulary/cgi/201211/deformationstyle>
      rdf:type void:Dataset ;
      rdfs:label "Deformation style vocabulary"^^xsd:string .
