# baseURI: http://resource.geosciml.org/classifierscheme/cgi/201211/descriptionpurpose
# imports: http://rdfs.org/ns/void
# imports: http://www.w3.org/2004/02/skos/core

@prefix DescriptionPurpose:  <http://resource.geosciml.org/classifier/cgi/descriptionpurpose/> .
@prefix cgi:     <http://resource.geosciml.org/classifierscheme/cgi/201211/> .
@prefix dc:      <http://purl.org/dc/elements/1.1/> .
@prefix owl:     <http://www.w3.org/2002/07/owl#> .
@prefix owl2xml:  <http://www.w3.org/2006/12/owl2-xml#> .
@prefix rdf:     <http://www.w3.org/1999/02/22-rdf-syntax-ns#> .
@prefix rdfs:    <http://www.w3.org/2000/01/rdf-schema#> .
@prefix skos:    <http://www.w3.org/2004/02/skos/core#> .
@prefix void:    <http://rdfs.org/ns/void#> .
@prefix xsd:     <http://www.w3.org/2001/XMLSchema#> .

DescriptionPurpose:
      rdf:type skos:Collection ;
      rdfs:label "description purpose concepts"@en ;
      skos:definition "This resource defines the concept space for description purpose concepts by extension; it includes all concepts in this conceptScheme, as well as concepts in previous versions of the scheme."@en ;
      skos:member DescriptionPurpose:defining_norm , DescriptionPurpose:instance , DescriptionPurpose:typical_norm ;
      skos:prefLabel "CGI Description Purpose"@en .

<http://resource.geosciml.org/classifier/cgi/descriptionpurpose/0001>
      rdf:type owl:NamedIndividual .

<http://resource.geosciml.org/classifier/cgi/descriptionpurpose/0002>
      rdf:type owl:NamedIndividual .

<http://resource.geosciml.org/classifier/cgi/descriptionpurpose/0003>
      rdf:type owl:NamedIndividual .

DescriptionPurpose:defining_norm
      rdf:type skos:Concept ;
      dc:source "GeoSciML UML model scope notes" ;
      skos:definition "A description that specifies properties sufficient to identify a new occurrence as belonging to the class represented by the description. Basically these are the 'sufficient conditions' for class membership. Used when presented with a query 'I have an outcrop with these properties; which geologic unit should I assign to the outcrop?' DefiningNorm has to do with the intension of a ControlledConcept." ;
      skos:exactMatch <http://resource.geosciml.org/classifier/cgi/descriptionpurpose/0001> ;
      skos:inScheme cgi:descriptionpurpose ;
      skos:prefLabel "defining norm" .

DescriptionPurpose:instance
      rdf:type skos:Concept ;
      dc:source "GeoSciML UML model scope notes" ;
      skos:definition "A description that is specific to a particular observed occurrence. This is 'raw data', and its classification may start out as very general. There are kinds of narrowly defined ControlledConcepts that might not allow 'instances' that are different from the DefiningNorm. It might be worth considering a different relationship between MappedFeature and an Instance GeologicEntity, with the GeologicEntity role being 'description'." ;
      skos:exactMatch <http://resource.geosciml.org/classifier/cgi/descriptionpurpose/0002> ;
      skos:inScheme cgi:descriptionpurpose ;
      skos:prefLabel "instance"@en .

DescriptionPurpose:typical_norm
      rdf:type skos:Concept ;
      dc:source "GeoSciML UML model scope notes" ;
      skos:definition "A description that specifies properties to be expected of some occurrence associated with the GeologicEntity. This description may include many properties that are not part of the DefiningNorm. For example, the fact that granite is typically light-colored is not a defining property, but is certainly a useful typical property. These kinds of descriptions would be used to address queries like 'This area is within a polygon classified as Podunk Formation; what sort of lithology am I most likely to encounter when I start digging?' The Podunk Formation may be defined by the presence of a certain ammonite... TypicalNorm description would be constructed as a summary over many Instance descriptions." ;
      skos:exactMatch <http://resource.geosciml.org/classifier/cgi/descriptionpurpose/0003> ;
      skos:inScheme cgi:descriptionpurpose ;
      skos:prefLabel "typical norm" .

cgi:descriptionpurpose
      rdf:type owl:Ontology , skos:ConceptScheme ;
      dc:creator "Concept Definition Task Group of IUGS CGI Interoperability Working Group (http://www.cgi-iugs.org/tech_collaboration/interoperability_working_group.html)" ;
      dc:format "application/rdf+xml" ;
      dc:identifier "http://resource.geosciml.org/classifierscheme/cgi/201211/descriptionpurpose" ;
      dc:language "en" ;
      dc:publisher "Concept Definition Task Group of IUGS CGI Interoperability Working Group (http://www.cgi-iugs.org/tech_collaboration/interoperability_working_group.html)" ;
      dc:title "CGI Description Purpose Terms Vocabulary"@en ;
      owl:imports <http://www.w3.org/2004/02/skos/core> , <http://rdfs.org/ns/void> ;
      owl:versionInfo "201211" ;
      skos:definition "This file contains the CGI Description Purpose codelist. Codes used for the specification of the intended purpose/level of abstraction for a given feature or object instance, ie the reason for the existence of the GeologicFeature. Values: Instance, TypicalNorm, IdentifyingNorm."@en ;
      skos:historyNote "2010-11-27 SMR update URN to http URI, create version 201202"@en , "2009-07-14. Generate SKOS encoding of vocabulary from Excel spreadsheet."@en , "2012-02-07 SMR update URI to replace numeric final token with English-language string as in original URN scheme."@en , "2010-02-08. SMR Clean up namespace declarations so concept URI's follow CGI URN scheme; concepts have URN, are not document fragments."@en , "2009-12-07 SMR Update metadata properties for version, creator, title, and format.  Change skos:HistoryNote to dc:source for information on origin of terms and definitions."@en , "2012-11-24 SMR Update to 201211 version; add collection entity, check all pref labels are lower case, remove owl:NamedIndividual and Owl:Thing rdf:types."@en , "2012-02-27 SMR add skos:exactMatch triples to map URIs for concepts in this vocabulary to number-token URIs in 201012 version of same concepts."@en ;
      skos:prefLabel "CGI Description Purpose Terms Vocabulary"@en .

<http://resource.geosciml.org/vocabulary/cgi/201211/descriptionpurpose>
      rdf:type void:Dataset ;
      rdfs:label "Description purpose vocabulary"^^xsd:string .

skos:ConceptScheme
      rdf:type owl:Class .
