# baseURI: http://resource.geosciml.org/classifierscheme/cgi/201211/determinationmethodorientation
# imports: http://rdfs.org/ns/void
# imports: http://www.w3.org/2004/02/skos/core

@prefix cgi:     <http://resource.geosciml.org/classifierscheme/cgi/201211/> .
@prefix dc:      <http://purl.org/dc/elements/1.1/> .
@prefix detmeth:  <http://resource.geosciml.org/classifier/cgi/determinationmethodorientation/> .
@prefix owl:     <http://www.w3.org/2002/07/owl#> .
@prefix owl2xml:  <http://www.w3.org/2006/12/owl2-xml#> .
@prefix rdf:     <http://www.w3.org/1999/02/22-rdf-syntax-ns#> .
@prefix rdfs:    <http://www.w3.org/2000/01/rdf-schema#> .
@prefix skos:    <http://www.w3.org/2004/02/skos/core#> .
@prefix void:    <http://rdfs.org/ns/void#> .
@prefix xsd:     <http://www.w3.org/2001/XMLSchema#> .

detmeth:
      rdf:type skos:Collection ;
      rdfs:label "orientation determination method concepts"@en ;
      skos:member detmeth:standard_on_site_measure , detmeth:measure_on_outcrop , detmeth:three_point_determination , detmeth:estimate_from_air_photo , detmeth:visual_surface_estimation_on_outcrop , detmeth:photogeologic_determination , detmeth:calculated_average_orientation , detmeth:estimate_from_distance , detmeth:method_unknown ;
      skos:prefLabel "CGI Orientation Determination Method"@en .

<http://resource.geosciml.org/classifier/cgi/determinationmethodorientation/0001>
      rdf:type owl:NamedIndividual .

<http://resource.geosciml.org/classifier/cgi/determinationmethodorientation/0002>
      rdf:type owl:NamedIndividual .

<http://resource.geosciml.org/classifier/cgi/determinationmethodorientation/0003>
      rdf:type owl:NamedIndividual .

<http://resource.geosciml.org/classifier/cgi/determinationmethodorientation/0004>
      rdf:type owl:NamedIndividual .

<http://resource.geosciml.org/classifier/cgi/determinationmethodorientation/0005>
      rdf:type owl:NamedIndividual .

<http://resource.geosciml.org/classifier/cgi/determinationmethodorientation/0006>
      rdf:type owl:NamedIndividual .

<http://resource.geosciml.org/classifier/cgi/determinationmethodorientation/0007>
      rdf:type owl:NamedIndividual .

<http://resource.geosciml.org/classifier/cgi/determinationmethodorientation/0008>
      rdf:type owl:NamedIndividual .

<http://resource.geosciml.org/classifier/cgi/determinationmethodorientation/0009>
      rdf:type owl:NamedIndividual .

detmeth:calculated_average_orientation
      rdf:type skos:Concept ;
      dc:source "this vocabulary"@en ;
      skos:definition "Orientation value is specified using a calculated average of a collection of related orientations (computer generalization)."@en ;
      skos:exactMatch <http://resource.geosciml.org/classifier/cgi/determinationmethodorientation/0001> ;
      skos:inScheme cgi:determinationmethodorientation ;
      skos:prefLabel "calculated average orientation"@en .

detmeth:estimate_from_air_photo
      rdf:type skos:Concept ;
      dc:source "this vocabulary"@en ;
      skos:definition "Orientation of a geologic structure estimated based on inspection or measurements on an air photograph."@en ;
      skos:exactMatch <http://resource.geosciml.org/classifier/cgi/determinationmethodorientation/0002> ;
      skos:inScheme cgi:determinationmethodorientation ;
      skos:prefLabel "estimate from air photo"@en .

detmeth:estimate_from_distance
      rdf:type skos:Concept ;
      dc:source "this vocabulary"@en ;
      skos:definition "Orientation of a geologic structure based on observation from a distance great enough to preclude direct inspection of the structure to determine orientation."@en ;
      skos:exactMatch <http://resource.geosciml.org/classifier/cgi/determinationmethodorientation/0003> ;
      skos:inScheme cgi:determinationmethodorientation ;
      skos:prefLabel "estimate from distance"@en .

detmeth:measure_on_outcrop
      rdf:type skos:Concept ;
      dc:source "this vocabulary"@en ;
      skos:definition "Orientation of surface or line is measured on an outcrop of that surface or line directly, e.g. by measuring a particular bedding surface, a 3-D exposure of a fold hinge, a particular stretched mineral grain in a foliation surface."@en ;
      skos:exactMatch <http://resource.geosciml.org/classifier/cgi/determinationmethodorientation/0004> ;
      skos:inScheme cgi:determinationmethodorientation ;
      skos:narrower detmeth:visual_surface_estimation_on_outcrop , detmeth:standard_on_site_measure ;
      skos:prefLabel "measure on outcrop"@en .

detmeth:method_unknown
      rdf:type skos:Concept ;
      dc:source "this vocabulary"@en ;
      skos:definition "use value qualifier to specify the kind of nil."@en ;
      skos:exactMatch <http://resource.geosciml.org/classifier/cgi/determinationmethodorientation/0005> ;
      skos:inScheme cgi:determinationmethodorientation ;
      skos:prefLabel "method unknown"@en .

detmeth:photogeologic_determination
      rdf:type skos:Concept ;
      dc:source "this vocabulary"@en ;
      skos:definition "Orientation determined based on measurements from aerial photography or satellite imagery (in conjunction with an elevation model."@en ;
      skos:exactMatch <http://resource.geosciml.org/classifier/cgi/determinationmethodorientation/0006> ;
      skos:inScheme cgi:determinationmethodorientation ;
      skos:prefLabel "photogeologic determination"@en .

detmeth:standard_on_site_measure
      rdf:type skos:Concept ;
      dc:source "this vocabulary"@en ;
      skos:broader detmeth:measure_on_outcrop ;
      skos:definition "Orientation measured using compass or other instrument directly on or at an outcrop of the structure."@en ;
      skos:exactMatch <http://resource.geosciml.org/classifier/cgi/determinationmethodorientation/0007> ;
      skos:inScheme cgi:determinationmethodorientation ;
      skos:prefLabel "standard on site measure"@en .

detmeth:three_point_determination
      rdf:type skos:Concept ;
      dc:source "this vocabulary"@en ;
      skos:definition "Orientation determined by fitting a plane to three or more points located on the geologic surface of interest."@en ;
      skos:exactMatch <http://resource.geosciml.org/classifier/cgi/determinationmethodorientation/0008> ;
      skos:inScheme cgi:determinationmethodorientation ;
      skos:prefLabel "three point determination"@en .

detmeth:visual_surface_estimation_on_outcrop
      rdf:type skos:Concept ;
      dc:source "this vocabulary"@en ;
      skos:broader detmeth:measure_on_outcrop ;
      skos:definition "Orientation of a surface is measured by visually averaging across one or more outcrops in a small area--e.g. approximating dip by looking down strike of beds, approximating strike by outcrop trace of one or more beds."@en ;
      skos:exactMatch <http://resource.geosciml.org/classifier/cgi/determinationmethodorientation/0009> ;
      skos:inScheme cgi:determinationmethodorientation ;
      skos:prefLabel "visual surface estimation on outcrop"@en .

cgi:determinationmethodorientation
      rdf:type owl:Ontology , skos:ConceptScheme ;
      dc:creator "Concept Definition Task Group of IUGS CGI Interoperability Working Group (http://www.cgi-iugs.org/tech_collaboration/interoperability_working_group.html)" ;
      dc:format "application/rdf+xml" ;
      dc:identifier "http://resource.geosciml.org/classifierscheme/cgi/201211/determinationmethodorientation" ;
      dc:language "en" ;
      dc:publisher "Concept Definition Task Group of IUGS CGI Interoperability Working Group (http://www.cgi-iugs.org/tech_collaboration/interoperability_working_group.html)" ;
      dc:title "CGI Determination Method for Orientation Term Vocabulary"@en ;
      owl:imports <http://www.w3.org/2004/02/skos/core> , <http://rdfs.org/ns/void> ;
      owl:versionInfo "201211" ;
      skos:definition "This file contains the CGI Determination methods vocabulary. Methods of measuring orientation of geometrical features in rock bodies. Describes the way the dip value was determined e.g. measured, inferred from dip slope etc."@en ;
      skos:historyNote "2012-11-24 SMR Update to 201211 version; add collection entity, check all pref labels are lower case, remove owl:NamedIndividual and Owl:Thing rdf:types."@en , "2010-02-08. SMR Clean up namespace declarations so concept URI's follow CGI URN scheme; concepts have URN, are not document fragments."@en , "2010 11 27 SMR convert identifiers from URN to http URI according to CGI URI scheme."@en , "2012-02-07 SMR update URI to replace numeric final token with English-language string as in original URN scheme."@en , "2009-07-14. Generate SKOS encoding of vocabulary from Excel spreadsheet."@en , "2012-02-27 SMR add skos:exactMatch triples to map URIs for concepts in this vocabulary to number-token URIs in 201012 version of same concepts."@en , "2010-02-12  Add narrower relationship links by adding skos:narrower link in Protege, defining skos:narrower as inverse of skos:broader, calculating with Pellet reasoner to add inferred axioms, and using 'file/Export inferred axioms as ontology' in Protege."@en ;
      skos:prefLabel "CGI Determination Method for Orientation Term Vocabulary"@en .

<http://resource.geosciml.org/vocabulary/cgi/201211/determinationmethodorientation>
      rdf:type void:Dataset ;
      rdfs:label "Determination method orientation vocabulary"^^xsd:string .

skos:ConceptScheme
      rdf:type owl:Class .
