# baseURI: http://resource.geosciml.org/classifierscheme/cgi/201211/featureobservationmethod
# imports: http://rdfs.org/ns/void
# imports: http://www.w3.org/2004/02/skos/core

@prefix cgi:     <http://resource.geosciml.org/classifierscheme/cgi/201211/> .
@prefix dc:      <http://purl.org/dc/elements/1.1/> .
@prefix featobs:  <http://resource.geosciml.org/classifier/cgi/featureobservationmethod/> .
@prefix owl:     <http://www.w3.org/2002/07/owl#> .
@prefix owl2xml:  <http://www.w3.org/2006/12/owl2-xml#> .
@prefix rdf:     <http://www.w3.org/1999/02/22-rdf-syntax-ns#> .
@prefix rdfs:    <http://www.w3.org/2000/01/rdf-schema#> .
@prefix skos:    <http://www.w3.org/2004/02/skos/core#> .
@prefix void:    <http://rdfs.org/ns/void#> .
@prefix xsd:     <http://www.w3.org/2001/XMLSchema#> .

featobs:
      rdf:type skos:Collection ;
      rdfs:label "feature observation method concepts"@en ;
      skos:definition "This resource defines the concept space for feature observation method concepts by extension; it includes all concepts in this conceptScheme, as well as concepts in previous versions of the scheme."@en ;
      skos:member featobs:drill_core_observation_measured_values , featobs:synthesis_of_multiple_outcrop_observations , featobs:outcrop_observation_estimated_values , featobs:indirect_method , featobs:direct_observation , featobs:remotely_sensed_data , featobs:synthesis_from_multiple_sources , featobs:borehole_cuttings_observation , featobs:outcrop_observation_measured_values , featobs:data_from_single_published_description , featobs:drill_core_observation_estimated_values , featobs:outcrop_observation , featobs:digital_conversion_from_published_source , featobs:borehole_geophysical_log_measurements , featobs:synthesis_of_multiple_published_descriptions , featobs:drill_core_observation ;
      skos:prefLabel "CGI Feature Observation Method"@en .

featobs:borehole_cuttings_observation
      rdf:type skos:Concept ;
      dc:source "this vocabulary"@en ;
      skos:broader featobs:direct_observation ;
      skos:definition "Data based on interpretation of borehole cuttings"@en ;
      skos:exactMatch <http://resource.geosciml.org/classifier/cgi/featureobservationmethod/0001> ;
      skos:inScheme cgi:featureobservationmethod ;
      skos:prefLabel "borehole cuttings observation" .

featobs:borehole_geophysical_log_measurements
      rdf:type skos:Concept ;
      dc:source "this vocabulary"@en ;
      skos:broader featobs:indirect_method ;
      skos:definition "Data based on interpretation of geophysical measurement obtained by borehole logging tools."@en ;
      skos:exactMatch <http://resource.geosciml.org/classifier/cgi/featureobservationmethod/0002> ;
      skos:inScheme cgi:featureobservationmethod ;
      skos:prefLabel "borehole geophysical log measurements" .

featobs:data_from_single_published_description
      rdf:type skos:Concept ;
      dc:source "this vocabulary"@en ;
      skos:broader featobs:digital_conversion_from_published_source ;
      skos:definition "Data are extracted from a publised description of the feature"@en ;
      skos:exactMatch <http://resource.geosciml.org/classifier/cgi/featureobservationmethod/0003> ;
      skos:inScheme cgi:featureobservationmethod ;
      skos:prefLabel "data from single published description" .

featobs:digital_conversion_from_published_source
      rdf:type skos:Concept ;
      dc:source "This vocabulary"@en ;
      skos:definition "Feature observation is based on published information, converted to a digital representation for database application"@en ;
      skos:exactMatch <http://resource.geosciml.org/classifier/cgi/featureobservationmethod/0004> ;
      skos:inScheme cgi:featureobservationmethod ;
      skos:narrower featobs:data_from_single_published_description , featobs:synthesis_of_multiple_published_descriptions ;
      skos:prefLabel "digital conversion from published source" ;
      skos:topConceptOf cgi:featureobservationmethod .

featobs:direct_observation
      rdf:type skos:Concept ;
      dc:source "this vocabulary"@en ;
      skos:definition "Feature observation is result of direct visual observation by a geologist"@en ;
      skos:exactMatch <http://resource.geosciml.org/classifier/cgi/featureobservationmethod/0005> ;
      skos:inScheme cgi:featureobservationmethod ;
      skos:narrower featobs:outcrop_observation , featobs:borehole_cuttings_observation , featobs:drill_core_observation ;
      skos:prefLabel "direct observation" ;
      skos:topConceptOf cgi:featureobservationmethod .

featobs:drill_core_observation
      rdf:type skos:Concept ;
      dc:source "this vocabulary"@en ;
      skos:broader featobs:direct_observation ;
      skos:definition "Data collected through observation of a single drill core interval."@en ;
      skos:exactMatch <http://resource.geosciml.org/classifier/cgi/featureobservationmethod/0006> ;
      skos:inScheme cgi:featureobservationmethod ;
      skos:narrower featobs:drill_core_observation_estimated_values , featobs:drill_core_observation_measured_values ;
      skos:prefLabel "drill core observation" .

featobs:drill_core_observation_estimated_values
      rdf:type skos:Concept ;
      dc:source "this vocabulary"@en ;
      skos:broader featobs:drill_core_observation ;
      skos:definition "Values for properties are estimated by observer."@en ;
      skos:exactMatch <http://resource.geosciml.org/classifier/cgi/featureobservationmethod/0007> ;
      skos:inScheme cgi:featureobservationmethod ;
      skos:prefLabel "drill core observation, estimated values" .

featobs:drill_core_observation_measured_values
      rdf:type skos:Concept ;
      dc:source "this vocabulary"@en ;
      skos:broader featobs:drill_core_observation ;
      skos:definition "Values for properties are measured using a device (compass, jacob staff, scintillometer, clinometer, ruler…)"@en ;
      skos:exactMatch <http://resource.geosciml.org/classifier/cgi/featureobservationmethod/0008> ;
      skos:inScheme cgi:featureobservationmethod ;
      skos:prefLabel "drill core observation, measured values" .

featobs:indirect_method
      rdf:type skos:Concept ;
      dc:source "this vocabulary"@en ;
      skos:definition "Feature observation based on inference from proxy observation"@en ;
      skos:exactMatch <http://resource.geosciml.org/classifier/cgi/featureobservationmethod/0009> ;
      skos:inScheme cgi:featureobservationmethod ;
      skos:narrower featobs:borehole_geophysical_log_measurements , featobs:remotely_sensed_data ;
      skos:prefLabel "indirect method" ;
      skos:topConceptOf cgi:featureobservationmethod .

featobs:outcrop_observation
      rdf:type skos:Concept ;
      dc:source "this vocabulary"@en ;
      skos:broader featobs:direct_observation ;
      skos:definition "Data collected in field through direct observation of a single outcrop. Observer defines scope of 'single outcrop'--may be one point location, or averaged over an extended but connected) area, e.g. a single polygon on a map. Direct observation may include observation using a remote camera (e.g. downhole viewer, submarine camera)"@en ;
      skos:exactMatch <http://resource.geosciml.org/classifier/cgi/featureobservationmethod/0010> ;
      skos:inScheme cgi:featureobservationmethod ;
      skos:narrower featobs:outcrop_observation_estimated_values , featobs:outcrop_observation_measured_values ;
      skos:prefLabel "outcrop observation" .

featobs:outcrop_observation_estimated_values
      rdf:type skos:Concept ;
      dc:source "this vocabulary"@en ;
      skos:broader featobs:outcrop_observation ;
      skos:definition "Values for properties are estimated by observer."@en ;
      skos:exactMatch <http://resource.geosciml.org/classifier/cgi/featureobservationmethod/0011> ;
      skos:inScheme cgi:featureobservationmethod ;
      skos:prefLabel "outcrop observation estimated values" .

featobs:outcrop_observation_measured_values
      rdf:type skos:Concept ;
      dc:source "this vocabulary"@en ;
      skos:broader featobs:outcrop_observation ;
      skos:definition "Values for properties are measured using a device (compass, jacob staff, scintillometer, clinometer, ruler…)"@en ;
      skos:exactMatch <http://resource.geosciml.org/classifier/cgi/featureobservationmethod/0012> ;
      skos:inScheme cgi:featureobservationmethod ;
      skos:prefLabel "outcrop observation measured values" .

featobs:remotely_sensed_data
      rdf:type skos:Concept ;
      dc:source "this vocabulary"@en ;
      skos:broader featobs:indirect_method ;
      skos:definition "Geologic unit or structure characterized based on remotely sensed data."@en ;
      skos:exactMatch <http://resource.geosciml.org/classifier/cgi/featureobservationmethod/0013> ;
      skos:inScheme cgi:featureobservationmethod ;
      skos:prefLabel "remotely sensed data" .

featobs:synthesis_from_multiple_sources
      rdf:type skos:Concept ;
      dc:source "this vocabulary"@en ;
      skos:definition "Feature observation is based on a synthesis of other observations by some compiler. The compiler may be the same individual that made the source observations."@en ;
      skos:exactMatch <http://resource.geosciml.org/classifier/cgi/featureobservationmethod/0014> ;
      skos:inScheme cgi:featureobservationmethod ;
      skos:narrower featobs:synthesis_of_multiple_outcrop_observations , featobs:synthesis_of_multiple_published_descriptions ;
      skos:prefLabel "synthesis from multiple sources" ;
      skos:topConceptOf cgi:featureobservationmethod .

featobs:synthesis_of_multiple_outcrop_observations
      rdf:type skos:Concept ;
      dc:source "this vocabulary"@en ;
      skos:broader featobs:synthesis_from_multiple_sources ;
      skos:definition "Data are the result of synthesis from multiple direct observations, posibly by more than one observer"@en ;
      skos:exactMatch <http://resource.geosciml.org/classifier/cgi/featureobservationmethod/0015> ;
      skos:inScheme cgi:featureobservationmethod ;
      skos:prefLabel "synthesis of multiple outcrop observations" .

featobs:synthesis_of_multiple_published_descriptions
      rdf:type skos:Concept ;
      dc:source "this vocabulary"@en ;
      skos:broader featobs:digital_conversion_from_published_source , featobs:synthesis_from_multiple_sources ;
      skos:definition "Data are the result of synthesis from multiple published descriptions"@en ;
      skos:exactMatch <http://resource.geosciml.org/classifier/cgi/featureobservationmethod/0016> ;
      skos:inScheme cgi:featureobservationmethod ;
      skos:prefLabel "synthesis of multiple published descriptions" .

cgi:featureobservationmethod
      rdf:type skos:ConceptScheme , owl:Ontology ;
      rdfs:comment "2010-02-04  SMR Start file produced from excel spreadsheet version of FeatureObservationMethod200811, using P. Golodonic xl2xml."@en ;
      dc:creator "Concept Definition Task Group of IUGS CGI Interoperability Working Group (http://www.cgi-iugs.org/tech_collaboration/interoperability_working_group.html)"@en ;
      dc:format "application/rdf+xml" ;
      dc:identifier "http://resource.geosciml.org/classifierscheme/cgi/201211/featureobservationmethod" ;
      dc:language "en" ;
      dc:publisher "Concept Definition Task Group of IUGS CGI Interoperability Working Group (http://www.cgi-iugs.org/tech_collaboration/interoperability_working_group.html)"@en ;
      dc:title "CGI Feature observation method terms"@en ;
      owl:imports <http://rdfs.org/ns/void> , <http://www.w3.org/2004/02/skos/core> ;
      owl:versionInfo "201211" ;
      skos:definition "This classifier scheme contains the CGI Feature Observation Method vocabulary, used to specify the approach to acquiring the collection of attribute value assignments that constitute an individual feature instance. Observation method is a convienence property that provides a quick and dirty approach to shortcut use of more comprehensive observation and measurement construct when data are reported using a feature view (as opposed to observation view)."@en ;
      skos:historyNote "2012-02-07 SMR update URI to replace numeric final token with English-language string as in original URN scheme."@en , "2010-11-28 SMR replace URN with http URI identifiers according to CGI URI scheme"@en , "2010-02-11 Add narrower relationship links by adding skos:narrower link in Protege, defining skos:narrower as inverse of skos:broader, calculating with Pellet reasoner to add inferred axioms, and using 'file/Export inferred axioms as ontology' in Protege."@en , "2010-02-04 SMR Updated from 2010 01 version by adding broader categories for 'digital conversion...', Direct observation, indirect method, and 'synthesis....'"@en , "2012-11-24 SMR Update to 201211 version; add collection entity, check all pref labels are lower case, remove owl:NamedIndividual and Owl:Thing rdf:types."@en ;
      skos:prefLabel "CGI Feature observation method"@en .

<http://resource.geosciml.org/vocabulary/cgi/201211/featureobservationmethod>
      rdf:type void:Dataset ;
      rdfs:label "Feature observation method vocabulary"^^xsd:string .
