<?xml version="1.0" encoding="UTF-8"?>
<rdf:RDF
	xmlns:cgi="http://resource.geosciml.org/classifierscheme/cgi/201211/"
	xmlns:dc="http://purl.org/dc/elements/1.1/"
	xmlns:featobs="http://resource.geosciml.org/classifier/cgi/featureobservationmethod/"
	xmlns:owl="http://www.w3.org/2002/07/owl#"
	xmlns:owl2xml="http://www.w3.org/2006/12/owl2-xml#"
	xmlns:rdf="http://www.w3.org/1999/02/22-rdf-syntax-ns#"
	xmlns:rdfs="http://www.w3.org/2000/01/rdf-schema#"
	xmlns:skos="http://www.w3.org/2004/02/skos/core#"
	xmlns:void="http://rdfs.org/ns/void#"
	xmlns:xsd="http://www.w3.org/2001/XMLSchema#">

<rdf:Description rdf:about="http://resource.geosciml.org/classifier/cgi/featureobservationmethod/">
	<rdf:type rdf:resource="http://www.w3.org/2004/02/skos/core#Collection"/>
	<rdfs:label xml:lang="en">feature observation method concepts</rdfs:label>
	<skos:definition xml:lang="en">This resource defines the concept space for feature observation method concepts by extension; it includes all concepts in this conceptScheme, as well as concepts in previous versions of the scheme.</skos:definition>
	<skos:member rdf:resource="http://resource.geosciml.org/classifier/cgi/featureobservationmethod/drill_core_observation_measured_values"/>
	<skos:member rdf:resource="http://resource.geosciml.org/classifier/cgi/featureobservationmethod/synthesis_of_multiple_outcrop_observations"/>
	<skos:member rdf:resource="http://resource.geosciml.org/classifier/cgi/featureobservationmethod/outcrop_observation_estimated_values"/>
	<skos:member rdf:resource="http://resource.geosciml.org/classifier/cgi/featureobservationmethod/indirect_method"/>
	<skos:member rdf:resource="http://resource.geosciml.org/classifier/cgi/featureobservationmethod/direct_observation"/>
	<skos:member rdf:resource="http://resource.geosciml.org/classifier/cgi/featureobservationmethod/remotely_sensed_data"/>
	<skos:member rdf:resource="http://resource.geosciml.org/classifier/cgi/featureobservationmethod/synthesis_from_multiple_sources"/>
	<skos:member rdf:resource="http://resource.geosciml.org/classifier/cgi/featureobservationmethod/borehole_cuttings_observation"/>
	<skos:member rdf:resource="http://resource.geosciml.org/classifier/cgi/featureobservationmethod/outcrop_observation_measured_values"/>
	<skos:member rdf:resource="http://resource.geosciml.org/classifier/cgi/featureobservationmethod/data_from_single_published_description"/>
	<skos:member rdf:resource="http://resource.geosciml.org/classifier/cgi/featureobservationmethod/drill_core_observation_estimated_values"/>
	<skos:member rdf:resource="http://resource.geosciml.org/classifier/cgi/featureobservationmethod/outcrop_observation"/>
	<skos:member rdf:resource="http://resource.geosciml.org/classifier/cgi/featureobservationmethod/digital_conversion_from_published_source"/>
	<skos:member rdf:resource="http://resource.geosciml.org/classifier/cgi/featureobservationmethod/borehole_geophysical_log_measurements"/>
	<skos:member rdf:resource="http://resource.geosciml.org/classifier/cgi/featureobservationmethod/synthesis_of_multiple_published_descriptions"/>
	<skos:member rdf:resource="http://resource.geosciml.org/classifier/cgi/featureobservationmethod/drill_core_observation"/>
	<skos:prefLabel xml:lang="en">CGI Feature Observation Method</skos:prefLabel>
</rdf:Description>

<rdf:Description rdf:about="http://resource.geosciml.org/classifier/cgi/featureobservationmethod/borehole_cuttings_observation">
	<rdf:type rdf:resource="http://www.w3.org/2004/02/skos/core#Concept"/>
	<dc:source xml:lang="en">this vocabulary</dc:source>
	<skos:broader rdf:resource="http://resource.geosciml.org/classifier/cgi/featureobservationmethod/direct_observation"/>
	<skos:definition xml:lang="en">Data based on interpretation of borehole cuttings</skos:definition>
	<skos:exactMatch rdf:resource="http://resource.geosciml.org/classifier/cgi/featureobservationmethod/0001"/>
	<skos:inScheme rdf:resource="http://resource.geosciml.org/classifierscheme/cgi/201211/featureobservationmethod"/>
	<skos:prefLabel>borehole cuttings observation</skos:prefLabel>
</rdf:Description>

<rdf:Description rdf:about="http://resource.geosciml.org/classifier/cgi/featureobservationmethod/borehole_geophysical_log_measurements">
	<rdf:type rdf:resource="http://www.w3.org/2004/02/skos/core#Concept"/>
	<dc:source xml:lang="en">this vocabulary</dc:source>
	<skos:broader rdf:resource="http://resource.geosciml.org/classifier/cgi/featureobservationmethod/indirect_method"/>
	<skos:definition xml:lang="en">Data based on interpretation of geophysical measurement obtained by borehole logging tools.</skos:definition>
	<skos:exactMatch rdf:resource="http://resource.geosciml.org/classifier/cgi/featureobservationmethod/0002"/>
	<skos:inScheme rdf:resource="http://resource.geosciml.org/classifierscheme/cgi/201211/featureobservationmethod"/>
	<skos:prefLabel>borehole geophysical log measurements</skos:prefLabel>
</rdf:Description>

<rdf:Description rdf:about="http://resource.geosciml.org/classifier/cgi/featureobservationmethod/data_from_single_published_description">
	<rdf:type rdf:resource="http://www.w3.org/2004/02/skos/core#Concept"/>
	<dc:source xml:lang="en">this vocabulary</dc:source>
	<skos:broader rdf:resource="http://resource.geosciml.org/classifier/cgi/featureobservationmethod/digital_conversion_from_published_source"/>
	<skos:definition xml:lang="en">Data are extracted from a publised description of the feature</skos:definition>
	<skos:exactMatch rdf:resource="http://resource.geosciml.org/classifier/cgi/featureobservationmethod/0003"/>
	<skos:inScheme rdf:resource="http://resource.geosciml.org/classifierscheme/cgi/201211/featureobservationmethod"/>
	<skos:prefLabel>data from single published description</skos:prefLabel>
</rdf:Description>

<rdf:Description rdf:about="http://resource.geosciml.org/classifier/cgi/featureobservationmethod/digital_conversion_from_published_source">
	<rdf:type rdf:resource="http://www.w3.org/2004/02/skos/core#Concept"/>
	<dc:source xml:lang="en">This vocabulary</dc:source>
	<skos:definition xml:lang="en">Feature observation is based on published information, converted to a digital representation for database application</skos:definition>
	<skos:exactMatch rdf:resource="http://resource.geosciml.org/classifier/cgi/featureobservationmethod/0004"/>
	<skos:inScheme rdf:resource="http://resource.geosciml.org/classifierscheme/cgi/201211/featureobservationmethod"/>
	<skos:narrower rdf:resource="http://resource.geosciml.org/classifier/cgi/featureobservationmethod/data_from_single_published_description"/>
	<skos:narrower rdf:resource="http://resource.geosciml.org/classifier/cgi/featureobservationmethod/synthesis_of_multiple_published_descriptions"/>
	<skos:prefLabel>digital conversion from published source</skos:prefLabel>
	<skos:topConceptOf rdf:resource="http://resource.geosciml.org/classifierscheme/cgi/201211/featureobservationmethod"/>
</rdf:Description>

<rdf:Description rdf:about="http://resource.geosciml.org/classifier/cgi/featureobservationmethod/direct_observation">
	<rdf:type rdf:resource="http://www.w3.org/2004/02/skos/core#Concept"/>
	<dc:source xml:lang="en">this vocabulary</dc:source>
	<skos:definition xml:lang="en">Feature observation is result of direct visual observation by a geologist</skos:definition>
	<skos:exactMatch rdf:resource="http://resource.geosciml.org/classifier/cgi/featureobservationmethod/0005"/>
	<skos:inScheme rdf:resource="http://resource.geosciml.org/classifierscheme/cgi/201211/featureobservationmethod"/>
	<skos:narrower rdf:resource="http://resource.geosciml.org/classifier/cgi/featureobservationmethod/outcrop_observation"/>
	<skos:narrower rdf:resource="http://resource.geosciml.org/classifier/cgi/featureobservationmethod/borehole_cuttings_observation"/>
	<skos:narrower rdf:resource="http://resource.geosciml.org/classifier/cgi/featureobservationmethod/drill_core_observation"/>
	<skos:prefLabel>direct observation</skos:prefLabel>
	<skos:topConceptOf rdf:resource="http://resource.geosciml.org/classifierscheme/cgi/201211/featureobservationmethod"/>
</rdf:Description>

<rdf:Description rdf:about="http://resource.geosciml.org/classifier/cgi/featureobservationmethod/drill_core_observation">
	<rdf:type rdf:resource="http://www.w3.org/2004/02/skos/core#Concept"/>
	<dc:source xml:lang="en">this vocabulary</dc:source>
	<skos:broader rdf:resource="http://resource.geosciml.org/classifier/cgi/featureobservationmethod/direct_observation"/>
	<skos:definition xml:lang="en">Data collected through observation of a single drill core interval.</skos:definition>
	<skos:exactMatch rdf:resource="http://resource.geosciml.org/classifier/cgi/featureobservationmethod/0006"/>
	<skos:inScheme rdf:resource="http://resource.geosciml.org/classifierscheme/cgi/201211/featureobservationmethod"/>
	<skos:narrower rdf:resource="http://resource.geosciml.org/classifier/cgi/featureobservationmethod/drill_core_observation_estimated_values"/>
	<skos:narrower rdf:resource="http://resource.geosciml.org/classifier/cgi/featureobservationmethod/drill_core_observation_measured_values"/>
	<skos:prefLabel>drill core observation</skos:prefLabel>
</rdf:Description>

<rdf:Description rdf:about="http://resource.geosciml.org/classifier/cgi/featureobservationmethod/drill_core_observation_estimated_values">
	<rdf:type rdf:resource="http://www.w3.org/2004/02/skos/core#Concept"/>
	<dc:source xml:lang="en">this vocabulary</dc:source>
	<skos:broader rdf:resource="http://resource.geosciml.org/classifier/cgi/featureobservationmethod/drill_core_observation"/>
	<skos:definition xml:lang="en">Values for properties are estimated by observer.</skos:definition>
	<skos:exactMatch rdf:resource="http://resource.geosciml.org/classifier/cgi/featureobservationmethod/0007"/>
	<skos:inScheme rdf:resource="http://resource.geosciml.org/classifierscheme/cgi/201211/featureobservationmethod"/>
	<skos:prefLabel>drill core observation, estimated values</skos:prefLabel>
</rdf:Description>

<rdf:Description rdf:about="http://resource.geosciml.org/classifier/cgi/featureobservationmethod/drill_core_observation_measured_values">
	<rdf:type rdf:resource="http://www.w3.org/2004/02/skos/core#Concept"/>
	<dc:source xml:lang="en">this vocabulary</dc:source>
	<skos:broader rdf:resource="http://resource.geosciml.org/classifier/cgi/featureobservationmethod/drill_core_observation"/>
	<skos:definition xml:lang="en">Values for properties are measured using a device (compass, jacob staff, scintillometer, clinometer, ruler…)</skos:definition>
	<skos:exactMatch rdf:resource="http://resource.geosciml.org/classifier/cgi/featureobservationmethod/0008"/>
	<skos:inScheme rdf:resource="http://resource.geosciml.org/classifierscheme/cgi/201211/featureobservationmethod"/>
	<skos:prefLabel>drill core observation, measured values</skos:prefLabel>
</rdf:Description>

<rdf:Description rdf:about="http://resource.geosciml.org/classifier/cgi/featureobservationmethod/indirect_method">
	<rdf:type rdf:resource="http://www.w3.org/2004/02/skos/core#Concept"/>
	<dc:source xml:lang="en">this vocabulary</dc:source>
	<skos:definition xml:lang="en">Feature observation based on inference from proxy observation</skos:definition>
	<skos:exactMatch rdf:resource="http://resource.geosciml.org/classifier/cgi/featureobservationmethod/0009"/>
	<skos:inScheme rdf:resource="http://resource.geosciml.org/classifierscheme/cgi/201211/featureobservationmethod"/>
	<skos:narrower rdf:resource="http://resource.geosciml.org/classifier/cgi/featureobservationmethod/borehole_geophysical_log_measurements"/>
	<skos:narrower rdf:resource="http://resource.geosciml.org/classifier/cgi/featureobservationmethod/remotely_sensed_data"/>
	<skos:prefLabel>indirect method</skos:prefLabel>
	<skos:topConceptOf rdf:resource="http://resource.geosciml.org/classifierscheme/cgi/201211/featureobservationmethod"/>
</rdf:Description>

<rdf:Description rdf:about="http://resource.geosciml.org/classifier/cgi/featureobservationmethod/outcrop_observation">
	<rdf:type rdf:resource="http://www.w3.org/2004/02/skos/core#Concept"/>
	<dc:source xml:lang="en">this vocabulary</dc:source>
	<skos:broader rdf:resource="http://resource.geosciml.org/classifier/cgi/featureobservationmethod/direct_observation"/>
	<skos:definition xml:lang="en">Data collected in field through direct observation of a single outcrop. Observer defines scope of 'single outcrop'--may be one point location, or averaged over an extended but connected) area, e.g. a single polygon on a map. Direct observation may include observation using a remote camera (e.g. downhole viewer, submarine camera)</skos:definition>
	<skos:exactMatch rdf:resource="http://resource.geosciml.org/classifier/cgi/featureobservationmethod/0010"/>
	<skos:inScheme rdf:resource="http://resource.geosciml.org/classifierscheme/cgi/201211/featureobservationmethod"/>
	<skos:narrower rdf:resource="http://resource.geosciml.org/classifier/cgi/featureobservationmethod/outcrop_observation_estimated_values"/>
	<skos:narrower rdf:resource="http://resource.geosciml.org/classifier/cgi/featureobservationmethod/outcrop_observation_measured_values"/>
	<skos:prefLabel>outcrop observation</skos:prefLabel>
</rdf:Description>

<rdf:Description rdf:about="http://resource.geosciml.org/classifier/cgi/featureobservationmethod/outcrop_observation_estimated_values">
	<rdf:type rdf:resource="http://www.w3.org/2004/02/skos/core#Concept"/>
	<dc:source xml:lang="en">this vocabulary</dc:source>
	<skos:broader rdf:resource="http://resource.geosciml.org/classifier/cgi/featureobservationmethod/outcrop_observation"/>
	<skos:definition xml:lang="en">Values for properties are estimated by observer.</skos:definition>
	<skos:exactMatch rdf:resource="http://resource.geosciml.org/classifier/cgi/featureobservationmethod/0011"/>
	<skos:inScheme rdf:resource="http://resource.geosciml.org/classifierscheme/cgi/201211/featureobservationmethod"/>
	<skos:prefLabel>outcrop observation estimated values</skos:prefLabel>
</rdf:Description>

<rdf:Description rdf:about="http://resource.geosciml.org/classifier/cgi/featureobservationmethod/outcrop_observation_measured_values">
	<rdf:type rdf:resource="http://www.w3.org/2004/02/skos/core#Concept"/>
	<dc:source xml:lang="en">this vocabulary</dc:source>
	<skos:broader rdf:resource="http://resource.geosciml.org/classifier/cgi/featureobservationmethod/outcrop_observation"/>
	<skos:definition xml:lang="en">Values for properties are measured using a device (compass, jacob staff, scintillometer, clinometer, ruler…)</skos:definition>
	<skos:exactMatch rdf:resource="http://resource.geosciml.org/classifier/cgi/featureobservationmethod/0012"/>
	<skos:inScheme rdf:resource="http://resource.geosciml.org/classifierscheme/cgi/201211/featureobservationmethod"/>
	<skos:prefLabel>outcrop observation measured values</skos:prefLabel>
</rdf:Description>

<rdf:Description rdf:about="http://resource.geosciml.org/classifier/cgi/featureobservationmethod/remotely_sensed_data">
	<rdf:type rdf:resource="http://www.w3.org/2004/02/skos/core#Concept"/>
	<dc:source xml:lang="en">this vocabulary</dc:source>
	<skos:broader rdf:resource="http://resource.geosciml.org/classifier/cgi/featureobservationmethod/indirect_method"/>
	<skos:definition xml:lang="en">Geologic unit or structure characterized based on remotely sensed data.</skos:definition>
	<skos:exactMatch rdf:resource="http://resource.geosciml.org/classifier/cgi/featureobservationmethod/0013"/>
	<skos:inScheme rdf:resource="http://resource.geosciml.org/classifierscheme/cgi/201211/featureobservationmethod"/>
	<skos:prefLabel>remotely sensed data</skos:prefLabel>
</rdf:Description>

<rdf:Description rdf:about="http://resource.geosciml.org/classifier/cgi/featureobservationmethod/synthesis_from_multiple_sources">
	<rdf:type rdf:resource="http://www.w3.org/2004/02/skos/core#Concept"/>
	<dc:source xml:lang="en">this vocabulary</dc:source>
	<skos:definition xml:lang="en">Feature observation is based on a synthesis of other observations by some compiler. The compiler may be the same individual that made the source observations.</skos:definition>
	<skos:exactMatch rdf:resource="http://resource.geosciml.org/classifier/cgi/featureobservationmethod/0014"/>
	<skos:inScheme rdf:resource="http://resource.geosciml.org/classifierscheme/cgi/201211/featureobservationmethod"/>
	<skos:narrower rdf:resource="http://resource.geosciml.org/classifier/cgi/featureobservationmethod/synthesis_of_multiple_outcrop_observations"/>
	<skos:narrower rdf:resource="http://resource.geosciml.org/classifier/cgi/featureobservationmethod/synthesis_of_multiple_published_descriptions"/>
	<skos:prefLabel>synthesis from multiple sources</skos:prefLabel>
	<skos:topConceptOf rdf:resource="http://resource.geosciml.org/classifierscheme/cgi/201211/featureobservationmethod"/>
</rdf:Description>

<rdf:Description rdf:about="http://resource.geosciml.org/classifier/cgi/featureobservationmethod/synthesis_of_multiple_outcrop_observations">
	<rdf:type rdf:resource="http://www.w3.org/2004/02/skos/core#Concept"/>
	<dc:source xml:lang="en">this vocabulary</dc:source>
	<skos:broader rdf:resource="http://resource.geosciml.org/classifier/cgi/featureobservationmethod/synthesis_from_multiple_sources"/>
	<skos:definition xml:lang="en">Data are the result of synthesis from multiple direct observations, posibly by more than one observer</skos:definition>
	<skos:exactMatch rdf:resource="http://resource.geosciml.org/classifier/cgi/featureobservationmethod/0015"/>
	<skos:inScheme rdf:resource="http://resource.geosciml.org/classifierscheme/cgi/201211/featureobservationmethod"/>
	<skos:prefLabel>synthesis of multiple outcrop observations</skos:prefLabel>
</rdf:Description>

<rdf:Description rdf:about="http://resource.geosciml.org/classifier/cgi/featureobservationmethod/synthesis_of_multiple_published_descriptions">
	<rdf:type rdf:resource="http://www.w3.org/2004/02/skos/core#Concept"/>
	<dc:source xml:lang="en">this vocabulary</dc:source>
	<skos:broader rdf:resource="http://resource.geosciml.org/classifier/cgi/featureobservationmethod/digital_conversion_from_published_source"/>
	<skos:broader rdf:resource="http://resource.geosciml.org/classifier/cgi/featureobservationmethod/synthesis_from_multiple_sources"/>
	<skos:definition xml:lang="en">Data are the result of synthesis from multiple published descriptions</skos:definition>
	<skos:exactMatch rdf:resource="http://resource.geosciml.org/classifier/cgi/featureobservationmethod/0016"/>
	<skos:inScheme rdf:resource="http://resource.geosciml.org/classifierscheme/cgi/201211/featureobservationmethod"/>
	<skos:prefLabel>synthesis of multiple published descriptions</skos:prefLabel>
</rdf:Description>

<rdf:Description rdf:about="http://resource.geosciml.org/classifierscheme/cgi/201211/featureobservationmethod">
	<rdf:type rdf:resource="http://www.w3.org/2004/02/skos/core#ConceptScheme"/>
	<rdf:type rdf:resource="http://www.w3.org/2002/07/owl#Ontology"/>
	<rdfs:comment xml:lang="en">2010-02-04  SMR Start file produced from excel spreadsheet version of FeatureObservationMethod200811, using P. Golodonic xl2xml.</rdfs:comment>
	<dc:creator xml:lang="en">Concept Definition Task Group of IUGS CGI Interoperability Working Group (http://www.cgi-iugs.org/tech_collaboration/interoperability_working_group.html)</dc:creator>
	<dc:format>application/rdf+xml</dc:format>
	<dc:identifier>http://resource.geosciml.org/classifierscheme/cgi/201211/featureobservationmethod</dc:identifier>
	<dc:language>en</dc:language>
	<dc:publisher xml:lang="en">Concept Definition Task Group of IUGS CGI Interoperability Working Group (http://www.cgi-iugs.org/tech_collaboration/interoperability_working_group.html)</dc:publisher>
	<dc:title xml:lang="en">CGI Feature observation method terms</dc:title>
	<owl:imports rdf:resource="http://rdfs.org/ns/void"/>
	<owl:imports rdf:resource="http://www.w3.org/2004/02/skos/core"/>
	<owl:versionInfo>201211</owl:versionInfo>
	<skos:definition xml:lang="en">This classifier scheme contains the CGI Feature Observation Method vocabulary, used to specify the approach to acquiring the collection of attribute value assignments that constitute an individual feature instance. Observation method is a convienence property that provides a quick and dirty approach to shortcut use of more comprehensive observation and measurement construct when data are reported using a feature view (as opposed to observation view).</skos:definition>
	<skos:historyNote xml:lang="en">2012-02-07 SMR update URI to replace numeric final token with English-language string as in original URN scheme.</skos:historyNote>
	<skos:historyNote xml:lang="en">2010-11-28 SMR replace URN with http URI identifiers according to CGI URI scheme</skos:historyNote>
	<skos:historyNote xml:lang="en">2010-02-11 Add narrower relationship links by adding skos:narrower link in Protege, defining skos:narrower as inverse of skos:broader, calculating with Pellet reasoner to add inferred axioms, and using 'file/Export inferred axioms as ontology' in Protege.</skos:historyNote>
	<skos:historyNote xml:lang="en">2010-02-04 SMR Updated from 2010 01 version by adding broader categories for 'digital conversion...', Direct observation, indirect method, and 'synthesis....'</skos:historyNote>
	<skos:historyNote xml:lang="en">2012-11-24 SMR Update to 201211 version; add collection entity, check all pref labels are lower case, remove owl:NamedIndividual and Owl:Thing rdf:types.</skos:historyNote>
	<skos:prefLabel xml:lang="en">CGI Feature observation method</skos:prefLabel>
</rdf:Description>

<rdf:Description rdf:about="http://resource.geosciml.org/vocabulary/cgi/201211/featureobservationmethod">
	<rdf:type rdf:resource="http://rdfs.org/ns/void#Dataset"/>
	<rdfs:label rdf:datatype="http://www.w3.org/2001/XMLSchema#string">Feature observation method vocabulary</rdfs:label>
</rdf:Description>

</rdf:RDF>