# baseURI: http://resource.geosciml.org/classifierscheme/cgi/201211/foliationtype
# imports: http://rdfs.org/ns/void
# imports: http://www.w3.org/2004/02/skos/core

@prefix cgi:     <http://resource.geosciml.org/classifierscheme/cgi/201211/> .
@prefix dc:      <http://purl.org/dc/elements/1.1/> .
@prefix foltyp:  <http://resource.geosciml.org/classifier/cgi/foliationtype/> .
@prefix owl:     <http://www.w3.org/2002/07/owl#> .
@prefix owl2xml:  <http://www.w3.org/2006/12/owl2-xml#> .
@prefix rdf:     <http://www.w3.org/1999/02/22-rdf-syntax-ns#> .
@prefix rdfs:    <http://www.w3.org/2000/01/rdf-schema#> .
@prefix skos:    <http://www.w3.org/2004/02/skos/core#> .
@prefix void:    <http://rdfs.org/ns/void#> .
@prefix xsd:     <http://www.w3.org/2001/XMLSchema#> .

foltyp:
      rdf:type skos:Collection ;
      rdfs:label "foliation type concepts"@en ;
      skos:definition "This resource defines the concept space for foliation type concepts by extension; it includes all concepts in this conceptScheme, as well as concepts in previous versions of the scheme."@en ;
      skos:member foltyp:layering , foltyp:sedimentary_layering , foltyp:domainal_cleavage , foltyp:cumulate_layering , foltyp:scaly_cleavage , foltyp:comb_layering , foltyp:tectonic_foliation , foltyp:cryptomicrobial_lamination , foltyp:crenulation_cleavage , foltyp:cleavage , foltyp:compound_metamorphic_foliation , foltyp:foliation , foltyp:lava_flow_banding , foltyp:transposed_bedding_layering , foltyp:mylonite_foliation , foltyp:generic_mylonitic_foliation , foltyp:rhythmic_layering , foltyp:metamorphic_layering , foltyp:discrete_disjunct_spaced_cleavage , foltyp:continuous_crenulation_cleavage , foltyp:flow_layering , foltyp:bedding_fabric , foltyp:igneous_textural_layering , foltyp:slaty_cleavage , foltyp:imbricated_clast_fabric , foltyp:metamorphic_layering_inherited_from_protolith , foltyp:varve_lamination , foltyp:phyllitic_cleavage , foltyp:flaser_structure , foltyp:anastomosing_spaced_cleavage , foltyp:close_joints , foltyp:c_fabric , foltyp:undulating_lamination , foltyp:ultramylonite_foliation , foltyp:impersistent_lamination , foltyp:metamorphic_differentiation_layering , foltyp:gneissic_layering , foltyp:fissile_lamination , foltyp:joint_fabric , foltyp:solution_cleavage , foltyp:s_fabric , foltyp:tectonic_layering , foltyp:disjunctive_cleavage , foltyp:cleavage_parallel_to_bedding , foltyp:discrete_crenulation_cleavage , foltyp:stromatic_layering , foltyp:rough_cleavage , foltyp:igneous_flow_foliation , foltyp:protomylonite_foliation , foltyp:parallel_bedding_lamination , foltyp:primary_igneous_foliation , foltyp:crude_or_indistinct_bedding , foltyp:ductile_shear_banding_foliation , foltyp:planar_lamination , foltyp:low_temperature_flow_foliation , foltyp:spaced_cleavage , foltyp:laminated_metamorphic_layering , foltyp:primary_foliation , foltyp:compositional_layering , foltyp:compound_folation , foltyp:irregular_lamination , foltyp:parallel_bedding , foltyp:stromatolitic_lamination , foltyp:discrete_cleavage , foltyp:vague_metamorphic_layering , foltyp:eutaxitic_foliation , foltyp:layered_mylonitic_foliation , foltyp:continuous_cleavage , foltyp:grain_shape_foliation , foltyp:igneous_layering , foltyp:schistosity , foltyp:mineralogical_layering , foltyp:igneous_lamination , foltyp:bedding_lamination_structure ;
      skos:prefLabel "CGI Foliation Type"@en .

foltyp:anastomosing_spaced_cleavage
      rdf:type skos:Concept ;
      dc:creator "Concept Definition Task Group of IUGS CGI Interoperability Working Group (http://www.cgi-iugs.org/tech_collaboration/interoperability_working_group.html)"@en ;
      dc:source "Geological Survey Victoria, Australia"^^xsd:string ;
      skos:broader foltyp:spaced_cleavage ;
      skos:definition "spaced cleavage domains branch and rejoin, creating lens-shaped microlithons."@en ;
      skos:exactMatch <http://resource.geosciml.org/classifier/cgi/foliationtype/0001> ;
      skos:inScheme cgi:foliationtype ;
      skos:prefLabel "anastomosing spaced cleavage"@en .

foltyp:bedding_fabric
      rdf:type skos:Concept ;
      dc:creator "Concept Definition Task Group of IUGS CGI Interoperability Working Group (http://www.cgi-iugs.org/tech_collaboration/interoperability_working_group.html)"@en ;
      dc:source "SLTTs 2004; this vocabulary" ;
      skos:broader foltyp:primary_foliation ;
      skos:definition "Fabric defined by textural or mineralogic variations in sediment produced by depositional processes. May be manifested by lamination structure within the sediment, or by layering in which the individual layers (beds) are bounded by discontinuities related to events in the depositional history."@en ;
      skos:exactMatch <http://resource.geosciml.org/classifier/cgi/foliationtype/0002> ;
      skos:inScheme cgi:foliationtype ;
      skos:narrower foltyp:parallel_bedding , foltyp:sedimentary_layering , foltyp:crude_or_indistinct_bedding , foltyp:bedding_lamination_structure ;
      skos:prefLabel "bedding fabric"@en .

foltyp:bedding_lamination_structure
      rdf:type skos:Concept ;
      dc:creator "Concept Definition Task Group of IUGS CGI Interoperability Working Group (http://www.cgi-iugs.org/tech_collaboration/interoperability_working_group.html)"@en ;
      dc:source "SLTTs 2004" ;
      skos:broader foltyp:bedding_fabric ;
      skos:definition "A surface internal to the containing sediment mass defined by textural or mineralogical variation, produced by sediment deposition process, and reflecting the orientation of the original depositional surface. Syn Laminated structure (SLTTs 2004)."@en ;
      skos:exactMatch <http://resource.geosciml.org/classifier/cgi/foliationtype/0003> ;
      skos:inScheme cgi:foliationtype ;
      skos:narrower foltyp:impersistent_lamination , foltyp:planar_lamination , foltyp:parallel_bedding_lamination , foltyp:undulating_lamination , foltyp:fissile_lamination , foltyp:cryptomicrobial_lamination , foltyp:irregular_lamination , foltyp:varve_lamination ;
      skos:prefLabel "bedding lamination structure"@en .

foltyp:c_fabric
      rdf:type skos:Concept ;
      dc:creator "Concept Definition Task Group of IUGS CGI Interoperability Working Group (http://www.cgi-iugs.org/tech_collaboration/interoperability_working_group.html)"@en ;
      dc:source "Geoscience Victoria, Australia" ;
      skos:broader foltyp:ductile_shear_banding_foliation ;
      skos:definition "Ductile shear banding foliation defined by spaced, discrete planar zones of high strain less than 1mm thick. commonly associated with a particle flattening ('S') fabric to form a mylonitic foliation."@en ;
      skos:exactMatch <http://resource.geosciml.org/classifier/cgi/foliationtype/0004> ;
      skos:inScheme cgi:foliationtype ;
      skos:prefLabel "c fabric"@en .

foltyp:cleavage
      rdf:type skos:Concept ;
      dc:creator "Concept Definition Task Group of IUGS CGI Interoperability Working Group (http://www.cgi-iugs.org/tech_collaboration/interoperability_working_group.html)"@en ;
      dc:source "Brodie, Kate, Fettes, Douglas, and Harte, Ben, 2007, Structural terms including fault rock terms, in Fettes, D., and Desmons, J., Metamorphic rocks-A classification and Glossary of Terms: Cambridge, UK, Cam-bridge University Press, p. 24-31."@en ;
      skos:broader foltyp:foliation ;
      skos:definition "A tectonic foliation in a rock characterized by a tendency for the rock to split along a regular set of parallel or sub-parallel closely spaced surfaces. Cleavage is a more general term than schistosity because schistosity need not be present in order for a rock to display cleavage. Cleavage domains or parting surfaces are not spaced more than 5 cm apart on average (Borradaille et al., 1982)"@en ;
      skos:exactMatch <http://resource.geosciml.org/classifier/cgi/foliationtype/0005> ;
      skos:inScheme cgi:foliationtype ;
      skos:narrower foltyp:crenulation_cleavage , foltyp:close_joints , foltyp:spaced_cleavage , foltyp:domainal_cleavage , foltyp:disjunctive_cleavage , foltyp:cleavage_parallel_to_bedding , foltyp:rough_cleavage , foltyp:continuous_cleavage ;
      skos:prefLabel "cleavage"@en .

foltyp:cleavage_parallel_to_bedding
      rdf:type skos:Concept ;
      dc:creator "Concept Definition Task Group of IUGS CGI Interoperability Working Group (http://www.cgi-iugs.org/tech_collaboration/interoperability_working_group.html)"@en ;
      dc:source "this vocabulary" ;
      skos:broader foltyp:cleavage , foltyp:compound_folation ;
      skos:definition "composite fabric in which a cleavage is developed parallel to bedding."@en ;
      skos:exactMatch <http://resource.geosciml.org/classifier/cgi/foliationtype/0006> ;
      skos:inScheme cgi:foliationtype ;
      skos:prefLabel "cleavage parallel to bedding"@en .

foltyp:close_joints
      rdf:type skos:Concept ;
      dc:creator "Concept Definition Task Group of IUGS CGI Interoperability Working Group (http://www.cgi-iugs.org/tech_collaboration/interoperability_working_group.html)"@en ;
      dc:source "Borradaile et al. 1982; This Vocabulary" ;
      skos:broader foltyp:cleavage , foltyp:joint_fabric ;
      skos:definition "Foliation defined by parting surfaces (cleavage domains) that have no apparent thickness, are spaced between 5 cm and 25 cm, and do not crenulate an older foliation. Fabric intermediate between typical cleavage and joints. Parting surfaces are regularly spaced, and penetrative on a 1-10 m scale. 5 cm upper limit on spacing of 'cleavage domains' in a 'cleavage 'fabric is suggested by Borradaile et al. [1982]."@en ;
      skos:exactMatch <http://resource.geosciml.org/classifier/cgi/foliationtype/0007> ;
      skos:inScheme cgi:foliationtype ;
      skos:prefLabel "close joints"@en .

foltyp:comb_layering
      rdf:type skos:Concept ;
      dc:creator "Concept Definition Task Group of IUGS CGI Interoperability Working Group (http://www.cgi-iugs.org/tech_collaboration/interoperability_working_group.html)"@en ;
      dc:source "Neuendorf et al. 2005; this vocabulary" ;
      skos:broader foltyp:layering ;
      skos:definition "Layering fabric defined by layers that have internal comb structure. Layer boundaries are the termination surfaces for the constituent crystals."@en ;
      skos:exactMatch <http://resource.geosciml.org/classifier/cgi/foliationtype/0008> ;
      skos:inScheme cgi:foliationtype ;
      skos:prefLabel "comb layering"@en .

foltyp:compositional_layering
      rdf:type skos:Concept ;
      dc:creator "Concept Definition Task Group of IUGS CGI Interoperability Working Group (http://www.cgi-iugs.org/tech_collaboration/interoperability_working_group.html)"@en ;
      dc:source "this vocabulary, submitted by British Antarctic Survey" ;
      skos:broader foltyp:layering ;
      skos:definition "Layering fabric defined by layers that have different mineralogic composition."@en ;
      skos:exactMatch <http://resource.geosciml.org/classifier/cgi/foliationtype/0009> ;
      skos:inScheme cgi:foliationtype ;
      skos:narrower foltyp:mineralogical_layering , foltyp:metamorphic_layering_inherited_from_protolith , foltyp:metamorphic_differentiation_layering ;
      skos:prefLabel "compositional layering"@en .

foltyp:compound_folation
      rdf:type skos:Concept ;
      dc:creator "Concept Definition Task Group of IUGS CGI Interoperability Working Group (http://www.cgi-iugs.org/tech_collaboration/interoperability_working_group.html)"@en ;
      dc:source "this vocabulary" ;
      skos:broader foltyp:foliation ;
      skos:definition "Foliation that includes fabric elements indicating classification with foliation types of different genetic origin, e.g. cleavage parallel to bedding is a compound fabric with a sedimentary foliation and a tectonic foliation. No connotation of genetic origin of fabric elements."@en ;
      skos:exactMatch <http://resource.geosciml.org/classifier/cgi/foliationtype/0010> ;
      skos:inScheme cgi:foliationtype ;
      skos:narrower foltyp:layered_mylonitic_foliation , foltyp:cleavage_parallel_to_bedding , foltyp:compound_metamorphic_foliation ;
      skos:prefLabel "compound folation"@en .

foltyp:compound_metamorphic_foliation
      rdf:type skos:Concept ;
      dc:creator "Concept Definition Task Group of IUGS CGI Interoperability Working Group (http://www.cgi-iugs.org/tech_collaboration/interoperability_working_group.html)"@en ;
      dc:source "this vocabulary" ;
      skos:broader foltyp:compound_folation ;
      skos:definition "A compound foliation in which the constituent fabric elements are of metamorphic origin."@en ;
      skos:exactMatch <http://resource.geosciml.org/classifier/cgi/foliationtype/0011> ;
      skos:inScheme cgi:foliationtype ;
      skos:prefLabel "compound metamorphic foliation"@en .

foltyp:continuous_cleavage
      rdf:type skos:Concept ;
      dc:creator "Concept Definition Task Group of IUGS CGI Interoperability Working Group (http://www.cgi-iugs.org/tech_collaboration/interoperability_working_group.html)"@en ;
      dc:source "Borradaile et al 1982" ;
      skos:broader foltyp:cleavage ;
      skos:definition "A cleavage that is statistically homogeneous down to the scale of individual mineral grains."@en ;
      skos:exactMatch <http://resource.geosciml.org/classifier/cgi/foliationtype/0012> ;
      skos:inScheme cgi:foliationtype ;
      skos:narrower foltyp:phyllitic_cleavage , foltyp:slaty_cleavage , foltyp:continuous_crenulation_cleavage ;
      skos:prefLabel "continuous cleavage"@en .

foltyp:continuous_crenulation_cleavage
      rdf:type skos:Concept ;
      dc:creator "Concept Definition Task Group of IUGS CGI Interoperability Working Group (http://www.cgi-iugs.org/tech_collaboration/interoperability_working_group.html)"@en ;
      dc:source "Borradaile et al 1982" ;
      skos:broader foltyp:continuous_cleavage , foltyp:crenulation_cleavage ;
      skos:definition "Cleavage defined by long, thin limbs of crenulation folds of pre-existing foliation, in which the boundaries between cleavage domains and lithons are gradational. Both the crenulation foliation and the crenulated (older) foliation are easily visible. Grades to spaced crenulation cleavage as boundaries of cleavage domains become sharp, and to schistosity or compositional layering as the crenulation foliation obscures the crenulated foliation to become the dominant fabric in the rock. In many rocks with continuous crenulation cleavage, the tendency to part along the cleavage may be weak, thus the rock may not technically meet the definition of 'cleavage as used in this vocabulary."@en ;
      skos:exactMatch <http://resource.geosciml.org/classifier/cgi/foliationtype/0013> ;
      skos:inScheme cgi:foliationtype ;
      skos:prefLabel "continuous crenulation cleavage" .

foltyp:crenulation_cleavage
      rdf:type skos:Concept ;
      dc:creator "Concept Definition Task Group of IUGS CGI Interoperability Working Group (http://www.cgi-iugs.org/tech_collaboration/interoperability_working_group.html)"@en ;
      dc:source "Brodie, Kate, Fettes, Douglas, and Harte, Ben, 2007, Structural terms including fault rock terms, in Fettes, D., and Desmons, J., Metamorphic rocks-A classification and Glossary of Terms: Cambridge, UK, Cam-bridge University Press, p. 24-31." ;
      skos:broader foltyp:cleavage ;
      skos:definition "Cleavage that is overprinted on an older foliation that is folded to some degree in association with development of the younger cleavage. Cleavage domains commonly associated with long limbs of crenulation folds, and hinge surfaces of folds are roughly parallel. Wavelength of crenulation folds is less than or equal to 1 cm. Cleavage defined by limbs of microfolds coincident with zones of mineral differentiation"@en ;
      skos:exactMatch <http://resource.geosciml.org/classifier/cgi/foliationtype/0014> ;
      skos:inScheme cgi:foliationtype ;
      skos:narrower foltyp:discrete_crenulation_cleavage , foltyp:continuous_crenulation_cleavage ;
      skos:prefLabel "crenulation cleavage" .

foltyp:crude_or_indistinct_bedding
      rdf:type skos:Concept ;
      dc:creator "Concept Definition Task Group of IUGS CGI Interoperability Working Group (http://www.cgi-iugs.org/tech_collaboration/interoperability_working_group.html)"@en ;
      dc:source "this vocabulary" ;
      skos:broader foltyp:bedding_fabric ;
      skos:definition "Bedding defined by surfaces that are not distinct, e.g. by gradational grain size variations."@en ;
      skos:exactMatch <http://resource.geosciml.org/classifier/cgi/foliationtype/0015> ;
      skos:inScheme cgi:foliationtype ;
      skos:prefLabel "crude or indistinct bedding"@en .

foltyp:cryptomicrobial_lamination
      rdf:type skos:Concept ;
      dc:creator "Concept Definition Task Group of IUGS CGI Interoperability Working Group (http://www.cgi-iugs.org/tech_collaboration/interoperability_working_group.html)"@en ;
      dc:source "GGIPAC; http://www.brs.gov.au/land&water/groundwater/result.internal_stratification.html" ;
      skos:broader foltyp:bedding_lamination_structure ;
      skos:definition "Fabric defined by fine laminae formed by the trapping of grains and lime precipitation in a microbial mat."@en ;
      skos:exactMatch <http://resource.geosciml.org/classifier/cgi/foliationtype/0016> ;
      skos:inScheme cgi:foliationtype ;
      skos:narrower foltyp:stromatolitic_lamination ;
      skos:prefLabel "cryptomicrobial lamination"@en .

foltyp:cumulate_layering
      rdf:type skos:Concept ;
      dc:creator "Concept Definition Task Group of IUGS CGI Interoperability Working Group (http://www.cgi-iugs.org/tech_collaboration/interoperability_working_group.html)"@en ;
      dc:source "Carmichael et al 1974; Best 1982" ;
      skos:broader foltyp:igneous_layering ;
      skos:definition "Layering in igneous rocks in which layers are characterized by variation in relative proportion of magmatically crystallized minerals. Typically a pattern of mineralogical variation will be repeated many times in a vertical section with layers of relatively consistent thickness. See photos in Best [1982] p. 176-177. Gravity-stratified layers typically have mafic minerals at the base and plagioclase at the top and are interpreted to form by crystal settling in magma."@en ;
      skos:exactMatch <http://resource.geosciml.org/classifier/cgi/foliationtype/0017> ;
      skos:inScheme cgi:foliationtype ;
      skos:prefLabel "cumulate layering"@en .

foltyp:discrete_cleavage
      rdf:type skos:Concept ;
      dc:creator "Concept Definition Task Group of IUGS CGI Interoperability Working Group (http://www.cgi-iugs.org/tech_collaboration/interoperability_working_group.html)"@en ;
      dc:source "Borradaile et al., 1982" ;
      skos:broader foltyp:spaced_cleavage ;
      skos:definition "Spaced cleavage in which cleavage domains have sharply defined edges."@en ;
      skos:exactMatch <http://resource.geosciml.org/classifier/cgi/foliationtype/0018> ;
      skos:inScheme cgi:foliationtype ;
      skos:prefLabel "discrete cleavage"@en .

foltyp:discrete_crenulation_cleavage
      rdf:type skos:Concept ;
      dc:creator "Concept Definition Task Group of IUGS CGI Interoperability Working Group (http://www.cgi-iugs.org/tech_collaboration/interoperability_working_group.html)"@en ;
      dc:source "Borradaile et al 1982" ;
      skos:broader foltyp:crenulation_cleavage , foltyp:spaced_cleavage ;
      skos:definition "Crenulation cleavage in which the cleavage domains have discrete boundaries. Amplitude of crenulation folds tends to be small."@en ;
      skos:exactMatch <http://resource.geosciml.org/classifier/cgi/foliationtype/0019> ;
      skos:inScheme cgi:foliationtype ;
      skos:prefLabel "discrete crenulation cleavage"@en .

foltyp:discrete_disjunct_spaced_cleavage
      rdf:type skos:Concept ;
      dc:creator "Concept Definition Task Group of IUGS CGI Interoperability Working Group (http://www.cgi-iugs.org/tech_collaboration/interoperability_working_group.html)"@en ;
      dc:source "Neuendorf et al. 2005; Borradaile et al. 1982." ;
      skos:broader foltyp:spaced_cleavage ;
      skos:definition "Disjunct spaced cleavage defined by discrete cleavage surfaces, typically in low-grade clastic rocks. Syn. Fracture cleavage."@en ;
      skos:exactMatch <http://resource.geosciml.org/classifier/cgi/foliationtype/0020> ;
      skos:inScheme cgi:foliationtype ;
      skos:prefLabel "discrete disjunct spaced cleavage"@en .

foltyp:disjunctive_cleavage
      rdf:type skos:Concept ;
      dc:creator "Concept Definition Task Group of IUGS CGI Interoperability Working Group (http://www.cgi-iugs.org/tech_collaboration/interoperability_working_group.html)"@en ;
      dc:source "Borradaile et al. 1982" ;
      skos:broader foltyp:cleavage ;
      skos:definition "A spaced cleavage independent of any pre-existing mineral orientation; cleavage in which there is no systematic relationship between a pre-existing preferred orientation and the superimposed cleavage. (Borradaile et al., 1982)"@en ;
      skos:exactMatch <http://resource.geosciml.org/classifier/cgi/foliationtype/0021> ;
      skos:inScheme cgi:foliationtype ;
      skos:prefLabel "disjunctive cleavage"@en .

foltyp:domainal_cleavage
      rdf:type skos:Concept ;
      dc:creator "Concept Definition Task Group of IUGS CGI Interoperability Working Group (http://www.cgi-iugs.org/tech_collaboration/interoperability_working_group.html)"@en ;
      dc:source "this vocabulary" ;
      skos:broader foltyp:cleavage ;
      skos:definition "Fabric in which domains of more strongly developed (closely spaced) cleavage are separated by lenses of weakly or non-cleaved rock. Typically observed on outcrop scale and used for geologic unit description"@en ;
      skos:exactMatch <http://resource.geosciml.org/classifier/cgi/foliationtype/0022> ;
      skos:inScheme cgi:foliationtype ;
      skos:prefLabel "domainal cleavage"@en .

foltyp:ductile_shear_banding_foliation
      rdf:type skos:Concept ;
      dc:creator "Concept Definition Task Group of IUGS CGI Interoperability Working Group (http://www.cgi-iugs.org/tech_collaboration/interoperability_working_group.html)"@en ;
      dc:source "Geoscience Victoria, Australia" ;
      skos:broader foltyp:foliation ;
      skos:definition "Foliation defined by regularly spaced ductile shear bands at the scale of descripiton."@en ;
      skos:exactMatch <http://resource.geosciml.org/classifier/cgi/foliationtype/0023> ;
      skos:inScheme cgi:foliationtype ;
      skos:narrower foltyp:c_fabric ;
      skos:prefLabel "ductile shear banding foliation"@en .

foltyp:eutaxitic_foliation
      rdf:type skos:Concept ;
      dc:creator "Concept Definition Task Group of IUGS CGI Interoperability Working Group (http://www.cgi-iugs.org/tech_collaboration/interoperability_working_group.html)"@en ;
      dc:source "Neuendorf et al. 2005; this vocabulary" ;
      skos:broader foltyp:primary_igneous_foliation ;
      skos:definition "Foliation defined by flattened pumice clasts or glass shards, aligned elongate lithic fragments, variations in composition, vesicularity, crystallinity, grain size, spherulite and lithophysae abundance, or the degree of devitrification in a welded tuff. This term denotes interpretation that foliation formed during compaction and welding of tuff."@en ;
      skos:exactMatch <http://resource.geosciml.org/classifier/cgi/foliationtype/0024> ;
      skos:inScheme cgi:foliationtype ;
      skos:prefLabel "eutaxitic foliation"@en .

foltyp:fissile_lamination
      rdf:type skos:Concept ;
      dc:creator "Concept Definition Task Group of IUGS CGI Interoperability Working Group (http://www.cgi-iugs.org/tech_collaboration/interoperability_working_group.html)"@en ;
      dc:source "SLTTs 2004; this vocabulary" ;
      skos:broader foltyp:bedding_lamination_structure ;
      skos:definition "Diffuse to distinct lamination in mudstones and mud, defined by the alignment of clay minerals. Lacks distinct very-fine scale layering and repetition of couplets that characterize varves. Essentially a continuous cleavage parallel to bedding, but considered a sedimentary structure related to sediment compaction during diagenesis."@en ;
      skos:exactMatch <http://resource.geosciml.org/classifier/cgi/foliationtype/0025> ;
      skos:inScheme cgi:foliationtype ;
      skos:prefLabel "fissile lamination"@en .

foltyp:flaser_structure
      rdf:type skos:Concept ;
      dc:creator "Concept Definition Task Group of IUGS CGI Interoperability Working Group (http://www.cgi-iugs.org/tech_collaboration/interoperability_working_group.html)"@en ;
      dc:source "Neuendorf et al. 2005" ;
      skos:broader foltyp:tectonic_foliation ;
      skos:definition "Tectonic foliation defined by lenses and layers of original or relatively unaltered granular minerals surrounded by a matrix of highly sheared and crushed material. No connotation of metamorphic grade."@en ;
      skos:exactMatch <http://resource.geosciml.org/classifier/cgi/foliationtype/0026> ;
      skos:inScheme cgi:foliationtype ;
      skos:prefLabel "flaser structure"@en .

foltyp:flow_layering
      rdf:type skos:Concept ;
      dc:creator "Concept Definition Task Group of IUGS CGI Interoperability Working Group (http://www.cgi-iugs.org/tech_collaboration/interoperability_working_group.html)"@en ;
      dc:source "this vocabulary" ;
      skos:broader foltyp:layering ;
      skos:definition "Layering produced by flow of magma, lava, or diapiric flow of sedimentary rock. Distinction from eutaxitic foliation may be difficult."@en ;
      skos:exactMatch <http://resource.geosciml.org/classifier/cgi/foliationtype/0027> ;
      skos:inScheme cgi:foliationtype ;
      skos:narrower foltyp:lava_flow_banding ;
      skos:prefLabel "flow layering"@en .

foltyp:foliation
      rdf:type skos:Concept ;
      dc:creator "Concept Definition Task Group of IUGS CGI Interoperability Working Group (http://www.cgi-iugs.org/tech_collaboration/interoperability_working_group.html)"@en ;
      dc:source "Jackson 1997" ;
      skos:definition "Fabric defined by the planar arrangement of textural or structural features (fabric elements)."@en ;
      skos:exactMatch <http://resource.geosciml.org/classifier/cgi/foliationtype/0028> ;
      skos:inScheme cgi:foliationtype ;
      skos:narrower foltyp:compound_folation , foltyp:layering , foltyp:joint_fabric , foltyp:tectonic_foliation , foltyp:cleavage , foltyp:low_temperature_flow_foliation , foltyp:grain_shape_foliation , foltyp:ductile_shear_banding_foliation , foltyp:schistosity , foltyp:primary_foliation ;
      skos:prefLabel "foliation"@en ;
      skos:topConceptOf cgi:foliationtype .

foltyp:generic_mylonitic_foliation
      rdf:type skos:Concept ;
      dc:creator "Concept Definition Task Group of IUGS CGI Interoperability Working Group (http://www.cgi-iugs.org/tech_collaboration/interoperability_working_group.html)"@en ;
      dc:source "NADM metamorphic rock vocabulary SLTTm1.0 2004" ;
      skos:broader foltyp:tectonic_foliation ;
      skos:definition "Foliation defined by the shapes of deformed mineral grains or grain aggregates having aspect ratios greater than 1.5:1, greater than 10 percent of the rock is composed of 'matrix' showing evidence of tectonic reduction in grain size, and the foliation and matrix are interpreted to be the product of continuous, crystal-plastic deformation processes. Generic class is used when data are insufficient to determine classification to protomylontic, mylonite, or ultramylonitc foliation, or to specify that any sort of mylontic foliation may be present."@en ;
      skos:exactMatch <http://resource.geosciml.org/classifier/cgi/foliationtype/0029> ;
      skos:inScheme cgi:foliationtype ;
      skos:narrower foltyp:mylonite_foliation , foltyp:ultramylonite_foliation , foltyp:protomylonite_foliation , foltyp:layered_mylonitic_foliation ;
      skos:prefLabel "generic mylonitic foliation"@en .

foltyp:gneissic_layering
      rdf:type skos:Concept ;
      dc:creator "Concept Definition Task Group of IUGS CGI Interoperability Working Group (http://www.cgi-iugs.org/tech_collaboration/interoperability_working_group.html)"@en ;
      dc:source "this vocabulary" ;
      skos:broader foltyp:metamorphic_layering ;
      skos:definition "compositional layering in a metamorphic rock; syn. gneissic banding"@en ;
      skos:exactMatch <http://resource.geosciml.org/classifier/cgi/foliationtype/0030> ;
      skos:inScheme cgi:foliationtype ;
      skos:prefLabel "gneissic layering"@en .

foltyp:grain_shape_foliation
      rdf:type skos:Concept ;
      dc:creator "Concept Definition Task Group of IUGS CGI Interoperability Working Group (http://www.cgi-iugs.org/tech_collaboration/interoperability_working_group.html)"@en ;
      dc:source "this vocabulary" ;
      skos:broader foltyp:foliation ;
      skos:definition "Foliation defined by the alignment of oblate particles, which may be detrital grains, crystals, or crystalline grain aggregates."@en ;
      skos:exactMatch <http://resource.geosciml.org/classifier/cgi/foliationtype/0031> ;
      skos:inScheme cgi:foliationtype ;
      skos:narrower foltyp:s_fabric , foltyp:imbricated_clast_fabric ;
      skos:prefLabel "grain shape foliation"@en .

foltyp:igneous_flow_foliation
      rdf:type skos:Concept ;
      dc:creator "Concept Definition Task Group of IUGS CGI Interoperability Working Group (http://www.cgi-iugs.org/tech_collaboration/interoperability_working_group.html)"@en ;
      dc:source "this vocabulary" ;
      skos:broader foltyp:primary_igneous_foliation ;
      skos:definition "Foliation interpreted to be due to flow in a body of magma or lava. Includes flow banding in lava, and foliation defined by aligned crystals in a phaneritic igneous rock.."@en ;
      skos:exactMatch <http://resource.geosciml.org/classifier/cgi/foliationtype/0032> ;
      skos:inScheme cgi:foliationtype ;
      skos:prefLabel "igneous flow foliation"@en .

foltyp:igneous_lamination
      rdf:type skos:Concept ;
      dc:creator "Concept Definition Task Group of IUGS CGI Interoperability Working Group (http://www.cgi-iugs.org/tech_collaboration/interoperability_working_group.html)"@en ;
      dc:source "this vocabulary" ;
      skos:broader foltyp:primary_igneous_foliation , foltyp:igneous_layering ;
      skos:definition "Foliation defined by surfaces of textural or mineralogical variation formed by igneous processes. If the lamination surfaces are regularly spaced, they may be used to define layers."@en ;
      skos:exactMatch <http://resource.geosciml.org/classifier/cgi/foliationtype/0033> ;
      skos:inScheme cgi:foliationtype ;
      skos:prefLabel "igneous lamination"@en .

foltyp:igneous_layering
      rdf:type skos:Concept ;
      dc:creator "Concept Definition Task Group of IUGS CGI Interoperability Working Group (http://www.cgi-iugs.org/tech_collaboration/interoperability_working_group.html)"@en ;
      dc:source "Geoscience Victoria, Australia" ;
      skos:broader foltyp:primary_igneous_foliation , foltyp:layering ;
      skos:definition "Layering that is the product of processes operating in magma or lava. syn. magmatic layering"@en ;
      skos:exactMatch <http://resource.geosciml.org/classifier/cgi/foliationtype/0034> ;
      skos:inScheme cgi:foliationtype ;
      skos:narrower foltyp:igneous_textural_layering , foltyp:igneous_lamination , foltyp:cumulate_layering , foltyp:lava_flow_banding , foltyp:rhythmic_layering ;
      skos:prefLabel "igneous layering"@en .

foltyp:igneous_textural_layering
      rdf:type skos:Concept ;
      dc:creator "Concept Definition Task Group of IUGS CGI Interoperability Working Group (http://www.cgi-iugs.org/tech_collaboration/interoperability_working_group.html)"@en ;
      dc:source "this vocabulary" ;
      skos:broader foltyp:igneous_layering ;
      skos:definition "Layering defined by grain size/ grain shape variations resulting from crystallization processes in igneous rock, most commonly observed in pegmatite/aplite dikes or bodies, and in Laramide leucogranites of Wilderness suite in Arizona."@en ;
      skos:exactMatch <http://resource.geosciml.org/classifier/cgi/foliationtype/0035> ;
      skos:inScheme cgi:foliationtype ;
      skos:prefLabel "igneous textural layering"@en .

foltyp:imbricated_clast_fabric
      rdf:type skos:Concept ;
      dc:creator "Concept Definition Task Group of IUGS CGI Interoperability Working Group (http://www.cgi-iugs.org/tech_collaboration/interoperability_working_group.html)"@en ;
      dc:source "based on Neuendorf et al 2005" ;
      skos:broader foltyp:grain_shape_foliation , foltyp:primary_foliation ;
      skos:definition "Fabric defined by long axis of tabular clasts stacked like shingles to define a surface that makes a small angle with the bedding surface. A depositional fabric formed by disk-shaped or elongate pebbles all tilted in the same direction; flat sides commonly dip upstream"@en ;
      skos:exactMatch <http://resource.geosciml.org/classifier/cgi/foliationtype/0036> ;
      skos:inScheme cgi:foliationtype ;
      skos:prefLabel "imbricated clast fabric"@en .

foltyp:impersistent_lamination
      rdf:type skos:Concept ;
      dc:creator "Concept Definition Task Group of IUGS CGI Interoperability Working Group (http://www.cgi-iugs.org/tech_collaboration/interoperability_working_group.html)"@en ;
      dc:source "this vocabulary" ;
      skos:broader foltyp:bedding_lamination_structure ;
      skos:definition "Lamination defined by discontinuous surfaces"@en ;
      skos:exactMatch <http://resource.geosciml.org/classifier/cgi/foliationtype/0037> ;
      skos:inScheme cgi:foliationtype ;
      skos:prefLabel "impersistent lamination"@en .

foltyp:irregular_lamination
      rdf:type skos:Concept ;
      dc:creator "Concept Definition Task Group of IUGS CGI Interoperability Working Group (http://www.cgi-iugs.org/tech_collaboration/interoperability_working_group.html)"@en ;
      dc:source "this vocabulary" ;
      skos:broader foltyp:bedding_lamination_structure ;
      skos:definition "Lamination fabric in which individual lamina or groups of lamina are warped in an irregular fashion, like a flattened peice of crumpled paper. A crude planar orientation is discernible."@en ;
      skos:exactMatch <http://resource.geosciml.org/classifier/cgi/foliationtype/0038> ;
      skos:inScheme cgi:foliationtype ;
      skos:prefLabel "irregular lamination"@en .

foltyp:joint_fabric
      rdf:type skos:Concept ;
      dc:creator "Concept Definition Task Group of IUGS CGI Interoperability Working Group (http://www.cgi-iugs.org/tech_collaboration/interoperability_working_group.html)"@en ;
      dc:source "Borradaile et al 1982" ;
      skos:broader foltyp:foliation ;
      skos:definition "Fabric defined by parting surfaces in rock that occur in crudely parallel orientation, spaced greater than 5 cm on average if in a very regular joint set. Spacing is more variable and alignment of surfaces is cruder that cleavage. Typically applies to geologic unit description."@en ;
      skos:exactMatch <http://resource.geosciml.org/classifier/cgi/foliationtype/0039> ;
      skos:inScheme cgi:foliationtype ;
      skos:narrower foltyp:close_joints ;
      skos:prefLabel "joint fabric"@en .

foltyp:laminated_metamorphic_layering
      rdf:type skos:Concept ;
      dc:creator "Concept Definition Task Group of IUGS CGI Interoperability Working Group (http://www.cgi-iugs.org/tech_collaboration/interoperability_working_group.html)"@en ;
      dc:source "Weiss 1972; Borradaile et al 1982; this vocabulary" ;
      skos:broader foltyp:metamorphic_layering ;
      skos:definition "Metamorphic layering in which the layers are less than 1 cm thick. See Weiss, L.E. [1972] plate 36 or Borraidaile et al [1982] plate 137A,B (page 331), plate140A (page 337) for examples."@en ;
      skos:exactMatch <http://resource.geosciml.org/classifier/cgi/foliationtype/0040> ;
      skos:inScheme cgi:foliationtype ;
      skos:prefLabel "laminated metamorphic layering"@en .

foltyp:lava_flow_banding
      rdf:type skos:Concept ;
      dc:creator "Concept Definition Task Group of IUGS CGI Interoperability Working Group (http://www.cgi-iugs.org/tech_collaboration/interoperability_working_group.html)"@en ;
      dc:source "GGIPAC, Australia" ;
      skos:broader foltyp:flow_layering , foltyp:igneous_layering ;
      skos:definition "Layering formed by laminar lava flow, defined by variations in composition, vesicularity, crystallinity, grainsize, spherulite and lithophysae abundance, degree of devitrification, colour, and/or parting surfaces; syn. flow lamination, flow banding"@en ;
      skos:exactMatch <http://resource.geosciml.org/classifier/cgi/foliationtype/0041> ;
      skos:inScheme cgi:foliationtype ;
      skos:prefLabel "lava flow banding"@en .

foltyp:layered_mylonitic_foliation
      rdf:type skos:Concept ;
      dc:creator "Concept Definition Task Group of IUGS CGI Interoperability Working Group (http://www.cgi-iugs.org/tech_collaboration/interoperability_working_group.html)"@en ;
      dc:source "this vocabulary" ;
      skos:broader foltyp:layering , foltyp:compound_folation , foltyp:generic_mylonitic_foliation ;
      skos:definition "compound foliation in which mylonitic foliation is present in rock that has continuous compositional layering. Continuous means individual layers can be traced more than 1 m."@en ;
      skos:exactMatch <http://resource.geosciml.org/classifier/cgi/foliationtype/0042> ;
      skos:inScheme cgi:foliationtype ;
      skos:prefLabel "layered mylonitic foliation"@en .

foltyp:layering
      rdf:type skos:Concept ;
      dc:creator "Concept Definition Task Group of IUGS CGI Interoperability Working Group (http://www.cgi-iugs.org/tech_collaboration/interoperability_working_group.html)"@en ;
      dc:source "this vocabulary" ;
      skos:broader foltyp:foliation ;
      skos:definition "Foliation defined by stacked, differentiable, sheet-like masses of material (layers), with no denotation of the nature (composition, grain size, grain shape...) or origin (igneous, sedimentary, metamorphic) of the layers."@en ;
      skos:exactMatch <http://resource.geosciml.org/classifier/cgi/foliationtype/0043> ;
      skos:inScheme cgi:foliationtype ;
      skos:narrower foltyp:igneous_layering , foltyp:sedimentary_layering , foltyp:metamorphic_layering , foltyp:layered_mylonitic_foliation , foltyp:compositional_layering , foltyp:flow_layering , foltyp:tectonic_layering , foltyp:comb_layering ;
      skos:prefLabel "layering"@en .

foltyp:low_temperature_flow_foliation
      rdf:type skos:Concept ;
      dc:creator "Concept Definition Task Group of IUGS CGI Interoperability Working Group (http://www.cgi-iugs.org/tech_collaboration/interoperability_working_group.html)"@en ;
      dc:source "this vocabulary" ;
      skos:broader foltyp:foliation ;
      skos:definition "Foliation interpreted to be due to flow in a body of rock (typically mudrock, salt, or anhydrite) under low-temperature (non-metamorphic) conditions, typically related to diapirism."@en ;
      skos:exactMatch <http://resource.geosciml.org/classifier/cgi/foliationtype/0044> ;
      skos:inScheme cgi:foliationtype ;
      skos:prefLabel "low temperature flow foliation"@en .

foltyp:metamorphic_differentiation_layering
      rdf:type skos:Concept ;
      dc:creator "Concept Definition Task Group of IUGS CGI Interoperability Working Group (http://www.cgi-iugs.org/tech_collaboration/interoperability_working_group.html)"@en ;
      dc:source "this vocabulary" ;
      skos:broader foltyp:compositional_layering , foltyp:metamorphic_layering ;
      skos:definition "Layering defined by mineralogical variations in a rock body interpreted to be result of solid-state reactions in rock body (metamorphic segregation)."@en ;
      skos:exactMatch <http://resource.geosciml.org/classifier/cgi/foliationtype/0045> ;
      skos:inScheme cgi:foliationtype ;
      skos:prefLabel "metamorphic differentiation layering"@en .

foltyp:metamorphic_layering
      rdf:type skos:Concept ;
      dc:creator "Concept Definition Task Group of IUGS CGI Interoperability Working Group (http://www.cgi-iugs.org/tech_collaboration/interoperability_working_group.html)"@en ;
      dc:source "this vocabulary" ;
      skos:broader foltyp:layering ;
      skos:definition "Layering of unspecified origin in a metamorphic rock. compositional or textural variations may be inherited from protolith, or result from metamorphic processes."@en ;
      skos:exactMatch <http://resource.geosciml.org/classifier/cgi/foliationtype/0046> ;
      skos:inScheme cgi:foliationtype ;
      skos:narrower foltyp:laminated_metamorphic_layering , foltyp:vague_metamorphic_layering , foltyp:metamorphic_layering_inherited_from_protolith , foltyp:gneissic_layering , foltyp:metamorphic_differentiation_layering , foltyp:stromatic_layering ;
      skos:prefLabel "metamorphic layering"@en .

foltyp:metamorphic_layering_inherited_from_protolith
      rdf:type skos:Concept ;
      dc:creator "Concept Definition Task Group of IUGS CGI Interoperability Working Group (http://www.cgi-iugs.org/tech_collaboration/interoperability_working_group.html)"@en ;
      dc:source "this vocabulary" ;
      skos:broader foltyp:metamorphic_layering , foltyp:compositional_layering ;
      skos:definition "Metamorphic layering in which layer differntiation is relict of compositional variations in the protolith, typically heterogeneous sedimentary or volcanic rock."@en ;
      skos:exactMatch <http://resource.geosciml.org/classifier/cgi/foliationtype/0047> ;
      skos:inScheme cgi:foliationtype ;
      skos:narrower foltyp:transposed_bedding_layering ;
      skos:prefLabel "metamorphic layering inherited from protolith"@en .

foltyp:mineralogical_layering
      rdf:type skos:Concept ;
      dc:creator "Concept Definition Task Group of IUGS CGI Interoperability Working Group (http://www.cgi-iugs.org/tech_collaboration/interoperability_working_group.html)"@en ;
      dc:source "this vocabulary" ;
      skos:broader foltyp:compositional_layering ;
      skos:definition "Generic layering defined by variations in mineralogy between individual sheets of material"@en ;
      skos:exactMatch <http://resource.geosciml.org/classifier/cgi/foliationtype/0048> ;
      skos:inScheme cgi:foliationtype ;
      skos:prefLabel "mineralogical layering"@en .

foltyp:mylonite_foliation
      rdf:type skos:Concept ;
      dc:creator "Concept Definition Task Group of IUGS CGI Interoperability Working Group (http://www.cgi-iugs.org/tech_collaboration/interoperability_working_group.html)"@en ;
      dc:source "SLTTm 2004; Sibson 1977" ;
      skos:broader foltyp:generic_mylonitic_foliation ;
      skos:definition "Generic mylonitic foliation in which 50-90 percent of rock is matrix due to tectonic grain size reduction processes. Planar fabric is very apparent due to flattening of mineral grains, development of shear surfaces, and alignment of tabular mineral grains. Lineation is typically present and easily observed."@en ;
      skos:exactMatch <http://resource.geosciml.org/classifier/cgi/foliationtype/0049> ;
      skos:inScheme cgi:foliationtype ;
      skos:prefLabel "mylonite foliation"@en .

foltyp:parallel_bedding
      rdf:type skos:Concept ;
      dc:creator "Concept Definition Task Group of IUGS CGI Interoperability Working Group (http://www.cgi-iugs.org/tech_collaboration/interoperability_working_group.html)"@en ;
      dc:source "SLTTs 2004" ;
      skos:broader foltyp:bedding_fabric ;
      skos:definition "Bedding defined by parallel surfaces. Bedding structure may be lamination or layering."@en ;
      skos:exactMatch <http://resource.geosciml.org/classifier/cgi/foliationtype/0050> ;
      skos:inScheme cgi:foliationtype ;
      skos:prefLabel "parallel bedding" .

foltyp:parallel_bedding_lamination
      rdf:type skos:Concept ;
      dc:creator "Concept Definition Task Group of IUGS CGI Interoperability Working Group (http://www.cgi-iugs.org/tech_collaboration/interoperability_working_group.html)"@en ;
      dc:source "this vocabulary" ;
      skos:broader foltyp:bedding_lamination_structure ;
      skos:definition "Bedding lamination structure in which all visible bedding surfaces are parallel."@en ;
      skos:exactMatch <http://resource.geosciml.org/classifier/cgi/foliationtype/0051> ;
      skos:inScheme cgi:foliationtype ;
      skos:prefLabel "parallel bedding lamination" .

foltyp:phyllitic_cleavage
      rdf:type skos:Concept ;
      dc:creator "Concept Definition Task Group of IUGS CGI Interoperability Working Group (http://www.cgi-iugs.org/tech_collaboration/interoperability_working_group.html)"@en ;
      dc:source "SLTTm 2004; Geoscience Victoria, Australia" ;
      skos:broader foltyp:continuous_cleavage ;
      skos:definition "Continuous cleavage in phyllitic rock; phyllosilicate mineral grains just barely visible, grain size midway between slaty cleavage and schist; typically has a satiny lustre."@en ;
      skos:exactMatch <http://resource.geosciml.org/classifier/cgi/foliationtype/0052> ;
      skos:inScheme cgi:foliationtype ;
      skos:prefLabel "phyllitic cleavage"@en .

foltyp:planar_lamination
      rdf:type skos:Concept ;
      dc:creator "Concept Definition Task Group of IUGS CGI Interoperability Working Group (http://www.cgi-iugs.org/tech_collaboration/interoperability_working_group.html)"@en ;
      dc:source "this vocabulary" ;
      skos:broader foltyp:bedding_lamination_structure ;
      skos:definition "Lamination that is defined by planar bedding surfaces at the scale of description."@en ;
      skos:exactMatch <http://resource.geosciml.org/classifier/cgi/foliationtype/0053> ;
      skos:inScheme cgi:foliationtype ;
      skos:prefLabel "planar lamination"@en .

foltyp:primary_foliation
      rdf:type skos:Concept ;
      dc:creator "Concept Definition Task Group of IUGS CGI Interoperability Working Group (http://www.cgi-iugs.org/tech_collaboration/interoperability_working_group.html)"@en ;
      dc:source "this vocabulary" ;
      skos:broader foltyp:foliation ;
      skos:definition "Foliation formed during original process of deposition or crystallization of an igneous or sedimentary material."@en ;
      skos:exactMatch <http://resource.geosciml.org/classifier/cgi/foliationtype/0054> ;
      skos:inScheme cgi:foliationtype ;
      skos:narrower foltyp:bedding_fabric , foltyp:imbricated_clast_fabric , foltyp:primary_igneous_foliation ;
      skos:prefLabel "primary foliation" .

foltyp:primary_igneous_foliation
      rdf:type skos:Concept ;
      dc:creator "Concept Definition Task Group of IUGS CGI Interoperability Working Group (http://www.cgi-iugs.org/tech_collaboration/interoperability_working_group.html)"@en ;
      dc:source "this vocabulary" ;
      skos:broader foltyp:primary_foliation ;
      skos:definition "Foliation interpreted to be the product of igneous processes, formed in the rock while melt was still present.."@en ;
      skos:exactMatch <http://resource.geosciml.org/classifier/cgi/foliationtype/0055> ;
      skos:inScheme cgi:foliationtype ;
      skos:narrower foltyp:igneous_flow_foliation , foltyp:igneous_lamination , foltyp:igneous_layering , foltyp:eutaxitic_foliation ;
      skos:prefLabel "primary igneous foliation"@en .

foltyp:protomylonite_foliation
      rdf:type skos:Concept ;
      dc:creator "Concept Definition Task Group of IUGS CGI Interoperability Working Group (http://www.cgi-iugs.org/tech_collaboration/interoperability_working_group.html)"@en ;
      dc:source "SLTTm 2004; Sibson 1977" ;
      skos:broader foltyp:generic_mylonitic_foliation ;
      skos:definition "Generic mylonitic foliation in which 10-50 percent of rock is matrix due to tectonic grain size reduction processes. Planar aspect of fabric may be quite subtle in weakly deformed rocks."@en ;
      skos:exactMatch <http://resource.geosciml.org/classifier/cgi/foliationtype/0056> ;
      skos:inScheme cgi:foliationtype ;
      skos:prefLabel "protomylonite foliation"@en .

foltyp:rhythmic_layering
      rdf:type skos:Concept ;
      dc:creator "Concept Definition Task Group of IUGS CGI Interoperability Working Group (http://www.cgi-iugs.org/tech_collaboration/interoperability_working_group.html)"@en ;
      dc:source "Jackson 1997" ;
      skos:broader foltyp:igneous_layering ;
      skos:definition "Layering in igneous rock defined by repeated gravity-stratified layers of typically mafic minerals at the base and plagioclase at the top; formed by crystal settling"@en ;
      skos:exactMatch <http://resource.geosciml.org/classifier/cgi/foliationtype/0057> ;
      skos:inScheme cgi:foliationtype ;
      skos:prefLabel "rhythmic layering"@en .

foltyp:rough_cleavage
      rdf:type skos:Concept ;
      dc:creator "Concept Definition Task Group of IUGS CGI Interoperability Working Group (http://www.cgi-iugs.org/tech_collaboration/interoperability_working_group.html)"@en ;
      dc:source "Neuendorf et al. 2005; Borradaile et al, 1990" ;
      skos:broader foltyp:cleavage ;
      skos:definition "Disjunct (Borradaile et al, 1990) cleavage characterized by short, discontinuous clavage surfaces, typically with concentrations of phyllosilicate minerals. common in micaceous sandstone."@en ;
      skos:exactMatch <http://resource.geosciml.org/classifier/cgi/foliationtype/0058> ;
      skos:inScheme cgi:foliationtype ;
      skos:prefLabel "rough cleavage"@en .

foltyp:s_fabric
      rdf:type skos:Concept ;
      dc:creator "Concept Definition Task Group of IUGS CGI Interoperability Working Group (http://www.cgi-iugs.org/tech_collaboration/interoperability_working_group.html)"@en ;
      dc:source "Geoscience Victoria, Australia" ;
      skos:broader foltyp:grain_shape_foliation , foltyp:tectonic_foliation ;
      skos:definition "Foliation in mylonite defined by alignment of tabular crystals or deformed mineral grains; often with sigmoid shape, typically curving into an associated ductile shear banding foliation (C fabric) with a consistent sense."@en ;
      skos:exactMatch <http://resource.geosciml.org/classifier/cgi/foliationtype/0059> ;
      skos:inScheme cgi:foliationtype ;
      skos:prefLabel "s fabric"@en .

foltyp:scaly_cleavage
      rdf:type skos:Concept ;
      dc:creator "Concept Definition Task Group of IUGS CGI Interoperability Working Group (http://www.cgi-iugs.org/tech_collaboration/interoperability_working_group.html)"@en ;
      dc:source "Based on Jackson 1997" ;
      skos:broader foltyp:spaced_cleavage ;
      skos:definition "Discrete, anastomosing spaced cleavage characterized by smooth and highly polished/slickensided cleavage surfaces that intersect with one another to form lensoid flakes, scales or chips. common in pelitic rocks in shear zones, melange, or deformed accretionary complexes."@en ;
      skos:exactMatch <http://resource.geosciml.org/classifier/cgi/foliationtype/0060> ;
      skos:inScheme cgi:foliationtype ;
      skos:prefLabel "scaly cleavage"@en .

foltyp:schistosity
      rdf:type skos:Concept ;
      dc:creator "Concept Definition Task Group of IUGS CGI Interoperability Working Group (http://www.cgi-iugs.org/tech_collaboration/interoperability_working_group.html)"@en ;
      dc:source "NADM metamorphic rock vocabulary SLTTm1.0 2004" ;
      skos:broader foltyp:foliation ;
      skos:definition "A fabric defined the parallel, planar arrangement of mineral grains having a platy, lamellar, or tabular crystallographic habit that are oriented in a continuous planar or rarely a linear fabric. Schistosity is commonly, but not necessarily, a crystalloblastic foliation. Platy mineral grains typically 1 to 10 mm across (Jackson, 1997), at smaller grain size grades into phyllitic cleavage. Schistosity is typically associated with a continuous cleavage due to the tendency to part parallel to the aligned mineral grains."@en ;
      skos:exactMatch <http://resource.geosciml.org/classifier/cgi/foliationtype/0061> ;
      skos:inScheme cgi:foliationtype ;
      skos:prefLabel "schistosity"@en .

foltyp:sedimentary_layering
      rdf:type skos:Concept ;
      dc:creator "Concept Definition Task Group of IUGS CGI Interoperability Working Group (http://www.cgi-iugs.org/tech_collaboration/interoperability_working_group.html)"@en ;
      dc:source "this vocabulary" ;
      skos:broader foltyp:bedding_fabric , foltyp:layering ;
      skos:definition "Layering resulting from primary sedimentary processes, in which the individual layers (beds) are bounded by discontinuities related to events in the depositional history."@en ;
      skos:exactMatch <http://resource.geosciml.org/classifier/cgi/foliationtype/0062> ;
      skos:inScheme cgi:foliationtype ;
      skos:prefLabel "sedimentary layering"@en .

foltyp:slaty_cleavage
      rdf:type skos:Concept ;
      dc:creator "Concept Definition Task Group of IUGS CGI Interoperability Working Group (http://www.cgi-iugs.org/tech_collaboration/interoperability_working_group.html)"@en ;
      dc:source "Brodie, Kate, Fettes, Douglas, and Harte, Ben, 2007, Structural terms including fault rock terms, in Fettes, D., and Desmons, J., Metamorphic rocks-A classification and Glossary of Terms: Cambridge, UK, Cam-bridge University Press, p. 24-31.; Jackson 1997" ;
      skos:broader foltyp:continuous_cleavage ;
      skos:definition "Continuous cleavage defined by aligned fine to very-fine grained phylosilicate mineral grains. The individual grains defining the fabric are too small to be seen by the unaided eye. Grades into phyllitic cleavage as grain size increases. Cleavage domains typically less than 100 micrometres wide; rock easily splits into slabs and thin plates."@en ;
      skos:exactMatch <http://resource.geosciml.org/classifier/cgi/foliationtype/0063> ;
      skos:inScheme cgi:foliationtype ;
      skos:prefLabel "slaty cleavage"@en .

foltyp:solution_cleavage
      rdf:type skos:Concept ;
      dc:creator "Concept Definition Task Group of IUGS CGI Interoperability Working Group (http://www.cgi-iugs.org/tech_collaboration/interoperability_working_group.html)"@en ;
      dc:source "Geoscience Victoria, Australia" ;
      skos:broader foltyp:spaced_cleavage ;
      skos:definition "Spaced cleavage forming an array of parallel to anastomosing, stylolitic to smooth, fracture-like partings formed by rock dissolution. Dissolution is indicated by discontinuity and offset of primary features that intersect cleavage surfaces, and typically by accumulation of insoluble residue along cleavage surface. Syn. stylolitic cleavage, pressure solution cleavage"@en ;
      skos:exactMatch <http://resource.geosciml.org/classifier/cgi/foliationtype/0064> ;
      skos:inScheme cgi:foliationtype ;
      skos:prefLabel "solution cleavage"@en .

foltyp:spaced_cleavage
      rdf:type skos:Concept ;
      dc:creator "Concept Definition Task Group of IUGS CGI Interoperability Working Group (http://www.cgi-iugs.org/tech_collaboration/interoperability_working_group.html)"@en ;
      dc:source "Borradaile et al. 1982" ;
      skos:broader foltyp:cleavage ;
      skos:definition "Cleavage in which cleavage domains are spaced at finite intervals as the scale of description. Microlithons of uncleaved rock separate cleavage domains."@en ;
      skos:exactMatch <http://resource.geosciml.org/classifier/cgi/foliationtype/0065> ;
      skos:inScheme cgi:foliationtype ;
      skos:narrower foltyp:scaly_cleavage , foltyp:discrete_crenulation_cleavage , foltyp:discrete_cleavage , foltyp:anastomosing_spaced_cleavage , foltyp:solution_cleavage , foltyp:discrete_disjunct_spaced_cleavage ;
      skos:prefLabel "spaced cleavage"@en .

foltyp:stromatic_layering
      rdf:type skos:Concept ;
      dc:creator "Concept Definition Task Group of IUGS CGI Interoperability Working Group (http://www.cgi-iugs.org/tech_collaboration/interoperability_working_group.html)"@en ;
      dc:source "Weiss 1972; Borradaile et al 1982; Neuendorf et al. 2005" ;
      skos:broader foltyp:metamorphic_layering ;
      skos:definition "Tectonic layering in which variations that distinguish the layers are the result of melt segregation during high-grade metamorphism; some layers have magmatic/igneous mineralogy. Plates 143 and 144, Borradaile et al [1982] (page 344-347) Syn. Migmatitic layering, lit-par-lit layering"@en ;
      skos:exactMatch <http://resource.geosciml.org/classifier/cgi/foliationtype/0066> ;
      skos:inScheme cgi:foliationtype ;
      skos:prefLabel "stromatic layering"@en .

foltyp:stromatolitic_lamination
      rdf:type skos:Concept ;
      dc:creator "Concept Definition Task Group of IUGS CGI Interoperability Working Group (http://www.cgi-iugs.org/tech_collaboration/interoperability_working_group.html)"@en ;
      dc:source "Based on Neuendorf et al 2005" ;
      skos:broader foltyp:cryptomicrobial_lamination ;
      skos:definition "Lamination produced by sediment trapping, binding and or precipitation by cyanophytes (blue-green algae)"@en ;
      skos:exactMatch <http://resource.geosciml.org/classifier/cgi/foliationtype/0067> ;
      skos:inScheme cgi:foliationtype ;
      skos:prefLabel "stromatolitic lamination"@en .

foltyp:tectonic_foliation
      rdf:type skos:Concept ;
      dc:creator "Concept Definition Task Group of IUGS CGI Interoperability Working Group (http://www.cgi-iugs.org/tech_collaboration/interoperability_working_group.html)"@en ;
      dc:source "this vocabulary" ;
      skos:broader foltyp:foliation ;
      skos:definition "Foliation in a rock body defined by physical components related to deformation subsequent to solidification of the rock."@en ;
      skos:exactMatch <http://resource.geosciml.org/classifier/cgi/foliationtype/0068> ;
      skos:inScheme cgi:foliationtype ;
      skos:narrower foltyp:s_fabric , foltyp:generic_mylonitic_foliation , foltyp:flaser_structure , foltyp:tectonic_layering ;
      skos:prefLabel "tectonic foliation"@en .

foltyp:tectonic_layering
      rdf:type skos:Concept ;
      dc:creator "Concept Definition Task Group of IUGS CGI Interoperability Working Group (http://www.cgi-iugs.org/tech_collaboration/interoperability_working_group.html)"@en ;
      dc:source "Weiss 1972; Borradaile et al 1982; this vocabulary" ;
      skos:broader foltyp:layering , foltyp:tectonic_foliation ;
      skos:definition "Layering defined by mineralogical or textural variations in a rock body that are interpreted to be related to deformation or metamorphism, commonly associated with layers that have sharp boundaries. Also known as gneissic foliation. See plates 142-145 (p. 342-349) in Borradaile et al [1982] and plate 46A to 49A in Weiss [1972]."@en ;
      skos:exactMatch <http://resource.geosciml.org/classifier/cgi/foliationtype/0069> ;
      skos:inScheme cgi:foliationtype ;
      skos:prefLabel "tectonic layering"@en .

foltyp:transposed_bedding_layering
      rdf:type skos:Concept ;
      dc:creator "Concept Definition Task Group of IUGS CGI Interoperability Working Group (http://www.cgi-iugs.org/tech_collaboration/interoperability_working_group.html)"@en ;
      dc:source "this vocabulary" ;
      skos:broader foltyp:metamorphic_layering_inherited_from_protolith ;
      skos:definition "Layering interpreted to have originated as sedimentary bedding that has been transposed as a result of metamorphism and deformation."@en ;
      skos:exactMatch <http://resource.geosciml.org/classifier/cgi/foliationtype/0070> ;
      skos:inScheme cgi:foliationtype ;
      skos:prefLabel "transposed bedding layering"@en .

foltyp:ultramylonite_foliation
      rdf:type skos:Concept ;
      dc:creator "Concept Definition Task Group of IUGS CGI Interoperability Working Group (http://www.cgi-iugs.org/tech_collaboration/interoperability_working_group.html)"@en ;
      dc:source "SLTTm 2004; Sibson 1977" ;
      skos:broader foltyp:generic_mylonitic_foliation ;
      skos:definition "Mylonitic foliation in which greater than 90 percent of rock is matrix due to tectonic grain size reduction processes. Typically rock is very-fine grained to aphanitic, with sparse porphyroclasts, and vague to prominent lamination on a mm scale."@en ;
      skos:exactMatch <http://resource.geosciml.org/classifier/cgi/foliationtype/0071> ;
      skos:inScheme cgi:foliationtype ;
      skos:prefLabel "ultramylonite foliation"@en .

foltyp:undulating_lamination
      rdf:type skos:Concept ;
      dc:creator "Concept Definition Task Group of IUGS CGI Interoperability Working Group (http://www.cgi-iugs.org/tech_collaboration/interoperability_working_group.html)"@en ;
      dc:source "this vocabulary" ;
      skos:broader foltyp:bedding_lamination_structure ;
      skos:definition "Gently curviplanar or wavy bedding lamination structure"@en ;
      skos:exactMatch <http://resource.geosciml.org/classifier/cgi/foliationtype/0072> ;
      skos:inScheme cgi:foliationtype ;
      skos:prefLabel "undulating lamination"@en .

foltyp:vague_metamorphic_layering
      rdf:type skos:Concept ;
      dc:creator "Concept Definition Task Group of IUGS CGI Interoperability Working Group (http://www.cgi-iugs.org/tech_collaboration/interoperability_working_group.html)"@en ;
      dc:source "Weiss 1972;Borradaile et al 1982; this vocabulary" ;
      skos:broader foltyp:metamorphic_layering ;
      skos:definition "Metamorphic layering of uncertain origin, defined by subtle mineralogical or textural variations, with gradational layer boundaries. See plate 142 in Borradaile et al [1982]."@en ;
      skos:exactMatch <http://resource.geosciml.org/classifier/cgi/foliationtype/0073> ;
      skos:inScheme cgi:foliationtype ;
      skos:prefLabel "vague metamorphic layering"@en .

foltyp:varve_lamination
      rdf:type skos:Concept ;
      dc:creator "Concept Definition Task Group of IUGS CGI Interoperability Working Group (http://www.cgi-iugs.org/tech_collaboration/interoperability_working_group.html)"@en ;
      dc:source "SLTTs 2004; Jackson 1997" ;
      skos:broader foltyp:bedding_lamination_structure ;
      skos:definition "Bedding defined by distinct, parallel laminae (layers less than 1 cm thick), typically occurring in sequences of distinct couplets (e.g. dark and light color). Generally interpreted as deposited from suspension in still water, with each lamina thought to be an annual sedimentation unit. Typically consists of mud-size sediment."@en ;
      skos:exactMatch <http://resource.geosciml.org/classifier/cgi/foliationtype/0074> ;
      skos:inScheme cgi:foliationtype ;
      skos:prefLabel "varve lamination"@en .

cgi:foliationtype
      rdf:type owl:Ontology , skos:ConceptScheme ;
      dc:contributor "Stephen M Richard" ;
      dc:creator "Concept Definition Task Group of IUGS CGI Interoperability Working Group (http://www.cgi-iugs.org/tech_collaboration/interoperability_working_group.html)"@en ;
      dc:date "2009-11-04" ;
      dc:description "This file contains the CGI Foliation type vocabulary. Use for soft typing GeoSciML GeologicStructure.Foliation elements. Generated from compilation."@en , "vocabulary for categories of planar fabric, for use in GeoSciML interchange documents"@en ;
      dc:format "application/rdf+xml" ;
      dc:identifier "http://resource.geosciml.org/classifierscheme/cgi/201211/foliationtype" ;
      dc:publisher "Concept Definition Task Group of IUGS CGI Interoperability Working Group (http://www.cgi-iugs.org/tech_collaboration/interoperability_working_group.html)"@en ;
      dc:subject "Planar fabrics in rocks"@en ;
      dc:title "CGI Foliation Type categories"@en ;
      owl:imports <http://www.w3.org/2004/02/skos/core> , <http://rdfs.org/ns/void> ;
      owl:versionInfo "201211" ;
      skos:definition "This file contains the CGI Foliation type vocabulary. Use for soft typing GeoSciML GeologicStructure.Foliation elements."@en ;
      skos:historyNote "2012-02-07 SMR update URI to replace numeric final token with English-language string as in original URN scheme."@en , "2010-02-11 Add narrower relationship links by adding skos:narrower link in Protege, defining skos:narrower as inverse of skos:broader, calculating with Pellet reasoner to add inferred axioms, and using 'file/Export inferred axioms as ontology' in Protege."@en , "2012-11-24 SMR Update to 201211 version; add collection entity, check all pref labels are lower case, remove owl:NamedIndividual and Owl:Thing rdf:types."@en , "2010-11-28 SMR Replace URN with http URI according to CGI URI scheme (https://www.seegrid.csiro.au/wiki/bin/view/CGIModel/PersistentIdentifiersInGeoSciMLServices#Identifier_value)"@en ;
      skos:prefLabel "FoliationType"@en .

<http://resource.geosciml.org/vocabulary/cgi/201211/foliationtype>
      rdf:type void:Dataset ;
      rdfs:label "Foliation type vocabulary"^^xsd:string .

skos:ConceptScheme
      rdf:type owl:Class .
