<?xml version="1.0" encoding="UTF-8"?>
<rdf:RDF
	xmlns:cgi="http://resource.geosciml.org/classifierscheme/cgi/201211/"
	xmlns:dc="http://purl.org/dc/elements/1.1/"
	xmlns:foltyp="http://resource.geosciml.org/classifier/cgi/foliationtype/"
	xmlns:owl="http://www.w3.org/2002/07/owl#"
	xmlns:owl2xml="http://www.w3.org/2006/12/owl2-xml#"
	xmlns:rdf="http://www.w3.org/1999/02/22-rdf-syntax-ns#"
	xmlns:rdfs="http://www.w3.org/2000/01/rdf-schema#"
	xmlns:skos="http://www.w3.org/2004/02/skos/core#"
	xmlns:void="http://rdfs.org/ns/void#"
	xmlns:xsd="http://www.w3.org/2001/XMLSchema#">

<rdf:Description rdf:about="http://resource.geosciml.org/classifier/cgi/foliationtype/">
	<rdf:type rdf:resource="http://www.w3.org/2004/02/skos/core#Collection"/>
	<rdfs:label xml:lang="en">foliation type concepts</rdfs:label>
	<skos:definition xml:lang="en">This resource defines the concept space for foliation type concepts by extension; it includes all concepts in this conceptScheme, as well as concepts in previous versions of the scheme.</skos:definition>
	<skos:member rdf:resource="http://resource.geosciml.org/classifier/cgi/foliationtype/layering"/>
	<skos:member rdf:resource="http://resource.geosciml.org/classifier/cgi/foliationtype/sedimentary_layering"/>
	<skos:member rdf:resource="http://resource.geosciml.org/classifier/cgi/foliationtype/domainal_cleavage"/>
	<skos:member rdf:resource="http://resource.geosciml.org/classifier/cgi/foliationtype/cumulate_layering"/>
	<skos:member rdf:resource="http://resource.geosciml.org/classifier/cgi/foliationtype/scaly_cleavage"/>
	<skos:member rdf:resource="http://resource.geosciml.org/classifier/cgi/foliationtype/comb_layering"/>
	<skos:member rdf:resource="http://resource.geosciml.org/classifier/cgi/foliationtype/tectonic_foliation"/>
	<skos:member rdf:resource="http://resource.geosciml.org/classifier/cgi/foliationtype/cryptomicrobial_lamination"/>
	<skos:member rdf:resource="http://resource.geosciml.org/classifier/cgi/foliationtype/crenulation_cleavage"/>
	<skos:member rdf:resource="http://resource.geosciml.org/classifier/cgi/foliationtype/cleavage"/>
	<skos:member rdf:resource="http://resource.geosciml.org/classifier/cgi/foliationtype/compound_metamorphic_foliation"/>
	<skos:member rdf:resource="http://resource.geosciml.org/classifier/cgi/foliationtype/foliation"/>
	<skos:member rdf:resource="http://resource.geosciml.org/classifier/cgi/foliationtype/lava_flow_banding"/>
	<skos:member rdf:resource="http://resource.geosciml.org/classifier/cgi/foliationtype/transposed_bedding_layering"/>
	<skos:member rdf:resource="http://resource.geosciml.org/classifier/cgi/foliationtype/mylonite_foliation"/>
	<skos:member rdf:resource="http://resource.geosciml.org/classifier/cgi/foliationtype/generic_mylonitic_foliation"/>
	<skos:member rdf:resource="http://resource.geosciml.org/classifier/cgi/foliationtype/rhythmic_layering"/>
	<skos:member rdf:resource="http://resource.geosciml.org/classifier/cgi/foliationtype/metamorphic_layering"/>
	<skos:member rdf:resource="http://resource.geosciml.org/classifier/cgi/foliationtype/discrete_disjunct_spaced_cleavage"/>
	<skos:member rdf:resource="http://resource.geosciml.org/classifier/cgi/foliationtype/continuous_crenulation_cleavage"/>
	<skos:member rdf:resource="http://resource.geosciml.org/classifier/cgi/foliationtype/flow_layering"/>
	<skos:member rdf:resource="http://resource.geosciml.org/classifier/cgi/foliationtype/bedding_fabric"/>
	<skos:member rdf:resource="http://resource.geosciml.org/classifier/cgi/foliationtype/igneous_textural_layering"/>
	<skos:member rdf:resource="http://resource.geosciml.org/classifier/cgi/foliationtype/slaty_cleavage"/>
	<skos:member rdf:resource="http://resource.geosciml.org/classifier/cgi/foliationtype/imbricated_clast_fabric"/>
	<skos:member rdf:resource="http://resource.geosciml.org/classifier/cgi/foliationtype/metamorphic_layering_inherited_from_protolith"/>
	<skos:member rdf:resource="http://resource.geosciml.org/classifier/cgi/foliationtype/varve_lamination"/>
	<skos:member rdf:resource="http://resource.geosciml.org/classifier/cgi/foliationtype/phyllitic_cleavage"/>
	<skos:member rdf:resource="http://resource.geosciml.org/classifier/cgi/foliationtype/flaser_structure"/>
	<skos:member rdf:resource="http://resource.geosciml.org/classifier/cgi/foliationtype/anastomosing_spaced_cleavage"/>
	<skos:member rdf:resource="http://resource.geosciml.org/classifier/cgi/foliationtype/close_joints"/>
	<skos:member rdf:resource="http://resource.geosciml.org/classifier/cgi/foliationtype/c_fabric"/>
	<skos:member rdf:resource="http://resource.geosciml.org/classifier/cgi/foliationtype/undulating_lamination"/>
	<skos:member rdf:resource="http://resource.geosciml.org/classifier/cgi/foliationtype/ultramylonite_foliation"/>
	<skos:member rdf:resource="http://resource.geosciml.org/classifier/cgi/foliationtype/impersistent_lamination"/>
	<skos:member rdf:resource="http://resource.geosciml.org/classifier/cgi/foliationtype/metamorphic_differentiation_layering"/>
	<skos:member rdf:resource="http://resource.geosciml.org/classifier/cgi/foliationtype/gneissic_layering"/>
	<skos:member rdf:resource="http://resource.geosciml.org/classifier/cgi/foliationtype/fissile_lamination"/>
	<skos:member rdf:resource="http://resource.geosciml.org/classifier/cgi/foliationtype/joint_fabric"/>
	<skos:member rdf:resource="http://resource.geosciml.org/classifier/cgi/foliationtype/solution_cleavage"/>
	<skos:member rdf:resource="http://resource.geosciml.org/classifier/cgi/foliationtype/s_fabric"/>
	<skos:member rdf:resource="http://resource.geosciml.org/classifier/cgi/foliationtype/tectonic_layering"/>
	<skos:member rdf:resource="http://resource.geosciml.org/classifier/cgi/foliationtype/disjunctive_cleavage"/>
	<skos:member rdf:resource="http://resource.geosciml.org/classifier/cgi/foliationtype/cleavage_parallel_to_bedding"/>
	<skos:member rdf:resource="http://resource.geosciml.org/classifier/cgi/foliationtype/discrete_crenulation_cleavage"/>
	<skos:member rdf:resource="http://resource.geosciml.org/classifier/cgi/foliationtype/stromatic_layering"/>
	<skos:member rdf:resource="http://resource.geosciml.org/classifier/cgi/foliationtype/rough_cleavage"/>
	<skos:member rdf:resource="http://resource.geosciml.org/classifier/cgi/foliationtype/igneous_flow_foliation"/>
	<skos:member rdf:resource="http://resource.geosciml.org/classifier/cgi/foliationtype/protomylonite_foliation"/>
	<skos:member rdf:resource="http://resource.geosciml.org/classifier/cgi/foliationtype/parallel_bedding_lamination"/>
	<skos:member rdf:resource="http://resource.geosciml.org/classifier/cgi/foliationtype/primary_igneous_foliation"/>
	<skos:member rdf:resource="http://resource.geosciml.org/classifier/cgi/foliationtype/crude_or_indistinct_bedding"/>
	<skos:member rdf:resource="http://resource.geosciml.org/classifier/cgi/foliationtype/ductile_shear_banding_foliation"/>
	<skos:member rdf:resource="http://resource.geosciml.org/classifier/cgi/foliationtype/planar_lamination"/>
	<skos:member rdf:resource="http://resource.geosciml.org/classifier/cgi/foliationtype/low_temperature_flow_foliation"/>
	<skos:member rdf:resource="http://resource.geosciml.org/classifier/cgi/foliationtype/spaced_cleavage"/>
	<skos:member rdf:resource="http://resource.geosciml.org/classifier/cgi/foliationtype/laminated_metamorphic_layering"/>
	<skos:member rdf:resource="http://resource.geosciml.org/classifier/cgi/foliationtype/primary_foliation"/>
	<skos:member rdf:resource="http://resource.geosciml.org/classifier/cgi/foliationtype/compositional_layering"/>
	<skos:member rdf:resource="http://resource.geosciml.org/classifier/cgi/foliationtype/compound_folation"/>
	<skos:member rdf:resource="http://resource.geosciml.org/classifier/cgi/foliationtype/irregular_lamination"/>
	<skos:member rdf:resource="http://resource.geosciml.org/classifier/cgi/foliationtype/parallel_bedding"/>
	<skos:member rdf:resource="http://resource.geosciml.org/classifier/cgi/foliationtype/stromatolitic_lamination"/>
	<skos:member rdf:resource="http://resource.geosciml.org/classifier/cgi/foliationtype/discrete_cleavage"/>
	<skos:member rdf:resource="http://resource.geosciml.org/classifier/cgi/foliationtype/vague_metamorphic_layering"/>
	<skos:member rdf:resource="http://resource.geosciml.org/classifier/cgi/foliationtype/eutaxitic_foliation"/>
	<skos:member rdf:resource="http://resource.geosciml.org/classifier/cgi/foliationtype/layered_mylonitic_foliation"/>
	<skos:member rdf:resource="http://resource.geosciml.org/classifier/cgi/foliationtype/continuous_cleavage"/>
	<skos:member rdf:resource="http://resource.geosciml.org/classifier/cgi/foliationtype/grain_shape_foliation"/>
	<skos:member rdf:resource="http://resource.geosciml.org/classifier/cgi/foliationtype/igneous_layering"/>
	<skos:member rdf:resource="http://resource.geosciml.org/classifier/cgi/foliationtype/schistosity"/>
	<skos:member rdf:resource="http://resource.geosciml.org/classifier/cgi/foliationtype/mineralogical_layering"/>
	<skos:member rdf:resource="http://resource.geosciml.org/classifier/cgi/foliationtype/igneous_lamination"/>
	<skos:member rdf:resource="http://resource.geosciml.org/classifier/cgi/foliationtype/bedding_lamination_structure"/>
	<skos:prefLabel xml:lang="en">CGI Foliation Type</skos:prefLabel>
</rdf:Description>

<rdf:Description rdf:about="http://resource.geosciml.org/classifier/cgi/foliationtype/anastomosing_spaced_cleavage">
	<rdf:type rdf:resource="http://www.w3.org/2004/02/skos/core#Concept"/>
	<dc:creator xml:lang="en">Concept Definition Task Group of IUGS CGI Interoperability Working Group (http://www.cgi-iugs.org/tech_collaboration/interoperability_working_group.html)</dc:creator>
	<dc:source rdf:datatype="http://www.w3.org/2001/XMLSchema#string">Geological Survey Victoria, Australia</dc:source>
	<skos:broader rdf:resource="http://resource.geosciml.org/classifier/cgi/foliationtype/spaced_cleavage"/>
	<skos:definition xml:lang="en">spaced cleavage domains branch and rejoin, creating lens-shaped microlithons.</skos:definition>
	<skos:exactMatch rdf:resource="http://resource.geosciml.org/classifier/cgi/foliationtype/0001"/>
	<skos:inScheme rdf:resource="http://resource.geosciml.org/classifierscheme/cgi/201211/foliationtype"/>
	<skos:prefLabel xml:lang="en">anastomosing spaced cleavage</skos:prefLabel>
</rdf:Description>

<rdf:Description rdf:about="http://resource.geosciml.org/classifier/cgi/foliationtype/bedding_fabric">
	<rdf:type rdf:resource="http://www.w3.org/2004/02/skos/core#Concept"/>
	<dc:creator xml:lang="en">Concept Definition Task Group of IUGS CGI Interoperability Working Group (http://www.cgi-iugs.org/tech_collaboration/interoperability_working_group.html)</dc:creator>
	<dc:source>SLTTs 2004; this vocabulary</dc:source>
	<skos:broader rdf:resource="http://resource.geosciml.org/classifier/cgi/foliationtype/primary_foliation"/>
	<skos:definition xml:lang="en">Fabric defined by textural or mineralogic variations in sediment produced by depositional processes. May be manifested by lamination structure within the sediment, or by layering in which the individual layers (beds) are bounded by discontinuities related to events in the depositional history.</skos:definition>
	<skos:exactMatch rdf:resource="http://resource.geosciml.org/classifier/cgi/foliationtype/0002"/>
	<skos:inScheme rdf:resource="http://resource.geosciml.org/classifierscheme/cgi/201211/foliationtype"/>
	<skos:narrower rdf:resource="http://resource.geosciml.org/classifier/cgi/foliationtype/parallel_bedding"/>
	<skos:narrower rdf:resource="http://resource.geosciml.org/classifier/cgi/foliationtype/sedimentary_layering"/>
	<skos:narrower rdf:resource="http://resource.geosciml.org/classifier/cgi/foliationtype/crude_or_indistinct_bedding"/>
	<skos:narrower rdf:resource="http://resource.geosciml.org/classifier/cgi/foliationtype/bedding_lamination_structure"/>
	<skos:prefLabel xml:lang="en">bedding fabric</skos:prefLabel>
</rdf:Description>

<rdf:Description rdf:about="http://resource.geosciml.org/classifier/cgi/foliationtype/bedding_lamination_structure">
	<rdf:type rdf:resource="http://www.w3.org/2004/02/skos/core#Concept"/>
	<dc:creator xml:lang="en">Concept Definition Task Group of IUGS CGI Interoperability Working Group (http://www.cgi-iugs.org/tech_collaboration/interoperability_working_group.html)</dc:creator>
	<dc:source>SLTTs 2004</dc:source>
	<skos:broader rdf:resource="http://resource.geosciml.org/classifier/cgi/foliationtype/bedding_fabric"/>
	<skos:definition xml:lang="en">A surface internal to the containing sediment mass defined by textural or mineralogical variation, produced by sediment deposition process, and reflecting the orientation of the original depositional surface. Syn Laminated structure (SLTTs 2004).</skos:definition>
	<skos:exactMatch rdf:resource="http://resource.geosciml.org/classifier/cgi/foliationtype/0003"/>
	<skos:inScheme rdf:resource="http://resource.geosciml.org/classifierscheme/cgi/201211/foliationtype"/>
	<skos:narrower rdf:resource="http://resource.geosciml.org/classifier/cgi/foliationtype/impersistent_lamination"/>
	<skos:narrower rdf:resource="http://resource.geosciml.org/classifier/cgi/foliationtype/planar_lamination"/>
	<skos:narrower rdf:resource="http://resource.geosciml.org/classifier/cgi/foliationtype/parallel_bedding_lamination"/>
	<skos:narrower rdf:resource="http://resource.geosciml.org/classifier/cgi/foliationtype/undulating_lamination"/>
	<skos:narrower rdf:resource="http://resource.geosciml.org/classifier/cgi/foliationtype/fissile_lamination"/>
	<skos:narrower rdf:resource="http://resource.geosciml.org/classifier/cgi/foliationtype/cryptomicrobial_lamination"/>
	<skos:narrower rdf:resource="http://resource.geosciml.org/classifier/cgi/foliationtype/irregular_lamination"/>
	<skos:narrower rdf:resource="http://resource.geosciml.org/classifier/cgi/foliationtype/varve_lamination"/>
	<skos:prefLabel xml:lang="en">bedding lamination structure</skos:prefLabel>
</rdf:Description>

<rdf:Description rdf:about="http://resource.geosciml.org/classifier/cgi/foliationtype/c_fabric">
	<rdf:type rdf:resource="http://www.w3.org/2004/02/skos/core#Concept"/>
	<dc:creator xml:lang="en">Concept Definition Task Group of IUGS CGI Interoperability Working Group (http://www.cgi-iugs.org/tech_collaboration/interoperability_working_group.html)</dc:creator>
	<dc:source>Geoscience Victoria, Australia</dc:source>
	<skos:broader rdf:resource="http://resource.geosciml.org/classifier/cgi/foliationtype/ductile_shear_banding_foliation"/>
	<skos:definition xml:lang="en">Ductile shear banding foliation defined by spaced, discrete planar zones of high strain less than 1mm thick. commonly associated with a particle flattening ('S') fabric to form a mylonitic foliation.</skos:definition>
	<skos:exactMatch rdf:resource="http://resource.geosciml.org/classifier/cgi/foliationtype/0004"/>
	<skos:inScheme rdf:resource="http://resource.geosciml.org/classifierscheme/cgi/201211/foliationtype"/>
	<skos:prefLabel xml:lang="en">c fabric</skos:prefLabel>
</rdf:Description>

<rdf:Description rdf:about="http://resource.geosciml.org/classifier/cgi/foliationtype/cleavage">
	<rdf:type rdf:resource="http://www.w3.org/2004/02/skos/core#Concept"/>
	<dc:creator xml:lang="en">Concept Definition Task Group of IUGS CGI Interoperability Working Group (http://www.cgi-iugs.org/tech_collaboration/interoperability_working_group.html)</dc:creator>
	<dc:source xml:lang="en">Brodie, Kate, Fettes, Douglas, and Harte, Ben, 2007, Structural terms including fault rock terms, in Fettes, D., and Desmons, J., Metamorphic rocks-A classification and Glossary of Terms: Cambridge, UK, Cam-bridge University Press, p. 24-31.</dc:source>
	<skos:broader rdf:resource="http://resource.geosciml.org/classifier/cgi/foliationtype/foliation"/>
	<skos:definition xml:lang="en">A tectonic foliation in a rock characterized by a tendency for the rock to split along a regular set of parallel or sub-parallel closely spaced surfaces. Cleavage is a more general term than schistosity because schistosity need not be present in order for a rock to display cleavage. Cleavage domains or parting surfaces are not spaced more than 5 cm apart on average (Borradaille et al., 1982)</skos:definition>
	<skos:exactMatch rdf:resource="http://resource.geosciml.org/classifier/cgi/foliationtype/0005"/>
	<skos:inScheme rdf:resource="http://resource.geosciml.org/classifierscheme/cgi/201211/foliationtype"/>
	<skos:narrower rdf:resource="http://resource.geosciml.org/classifier/cgi/foliationtype/crenulation_cleavage"/>
	<skos:narrower rdf:resource="http://resource.geosciml.org/classifier/cgi/foliationtype/close_joints"/>
	<skos:narrower rdf:resource="http://resource.geosciml.org/classifier/cgi/foliationtype/spaced_cleavage"/>
	<skos:narrower rdf:resource="http://resource.geosciml.org/classifier/cgi/foliationtype/domainal_cleavage"/>
	<skos:narrower rdf:resource="http://resource.geosciml.org/classifier/cgi/foliationtype/disjunctive_cleavage"/>
	<skos:narrower rdf:resource="http://resource.geosciml.org/classifier/cgi/foliationtype/cleavage_parallel_to_bedding"/>
	<skos:narrower rdf:resource="http://resource.geosciml.org/classifier/cgi/foliationtype/rough_cleavage"/>
	<skos:narrower rdf:resource="http://resource.geosciml.org/classifier/cgi/foliationtype/continuous_cleavage"/>
	<skos:prefLabel xml:lang="en">cleavage</skos:prefLabel>
</rdf:Description>

<rdf:Description rdf:about="http://resource.geosciml.org/classifier/cgi/foliationtype/cleavage_parallel_to_bedding">
	<rdf:type rdf:resource="http://www.w3.org/2004/02/skos/core#Concept"/>
	<dc:creator xml:lang="en">Concept Definition Task Group of IUGS CGI Interoperability Working Group (http://www.cgi-iugs.org/tech_collaboration/interoperability_working_group.html)</dc:creator>
	<dc:source>this vocabulary</dc:source>
	<skos:broader rdf:resource="http://resource.geosciml.org/classifier/cgi/foliationtype/cleavage"/>
	<skos:broader rdf:resource="http://resource.geosciml.org/classifier/cgi/foliationtype/compound_folation"/>
	<skos:definition xml:lang="en">composite fabric in which a cleavage is developed parallel to bedding.</skos:definition>
	<skos:exactMatch rdf:resource="http://resource.geosciml.org/classifier/cgi/foliationtype/0006"/>
	<skos:inScheme rdf:resource="http://resource.geosciml.org/classifierscheme/cgi/201211/foliationtype"/>
	<skos:prefLabel xml:lang="en">cleavage parallel to bedding</skos:prefLabel>
</rdf:Description>

<rdf:Description rdf:about="http://resource.geosciml.org/classifier/cgi/foliationtype/close_joints">
	<rdf:type rdf:resource="http://www.w3.org/2004/02/skos/core#Concept"/>
	<dc:creator xml:lang="en">Concept Definition Task Group of IUGS CGI Interoperability Working Group (http://www.cgi-iugs.org/tech_collaboration/interoperability_working_group.html)</dc:creator>
	<dc:source>Borradaile et al. 1982; This Vocabulary</dc:source>
	<skos:broader rdf:resource="http://resource.geosciml.org/classifier/cgi/foliationtype/cleavage"/>
	<skos:broader rdf:resource="http://resource.geosciml.org/classifier/cgi/foliationtype/joint_fabric"/>
	<skos:definition xml:lang="en">Foliation defined by parting surfaces (cleavage domains) that have no apparent thickness, are spaced between 5 cm and 25 cm, and do not crenulate an older foliation. Fabric intermediate between typical cleavage and joints. Parting surfaces are regularly spaced, and penetrative on a 1-10 m scale. 5 cm upper limit on spacing of 'cleavage domains' in a 'cleavage 'fabric is suggested by Borradaile et al. [1982].</skos:definition>
	<skos:exactMatch rdf:resource="http://resource.geosciml.org/classifier/cgi/foliationtype/0007"/>
	<skos:inScheme rdf:resource="http://resource.geosciml.org/classifierscheme/cgi/201211/foliationtype"/>
	<skos:prefLabel xml:lang="en">close joints</skos:prefLabel>
</rdf:Description>

<rdf:Description rdf:about="http://resource.geosciml.org/classifier/cgi/foliationtype/comb_layering">
	<rdf:type rdf:resource="http://www.w3.org/2004/02/skos/core#Concept"/>
	<dc:creator xml:lang="en">Concept Definition Task Group of IUGS CGI Interoperability Working Group (http://www.cgi-iugs.org/tech_collaboration/interoperability_working_group.html)</dc:creator>
	<dc:source>Neuendorf et al. 2005; this vocabulary</dc:source>
	<skos:broader rdf:resource="http://resource.geosciml.org/classifier/cgi/foliationtype/layering"/>
	<skos:definition xml:lang="en">Layering fabric defined by layers that have internal comb structure. Layer boundaries are the termination surfaces for the constituent crystals.</skos:definition>
	<skos:exactMatch rdf:resource="http://resource.geosciml.org/classifier/cgi/foliationtype/0008"/>
	<skos:inScheme rdf:resource="http://resource.geosciml.org/classifierscheme/cgi/201211/foliationtype"/>
	<skos:prefLabel xml:lang="en">comb layering</skos:prefLabel>
</rdf:Description>

<rdf:Description rdf:about="http://resource.geosciml.org/classifier/cgi/foliationtype/compositional_layering">
	<rdf:type rdf:resource="http://www.w3.org/2004/02/skos/core#Concept"/>
	<dc:creator xml:lang="en">Concept Definition Task Group of IUGS CGI Interoperability Working Group (http://www.cgi-iugs.org/tech_collaboration/interoperability_working_group.html)</dc:creator>
	<dc:source>this vocabulary, submitted by British Antarctic Survey</dc:source>
	<skos:broader rdf:resource="http://resource.geosciml.org/classifier/cgi/foliationtype/layering"/>
	<skos:definition xml:lang="en">Layering fabric defined by layers that have different mineralogic composition.</skos:definition>
	<skos:exactMatch rdf:resource="http://resource.geosciml.org/classifier/cgi/foliationtype/0009"/>
	<skos:inScheme rdf:resource="http://resource.geosciml.org/classifierscheme/cgi/201211/foliationtype"/>
	<skos:narrower rdf:resource="http://resource.geosciml.org/classifier/cgi/foliationtype/mineralogical_layering"/>
	<skos:narrower rdf:resource="http://resource.geosciml.org/classifier/cgi/foliationtype/metamorphic_layering_inherited_from_protolith"/>
	<skos:narrower rdf:resource="http://resource.geosciml.org/classifier/cgi/foliationtype/metamorphic_differentiation_layering"/>
	<skos:prefLabel xml:lang="en">compositional layering</skos:prefLabel>
</rdf:Description>

<rdf:Description rdf:about="http://resource.geosciml.org/classifier/cgi/foliationtype/compound_folation">
	<rdf:type rdf:resource="http://www.w3.org/2004/02/skos/core#Concept"/>
	<dc:creator xml:lang="en">Concept Definition Task Group of IUGS CGI Interoperability Working Group (http://www.cgi-iugs.org/tech_collaboration/interoperability_working_group.html)</dc:creator>
	<dc:source>this vocabulary</dc:source>
	<skos:broader rdf:resource="http://resource.geosciml.org/classifier/cgi/foliationtype/foliation"/>
	<skos:definition xml:lang="en">Foliation that includes fabric elements indicating classification with foliation types of different genetic origin, e.g. cleavage parallel to bedding is a compound fabric with a sedimentary foliation and a tectonic foliation. No connotation of genetic origin of fabric elements.</skos:definition>
	<skos:exactMatch rdf:resource="http://resource.geosciml.org/classifier/cgi/foliationtype/0010"/>
	<skos:inScheme rdf:resource="http://resource.geosciml.org/classifierscheme/cgi/201211/foliationtype"/>
	<skos:narrower rdf:resource="http://resource.geosciml.org/classifier/cgi/foliationtype/layered_mylonitic_foliation"/>
	<skos:narrower rdf:resource="http://resource.geosciml.org/classifier/cgi/foliationtype/cleavage_parallel_to_bedding"/>
	<skos:narrower rdf:resource="http://resource.geosciml.org/classifier/cgi/foliationtype/compound_metamorphic_foliation"/>
	<skos:prefLabel xml:lang="en">compound folation</skos:prefLabel>
</rdf:Description>

<rdf:Description rdf:about="http://resource.geosciml.org/classifier/cgi/foliationtype/compound_metamorphic_foliation">
	<rdf:type rdf:resource="http://www.w3.org/2004/02/skos/core#Concept"/>
	<dc:creator xml:lang="en">Concept Definition Task Group of IUGS CGI Interoperability Working Group (http://www.cgi-iugs.org/tech_collaboration/interoperability_working_group.html)</dc:creator>
	<dc:source>this vocabulary</dc:source>
	<skos:broader rdf:resource="http://resource.geosciml.org/classifier/cgi/foliationtype/compound_folation"/>
	<skos:definition xml:lang="en">A compound foliation in which the constituent fabric elements are of metamorphic origin.</skos:definition>
	<skos:exactMatch rdf:resource="http://resource.geosciml.org/classifier/cgi/foliationtype/0011"/>
	<skos:inScheme rdf:resource="http://resource.geosciml.org/classifierscheme/cgi/201211/foliationtype"/>
	<skos:prefLabel xml:lang="en">compound metamorphic foliation</skos:prefLabel>
</rdf:Description>

<rdf:Description rdf:about="http://resource.geosciml.org/classifier/cgi/foliationtype/continuous_cleavage">
	<rdf:type rdf:resource="http://www.w3.org/2004/02/skos/core#Concept"/>
	<dc:creator xml:lang="en">Concept Definition Task Group of IUGS CGI Interoperability Working Group (http://www.cgi-iugs.org/tech_collaboration/interoperability_working_group.html)</dc:creator>
	<dc:source>Borradaile et al 1982</dc:source>
	<skos:broader rdf:resource="http://resource.geosciml.org/classifier/cgi/foliationtype/cleavage"/>
	<skos:definition xml:lang="en">A cleavage that is statistically homogeneous down to the scale of individual mineral grains.</skos:definition>
	<skos:exactMatch rdf:resource="http://resource.geosciml.org/classifier/cgi/foliationtype/0012"/>
	<skos:inScheme rdf:resource="http://resource.geosciml.org/classifierscheme/cgi/201211/foliationtype"/>
	<skos:narrower rdf:resource="http://resource.geosciml.org/classifier/cgi/foliationtype/phyllitic_cleavage"/>
	<skos:narrower rdf:resource="http://resource.geosciml.org/classifier/cgi/foliationtype/slaty_cleavage"/>
	<skos:narrower rdf:resource="http://resource.geosciml.org/classifier/cgi/foliationtype/continuous_crenulation_cleavage"/>
	<skos:prefLabel xml:lang="en">continuous cleavage</skos:prefLabel>
</rdf:Description>

<rdf:Description rdf:about="http://resource.geosciml.org/classifier/cgi/foliationtype/continuous_crenulation_cleavage">
	<rdf:type rdf:resource="http://www.w3.org/2004/02/skos/core#Concept"/>
	<dc:creator xml:lang="en">Concept Definition Task Group of IUGS CGI Interoperability Working Group (http://www.cgi-iugs.org/tech_collaboration/interoperability_working_group.html)</dc:creator>
	<dc:source>Borradaile et al 1982</dc:source>
	<skos:broader rdf:resource="http://resource.geosciml.org/classifier/cgi/foliationtype/continuous_cleavage"/>
	<skos:broader rdf:resource="http://resource.geosciml.org/classifier/cgi/foliationtype/crenulation_cleavage"/>
	<skos:definition xml:lang="en">Cleavage defined by long, thin limbs of crenulation folds of pre-existing foliation, in which the boundaries between cleavage domains and lithons are gradational. Both the crenulation foliation and the crenulated (older) foliation are easily visible. Grades to spaced crenulation cleavage as boundaries of cleavage domains become sharp, and to schistosity or compositional layering as the crenulation foliation obscures the crenulated foliation to become the dominant fabric in the rock. In many rocks with continuous crenulation cleavage, the tendency to part along the cleavage may be weak, thus the rock may not technically meet the definition of 'cleavage as used in this vocabulary.</skos:definition>
	<skos:exactMatch rdf:resource="http://resource.geosciml.org/classifier/cgi/foliationtype/0013"/>
	<skos:inScheme rdf:resource="http://resource.geosciml.org/classifierscheme/cgi/201211/foliationtype"/>
	<skos:prefLabel>continuous crenulation cleavage</skos:prefLabel>
</rdf:Description>

<rdf:Description rdf:about="http://resource.geosciml.org/classifier/cgi/foliationtype/crenulation_cleavage">
	<rdf:type rdf:resource="http://www.w3.org/2004/02/skos/core#Concept"/>
	<dc:creator xml:lang="en">Concept Definition Task Group of IUGS CGI Interoperability Working Group (http://www.cgi-iugs.org/tech_collaboration/interoperability_working_group.html)</dc:creator>
	<dc:source>Brodie, Kate, Fettes, Douglas, and Harte, Ben, 2007, Structural terms including fault rock terms, in Fettes, D., and Desmons, J., Metamorphic rocks-A classification and Glossary of Terms: Cambridge, UK, Cam-bridge University Press, p. 24-31.</dc:source>
	<skos:broader rdf:resource="http://resource.geosciml.org/classifier/cgi/foliationtype/cleavage"/>
	<skos:definition xml:lang="en">Cleavage that is overprinted on an older foliation that is folded to some degree in association with development of the younger cleavage. Cleavage domains commonly associated with long limbs of crenulation folds, and hinge surfaces of folds are roughly parallel. Wavelength of crenulation folds is less than or equal to 1 cm. Cleavage defined by limbs of microfolds coincident with zones of mineral differentiation</skos:definition>
	<skos:exactMatch rdf:resource="http://resource.geosciml.org/classifier/cgi/foliationtype/0014"/>
	<skos:inScheme rdf:resource="http://resource.geosciml.org/classifierscheme/cgi/201211/foliationtype"/>
	<skos:narrower rdf:resource="http://resource.geosciml.org/classifier/cgi/foliationtype/discrete_crenulation_cleavage"/>
	<skos:narrower rdf:resource="http://resource.geosciml.org/classifier/cgi/foliationtype/continuous_crenulation_cleavage"/>
	<skos:prefLabel>crenulation cleavage</skos:prefLabel>
</rdf:Description>

<rdf:Description rdf:about="http://resource.geosciml.org/classifier/cgi/foliationtype/crude_or_indistinct_bedding">
	<rdf:type rdf:resource="http://www.w3.org/2004/02/skos/core#Concept"/>
	<dc:creator xml:lang="en">Concept Definition Task Group of IUGS CGI Interoperability Working Group (http://www.cgi-iugs.org/tech_collaboration/interoperability_working_group.html)</dc:creator>
	<dc:source>this vocabulary</dc:source>
	<skos:broader rdf:resource="http://resource.geosciml.org/classifier/cgi/foliationtype/bedding_fabric"/>
	<skos:definition xml:lang="en">Bedding defined by surfaces that are not distinct, e.g. by gradational grain size variations.</skos:definition>
	<skos:exactMatch rdf:resource="http://resource.geosciml.org/classifier/cgi/foliationtype/0015"/>
	<skos:inScheme rdf:resource="http://resource.geosciml.org/classifierscheme/cgi/201211/foliationtype"/>
	<skos:prefLabel xml:lang="en">crude or indistinct bedding</skos:prefLabel>
</rdf:Description>

<rdf:Description rdf:about="http://resource.geosciml.org/classifier/cgi/foliationtype/cryptomicrobial_lamination">
	<rdf:type rdf:resource="http://www.w3.org/2004/02/skos/core#Concept"/>
	<dc:creator xml:lang="en">Concept Definition Task Group of IUGS CGI Interoperability Working Group (http://www.cgi-iugs.org/tech_collaboration/interoperability_working_group.html)</dc:creator>
	<dc:source>GGIPAC; http://www.brs.gov.au/land&amp;water/groundwater/result.internal_stratification.html</dc:source>
	<skos:broader rdf:resource="http://resource.geosciml.org/classifier/cgi/foliationtype/bedding_lamination_structure"/>
	<skos:definition xml:lang="en">Fabric defined by fine laminae formed by the trapping of grains and lime precipitation in a microbial mat.</skos:definition>
	<skos:exactMatch rdf:resource="http://resource.geosciml.org/classifier/cgi/foliationtype/0016"/>
	<skos:inScheme rdf:resource="http://resource.geosciml.org/classifierscheme/cgi/201211/foliationtype"/>
	<skos:narrower rdf:resource="http://resource.geosciml.org/classifier/cgi/foliationtype/stromatolitic_lamination"/>
	<skos:prefLabel xml:lang="en">cryptomicrobial lamination</skos:prefLabel>
</rdf:Description>

<rdf:Description rdf:about="http://resource.geosciml.org/classifier/cgi/foliationtype/cumulate_layering">
	<rdf:type rdf:resource="http://www.w3.org/2004/02/skos/core#Concept"/>
	<dc:creator xml:lang="en">Concept Definition Task Group of IUGS CGI Interoperability Working Group (http://www.cgi-iugs.org/tech_collaboration/interoperability_working_group.html)</dc:creator>
	<dc:source>Carmichael et al 1974; Best 1982</dc:source>
	<skos:broader rdf:resource="http://resource.geosciml.org/classifier/cgi/foliationtype/igneous_layering"/>
	<skos:definition xml:lang="en">Layering in igneous rocks in which layers are characterized by variation in relative proportion of magmatically crystallized minerals. Typically a pattern of mineralogical variation will be repeated many times in a vertical section with layers of relatively consistent thickness. See photos in Best [1982] p. 176-177. Gravity-stratified layers typically have mafic minerals at the base and plagioclase at the top and are interpreted to form by crystal settling in magma.</skos:definition>
	<skos:exactMatch rdf:resource="http://resource.geosciml.org/classifier/cgi/foliationtype/0017"/>
	<skos:inScheme rdf:resource="http://resource.geosciml.org/classifierscheme/cgi/201211/foliationtype"/>
	<skos:prefLabel xml:lang="en">cumulate layering</skos:prefLabel>
</rdf:Description>

<rdf:Description rdf:about="http://resource.geosciml.org/classifier/cgi/foliationtype/discrete_cleavage">
	<rdf:type rdf:resource="http://www.w3.org/2004/02/skos/core#Concept"/>
	<dc:creator xml:lang="en">Concept Definition Task Group of IUGS CGI Interoperability Working Group (http://www.cgi-iugs.org/tech_collaboration/interoperability_working_group.html)</dc:creator>
	<dc:source>Borradaile et al., 1982</dc:source>
	<skos:broader rdf:resource="http://resource.geosciml.org/classifier/cgi/foliationtype/spaced_cleavage"/>
	<skos:definition xml:lang="en">Spaced cleavage in which cleavage domains have sharply defined edges.</skos:definition>
	<skos:exactMatch rdf:resource="http://resource.geosciml.org/classifier/cgi/foliationtype/0018"/>
	<skos:inScheme rdf:resource="http://resource.geosciml.org/classifierscheme/cgi/201211/foliationtype"/>
	<skos:prefLabel xml:lang="en">discrete cleavage</skos:prefLabel>
</rdf:Description>

<rdf:Description rdf:about="http://resource.geosciml.org/classifier/cgi/foliationtype/discrete_crenulation_cleavage">
	<rdf:type rdf:resource="http://www.w3.org/2004/02/skos/core#Concept"/>
	<dc:creator xml:lang="en">Concept Definition Task Group of IUGS CGI Interoperability Working Group (http://www.cgi-iugs.org/tech_collaboration/interoperability_working_group.html)</dc:creator>
	<dc:source>Borradaile et al 1982</dc:source>
	<skos:broader rdf:resource="http://resource.geosciml.org/classifier/cgi/foliationtype/crenulation_cleavage"/>
	<skos:broader rdf:resource="http://resource.geosciml.org/classifier/cgi/foliationtype/spaced_cleavage"/>
	<skos:definition xml:lang="en">Crenulation cleavage in which the cleavage domains have discrete boundaries. Amplitude of crenulation folds tends to be small.</skos:definition>
	<skos:exactMatch rdf:resource="http://resource.geosciml.org/classifier/cgi/foliationtype/0019"/>
	<skos:inScheme rdf:resource="http://resource.geosciml.org/classifierscheme/cgi/201211/foliationtype"/>
	<skos:prefLabel xml:lang="en">discrete crenulation cleavage</skos:prefLabel>
</rdf:Description>

<rdf:Description rdf:about="http://resource.geosciml.org/classifier/cgi/foliationtype/discrete_disjunct_spaced_cleavage">
	<rdf:type rdf:resource="http://www.w3.org/2004/02/skos/core#Concept"/>
	<dc:creator xml:lang="en">Concept Definition Task Group of IUGS CGI Interoperability Working Group (http://www.cgi-iugs.org/tech_collaboration/interoperability_working_group.html)</dc:creator>
	<dc:source>Neuendorf et al. 2005; Borradaile et al. 1982.</dc:source>
	<skos:broader rdf:resource="http://resource.geosciml.org/classifier/cgi/foliationtype/spaced_cleavage"/>
	<skos:definition xml:lang="en">Disjunct spaced cleavage defined by discrete cleavage surfaces, typically in low-grade clastic rocks. Syn. Fracture cleavage.</skos:definition>
	<skos:exactMatch rdf:resource="http://resource.geosciml.org/classifier/cgi/foliationtype/0020"/>
	<skos:inScheme rdf:resource="http://resource.geosciml.org/classifierscheme/cgi/201211/foliationtype"/>
	<skos:prefLabel xml:lang="en">discrete disjunct spaced cleavage</skos:prefLabel>
</rdf:Description>

<rdf:Description rdf:about="http://resource.geosciml.org/classifier/cgi/foliationtype/disjunctive_cleavage">
	<rdf:type rdf:resource="http://www.w3.org/2004/02/skos/core#Concept"/>
	<dc:creator xml:lang="en">Concept Definition Task Group of IUGS CGI Interoperability Working Group (http://www.cgi-iugs.org/tech_collaboration/interoperability_working_group.html)</dc:creator>
	<dc:source>Borradaile et al. 1982</dc:source>
	<skos:broader rdf:resource="http://resource.geosciml.org/classifier/cgi/foliationtype/cleavage"/>
	<skos:definition xml:lang="en">A spaced cleavage independent of any pre-existing mineral orientation; cleavage in which there is no systematic relationship between a pre-existing preferred orientation and the superimposed cleavage. (Borradaile et al., 1982)</skos:definition>
	<skos:exactMatch rdf:resource="http://resource.geosciml.org/classifier/cgi/foliationtype/0021"/>
	<skos:inScheme rdf:resource="http://resource.geosciml.org/classifierscheme/cgi/201211/foliationtype"/>
	<skos:prefLabel xml:lang="en">disjunctive cleavage</skos:prefLabel>
</rdf:Description>

<rdf:Description rdf:about="http://resource.geosciml.org/classifier/cgi/foliationtype/domainal_cleavage">
	<rdf:type rdf:resource="http://www.w3.org/2004/02/skos/core#Concept"/>
	<dc:creator xml:lang="en">Concept Definition Task Group of IUGS CGI Interoperability Working Group (http://www.cgi-iugs.org/tech_collaboration/interoperability_working_group.html)</dc:creator>
	<dc:source>this vocabulary</dc:source>
	<skos:broader rdf:resource="http://resource.geosciml.org/classifier/cgi/foliationtype/cleavage"/>
	<skos:definition xml:lang="en">Fabric in which domains of more strongly developed (closely spaced) cleavage are separated by lenses of weakly or non-cleaved rock. Typically observed on outcrop scale and used for geologic unit description</skos:definition>
	<skos:exactMatch rdf:resource="http://resource.geosciml.org/classifier/cgi/foliationtype/0022"/>
	<skos:inScheme rdf:resource="http://resource.geosciml.org/classifierscheme/cgi/201211/foliationtype"/>
	<skos:prefLabel xml:lang="en">domainal cleavage</skos:prefLabel>
</rdf:Description>

<rdf:Description rdf:about="http://resource.geosciml.org/classifier/cgi/foliationtype/ductile_shear_banding_foliation">
	<rdf:type rdf:resource="http://www.w3.org/2004/02/skos/core#Concept"/>
	<dc:creator xml:lang="en">Concept Definition Task Group of IUGS CGI Interoperability Working Group (http://www.cgi-iugs.org/tech_collaboration/interoperability_working_group.html)</dc:creator>
	<dc:source>Geoscience Victoria, Australia</dc:source>
	<skos:broader rdf:resource="http://resource.geosciml.org/classifier/cgi/foliationtype/foliation"/>
	<skos:definition xml:lang="en">Foliation defined by regularly spaced ductile shear bands at the scale of descripiton.</skos:definition>
	<skos:exactMatch rdf:resource="http://resource.geosciml.org/classifier/cgi/foliationtype/0023"/>
	<skos:inScheme rdf:resource="http://resource.geosciml.org/classifierscheme/cgi/201211/foliationtype"/>
	<skos:narrower rdf:resource="http://resource.geosciml.org/classifier/cgi/foliationtype/c_fabric"/>
	<skos:prefLabel xml:lang="en">ductile shear banding foliation</skos:prefLabel>
</rdf:Description>

<rdf:Description rdf:about="http://resource.geosciml.org/classifier/cgi/foliationtype/eutaxitic_foliation">
	<rdf:type rdf:resource="http://www.w3.org/2004/02/skos/core#Concept"/>
	<dc:creator xml:lang="en">Concept Definition Task Group of IUGS CGI Interoperability Working Group (http://www.cgi-iugs.org/tech_collaboration/interoperability_working_group.html)</dc:creator>
	<dc:source>Neuendorf et al. 2005; this vocabulary</dc:source>
	<skos:broader rdf:resource="http://resource.geosciml.org/classifier/cgi/foliationtype/primary_igneous_foliation"/>
	<skos:definition xml:lang="en">Foliation defined by flattened pumice clasts or glass shards, aligned elongate lithic fragments, variations in composition, vesicularity, crystallinity, grain size, spherulite and lithophysae abundance, or the degree of devitrification in a welded tuff. This term denotes interpretation that foliation formed during compaction and welding of tuff.</skos:definition>
	<skos:exactMatch rdf:resource="http://resource.geosciml.org/classifier/cgi/foliationtype/0024"/>
	<skos:inScheme rdf:resource="http://resource.geosciml.org/classifierscheme/cgi/201211/foliationtype"/>
	<skos:prefLabel xml:lang="en">eutaxitic foliation</skos:prefLabel>
</rdf:Description>

<rdf:Description rdf:about="http://resource.geosciml.org/classifier/cgi/foliationtype/fissile_lamination">
	<rdf:type rdf:resource="http://www.w3.org/2004/02/skos/core#Concept"/>
	<dc:creator xml:lang="en">Concept Definition Task Group of IUGS CGI Interoperability Working Group (http://www.cgi-iugs.org/tech_collaboration/interoperability_working_group.html)</dc:creator>
	<dc:source>SLTTs 2004; this vocabulary</dc:source>
	<skos:broader rdf:resource="http://resource.geosciml.org/classifier/cgi/foliationtype/bedding_lamination_structure"/>
	<skos:definition xml:lang="en">Diffuse to distinct lamination in mudstones and mud, defined by the alignment of clay minerals. Lacks distinct very-fine scale layering and repetition of couplets that characterize varves. Essentially a continuous cleavage parallel to bedding, but considered a sedimentary structure related to sediment compaction during diagenesis.</skos:definition>
	<skos:exactMatch rdf:resource="http://resource.geosciml.org/classifier/cgi/foliationtype/0025"/>
	<skos:inScheme rdf:resource="http://resource.geosciml.org/classifierscheme/cgi/201211/foliationtype"/>
	<skos:prefLabel xml:lang="en">fissile lamination</skos:prefLabel>
</rdf:Description>

<rdf:Description rdf:about="http://resource.geosciml.org/classifier/cgi/foliationtype/flaser_structure">
	<rdf:type rdf:resource="http://www.w3.org/2004/02/skos/core#Concept"/>
	<dc:creator xml:lang="en">Concept Definition Task Group of IUGS CGI Interoperability Working Group (http://www.cgi-iugs.org/tech_collaboration/interoperability_working_group.html)</dc:creator>
	<dc:source>Neuendorf et al. 2005</dc:source>
	<skos:broader rdf:resource="http://resource.geosciml.org/classifier/cgi/foliationtype/tectonic_foliation"/>
	<skos:definition xml:lang="en">Tectonic foliation defined by lenses and layers of original or relatively unaltered granular minerals surrounded by a matrix of highly sheared and crushed material. No connotation of metamorphic grade.</skos:definition>
	<skos:exactMatch rdf:resource="http://resource.geosciml.org/classifier/cgi/foliationtype/0026"/>
	<skos:inScheme rdf:resource="http://resource.geosciml.org/classifierscheme/cgi/201211/foliationtype"/>
	<skos:prefLabel xml:lang="en">flaser structure</skos:prefLabel>
</rdf:Description>

<rdf:Description rdf:about="http://resource.geosciml.org/classifier/cgi/foliationtype/flow_layering">
	<rdf:type rdf:resource="http://www.w3.org/2004/02/skos/core#Concept"/>
	<dc:creator xml:lang="en">Concept Definition Task Group of IUGS CGI Interoperability Working Group (http://www.cgi-iugs.org/tech_collaboration/interoperability_working_group.html)</dc:creator>
	<dc:source>this vocabulary</dc:source>
	<skos:broader rdf:resource="http://resource.geosciml.org/classifier/cgi/foliationtype/layering"/>
	<skos:definition xml:lang="en">Layering produced by flow of magma, lava, or diapiric flow of sedimentary rock. Distinction from eutaxitic foliation may be difficult.</skos:definition>
	<skos:exactMatch rdf:resource="http://resource.geosciml.org/classifier/cgi/foliationtype/0027"/>
	<skos:inScheme rdf:resource="http://resource.geosciml.org/classifierscheme/cgi/201211/foliationtype"/>
	<skos:narrower rdf:resource="http://resource.geosciml.org/classifier/cgi/foliationtype/lava_flow_banding"/>
	<skos:prefLabel xml:lang="en">flow layering</skos:prefLabel>
</rdf:Description>

<rdf:Description rdf:about="http://resource.geosciml.org/classifier/cgi/foliationtype/foliation">
	<rdf:type rdf:resource="http://www.w3.org/2004/02/skos/core#Concept"/>
	<dc:creator xml:lang="en">Concept Definition Task Group of IUGS CGI Interoperability Working Group (http://www.cgi-iugs.org/tech_collaboration/interoperability_working_group.html)</dc:creator>
	<dc:source>Jackson 1997</dc:source>
	<skos:definition xml:lang="en">Fabric defined by the planar arrangement of textural or structural features (fabric elements).</skos:definition>
	<skos:exactMatch rdf:resource="http://resource.geosciml.org/classifier/cgi/foliationtype/0028"/>
	<skos:inScheme rdf:resource="http://resource.geosciml.org/classifierscheme/cgi/201211/foliationtype"/>
	<skos:narrower rdf:resource="http://resource.geosciml.org/classifier/cgi/foliationtype/compound_folation"/>
	<skos:narrower rdf:resource="http://resource.geosciml.org/classifier/cgi/foliationtype/layering"/>
	<skos:narrower rdf:resource="http://resource.geosciml.org/classifier/cgi/foliationtype/joint_fabric"/>
	<skos:narrower rdf:resource="http://resource.geosciml.org/classifier/cgi/foliationtype/tectonic_foliation"/>
	<skos:narrower rdf:resource="http://resource.geosciml.org/classifier/cgi/foliationtype/cleavage"/>
	<skos:narrower rdf:resource="http://resource.geosciml.org/classifier/cgi/foliationtype/low_temperature_flow_foliation"/>
	<skos:narrower rdf:resource="http://resource.geosciml.org/classifier/cgi/foliationtype/grain_shape_foliation"/>
	<skos:narrower rdf:resource="http://resource.geosciml.org/classifier/cgi/foliationtype/ductile_shear_banding_foliation"/>
	<skos:narrower rdf:resource="http://resource.geosciml.org/classifier/cgi/foliationtype/schistosity"/>
	<skos:narrower rdf:resource="http://resource.geosciml.org/classifier/cgi/foliationtype/primary_foliation"/>
	<skos:prefLabel xml:lang="en">foliation</skos:prefLabel>
	<skos:topConceptOf rdf:resource="http://resource.geosciml.org/classifierscheme/cgi/201211/foliationtype"/>
</rdf:Description>

<rdf:Description rdf:about="http://resource.geosciml.org/classifier/cgi/foliationtype/generic_mylonitic_foliation">
	<rdf:type rdf:resource="http://www.w3.org/2004/02/skos/core#Concept"/>
	<dc:creator xml:lang="en">Concept Definition Task Group of IUGS CGI Interoperability Working Group (http://www.cgi-iugs.org/tech_collaboration/interoperability_working_group.html)</dc:creator>
	<dc:source>NADM metamorphic rock vocabulary SLTTm1.0 2004</dc:source>
	<skos:broader rdf:resource="http://resource.geosciml.org/classifier/cgi/foliationtype/tectonic_foliation"/>
	<skos:definition xml:lang="en">Foliation defined by the shapes of deformed mineral grains or grain aggregates having aspect ratios greater than 1.5:1, greater than 10 percent of the rock is composed of 'matrix' showing evidence of tectonic reduction in grain size, and the foliation and matrix are interpreted to be the product of continuous, crystal-plastic deformation processes. Generic class is used when data are insufficient to determine classification to protomylontic, mylonite, or ultramylonitc foliation, or to specify that any sort of mylontic foliation may be present.</skos:definition>
	<skos:exactMatch rdf:resource="http://resource.geosciml.org/classifier/cgi/foliationtype/0029"/>
	<skos:inScheme rdf:resource="http://resource.geosciml.org/classifierscheme/cgi/201211/foliationtype"/>
	<skos:narrower rdf:resource="http://resource.geosciml.org/classifier/cgi/foliationtype/mylonite_foliation"/>
	<skos:narrower rdf:resource="http://resource.geosciml.org/classifier/cgi/foliationtype/ultramylonite_foliation"/>
	<skos:narrower rdf:resource="http://resource.geosciml.org/classifier/cgi/foliationtype/protomylonite_foliation"/>
	<skos:narrower rdf:resource="http://resource.geosciml.org/classifier/cgi/foliationtype/layered_mylonitic_foliation"/>
	<skos:prefLabel xml:lang="en">generic mylonitic foliation</skos:prefLabel>
</rdf:Description>

<rdf:Description rdf:about="http://resource.geosciml.org/classifier/cgi/foliationtype/gneissic_layering">
	<rdf:type rdf:resource="http://www.w3.org/2004/02/skos/core#Concept"/>
	<dc:creator xml:lang="en">Concept Definition Task Group of IUGS CGI Interoperability Working Group (http://www.cgi-iugs.org/tech_collaboration/interoperability_working_group.html)</dc:creator>
	<dc:source>this vocabulary</dc:source>
	<skos:broader rdf:resource="http://resource.geosciml.org/classifier/cgi/foliationtype/metamorphic_layering"/>
	<skos:definition xml:lang="en">compositional layering in a metamorphic rock; syn. gneissic banding</skos:definition>
	<skos:exactMatch rdf:resource="http://resource.geosciml.org/classifier/cgi/foliationtype/0030"/>
	<skos:inScheme rdf:resource="http://resource.geosciml.org/classifierscheme/cgi/201211/foliationtype"/>
	<skos:prefLabel xml:lang="en">gneissic layering</skos:prefLabel>
</rdf:Description>

<rdf:Description rdf:about="http://resource.geosciml.org/classifier/cgi/foliationtype/grain_shape_foliation">
	<rdf:type rdf:resource="http://www.w3.org/2004/02/skos/core#Concept"/>
	<dc:creator xml:lang="en">Concept Definition Task Group of IUGS CGI Interoperability Working Group (http://www.cgi-iugs.org/tech_collaboration/interoperability_working_group.html)</dc:creator>
	<dc:source>this vocabulary</dc:source>
	<skos:broader rdf:resource="http://resource.geosciml.org/classifier/cgi/foliationtype/foliation"/>
	<skos:definition xml:lang="en">Foliation defined by the alignment of oblate particles, which may be detrital grains, crystals, or crystalline grain aggregates.</skos:definition>
	<skos:exactMatch rdf:resource="http://resource.geosciml.org/classifier/cgi/foliationtype/0031"/>
	<skos:inScheme rdf:resource="http://resource.geosciml.org/classifierscheme/cgi/201211/foliationtype"/>
	<skos:narrower rdf:resource="http://resource.geosciml.org/classifier/cgi/foliationtype/s_fabric"/>
	<skos:narrower rdf:resource="http://resource.geosciml.org/classifier/cgi/foliationtype/imbricated_clast_fabric"/>
	<skos:prefLabel xml:lang="en">grain shape foliation</skos:prefLabel>
</rdf:Description>

<rdf:Description rdf:about="http://resource.geosciml.org/classifier/cgi/foliationtype/igneous_flow_foliation">
	<rdf:type rdf:resource="http://www.w3.org/2004/02/skos/core#Concept"/>
	<dc:creator xml:lang="en">Concept Definition Task Group of IUGS CGI Interoperability Working Group (http://www.cgi-iugs.org/tech_collaboration/interoperability_working_group.html)</dc:creator>
	<dc:source>this vocabulary</dc:source>
	<skos:broader rdf:resource="http://resource.geosciml.org/classifier/cgi/foliationtype/primary_igneous_foliation"/>
	<skos:definition xml:lang="en">Foliation interpreted to be due to flow in a body of magma or lava. Includes flow banding in lava, and foliation defined by aligned crystals in a phaneritic igneous rock..</skos:definition>
	<skos:exactMatch rdf:resource="http://resource.geosciml.org/classifier/cgi/foliationtype/0032"/>
	<skos:inScheme rdf:resource="http://resource.geosciml.org/classifierscheme/cgi/201211/foliationtype"/>
	<skos:prefLabel xml:lang="en">igneous flow foliation</skos:prefLabel>
</rdf:Description>

<rdf:Description rdf:about="http://resource.geosciml.org/classifier/cgi/foliationtype/igneous_lamination">
	<rdf:type rdf:resource="http://www.w3.org/2004/02/skos/core#Concept"/>
	<dc:creator xml:lang="en">Concept Definition Task Group of IUGS CGI Interoperability Working Group (http://www.cgi-iugs.org/tech_collaboration/interoperability_working_group.html)</dc:creator>
	<dc:source>this vocabulary</dc:source>
	<skos:broader rdf:resource="http://resource.geosciml.org/classifier/cgi/foliationtype/primary_igneous_foliation"/>
	<skos:broader rdf:resource="http://resource.geosciml.org/classifier/cgi/foliationtype/igneous_layering"/>
	<skos:definition xml:lang="en">Foliation defined by surfaces of textural or mineralogical variation formed by igneous processes. If the lamination surfaces are regularly spaced, they may be used to define layers.</skos:definition>
	<skos:exactMatch rdf:resource="http://resource.geosciml.org/classifier/cgi/foliationtype/0033"/>
	<skos:inScheme rdf:resource="http://resource.geosciml.org/classifierscheme/cgi/201211/foliationtype"/>
	<skos:prefLabel xml:lang="en">igneous lamination</skos:prefLabel>
</rdf:Description>

<rdf:Description rdf:about="http://resource.geosciml.org/classifier/cgi/foliationtype/igneous_layering">
	<rdf:type rdf:resource="http://www.w3.org/2004/02/skos/core#Concept"/>
	<dc:creator xml:lang="en">Concept Definition Task Group of IUGS CGI Interoperability Working Group (http://www.cgi-iugs.org/tech_collaboration/interoperability_working_group.html)</dc:creator>
	<dc:source>Geoscience Victoria, Australia</dc:source>
	<skos:broader rdf:resource="http://resource.geosciml.org/classifier/cgi/foliationtype/primary_igneous_foliation"/>
	<skos:broader rdf:resource="http://resource.geosciml.org/classifier/cgi/foliationtype/layering"/>
	<skos:definition xml:lang="en">Layering that is the product of processes operating in magma or lava. syn. magmatic layering</skos:definition>
	<skos:exactMatch rdf:resource="http://resource.geosciml.org/classifier/cgi/foliationtype/0034"/>
	<skos:inScheme rdf:resource="http://resource.geosciml.org/classifierscheme/cgi/201211/foliationtype"/>
	<skos:narrower rdf:resource="http://resource.geosciml.org/classifier/cgi/foliationtype/igneous_textural_layering"/>
	<skos:narrower rdf:resource="http://resource.geosciml.org/classifier/cgi/foliationtype/igneous_lamination"/>
	<skos:narrower rdf:resource="http://resource.geosciml.org/classifier/cgi/foliationtype/cumulate_layering"/>
	<skos:narrower rdf:resource="http://resource.geosciml.org/classifier/cgi/foliationtype/lava_flow_banding"/>
	<skos:narrower rdf:resource="http://resource.geosciml.org/classifier/cgi/foliationtype/rhythmic_layering"/>
	<skos:prefLabel xml:lang="en">igneous layering</skos:prefLabel>
</rdf:Description>

<rdf:Description rdf:about="http://resource.geosciml.org/classifier/cgi/foliationtype/igneous_textural_layering">
	<rdf:type rdf:resource="http://www.w3.org/2004/02/skos/core#Concept"/>
	<dc:creator xml:lang="en">Concept Definition Task Group of IUGS CGI Interoperability Working Group (http://www.cgi-iugs.org/tech_collaboration/interoperability_working_group.html)</dc:creator>
	<dc:source>this vocabulary</dc:source>
	<skos:broader rdf:resource="http://resource.geosciml.org/classifier/cgi/foliationtype/igneous_layering"/>
	<skos:definition xml:lang="en">Layering defined by grain size/ grain shape variations resulting from crystallization processes in igneous rock, most commonly observed in pegmatite/aplite dikes or bodies, and in Laramide leucogranites of Wilderness suite in Arizona.</skos:definition>
	<skos:exactMatch rdf:resource="http://resource.geosciml.org/classifier/cgi/foliationtype/0035"/>
	<skos:inScheme rdf:resource="http://resource.geosciml.org/classifierscheme/cgi/201211/foliationtype"/>
	<skos:prefLabel xml:lang="en">igneous textural layering</skos:prefLabel>
</rdf:Description>

<rdf:Description rdf:about="http://resource.geosciml.org/classifier/cgi/foliationtype/imbricated_clast_fabric">
	<rdf:type rdf:resource="http://www.w3.org/2004/02/skos/core#Concept"/>
	<dc:creator xml:lang="en">Concept Definition Task Group of IUGS CGI Interoperability Working Group (http://www.cgi-iugs.org/tech_collaboration/interoperability_working_group.html)</dc:creator>
	<dc:source>based on Neuendorf et al 2005</dc:source>
	<skos:broader rdf:resource="http://resource.geosciml.org/classifier/cgi/foliationtype/grain_shape_foliation"/>
	<skos:broader rdf:resource="http://resource.geosciml.org/classifier/cgi/foliationtype/primary_foliation"/>
	<skos:definition xml:lang="en">Fabric defined by long axis of tabular clasts stacked like shingles to define a surface that makes a small angle with the bedding surface. A depositional fabric formed by disk-shaped or elongate pebbles all tilted in the same direction; flat sides commonly dip upstream</skos:definition>
	<skos:exactMatch rdf:resource="http://resource.geosciml.org/classifier/cgi/foliationtype/0036"/>
	<skos:inScheme rdf:resource="http://resource.geosciml.org/classifierscheme/cgi/201211/foliationtype"/>
	<skos:prefLabel xml:lang="en">imbricated clast fabric</skos:prefLabel>
</rdf:Description>

<rdf:Description rdf:about="http://resource.geosciml.org/classifier/cgi/foliationtype/impersistent_lamination">
	<rdf:type rdf:resource="http://www.w3.org/2004/02/skos/core#Concept"/>
	<dc:creator xml:lang="en">Concept Definition Task Group of IUGS CGI Interoperability Working Group (http://www.cgi-iugs.org/tech_collaboration/interoperability_working_group.html)</dc:creator>
	<dc:source>this vocabulary</dc:source>
	<skos:broader rdf:resource="http://resource.geosciml.org/classifier/cgi/foliationtype/bedding_lamination_structure"/>
	<skos:definition xml:lang="en">Lamination defined by discontinuous surfaces</skos:definition>
	<skos:exactMatch rdf:resource="http://resource.geosciml.org/classifier/cgi/foliationtype/0037"/>
	<skos:inScheme rdf:resource="http://resource.geosciml.org/classifierscheme/cgi/201211/foliationtype"/>
	<skos:prefLabel xml:lang="en">impersistent lamination</skos:prefLabel>
</rdf:Description>

<rdf:Description rdf:about="http://resource.geosciml.org/classifier/cgi/foliationtype/irregular_lamination">
	<rdf:type rdf:resource="http://www.w3.org/2004/02/skos/core#Concept"/>
	<dc:creator xml:lang="en">Concept Definition Task Group of IUGS CGI Interoperability Working Group (http://www.cgi-iugs.org/tech_collaboration/interoperability_working_group.html)</dc:creator>
	<dc:source>this vocabulary</dc:source>
	<skos:broader rdf:resource="http://resource.geosciml.org/classifier/cgi/foliationtype/bedding_lamination_structure"/>
	<skos:definition xml:lang="en">Lamination fabric in which individual lamina or groups of lamina are warped in an irregular fashion, like a flattened peice of crumpled paper. A crude planar orientation is discernible.</skos:definition>
	<skos:exactMatch rdf:resource="http://resource.geosciml.org/classifier/cgi/foliationtype/0038"/>
	<skos:inScheme rdf:resource="http://resource.geosciml.org/classifierscheme/cgi/201211/foliationtype"/>
	<skos:prefLabel xml:lang="en">irregular lamination</skos:prefLabel>
</rdf:Description>

<rdf:Description rdf:about="http://resource.geosciml.org/classifier/cgi/foliationtype/joint_fabric">
	<rdf:type rdf:resource="http://www.w3.org/2004/02/skos/core#Concept"/>
	<dc:creator xml:lang="en">Concept Definition Task Group of IUGS CGI Interoperability Working Group (http://www.cgi-iugs.org/tech_collaboration/interoperability_working_group.html)</dc:creator>
	<dc:source>Borradaile et al 1982</dc:source>
	<skos:broader rdf:resource="http://resource.geosciml.org/classifier/cgi/foliationtype/foliation"/>
	<skos:definition xml:lang="en">Fabric defined by parting surfaces in rock that occur in crudely parallel orientation, spaced greater than 5 cm on average if in a very regular joint set. Spacing is more variable and alignment of surfaces is cruder that cleavage. Typically applies to geologic unit description.</skos:definition>
	<skos:exactMatch rdf:resource="http://resource.geosciml.org/classifier/cgi/foliationtype/0039"/>
	<skos:inScheme rdf:resource="http://resource.geosciml.org/classifierscheme/cgi/201211/foliationtype"/>
	<skos:narrower rdf:resource="http://resource.geosciml.org/classifier/cgi/foliationtype/close_joints"/>
	<skos:prefLabel xml:lang="en">joint fabric</skos:prefLabel>
</rdf:Description>

<rdf:Description rdf:about="http://resource.geosciml.org/classifier/cgi/foliationtype/laminated_metamorphic_layering">
	<rdf:type rdf:resource="http://www.w3.org/2004/02/skos/core#Concept"/>
	<dc:creator xml:lang="en">Concept Definition Task Group of IUGS CGI Interoperability Working Group (http://www.cgi-iugs.org/tech_collaboration/interoperability_working_group.html)</dc:creator>
	<dc:source>Weiss 1972; Borradaile et al 1982; this vocabulary</dc:source>
	<skos:broader rdf:resource="http://resource.geosciml.org/classifier/cgi/foliationtype/metamorphic_layering"/>
	<skos:definition xml:lang="en">Metamorphic layering in which the layers are less than 1 cm thick. See Weiss, L.E. [1972] plate 36 or Borraidaile et al [1982] plate 137A,B (page 331), plate140A (page 337) for examples.</skos:definition>
	<skos:exactMatch rdf:resource="http://resource.geosciml.org/classifier/cgi/foliationtype/0040"/>
	<skos:inScheme rdf:resource="http://resource.geosciml.org/classifierscheme/cgi/201211/foliationtype"/>
	<skos:prefLabel xml:lang="en">laminated metamorphic layering</skos:prefLabel>
</rdf:Description>

<rdf:Description rdf:about="http://resource.geosciml.org/classifier/cgi/foliationtype/lava_flow_banding">
	<rdf:type rdf:resource="http://www.w3.org/2004/02/skos/core#Concept"/>
	<dc:creator xml:lang="en">Concept Definition Task Group of IUGS CGI Interoperability Working Group (http://www.cgi-iugs.org/tech_collaboration/interoperability_working_group.html)</dc:creator>
	<dc:source>GGIPAC, Australia</dc:source>
	<skos:broader rdf:resource="http://resource.geosciml.org/classifier/cgi/foliationtype/flow_layering"/>
	<skos:broader rdf:resource="http://resource.geosciml.org/classifier/cgi/foliationtype/igneous_layering"/>
	<skos:definition xml:lang="en">Layering formed by laminar lava flow, defined by variations in composition, vesicularity, crystallinity, grainsize, spherulite and lithophysae abundance, degree of devitrification, colour, and/or parting surfaces; syn. flow lamination, flow banding</skos:definition>
	<skos:exactMatch rdf:resource="http://resource.geosciml.org/classifier/cgi/foliationtype/0041"/>
	<skos:inScheme rdf:resource="http://resource.geosciml.org/classifierscheme/cgi/201211/foliationtype"/>
	<skos:prefLabel xml:lang="en">lava flow banding</skos:prefLabel>
</rdf:Description>

<rdf:Description rdf:about="http://resource.geosciml.org/classifier/cgi/foliationtype/layered_mylonitic_foliation">
	<rdf:type rdf:resource="http://www.w3.org/2004/02/skos/core#Concept"/>
	<dc:creator xml:lang="en">Concept Definition Task Group of IUGS CGI Interoperability Working Group (http://www.cgi-iugs.org/tech_collaboration/interoperability_working_group.html)</dc:creator>
	<dc:source>this vocabulary</dc:source>
	<skos:broader rdf:resource="http://resource.geosciml.org/classifier/cgi/foliationtype/layering"/>
	<skos:broader rdf:resource="http://resource.geosciml.org/classifier/cgi/foliationtype/compound_folation"/>
	<skos:broader rdf:resource="http://resource.geosciml.org/classifier/cgi/foliationtype/generic_mylonitic_foliation"/>
	<skos:definition xml:lang="en">compound foliation in which mylonitic foliation is present in rock that has continuous compositional layering. Continuous means individual layers can be traced more than 1 m.</skos:definition>
	<skos:exactMatch rdf:resource="http://resource.geosciml.org/classifier/cgi/foliationtype/0042"/>
	<skos:inScheme rdf:resource="http://resource.geosciml.org/classifierscheme/cgi/201211/foliationtype"/>
	<skos:prefLabel xml:lang="en">layered mylonitic foliation</skos:prefLabel>
</rdf:Description>

<rdf:Description rdf:about="http://resource.geosciml.org/classifier/cgi/foliationtype/layering">
	<rdf:type rdf:resource="http://www.w3.org/2004/02/skos/core#Concept"/>
	<dc:creator xml:lang="en">Concept Definition Task Group of IUGS CGI Interoperability Working Group (http://www.cgi-iugs.org/tech_collaboration/interoperability_working_group.html)</dc:creator>
	<dc:source>this vocabulary</dc:source>
	<skos:broader rdf:resource="http://resource.geosciml.org/classifier/cgi/foliationtype/foliation"/>
	<skos:definition xml:lang="en">Foliation defined by stacked, differentiable, sheet-like masses of material (layers), with no denotation of the nature (composition, grain size, grain shape...) or origin (igneous, sedimentary, metamorphic) of the layers.</skos:definition>
	<skos:exactMatch rdf:resource="http://resource.geosciml.org/classifier/cgi/foliationtype/0043"/>
	<skos:inScheme rdf:resource="http://resource.geosciml.org/classifierscheme/cgi/201211/foliationtype"/>
	<skos:narrower rdf:resource="http://resource.geosciml.org/classifier/cgi/foliationtype/igneous_layering"/>
	<skos:narrower rdf:resource="http://resource.geosciml.org/classifier/cgi/foliationtype/sedimentary_layering"/>
	<skos:narrower rdf:resource="http://resource.geosciml.org/classifier/cgi/foliationtype/metamorphic_layering"/>
	<skos:narrower rdf:resource="http://resource.geosciml.org/classifier/cgi/foliationtype/layered_mylonitic_foliation"/>
	<skos:narrower rdf:resource="http://resource.geosciml.org/classifier/cgi/foliationtype/compositional_layering"/>
	<skos:narrower rdf:resource="http://resource.geosciml.org/classifier/cgi/foliationtype/flow_layering"/>
	<skos:narrower rdf:resource="http://resource.geosciml.org/classifier/cgi/foliationtype/tectonic_layering"/>
	<skos:narrower rdf:resource="http://resource.geosciml.org/classifier/cgi/foliationtype/comb_layering"/>
	<skos:prefLabel xml:lang="en">layering</skos:prefLabel>
</rdf:Description>

<rdf:Description rdf:about="http://resource.geosciml.org/classifier/cgi/foliationtype/low_temperature_flow_foliation">
	<rdf:type rdf:resource="http://www.w3.org/2004/02/skos/core#Concept"/>
	<dc:creator xml:lang="en">Concept Definition Task Group of IUGS CGI Interoperability Working Group (http://www.cgi-iugs.org/tech_collaboration/interoperability_working_group.html)</dc:creator>
	<dc:source>this vocabulary</dc:source>
	<skos:broader rdf:resource="http://resource.geosciml.org/classifier/cgi/foliationtype/foliation"/>
	<skos:definition xml:lang="en">Foliation interpreted to be due to flow in a body of rock (typically mudrock, salt, or anhydrite) under low-temperature (non-metamorphic) conditions, typically related to diapirism.</skos:definition>
	<skos:exactMatch rdf:resource="http://resource.geosciml.org/classifier/cgi/foliationtype/0044"/>
	<skos:inScheme rdf:resource="http://resource.geosciml.org/classifierscheme/cgi/201211/foliationtype"/>
	<skos:prefLabel xml:lang="en">low temperature flow foliation</skos:prefLabel>
</rdf:Description>

<rdf:Description rdf:about="http://resource.geosciml.org/classifier/cgi/foliationtype/metamorphic_differentiation_layering">
	<rdf:type rdf:resource="http://www.w3.org/2004/02/skos/core#Concept"/>
	<dc:creator xml:lang="en">Concept Definition Task Group of IUGS CGI Interoperability Working Group (http://www.cgi-iugs.org/tech_collaboration/interoperability_working_group.html)</dc:creator>
	<dc:source>this vocabulary</dc:source>
	<skos:broader rdf:resource="http://resource.geosciml.org/classifier/cgi/foliationtype/compositional_layering"/>
	<skos:broader rdf:resource="http://resource.geosciml.org/classifier/cgi/foliationtype/metamorphic_layering"/>
	<skos:definition xml:lang="en">Layering defined by mineralogical variations in a rock body interpreted to be result of solid-state reactions in rock body (metamorphic segregation).</skos:definition>
	<skos:exactMatch rdf:resource="http://resource.geosciml.org/classifier/cgi/foliationtype/0045"/>
	<skos:inScheme rdf:resource="http://resource.geosciml.org/classifierscheme/cgi/201211/foliationtype"/>
	<skos:prefLabel xml:lang="en">metamorphic differentiation layering</skos:prefLabel>
</rdf:Description>

<rdf:Description rdf:about="http://resource.geosciml.org/classifier/cgi/foliationtype/metamorphic_layering">
	<rdf:type rdf:resource="http://www.w3.org/2004/02/skos/core#Concept"/>
	<dc:creator xml:lang="en">Concept Definition Task Group of IUGS CGI Interoperability Working Group (http://www.cgi-iugs.org/tech_collaboration/interoperability_working_group.html)</dc:creator>
	<dc:source>this vocabulary</dc:source>
	<skos:broader rdf:resource="http://resource.geosciml.org/classifier/cgi/foliationtype/layering"/>
	<skos:definition xml:lang="en">Layering of unspecified origin in a metamorphic rock. compositional or textural variations may be inherited from protolith, or result from metamorphic processes.</skos:definition>
	<skos:exactMatch rdf:resource="http://resource.geosciml.org/classifier/cgi/foliationtype/0046"/>
	<skos:inScheme rdf:resource="http://resource.geosciml.org/classifierscheme/cgi/201211/foliationtype"/>
	<skos:narrower rdf:resource="http://resource.geosciml.org/classifier/cgi/foliationtype/laminated_metamorphic_layering"/>
	<skos:narrower rdf:resource="http://resource.geosciml.org/classifier/cgi/foliationtype/vague_metamorphic_layering"/>
	<skos:narrower rdf:resource="http://resource.geosciml.org/classifier/cgi/foliationtype/metamorphic_layering_inherited_from_protolith"/>
	<skos:narrower rdf:resource="http://resource.geosciml.org/classifier/cgi/foliationtype/gneissic_layering"/>
	<skos:narrower rdf:resource="http://resource.geosciml.org/classifier/cgi/foliationtype/metamorphic_differentiation_layering"/>
	<skos:narrower rdf:resource="http://resource.geosciml.org/classifier/cgi/foliationtype/stromatic_layering"/>
	<skos:prefLabel xml:lang="en">metamorphic layering</skos:prefLabel>
</rdf:Description>

<rdf:Description rdf:about="http://resource.geosciml.org/classifier/cgi/foliationtype/metamorphic_layering_inherited_from_protolith">
	<rdf:type rdf:resource="http://www.w3.org/2004/02/skos/core#Concept"/>
	<dc:creator xml:lang="en">Concept Definition Task Group of IUGS CGI Interoperability Working Group (http://www.cgi-iugs.org/tech_collaboration/interoperability_working_group.html)</dc:creator>
	<dc:source>this vocabulary</dc:source>
	<skos:broader rdf:resource="http://resource.geosciml.org/classifier/cgi/foliationtype/metamorphic_layering"/>
	<skos:broader rdf:resource="http://resource.geosciml.org/classifier/cgi/foliationtype/compositional_layering"/>
	<skos:definition xml:lang="en">Metamorphic layering in which layer differntiation is relict of compositional variations in the protolith, typically heterogeneous sedimentary or volcanic rock.</skos:definition>
	<skos:exactMatch rdf:resource="http://resource.geosciml.org/classifier/cgi/foliationtype/0047"/>
	<skos:inScheme rdf:resource="http://resource.geosciml.org/classifierscheme/cgi/201211/foliationtype"/>
	<skos:narrower rdf:resource="http://resource.geosciml.org/classifier/cgi/foliationtype/transposed_bedding_layering"/>
	<skos:prefLabel xml:lang="en">metamorphic layering inherited from protolith</skos:prefLabel>
</rdf:Description>

<rdf:Description rdf:about="http://resource.geosciml.org/classifier/cgi/foliationtype/mineralogical_layering">
	<rdf:type rdf:resource="http://www.w3.org/2004/02/skos/core#Concept"/>
	<dc:creator xml:lang="en">Concept Definition Task Group of IUGS CGI Interoperability Working Group (http://www.cgi-iugs.org/tech_collaboration/interoperability_working_group.html)</dc:creator>
	<dc:source>this vocabulary</dc:source>
	<skos:broader rdf:resource="http://resource.geosciml.org/classifier/cgi/foliationtype/compositional_layering"/>
	<skos:definition xml:lang="en">Generic layering defined by variations in mineralogy between individual sheets of material</skos:definition>
	<skos:exactMatch rdf:resource="http://resource.geosciml.org/classifier/cgi/foliationtype/0048"/>
	<skos:inScheme rdf:resource="http://resource.geosciml.org/classifierscheme/cgi/201211/foliationtype"/>
	<skos:prefLabel xml:lang="en">mineralogical layering</skos:prefLabel>
</rdf:Description>

<rdf:Description rdf:about="http://resource.geosciml.org/classifier/cgi/foliationtype/mylonite_foliation">
	<rdf:type rdf:resource="http://www.w3.org/2004/02/skos/core#Concept"/>
	<dc:creator xml:lang="en">Concept Definition Task Group of IUGS CGI Interoperability Working Group (http://www.cgi-iugs.org/tech_collaboration/interoperability_working_group.html)</dc:creator>
	<dc:source>SLTTm 2004; Sibson 1977</dc:source>
	<skos:broader rdf:resource="http://resource.geosciml.org/classifier/cgi/foliationtype/generic_mylonitic_foliation"/>
	<skos:definition xml:lang="en">Generic mylonitic foliation in which 50-90 percent of rock is matrix due to tectonic grain size reduction processes. Planar fabric is very apparent due to flattening of mineral grains, development of shear surfaces, and alignment of tabular mineral grains. Lineation is typically present and easily observed.</skos:definition>
	<skos:exactMatch rdf:resource="http://resource.geosciml.org/classifier/cgi/foliationtype/0049"/>
	<skos:inScheme rdf:resource="http://resource.geosciml.org/classifierscheme/cgi/201211/foliationtype"/>
	<skos:prefLabel xml:lang="en">mylonite foliation</skos:prefLabel>
</rdf:Description>

<rdf:Description rdf:about="http://resource.geosciml.org/classifier/cgi/foliationtype/parallel_bedding">
	<rdf:type rdf:resource="http://www.w3.org/2004/02/skos/core#Concept"/>
	<dc:creator xml:lang="en">Concept Definition Task Group of IUGS CGI Interoperability Working Group (http://www.cgi-iugs.org/tech_collaboration/interoperability_working_group.html)</dc:creator>
	<dc:source>SLTTs 2004</dc:source>
	<skos:broader rdf:resource="http://resource.geosciml.org/classifier/cgi/foliationtype/bedding_fabric"/>
	<skos:definition xml:lang="en">Bedding defined by parallel surfaces. Bedding structure may be lamination or layering.</skos:definition>
	<skos:exactMatch rdf:resource="http://resource.geosciml.org/classifier/cgi/foliationtype/0050"/>
	<skos:inScheme rdf:resource="http://resource.geosciml.org/classifierscheme/cgi/201211/foliationtype"/>
	<skos:prefLabel>parallel bedding</skos:prefLabel>
</rdf:Description>

<rdf:Description rdf:about="http://resource.geosciml.org/classifier/cgi/foliationtype/parallel_bedding_lamination">
	<rdf:type rdf:resource="http://www.w3.org/2004/02/skos/core#Concept"/>
	<dc:creator xml:lang="en">Concept Definition Task Group of IUGS CGI Interoperability Working Group (http://www.cgi-iugs.org/tech_collaboration/interoperability_working_group.html)</dc:creator>
	<dc:source>this vocabulary</dc:source>
	<skos:broader rdf:resource="http://resource.geosciml.org/classifier/cgi/foliationtype/bedding_lamination_structure"/>
	<skos:definition xml:lang="en">Bedding lamination structure in which all visible bedding surfaces are parallel.</skos:definition>
	<skos:exactMatch rdf:resource="http://resource.geosciml.org/classifier/cgi/foliationtype/0051"/>
	<skos:inScheme rdf:resource="http://resource.geosciml.org/classifierscheme/cgi/201211/foliationtype"/>
	<skos:prefLabel>parallel bedding lamination</skos:prefLabel>
</rdf:Description>

<rdf:Description rdf:about="http://resource.geosciml.org/classifier/cgi/foliationtype/phyllitic_cleavage">
	<rdf:type rdf:resource="http://www.w3.org/2004/02/skos/core#Concept"/>
	<dc:creator xml:lang="en">Concept Definition Task Group of IUGS CGI Interoperability Working Group (http://www.cgi-iugs.org/tech_collaboration/interoperability_working_group.html)</dc:creator>
	<dc:source>SLTTm 2004; Geoscience Victoria, Australia</dc:source>
	<skos:broader rdf:resource="http://resource.geosciml.org/classifier/cgi/foliationtype/continuous_cleavage"/>
	<skos:definition xml:lang="en">Continuous cleavage in phyllitic rock; phyllosilicate mineral grains just barely visible, grain size midway between slaty cleavage and schist; typically has a satiny lustre.</skos:definition>
	<skos:exactMatch rdf:resource="http://resource.geosciml.org/classifier/cgi/foliationtype/0052"/>
	<skos:inScheme rdf:resource="http://resource.geosciml.org/classifierscheme/cgi/201211/foliationtype"/>
	<skos:prefLabel xml:lang="en">phyllitic cleavage</skos:prefLabel>
</rdf:Description>

<rdf:Description rdf:about="http://resource.geosciml.org/classifier/cgi/foliationtype/planar_lamination">
	<rdf:type rdf:resource="http://www.w3.org/2004/02/skos/core#Concept"/>
	<dc:creator xml:lang="en">Concept Definition Task Group of IUGS CGI Interoperability Working Group (http://www.cgi-iugs.org/tech_collaboration/interoperability_working_group.html)</dc:creator>
	<dc:source>this vocabulary</dc:source>
	<skos:broader rdf:resource="http://resource.geosciml.org/classifier/cgi/foliationtype/bedding_lamination_structure"/>
	<skos:definition xml:lang="en">Lamination that is defined by planar bedding surfaces at the scale of description.</skos:definition>
	<skos:exactMatch rdf:resource="http://resource.geosciml.org/classifier/cgi/foliationtype/0053"/>
	<skos:inScheme rdf:resource="http://resource.geosciml.org/classifierscheme/cgi/201211/foliationtype"/>
	<skos:prefLabel xml:lang="en">planar lamination</skos:prefLabel>
</rdf:Description>

<rdf:Description rdf:about="http://resource.geosciml.org/classifier/cgi/foliationtype/primary_foliation">
	<rdf:type rdf:resource="http://www.w3.org/2004/02/skos/core#Concept"/>
	<dc:creator xml:lang="en">Concept Definition Task Group of IUGS CGI Interoperability Working Group (http://www.cgi-iugs.org/tech_collaboration/interoperability_working_group.html)</dc:creator>
	<dc:source>this vocabulary</dc:source>
	<skos:broader rdf:resource="http://resource.geosciml.org/classifier/cgi/foliationtype/foliation"/>
	<skos:definition xml:lang="en">Foliation formed during original process of deposition or crystallization of an igneous or sedimentary material.</skos:definition>
	<skos:exactMatch rdf:resource="http://resource.geosciml.org/classifier/cgi/foliationtype/0054"/>
	<skos:inScheme rdf:resource="http://resource.geosciml.org/classifierscheme/cgi/201211/foliationtype"/>
	<skos:narrower rdf:resource="http://resource.geosciml.org/classifier/cgi/foliationtype/bedding_fabric"/>
	<skos:narrower rdf:resource="http://resource.geosciml.org/classifier/cgi/foliationtype/imbricated_clast_fabric"/>
	<skos:narrower rdf:resource="http://resource.geosciml.org/classifier/cgi/foliationtype/primary_igneous_foliation"/>
	<skos:prefLabel>primary foliation</skos:prefLabel>
</rdf:Description>

<rdf:Description rdf:about="http://resource.geosciml.org/classifier/cgi/foliationtype/primary_igneous_foliation">
	<rdf:type rdf:resource="http://www.w3.org/2004/02/skos/core#Concept"/>
	<dc:creator xml:lang="en">Concept Definition Task Group of IUGS CGI Interoperability Working Group (http://www.cgi-iugs.org/tech_collaboration/interoperability_working_group.html)</dc:creator>
	<dc:source>this vocabulary</dc:source>
	<skos:broader rdf:resource="http://resource.geosciml.org/classifier/cgi/foliationtype/primary_foliation"/>
	<skos:definition xml:lang="en">Foliation interpreted to be the product of igneous processes, formed in the rock while melt was still present..</skos:definition>
	<skos:exactMatch rdf:resource="http://resource.geosciml.org/classifier/cgi/foliationtype/0055"/>
	<skos:inScheme rdf:resource="http://resource.geosciml.org/classifierscheme/cgi/201211/foliationtype"/>
	<skos:narrower rdf:resource="http://resource.geosciml.org/classifier/cgi/foliationtype/igneous_flow_foliation"/>
	<skos:narrower rdf:resource="http://resource.geosciml.org/classifier/cgi/foliationtype/igneous_lamination"/>
	<skos:narrower rdf:resource="http://resource.geosciml.org/classifier/cgi/foliationtype/igneous_layering"/>
	<skos:narrower rdf:resource="http://resource.geosciml.org/classifier/cgi/foliationtype/eutaxitic_foliation"/>
	<skos:prefLabel xml:lang="en">primary igneous foliation</skos:prefLabel>
</rdf:Description>

<rdf:Description rdf:about="http://resource.geosciml.org/classifier/cgi/foliationtype/protomylonite_foliation">
	<rdf:type rdf:resource="http://www.w3.org/2004/02/skos/core#Concept"/>
	<dc:creator xml:lang="en">Concept Definition Task Group of IUGS CGI Interoperability Working Group (http://www.cgi-iugs.org/tech_collaboration/interoperability_working_group.html)</dc:creator>
	<dc:source>SLTTm 2004; Sibson 1977</dc:source>
	<skos:broader rdf:resource="http://resource.geosciml.org/classifier/cgi/foliationtype/generic_mylonitic_foliation"/>
	<skos:definition xml:lang="en">Generic mylonitic foliation in which 10-50 percent of rock is matrix due to tectonic grain size reduction processes. Planar aspect of fabric may be quite subtle in weakly deformed rocks.</skos:definition>
	<skos:exactMatch rdf:resource="http://resource.geosciml.org/classifier/cgi/foliationtype/0056"/>
	<skos:inScheme rdf:resource="http://resource.geosciml.org/classifierscheme/cgi/201211/foliationtype"/>
	<skos:prefLabel xml:lang="en">protomylonite foliation</skos:prefLabel>
</rdf:Description>

<rdf:Description rdf:about="http://resource.geosciml.org/classifier/cgi/foliationtype/rhythmic_layering">
	<rdf:type rdf:resource="http://www.w3.org/2004/02/skos/core#Concept"/>
	<dc:creator xml:lang="en">Concept Definition Task Group of IUGS CGI Interoperability Working Group (http://www.cgi-iugs.org/tech_collaboration/interoperability_working_group.html)</dc:creator>
	<dc:source>Jackson 1997</dc:source>
	<skos:broader rdf:resource="http://resource.geosciml.org/classifier/cgi/foliationtype/igneous_layering"/>
	<skos:definition xml:lang="en">Layering in igneous rock defined by repeated gravity-stratified layers of typically mafic minerals at the base and plagioclase at the top; formed by crystal settling</skos:definition>
	<skos:exactMatch rdf:resource="http://resource.geosciml.org/classifier/cgi/foliationtype/0057"/>
	<skos:inScheme rdf:resource="http://resource.geosciml.org/classifierscheme/cgi/201211/foliationtype"/>
	<skos:prefLabel xml:lang="en">rhythmic layering</skos:prefLabel>
</rdf:Description>

<rdf:Description rdf:about="http://resource.geosciml.org/classifier/cgi/foliationtype/rough_cleavage">
	<rdf:type rdf:resource="http://www.w3.org/2004/02/skos/core#Concept"/>
	<dc:creator xml:lang="en">Concept Definition Task Group of IUGS CGI Interoperability Working Group (http://www.cgi-iugs.org/tech_collaboration/interoperability_working_group.html)</dc:creator>
	<dc:source>Neuendorf et al. 2005; Borradaile et al, 1990</dc:source>
	<skos:broader rdf:resource="http://resource.geosciml.org/classifier/cgi/foliationtype/cleavage"/>
	<skos:definition xml:lang="en">Disjunct (Borradaile et al, 1990) cleavage characterized by short, discontinuous clavage surfaces, typically with concentrations of phyllosilicate minerals. common in micaceous sandstone.</skos:definition>
	<skos:exactMatch rdf:resource="http://resource.geosciml.org/classifier/cgi/foliationtype/0058"/>
	<skos:inScheme rdf:resource="http://resource.geosciml.org/classifierscheme/cgi/201211/foliationtype"/>
	<skos:prefLabel xml:lang="en">rough cleavage</skos:prefLabel>
</rdf:Description>

<rdf:Description rdf:about="http://resource.geosciml.org/classifier/cgi/foliationtype/s_fabric">
	<rdf:type rdf:resource="http://www.w3.org/2004/02/skos/core#Concept"/>
	<dc:creator xml:lang="en">Concept Definition Task Group of IUGS CGI Interoperability Working Group (http://www.cgi-iugs.org/tech_collaboration/interoperability_working_group.html)</dc:creator>
	<dc:source>Geoscience Victoria, Australia</dc:source>
	<skos:broader rdf:resource="http://resource.geosciml.org/classifier/cgi/foliationtype/grain_shape_foliation"/>
	<skos:broader rdf:resource="http://resource.geosciml.org/classifier/cgi/foliationtype/tectonic_foliation"/>
	<skos:definition xml:lang="en">Foliation in mylonite defined by alignment of tabular crystals or deformed mineral grains; often with sigmoid shape, typically curving into an associated ductile shear banding foliation (C fabric) with a consistent sense.</skos:definition>
	<skos:exactMatch rdf:resource="http://resource.geosciml.org/classifier/cgi/foliationtype/0059"/>
	<skos:inScheme rdf:resource="http://resource.geosciml.org/classifierscheme/cgi/201211/foliationtype"/>
	<skos:prefLabel xml:lang="en">s fabric</skos:prefLabel>
</rdf:Description>

<rdf:Description rdf:about="http://resource.geosciml.org/classifier/cgi/foliationtype/scaly_cleavage">
	<rdf:type rdf:resource="http://www.w3.org/2004/02/skos/core#Concept"/>
	<dc:creator xml:lang="en">Concept Definition Task Group of IUGS CGI Interoperability Working Group (http://www.cgi-iugs.org/tech_collaboration/interoperability_working_group.html)</dc:creator>
	<dc:source>Based on Jackson 1997</dc:source>
	<skos:broader rdf:resource="http://resource.geosciml.org/classifier/cgi/foliationtype/spaced_cleavage"/>
	<skos:definition xml:lang="en">Discrete, anastomosing spaced cleavage characterized by smooth and highly polished/slickensided cleavage surfaces that intersect with one another to form lensoid flakes, scales or chips. common in pelitic rocks in shear zones, melange, or deformed accretionary complexes.</skos:definition>
	<skos:exactMatch rdf:resource="http://resource.geosciml.org/classifier/cgi/foliationtype/0060"/>
	<skos:inScheme rdf:resource="http://resource.geosciml.org/classifierscheme/cgi/201211/foliationtype"/>
	<skos:prefLabel xml:lang="en">scaly cleavage</skos:prefLabel>
</rdf:Description>

<rdf:Description rdf:about="http://resource.geosciml.org/classifier/cgi/foliationtype/schistosity">
	<rdf:type rdf:resource="http://www.w3.org/2004/02/skos/core#Concept"/>
	<dc:creator xml:lang="en">Concept Definition Task Group of IUGS CGI Interoperability Working Group (http://www.cgi-iugs.org/tech_collaboration/interoperability_working_group.html)</dc:creator>
	<dc:source>NADM metamorphic rock vocabulary SLTTm1.0 2004</dc:source>
	<skos:broader rdf:resource="http://resource.geosciml.org/classifier/cgi/foliationtype/foliation"/>
	<skos:definition xml:lang="en">A fabric defined the parallel, planar arrangement of mineral grains having a platy, lamellar, or tabular crystallographic habit that are oriented in a continuous planar or rarely a linear fabric. Schistosity is commonly, but not necessarily, a crystalloblastic foliation. Platy mineral grains typically 1 to 10 mm across (Jackson, 1997), at smaller grain size grades into phyllitic cleavage. Schistosity is typically associated with a continuous cleavage due to the tendency to part parallel to the aligned mineral grains.</skos:definition>
	<skos:exactMatch rdf:resource="http://resource.geosciml.org/classifier/cgi/foliationtype/0061"/>
	<skos:inScheme rdf:resource="http://resource.geosciml.org/classifierscheme/cgi/201211/foliationtype"/>
	<skos:prefLabel xml:lang="en">schistosity</skos:prefLabel>
</rdf:Description>

<rdf:Description rdf:about="http://resource.geosciml.org/classifier/cgi/foliationtype/sedimentary_layering">
	<rdf:type rdf:resource="http://www.w3.org/2004/02/skos/core#Concept"/>
	<dc:creator xml:lang="en">Concept Definition Task Group of IUGS CGI Interoperability Working Group (http://www.cgi-iugs.org/tech_collaboration/interoperability_working_group.html)</dc:creator>
	<dc:source>this vocabulary</dc:source>
	<skos:broader rdf:resource="http://resource.geosciml.org/classifier/cgi/foliationtype/bedding_fabric"/>
	<skos:broader rdf:resource="http://resource.geosciml.org/classifier/cgi/foliationtype/layering"/>
	<skos:definition xml:lang="en">Layering resulting from primary sedimentary processes, in which the individual layers (beds) are bounded by discontinuities related to events in the depositional history.</skos:definition>
	<skos:exactMatch rdf:resource="http://resource.geosciml.org/classifier/cgi/foliationtype/0062"/>
	<skos:inScheme rdf:resource="http://resource.geosciml.org/classifierscheme/cgi/201211/foliationtype"/>
	<skos:prefLabel xml:lang="en">sedimentary layering</skos:prefLabel>
</rdf:Description>

<rdf:Description rdf:about="http://resource.geosciml.org/classifier/cgi/foliationtype/slaty_cleavage">
	<rdf:type rdf:resource="http://www.w3.org/2004/02/skos/core#Concept"/>
	<dc:creator xml:lang="en">Concept Definition Task Group of IUGS CGI Interoperability Working Group (http://www.cgi-iugs.org/tech_collaboration/interoperability_working_group.html)</dc:creator>
	<dc:source>Brodie, Kate, Fettes, Douglas, and Harte, Ben, 2007, Structural terms including fault rock terms, in Fettes, D., and Desmons, J., Metamorphic rocks-A classification and Glossary of Terms: Cambridge, UK, Cam-bridge University Press, p. 24-31.; Jackson 1997</dc:source>
	<skos:broader rdf:resource="http://resource.geosciml.org/classifier/cgi/foliationtype/continuous_cleavage"/>
	<skos:definition xml:lang="en">Continuous cleavage defined by aligned fine to very-fine grained phylosilicate mineral grains. The individual grains defining the fabric are too small to be seen by the unaided eye. Grades into phyllitic cleavage as grain size increases. Cleavage domains typically less than 100 micrometres wide; rock easily splits into slabs and thin plates.</skos:definition>
	<skos:exactMatch rdf:resource="http://resource.geosciml.org/classifier/cgi/foliationtype/0063"/>
	<skos:inScheme rdf:resource="http://resource.geosciml.org/classifierscheme/cgi/201211/foliationtype"/>
	<skos:prefLabel xml:lang="en">slaty cleavage</skos:prefLabel>
</rdf:Description>

<rdf:Description rdf:about="http://resource.geosciml.org/classifier/cgi/foliationtype/solution_cleavage">
	<rdf:type rdf:resource="http://www.w3.org/2004/02/skos/core#Concept"/>
	<dc:creator xml:lang="en">Concept Definition Task Group of IUGS CGI Interoperability Working Group (http://www.cgi-iugs.org/tech_collaboration/interoperability_working_group.html)</dc:creator>
	<dc:source>Geoscience Victoria, Australia</dc:source>
	<skos:broader rdf:resource="http://resource.geosciml.org/classifier/cgi/foliationtype/spaced_cleavage"/>
	<skos:definition xml:lang="en">Spaced cleavage forming an array of parallel to anastomosing, stylolitic to smooth, fracture-like partings formed by rock dissolution. Dissolution is indicated by discontinuity and offset of primary features that intersect cleavage surfaces, and typically by accumulation of insoluble residue along cleavage surface. Syn. stylolitic cleavage, pressure solution cleavage</skos:definition>
	<skos:exactMatch rdf:resource="http://resource.geosciml.org/classifier/cgi/foliationtype/0064"/>
	<skos:inScheme rdf:resource="http://resource.geosciml.org/classifierscheme/cgi/201211/foliationtype"/>
	<skos:prefLabel xml:lang="en">solution cleavage</skos:prefLabel>
</rdf:Description>

<rdf:Description rdf:about="http://resource.geosciml.org/classifier/cgi/foliationtype/spaced_cleavage">
	<rdf:type rdf:resource="http://www.w3.org/2004/02/skos/core#Concept"/>
	<dc:creator xml:lang="en">Concept Definition Task Group of IUGS CGI Interoperability Working Group (http://www.cgi-iugs.org/tech_collaboration/interoperability_working_group.html)</dc:creator>
	<dc:source>Borradaile et al. 1982</dc:source>
	<skos:broader rdf:resource="http://resource.geosciml.org/classifier/cgi/foliationtype/cleavage"/>
	<skos:definition xml:lang="en">Cleavage in which cleavage domains are spaced at finite intervals as the scale of description. Microlithons of uncleaved rock separate cleavage domains.</skos:definition>
	<skos:exactMatch rdf:resource="http://resource.geosciml.org/classifier/cgi/foliationtype/0065"/>
	<skos:inScheme rdf:resource="http://resource.geosciml.org/classifierscheme/cgi/201211/foliationtype"/>
	<skos:narrower rdf:resource="http://resource.geosciml.org/classifier/cgi/foliationtype/scaly_cleavage"/>
	<skos:narrower rdf:resource="http://resource.geosciml.org/classifier/cgi/foliationtype/discrete_crenulation_cleavage"/>
	<skos:narrower rdf:resource="http://resource.geosciml.org/classifier/cgi/foliationtype/discrete_cleavage"/>
	<skos:narrower rdf:resource="http://resource.geosciml.org/classifier/cgi/foliationtype/anastomosing_spaced_cleavage"/>
	<skos:narrower rdf:resource="http://resource.geosciml.org/classifier/cgi/foliationtype/solution_cleavage"/>
	<skos:narrower rdf:resource="http://resource.geosciml.org/classifier/cgi/foliationtype/discrete_disjunct_spaced_cleavage"/>
	<skos:prefLabel xml:lang="en">spaced cleavage</skos:prefLabel>
</rdf:Description>

<rdf:Description rdf:about="http://resource.geosciml.org/classifier/cgi/foliationtype/stromatic_layering">
	<rdf:type rdf:resource="http://www.w3.org/2004/02/skos/core#Concept"/>
	<dc:creator xml:lang="en">Concept Definition Task Group of IUGS CGI Interoperability Working Group (http://www.cgi-iugs.org/tech_collaboration/interoperability_working_group.html)</dc:creator>
	<dc:source>Weiss 1972; Borradaile et al 1982; Neuendorf et al. 2005</dc:source>
	<skos:broader rdf:resource="http://resource.geosciml.org/classifier/cgi/foliationtype/metamorphic_layering"/>
	<skos:definition xml:lang="en">Tectonic layering in which variations that distinguish the layers are the result of melt segregation during high-grade metamorphism; some layers have magmatic/igneous mineralogy. Plates 143 and 144, Borradaile et al [1982] (page 344-347) Syn. Migmatitic layering, lit-par-lit layering</skos:definition>
	<skos:exactMatch rdf:resource="http://resource.geosciml.org/classifier/cgi/foliationtype/0066"/>
	<skos:inScheme rdf:resource="http://resource.geosciml.org/classifierscheme/cgi/201211/foliationtype"/>
	<skos:prefLabel xml:lang="en">stromatic layering</skos:prefLabel>
</rdf:Description>

<rdf:Description rdf:about="http://resource.geosciml.org/classifier/cgi/foliationtype/stromatolitic_lamination">
	<rdf:type rdf:resource="http://www.w3.org/2004/02/skos/core#Concept"/>
	<dc:creator xml:lang="en">Concept Definition Task Group of IUGS CGI Interoperability Working Group (http://www.cgi-iugs.org/tech_collaboration/interoperability_working_group.html)</dc:creator>
	<dc:source>Based on Neuendorf et al 2005</dc:source>
	<skos:broader rdf:resource="http://resource.geosciml.org/classifier/cgi/foliationtype/cryptomicrobial_lamination"/>
	<skos:definition xml:lang="en">Lamination produced by sediment trapping, binding and or precipitation by cyanophytes (blue-green algae)</skos:definition>
	<skos:exactMatch rdf:resource="http://resource.geosciml.org/classifier/cgi/foliationtype/0067"/>
	<skos:inScheme rdf:resource="http://resource.geosciml.org/classifierscheme/cgi/201211/foliationtype"/>
	<skos:prefLabel xml:lang="en">stromatolitic lamination</skos:prefLabel>
</rdf:Description>

<rdf:Description rdf:about="http://resource.geosciml.org/classifier/cgi/foliationtype/tectonic_foliation">
	<rdf:type rdf:resource="http://www.w3.org/2004/02/skos/core#Concept"/>
	<dc:creator xml:lang="en">Concept Definition Task Group of IUGS CGI Interoperability Working Group (http://www.cgi-iugs.org/tech_collaboration/interoperability_working_group.html)</dc:creator>
	<dc:source>this vocabulary</dc:source>
	<skos:broader rdf:resource="http://resource.geosciml.org/classifier/cgi/foliationtype/foliation"/>
	<skos:definition xml:lang="en">Foliation in a rock body defined by physical components related to deformation subsequent to solidification of the rock.</skos:definition>
	<skos:exactMatch rdf:resource="http://resource.geosciml.org/classifier/cgi/foliationtype/0068"/>
	<skos:inScheme rdf:resource="http://resource.geosciml.org/classifierscheme/cgi/201211/foliationtype"/>
	<skos:narrower rdf:resource="http://resource.geosciml.org/classifier/cgi/foliationtype/s_fabric"/>
	<skos:narrower rdf:resource="http://resource.geosciml.org/classifier/cgi/foliationtype/generic_mylonitic_foliation"/>
	<skos:narrower rdf:resource="http://resource.geosciml.org/classifier/cgi/foliationtype/flaser_structure"/>
	<skos:narrower rdf:resource="http://resource.geosciml.org/classifier/cgi/foliationtype/tectonic_layering"/>
	<skos:prefLabel xml:lang="en">tectonic foliation</skos:prefLabel>
</rdf:Description>

<rdf:Description rdf:about="http://resource.geosciml.org/classifier/cgi/foliationtype/tectonic_layering">
	<rdf:type rdf:resource="http://www.w3.org/2004/02/skos/core#Concept"/>
	<dc:creator xml:lang="en">Concept Definition Task Group of IUGS CGI Interoperability Working Group (http://www.cgi-iugs.org/tech_collaboration/interoperability_working_group.html)</dc:creator>
	<dc:source>Weiss 1972; Borradaile et al 1982; this vocabulary</dc:source>
	<skos:broader rdf:resource="http://resource.geosciml.org/classifier/cgi/foliationtype/layering"/>
	<skos:broader rdf:resource="http://resource.geosciml.org/classifier/cgi/foliationtype/tectonic_foliation"/>
	<skos:definition xml:lang="en">Layering defined by mineralogical or textural variations in a rock body that are interpreted to be related to deformation or metamorphism, commonly associated with layers that have sharp boundaries. Also known as gneissic foliation. See plates 142-145 (p. 342-349) in Borradaile et al [1982] and plate 46A to 49A in Weiss [1972].</skos:definition>
	<skos:exactMatch rdf:resource="http://resource.geosciml.org/classifier/cgi/foliationtype/0069"/>
	<skos:inScheme rdf:resource="http://resource.geosciml.org/classifierscheme/cgi/201211/foliationtype"/>
	<skos:prefLabel xml:lang="en">tectonic layering</skos:prefLabel>
</rdf:Description>

<rdf:Description rdf:about="http://resource.geosciml.org/classifier/cgi/foliationtype/transposed_bedding_layering">
	<rdf:type rdf:resource="http://www.w3.org/2004/02/skos/core#Concept"/>
	<dc:creator xml:lang="en">Concept Definition Task Group of IUGS CGI Interoperability Working Group (http://www.cgi-iugs.org/tech_collaboration/interoperability_working_group.html)</dc:creator>
	<dc:source>this vocabulary</dc:source>
	<skos:broader rdf:resource="http://resource.geosciml.org/classifier/cgi/foliationtype/metamorphic_layering_inherited_from_protolith"/>
	<skos:definition xml:lang="en">Layering interpreted to have originated as sedimentary bedding that has been transposed as a result of metamorphism and deformation.</skos:definition>
	<skos:exactMatch rdf:resource="http://resource.geosciml.org/classifier/cgi/foliationtype/0070"/>
	<skos:inScheme rdf:resource="http://resource.geosciml.org/classifierscheme/cgi/201211/foliationtype"/>
	<skos:prefLabel xml:lang="en">transposed bedding layering</skos:prefLabel>
</rdf:Description>

<rdf:Description rdf:about="http://resource.geosciml.org/classifier/cgi/foliationtype/ultramylonite_foliation">
	<rdf:type rdf:resource="http://www.w3.org/2004/02/skos/core#Concept"/>
	<dc:creator xml:lang="en">Concept Definition Task Group of IUGS CGI Interoperability Working Group (http://www.cgi-iugs.org/tech_collaboration/interoperability_working_group.html)</dc:creator>
	<dc:source>SLTTm 2004; Sibson 1977</dc:source>
	<skos:broader rdf:resource="http://resource.geosciml.org/classifier/cgi/foliationtype/generic_mylonitic_foliation"/>
	<skos:definition xml:lang="en">Mylonitic foliation in which greater than 90 percent of rock is matrix due to tectonic grain size reduction processes. Typically rock is very-fine grained to aphanitic, with sparse porphyroclasts, and vague to prominent lamination on a mm scale.</skos:definition>
	<skos:exactMatch rdf:resource="http://resource.geosciml.org/classifier/cgi/foliationtype/0071"/>
	<skos:inScheme rdf:resource="http://resource.geosciml.org/classifierscheme/cgi/201211/foliationtype"/>
	<skos:prefLabel xml:lang="en">ultramylonite foliation</skos:prefLabel>
</rdf:Description>

<rdf:Description rdf:about="http://resource.geosciml.org/classifier/cgi/foliationtype/undulating_lamination">
	<rdf:type rdf:resource="http://www.w3.org/2004/02/skos/core#Concept"/>
	<dc:creator xml:lang="en">Concept Definition Task Group of IUGS CGI Interoperability Working Group (http://www.cgi-iugs.org/tech_collaboration/interoperability_working_group.html)</dc:creator>
	<dc:source>this vocabulary</dc:source>
	<skos:broader rdf:resource="http://resource.geosciml.org/classifier/cgi/foliationtype/bedding_lamination_structure"/>
	<skos:definition xml:lang="en">Gently curviplanar or wavy bedding lamination structure</skos:definition>
	<skos:exactMatch rdf:resource="http://resource.geosciml.org/classifier/cgi/foliationtype/0072"/>
	<skos:inScheme rdf:resource="http://resource.geosciml.org/classifierscheme/cgi/201211/foliationtype"/>
	<skos:prefLabel xml:lang="en">undulating lamination</skos:prefLabel>
</rdf:Description>

<rdf:Description rdf:about="http://resource.geosciml.org/classifier/cgi/foliationtype/vague_metamorphic_layering">
	<rdf:type rdf:resource="http://www.w3.org/2004/02/skos/core#Concept"/>
	<dc:creator xml:lang="en">Concept Definition Task Group of IUGS CGI Interoperability Working Group (http://www.cgi-iugs.org/tech_collaboration/interoperability_working_group.html)</dc:creator>
	<dc:source>Weiss 1972;Borradaile et al 1982; this vocabulary</dc:source>
	<skos:broader rdf:resource="http://resource.geosciml.org/classifier/cgi/foliationtype/metamorphic_layering"/>
	<skos:definition xml:lang="en">Metamorphic layering of uncertain origin, defined by subtle mineralogical or textural variations, with gradational layer boundaries. See plate 142 in Borradaile et al [1982].</skos:definition>
	<skos:exactMatch rdf:resource="http://resource.geosciml.org/classifier/cgi/foliationtype/0073"/>
	<skos:inScheme rdf:resource="http://resource.geosciml.org/classifierscheme/cgi/201211/foliationtype"/>
	<skos:prefLabel xml:lang="en">vague metamorphic layering</skos:prefLabel>
</rdf:Description>

<rdf:Description rdf:about="http://resource.geosciml.org/classifier/cgi/foliationtype/varve_lamination">
	<rdf:type rdf:resource="http://www.w3.org/2004/02/skos/core#Concept"/>
	<dc:creator xml:lang="en">Concept Definition Task Group of IUGS CGI Interoperability Working Group (http://www.cgi-iugs.org/tech_collaboration/interoperability_working_group.html)</dc:creator>
	<dc:source>SLTTs 2004; Jackson 1997</dc:source>
	<skos:broader rdf:resource="http://resource.geosciml.org/classifier/cgi/foliationtype/bedding_lamination_structure"/>
	<skos:definition xml:lang="en">Bedding defined by distinct, parallel laminae (layers less than 1 cm thick), typically occurring in sequences of distinct couplets (e.g. dark and light color). Generally interpreted as deposited from suspension in still water, with each lamina thought to be an annual sedimentation unit. Typically consists of mud-size sediment.</skos:definition>
	<skos:exactMatch rdf:resource="http://resource.geosciml.org/classifier/cgi/foliationtype/0074"/>
	<skos:inScheme rdf:resource="http://resource.geosciml.org/classifierscheme/cgi/201211/foliationtype"/>
	<skos:prefLabel xml:lang="en">varve lamination</skos:prefLabel>
</rdf:Description>

<rdf:Description rdf:about="http://resource.geosciml.org/classifierscheme/cgi/201211/foliationtype">
	<rdf:type rdf:resource="http://www.w3.org/2002/07/owl#Ontology"/>
	<rdf:type rdf:resource="http://www.w3.org/2004/02/skos/core#ConceptScheme"/>
	<dc:contributor>Stephen M Richard</dc:contributor>
	<dc:creator xml:lang="en">Concept Definition Task Group of IUGS CGI Interoperability Working Group (http://www.cgi-iugs.org/tech_collaboration/interoperability_working_group.html)</dc:creator>
	<dc:date>2009-11-04</dc:date>
	<dc:description xml:lang="en">This file contains the CGI Foliation type vocabulary. Use for soft typing GeoSciML GeologicStructure.Foliation elements. Generated from compilation.</dc:description>
	<dc:description xml:lang="en">vocabulary for categories of planar fabric, for use in GeoSciML interchange documents</dc:description>
	<dc:format>application/rdf+xml</dc:format>
	<dc:identifier>http://resource.geosciml.org/classifierscheme/cgi/201211/foliationtype</dc:identifier>
	<dc:publisher xml:lang="en">Concept Definition Task Group of IUGS CGI Interoperability Working Group (http://www.cgi-iugs.org/tech_collaboration/interoperability_working_group.html)</dc:publisher>
	<dc:subject xml:lang="en">Planar fabrics in rocks</dc:subject>
	<dc:title xml:lang="en">CGI Foliation Type categories</dc:title>
	<owl:imports rdf:resource="http://www.w3.org/2004/02/skos/core"/>
	<owl:imports rdf:resource="http://rdfs.org/ns/void"/>
	<owl:versionInfo>201211</owl:versionInfo>
	<skos:definition xml:lang="en">This file contains the CGI Foliation type vocabulary. Use for soft typing GeoSciML GeologicStructure.Foliation elements.</skos:definition>
	<skos:historyNote xml:lang="en">2012-02-07 SMR update URI to replace numeric final token with English-language string as in original URN scheme.</skos:historyNote>
	<skos:historyNote xml:lang="en">2010-02-11 Add narrower relationship links by adding skos:narrower link in Protege, defining skos:narrower as inverse of skos:broader, calculating with Pellet reasoner to add inferred axioms, and using 'file/Export inferred axioms as ontology' in Protege.</skos:historyNote>
	<skos:historyNote xml:lang="en">2012-11-24 SMR Update to 201211 version; add collection entity, check all pref labels are lower case, remove owl:NamedIndividual and Owl:Thing rdf:types.</skos:historyNote>
	<skos:historyNote xml:lang="en">2010-11-28 SMR Replace URN with http URI according to CGI URI scheme (https://www.seegrid.csiro.au/wiki/bin/view/CGIModel/PersistentIdentifiersInGeoSciMLServices#Identifier_value)</skos:historyNote>
	<skos:prefLabel xml:lang="en">FoliationType</skos:prefLabel>
</rdf:Description>

<rdf:Description rdf:about="http://resource.geosciml.org/vocabulary/cgi/201211/foliationtype">
	<rdf:type rdf:resource="http://rdfs.org/ns/void#Dataset"/>
	<rdfs:label rdf:datatype="http://www.w3.org/2001/XMLSchema#string">Foliation type vocabulary</rdfs:label>
</rdf:Description>

<rdf:Description rdf:about="http://www.w3.org/2004/02/skos/core#ConceptScheme">
	<rdf:type rdf:resource="http://www.w3.org/2002/07/owl#Class"/>
</rdf:Description>

</rdf:RDF>