<?xml version="1.0" encoding="UTF-8"?>
<rdf:RDF
	xmlns="http://resource.geosciml.org/classifierscheme/cgi/201211/metamorphicfacies#"
	xmlns:cgi="http://resource.geosciml.org/classifierscheme/cgi/201211/"
	xmlns:dc="http://purl.org/dc/elements/1.1/"
	xmlns:metafac="http://resource.geosciml.org/classifier/cgi/metamorphicfacies/"
	xmlns:owl="http://www.w3.org/2002/07/owl#"
	xmlns:owl2xml="http://www.w3.org/2006/12/owl2-xml#"
	xmlns:rdf="http://www.w3.org/1999/02/22-rdf-syntax-ns#"
	xmlns:rdfs="http://www.w3.org/2000/01/rdf-schema#"
	xmlns:skos="http://www.w3.org/2004/02/skos/core#"
	xmlns:void="http://rdfs.org/ns/void#"
	xmlns:xsd="http://www.w3.org/2001/XMLSchema#">

<rdf:Description rdf:about="http://resource.geosciml.org/classifier/cgi/metamorphicfacies/">
	<rdf:type rdf:resource="http://www.w3.org/2004/02/skos/core#Collection"/>
	<rdfs:label xml:lang="en">metamorphic facies concepts</rdfs:label>
	<skos:definition xml:lang="en">This resource defines the concept space for metamorphic facies concepts by extension; it includes all concepts in this conceptScheme, as well as concepts in previous versions of the scheme.</skos:definition>
	<skos:member rdf:resource="http://resource.geosciml.org/classifier/cgi/metamorphicfacies/no_metamorphic_minerals"/>
	<skos:member rdf:resource="http://resource.geosciml.org/classifier/cgi/metamorphicfacies/epidote_amphibolite_metamorphic_facies"/>
	<skos:member rdf:resource="http://resource.geosciml.org/classifier/cgi/metamorphicfacies/glaucophane_schist_facies"/>
	<skos:member rdf:resource="http://resource.geosciml.org/classifier/cgi/metamorphicfacies/zeolite_metamorphic_facies"/>
	<skos:member rdf:resource="http://resource.geosciml.org/classifier/cgi/metamorphicfacies/sanidinite_metamorphic_facies"/>
	<skos:member rdf:resource="http://resource.geosciml.org/classifier/cgi/metamorphicfacies/amphibolite_metamorphic_facies"/>
	<skos:member rdf:resource="http://resource.geosciml.org/classifier/cgi/metamorphicfacies/greenschist_metamorphic_facies"/>
	<skos:member rdf:resource="http://resource.geosciml.org/classifier/cgi/metamorphicfacies/granulite_facies"/>
	<skos:member rdf:resource="http://resource.geosciml.org/classifier/cgi/metamorphicfacies/metamorphic_facies_unknown"/>
	<skos:member rdf:resource="http://resource.geosciml.org/classifier/cgi/metamorphicfacies/pyroxene_hornfels_metamorphic_facies"/>
	<skos:member rdf:resource="http://resource.geosciml.org/classifier/cgi/metamorphicfacies/metamorphic_facies_not_specified"/>
	<skos:member rdf:resource="http://resource.geosciml.org/classifier/cgi/metamorphicfacies/eclogite_metamorphic_facies"/>
	<skos:member rdf:resource="http://resource.geosciml.org/classifier/cgi/metamorphicfacies/subgreenschist_metamorphic_facies"/>
	<skos:prefLabel xml:lang="en">CGI Metamorphic Facies</skos:prefLabel>
</rdf:Description>

<rdf:Description rdf:about="http://resource.geosciml.org/classifier/cgi/metamorphicfacies/0001">
	<rdf:type rdf:resource="http://www.w3.org/2002/07/owl#NamedIndividual"/>
</rdf:Description>

<rdf:Description rdf:about="http://resource.geosciml.org/classifier/cgi/metamorphicfacies/0002">
	<rdf:type rdf:resource="http://www.w3.org/2002/07/owl#NamedIndividual"/>
</rdf:Description>

<rdf:Description rdf:about="http://resource.geosciml.org/classifier/cgi/metamorphicfacies/0003">
	<rdf:type rdf:resource="http://www.w3.org/2002/07/owl#NamedIndividual"/>
</rdf:Description>

<rdf:Description rdf:about="http://resource.geosciml.org/classifier/cgi/metamorphicfacies/0004">
	<rdf:type rdf:resource="http://www.w3.org/2002/07/owl#NamedIndividual"/>
</rdf:Description>

<rdf:Description rdf:about="http://resource.geosciml.org/classifier/cgi/metamorphicfacies/0005">
	<rdf:type rdf:resource="http://www.w3.org/2002/07/owl#NamedIndividual"/>
</rdf:Description>

<rdf:Description rdf:about="http://resource.geosciml.org/classifier/cgi/metamorphicfacies/0006">
	<rdf:type rdf:resource="http://www.w3.org/2002/07/owl#NamedIndividual"/>
</rdf:Description>

<rdf:Description rdf:about="http://resource.geosciml.org/classifier/cgi/metamorphicfacies/0007">
	<rdf:type rdf:resource="http://www.w3.org/2002/07/owl#NamedIndividual"/>
</rdf:Description>

<rdf:Description rdf:about="http://resource.geosciml.org/classifier/cgi/metamorphicfacies/0008">
	<rdf:type rdf:resource="http://www.w3.org/2002/07/owl#NamedIndividual"/>
</rdf:Description>

<rdf:Description rdf:about="http://resource.geosciml.org/classifier/cgi/metamorphicfacies/0009">
	<rdf:type rdf:resource="http://www.w3.org/2002/07/owl#NamedIndividual"/>
</rdf:Description>

<rdf:Description rdf:about="http://resource.geosciml.org/classifier/cgi/metamorphicfacies/0010">
	<rdf:type rdf:resource="http://www.w3.org/2002/07/owl#NamedIndividual"/>
</rdf:Description>

<rdf:Description rdf:about="http://resource.geosciml.org/classifier/cgi/metamorphicfacies/0011">
	<rdf:type rdf:resource="http://www.w3.org/2002/07/owl#NamedIndividual"/>
</rdf:Description>

<rdf:Description rdf:about="http://resource.geosciml.org/classifier/cgi/metamorphicfacies/0012">
	<rdf:type rdf:resource="http://www.w3.org/2002/07/owl#NamedIndividual"/>
</rdf:Description>

<rdf:Description rdf:about="http://resource.geosciml.org/classifier/cgi/metamorphicfacies/0013">
	<rdf:type rdf:resource="http://www.w3.org/2002/07/owl#NamedIndividual"/>
</rdf:Description>

<rdf:Description rdf:about="http://resource.geosciml.org/classifier/cgi/metamorphicfacies/amphibolite_metamorphic_facies">
	<rdf:type rdf:resource="http://www.w3.org/2004/02/skos/core#Concept"/>
	<dc:creator xml:lang="en">Concept Definition Task Group of IUGS CGI Interoperability Working Group (http://www.cgi-iugs.org/tech_collaboration/interoperability_working_group.html)</dc:creator>
	<dc:source>Smulikowski et al. 2003; Fettes and Desmons 2007</dc:source>
	<skos:broader rdf:resource="http://resource.geosciml.org/classifier/cgi/metamorphicfacies/metamorphic_facies_not_specified"/>
	<skos:definition xml:lang="en">Metamorphic facies characterized in rocks of basaltic composition by hornblende-plagioclase (plagioclase more calcic than An17).</skos:definition>
	<skos:exactMatch rdf:resource="http://resource.geosciml.org/classifier/cgi/metamorphicfacies/0001"/>
	<skos:inScheme rdf:resource="http://resource.geosciml.org/classifierscheme/cgi/201211/metamorphicfacies"/>
	<skos:prefLabel xml:lang="en">amphibolite metamorphic facies</skos:prefLabel>
</rdf:Description>

<rdf:Description rdf:about="http://resource.geosciml.org/classifier/cgi/metamorphicfacies/eclogite_metamorphic_facies">
	<rdf:type rdf:resource="http://www.w3.org/2004/02/skos/core#Concept"/>
	<dc:creator xml:lang="en">Concept Definition Task Group of IUGS CGI Interoperability Working Group (http://www.cgi-iugs.org/tech_collaboration/interoperability_working_group.html)</dc:creator>
	<dc:source xml:lang="en">Fettes and Desmons 2007</dc:source>
	<skos:broader rdf:resource="http://resource.geosciml.org/classifier/cgi/metamorphicfacies/metamorphic_facies_not_specified"/>
	<skos:definition xml:lang="en">omphacite-garnet-quartz (no plagioclase, olivine stable with garnet); assemblage for rocks of basaltic composition</skos:definition>
	<skos:exactMatch rdf:resource="http://resource.geosciml.org/classifier/cgi/metamorphicfacies/0002"/>
	<skos:inScheme rdf:resource="http://resource.geosciml.org/classifierscheme/cgi/201211/metamorphicfacies"/>
	<skos:prefLabel xml:lang="en">eclogite metamorphic facies</skos:prefLabel>
</rdf:Description>

<rdf:Description rdf:about="http://resource.geosciml.org/classifier/cgi/metamorphicfacies/epidote_amphibolite_metamorphic_facies">
	<rdf:type rdf:resource="http://www.w3.org/2004/02/skos/core#Concept"/>
	<dc:creator xml:lang="en">Concept Definition Task Group of IUGS CGI Interoperability Working Group (http://www.cgi-iugs.org/tech_collaboration/interoperability_working_group.html)</dc:creator>
	<dc:source xml:lang="en">Fettes and Desmons 2007</dc:source>
	<skos:broader rdf:resource="http://resource.geosciml.org/classifier/cgi/metamorphicfacies/metamorphic_facies_not_specified"/>
	<skos:definition xml:lang="en">hornblende-albite-epidote(-chlorite); assemblage for rocks of basaltic composition</skos:definition>
	<skos:exactMatch rdf:resource="http://resource.geosciml.org/classifier/cgi/metamorphicfacies/0003"/>
	<skos:inScheme rdf:resource="http://resource.geosciml.org/classifierscheme/cgi/201211/metamorphicfacies"/>
	<skos:prefLabel xml:lang="en">epidote amphibolite metamorphic facies</skos:prefLabel>
</rdf:Description>

<rdf:Description rdf:about="http://resource.geosciml.org/classifier/cgi/metamorphicfacies/glaucophane_schist_facies">
	<rdf:type rdf:resource="http://www.w3.org/2004/02/skos/core#Concept"/>
	<dc:creator xml:lang="en">Concept Definition Task Group of IUGS CGI Interoperability Working Group (http://www.cgi-iugs.org/tech_collaboration/interoperability_working_group.html)</dc:creator>
	<dc:source xml:lang="en">Smulikowski et al., 2003; Fettes and Desmons 2007</dc:source>
	<skos:broader rdf:resource="http://resource.geosciml.org/classifier/cgi/metamorphicfacies/metamorphic_facies_not_specified"/>
	<skos:definition xml:lang="en">Metamorphic facies characterized in rocks of basaltic composition by glaucophane-epidote (-garnet), glaucophane-lawsonite, or glaucophane-lawsonite-jadeite.</skos:definition>
	<skos:exactMatch rdf:resource="http://resource.geosciml.org/classifier/cgi/metamorphicfacies/0004"/>
	<skos:inScheme rdf:resource="http://resource.geosciml.org/classifierscheme/cgi/201211/metamorphicfacies"/>
	<skos:prefLabel xml:lang="en">glaucophane schist facies</skos:prefLabel>
</rdf:Description>

<rdf:Description rdf:about="http://resource.geosciml.org/classifier/cgi/metamorphicfacies/granulite_facies">
	<rdf:type rdf:resource="http://www.w3.org/2004/02/skos/core#Concept"/>
	<dc:creator xml:lang="en">Concept Definition Task Group of IUGS CGI Interoperability Working Group (http://www.cgi-iugs.org/tech_collaboration/interoperability_working_group.html)</dc:creator>
	<dc:source xml:lang="en">Smulikowski et al., 2003; Fettes and Desmons 2007</dc:source>
	<skos:broader rdf:resource="http://resource.geosciml.org/classifier/cgi/metamorphicfacies/metamorphic_facies_not_specified"/>
	<skos:definition xml:lang="en">Metamorphic facies characterized in rocks of basaltic composition by the mineral assemblage clinopyroxene-orthopyroxene-plagioclase (olivine not stable with plagioclase or with garnet), or especially high-temperature varieties or polymorphs of minerals (e</skos:definition>
	<skos:exactMatch rdf:resource="http://resource.geosciml.org/classifier/cgi/metamorphicfacies/0005"/>
	<skos:inScheme rdf:resource="http://resource.geosciml.org/classifierscheme/cgi/201211/metamorphicfacies"/>
	<skos:prefLabel xml:lang="en">granulite facies</skos:prefLabel>
</rdf:Description>

<rdf:Description rdf:about="http://resource.geosciml.org/classifier/cgi/metamorphicfacies/greenschist_metamorphic_facies">
	<rdf:type rdf:resource="http://www.w3.org/2004/02/skos/core#Concept"/>
	<dc:creator xml:lang="en">Concept Definition Task Group of IUGS CGI Interoperability Working Group (http://www.cgi-iugs.org/tech_collaboration/interoperability_working_group.html)</dc:creator>
	<dc:source xml:lang="en">Smulikowski et al., 2003; Fettes and Desmons 2007</dc:source>
	<skos:broader rdf:resource="http://resource.geosciml.org/classifier/cgi/metamorphicfacies/metamorphic_facies_not_specified"/>
	<skos:definition xml:lang="en">Metamorphic facies characterized in rocks of basaltic composition by actinolite-albite-epidote-chlorite (an epidote group mineral is the diagnostic Ca-Al silicate rather than prehnite or pumpellyite).</skos:definition>
	<skos:exactMatch rdf:resource="http://resource.geosciml.org/classifier/cgi/metamorphicfacies/0006"/>
	<skos:inScheme rdf:resource="http://resource.geosciml.org/classifierscheme/cgi/201211/metamorphicfacies"/>
	<skos:prefLabel xml:lang="en">greenschist metamorphic facies</skos:prefLabel>
</rdf:Description>

<rdf:Description rdf:about="http://resource.geosciml.org/classifier/cgi/metamorphicfacies/metamorphic_facies_not_specified">
	<rdf:type rdf:resource="http://www.w3.org/2004/02/skos/core#Concept"/>
	<dc:creator xml:lang="en">Concept Definition Task Group of IUGS CGI Interoperability Working Group (http://www.cgi-iugs.org/tech_collaboration/interoperability_working_group.html)</dc:creator>
	<dc:source xml:lang="en">this vocabulary</dc:source>
	<skos:definition xml:lang="en">Metamorphosed, but facies not specified in more detail. For use in normative description to indicate that any metamorphic facies value is valid.</skos:definition>
	<skos:exactMatch rdf:resource="http://resource.geosciml.org/classifier/cgi/metamorphicfacies/0007"/>
	<skos:inScheme rdf:resource="http://resource.geosciml.org/classifierscheme/cgi/201211/metamorphicfacies"/>
	<skos:narrower rdf:resource="http://resource.geosciml.org/classifier/cgi/metamorphicfacies/eclogite_metamorphic_facies"/>
	<skos:narrower rdf:resource="http://resource.geosciml.org/classifier/cgi/metamorphicfacies/zeolite_metamorphic_facies"/>
	<skos:narrower rdf:resource="http://resource.geosciml.org/classifier/cgi/metamorphicfacies/epidote_amphibolite_metamorphic_facies"/>
	<skos:narrower rdf:resource="http://resource.geosciml.org/classifier/cgi/metamorphicfacies/glaucophane_schist_facies"/>
	<skos:narrower rdf:resource="http://resource.geosciml.org/classifier/cgi/metamorphicfacies/greenschist_metamorphic_facies"/>
	<skos:narrower rdf:resource="http://resource.geosciml.org/classifier/cgi/metamorphicfacies/granulite_facies"/>
	<skos:narrower rdf:resource="http://resource.geosciml.org/classifier/cgi/metamorphicfacies/sanidinite_metamorphic_facies"/>
	<skos:narrower rdf:resource="http://resource.geosciml.org/classifier/cgi/metamorphicfacies/pyroxene_hornfels_metamorphic_facies"/>
	<skos:narrower rdf:resource="http://resource.geosciml.org/classifier/cgi/metamorphicfacies/subgreenschist_metamorphic_facies"/>
	<skos:narrower rdf:resource="http://resource.geosciml.org/classifier/cgi/metamorphicfacies/amphibolite_metamorphic_facies"/>
	<skos:prefLabel xml:lang="en">metamorphic facies not specified</skos:prefLabel>
	<skos:topConceptOf rdf:resource="http://resource.geosciml.org/classifierscheme/cgi/201211/metamorphicfacies"/>
</rdf:Description>

<rdf:Description rdf:about="http://resource.geosciml.org/classifier/cgi/metamorphicfacies/metamorphic_facies_unknown">
	<rdf:type rdf:resource="http://www.w3.org/2004/02/skos/core#Concept"/>
	<dc:creator xml:lang="en">Concept Definition Task Group of IUGS CGI Interoperability Working Group (http://www.cgi-iugs.org/tech_collaboration/interoperability_working_group.html)</dc:creator>
	<dc:source xml:lang="en">this vocabulary</dc:source>
	<skos:definition xml:lang="en">For use in instance descriptions to indicate that no data are available to constrain metamorphic facies.  May be metamorphosed or non-metamorphosed.</skos:definition>
	<skos:exactMatch rdf:resource="http://resource.geosciml.org/classifier/cgi/metamorphicfacies/0008"/>
	<skos:inScheme rdf:resource="http://resource.geosciml.org/classifierscheme/cgi/201211/metamorphicfacies"/>
	<skos:prefLabel xml:lang="en">metamorphic facies unknown</skos:prefLabel>
	<skos:topConceptOf rdf:resource="http://resource.geosciml.org/classifierscheme/cgi/201211/metamorphicfacies"/>
</rdf:Description>

<rdf:Description rdf:about="http://resource.geosciml.org/classifier/cgi/metamorphicfacies/no_metamorphic_minerals">
	<rdf:type rdf:resource="http://www.w3.org/2004/02/skos/core#Concept"/>
	<dc:creator xml:lang="en">Concept Definition Task Group of IUGS CGI Interoperability Working Group (http://www.cgi-iugs.org/tech_collaboration/interoperability_working_group.html)</dc:creator>
	<dc:source xml:lang="en">this vocabulary</dc:source>
	<skos:definition xml:lang="en">Corresponds to non-metamorphosed condition; since metamorphic facies classification is based on mineral assemblages, absence of metamorphic minerals means that the classification does not apply.</skos:definition>
	<skos:exactMatch rdf:resource="http://resource.geosciml.org/classifier/cgi/metamorphicfacies/0009"/>
	<skos:inScheme rdf:resource="http://resource.geosciml.org/classifierscheme/cgi/201211/metamorphicfacies"/>
	<skos:prefLabel xml:lang="en">no metamorphic minerals</skos:prefLabel>
	<skos:topConceptOf rdf:resource="http://resource.geosciml.org/classifierscheme/cgi/201211/metamorphicfacies"/>
</rdf:Description>

<rdf:Description rdf:about="http://resource.geosciml.org/classifier/cgi/metamorphicfacies/pyroxene_hornfels_metamorphic_facies">
	<rdf:type rdf:resource="http://www.w3.org/2004/02/skos/core#Concept"/>
	<dc:creator xml:lang="en">Concept Definition Task Group of IUGS CGI Interoperability Working Group (http://www.cgi-iugs.org/tech_collaboration/interoperability_working_group.html)</dc:creator>
	<dc:source xml:lang="en">Smulikowski et al. 2003;Fettes and Desmons 2007</dc:source>
	<skos:broader rdf:resource="http://resource.geosciml.org/classifier/cgi/metamorphicfacies/metamorphic_facies_not_specified"/>
	<skos:definition xml:lang="en">Metamorphic facies characterized in rocks of basaltic composition by clinopyroxene-orthopyroxene-plagioclase (olivine stable with plagioclase).</skos:definition>
	<skos:exactMatch rdf:resource="http://resource.geosciml.org/classifier/cgi/metamorphicfacies/0010"/>
	<skos:inScheme rdf:resource="http://resource.geosciml.org/classifierscheme/cgi/201211/metamorphicfacies"/>
	<skos:prefLabel xml:lang="en">pyroxene hornfels metamorphic facies</skos:prefLabel>
</rdf:Description>

<rdf:Description rdf:about="http://resource.geosciml.org/classifier/cgi/metamorphicfacies/sanidinite_metamorphic_facies">
	<rdf:type rdf:resource="http://www.w3.org/2004/02/skos/core#Concept"/>
	<dc:creator xml:lang="en">Concept Definition Task Group of IUGS CGI Interoperability Working Group (http://www.cgi-iugs.org/tech_collaboration/interoperability_working_group.html)</dc:creator>
	<dc:source xml:lang="en">Fettes and Desmons 2007</dc:source>
	<skos:broader rdf:resource="http://resource.geosciml.org/classifier/cgi/metamorphicfacies/metamorphic_facies_not_specified"/>
	<skos:definition xml:lang="en">distinguished from the pyroxene hornfels facies by the occurrence of especially high-temperature varieties and polymorphs of minerals (eg. pigeonite, K-rich labradorite); assemblage for rocks of basaltic composition</skos:definition>
	<skos:exactMatch rdf:resource="http://resource.geosciml.org/classifier/cgi/metamorphicfacies/0011"/>
	<skos:inScheme rdf:resource="http://resource.geosciml.org/classifierscheme/cgi/201211/metamorphicfacies"/>
	<skos:prefLabel xml:lang="en">sanidinite metamorphic facies</skos:prefLabel>
</rdf:Description>

<rdf:Description rdf:about="http://resource.geosciml.org/classifier/cgi/metamorphicfacies/subgreenschist_metamorphic_facies">
	<rdf:type rdf:resource="http://www.w3.org/2004/02/skos/core#Concept"/>
	<dc:creator xml:lang="en">Concept Definition Task Group of IUGS CGI Interoperability Working Group (http://www.cgi-iugs.org/tech_collaboration/interoperability_working_group.html)</dc:creator>
	<dc:source xml:lang="en">Smulikowski et al. 2003; Fettes and Desmons 2007</dc:source>
	<skos:broader rdf:resource="http://resource.geosciml.org/classifier/cgi/metamorphicfacies/metamorphic_facies_not_specified"/>
	<skos:definition xml:lang="en">Metamorphic facies characterized in rocks of basaltic composition by prehnite-pumpellyite, pumpellyite-actinolite, prehnite-actinolite (prehnite and pumpellyite are the diagnostic Ca-Al silicates rather than minerals of the epidote or zeolite groups).</skos:definition>
	<skos:exactMatch rdf:resource="http://resource.geosciml.org/classifier/cgi/metamorphicfacies/0012"/>
	<skos:inScheme rdf:resource="http://resource.geosciml.org/classifierscheme/cgi/201211/metamorphicfacies"/>
	<skos:prefLabel xml:lang="en">subgreenschist metamorphic facies</skos:prefLabel>
</rdf:Description>

<rdf:Description rdf:about="http://resource.geosciml.org/classifier/cgi/metamorphicfacies/zeolite_metamorphic_facies">
	<rdf:type rdf:resource="http://www.w3.org/2004/02/skos/core#Concept"/>
	<dc:creator xml:lang="en">Concept Definition Task Group of IUGS CGI Interoperability Working Group (http://www.cgi-iugs.org/tech_collaboration/interoperability_working_group.html)</dc:creator>
	<dc:source xml:lang="en">Smulikowski et al. 2003; Fettes and Desmons 2007</dc:source>
	<skos:broader rdf:resource="http://resource.geosciml.org/classifier/cgi/metamorphicfacies/metamorphic_facies_not_specified"/>
	<skos:definition xml:lang="en">Metamorphic facies characterized in rocks of basaltic composition by zeolite minerals such as laumontite and heulandites (in place of other Ca-Al silicates such as prehnite, pumpellyite and epidote).</skos:definition>
	<skos:exactMatch rdf:resource="http://resource.geosciml.org/classifier/cgi/metamorphicfacies/0013"/>
	<skos:inScheme rdf:resource="http://resource.geosciml.org/classifierscheme/cgi/201211/metamorphicfacies"/>
	<skos:prefLabel xml:lang="en">zeolite metamorphic facies</skos:prefLabel>
</rdf:Description>

<rdf:Description rdf:about="http://resource.geosciml.org/classifierscheme/cgi/201211/metamorphicfacies">
	<rdf:type rdf:resource="http://www.w3.org/2002/07/owl#Ontology"/>
	<rdf:type rdf:resource="http://www.w3.org/2004/02/skos/core#ConceptScheme"/>
	<dc:creator xml:lang="en">Concept Definition Task Group of IUGS CGI Interoperability Working Group (http://www.cgi-iugs.org/tech_collaboration/interoperability_working_group.html)</dc:creator>
	<dc:format rdf:datatype="http://www.w3.org/2001/XMLSchema#string">application/rdf+xml</dc:format>
	<dc:identifier>http://resource.geosciml.org/classifierscheme/cgi/201211/metamorphicfacies</dc:identifier>
	<dc:language>en</dc:language>
	<dc:publisher xml:lang="en">Concept Definition Task Group of IUGS CGI Interoperability Working Group (http://www.cgi-iugs.org/tech_collaboration/interoperability_working_group.html)</dc:publisher>
	<dc:title xml:lang="en">CGI Metamorphic Facies Categories</dc:title>
	<owl:imports rdf:resource="http://rdfs.org/ns/void"/>
	<owl:imports rdf:resource="http://www.w3.org/2004/02/skos/core"/>
	<owl:versionInfo>201211</owl:versionInfo>
	<skos:definition xml:lang="en">This file contains the CGI metamorphic facies vocabulary; vocabulary is based on Fettes and Desmons, 2007. Use to populate metamorphic facies property in metamorphic description</skos:definition>
	<skos:historyNote xml:lang="en">2012-02-27 SMR add skos:exactMatch triples associating URIs with number token URI in 201012 version.</skos:historyNote>
	<skos:historyNote xml:lang="en">2012-11-24 SMR Update to 201211 version; add collection entity, check all pref labels are lower case, remove owl:NamedIndividual and Owl:Thing rdf:types.</skos:historyNote>
	<skos:historyNote xml:lang="en">2012-02-07 SMR update URI to replace numeric final token with English-language string as in original URN scheme.</skos:historyNote>
	<skos:historyNote xml:lang="en">2010-02-11 Add narrower relationship links by adding skos:narrower link in Protege, defining skos:narrower as inverse of skos:broader, calculating with Pellet reasoner to add inferred axioms, and using 'file/Export inferred axioms as ontology' in Protege.</skos:historyNote>
	<skos:historyNote xml:lang="en">2010-11-28 SMR Replace URN identifiers with http URI identifiers according to CGI URI scheme (see https://www.seegrid.csiro.au/wiki/bin/view/CGIModel/PersistentIdentifiersInGeoSciMLServices)</skos:historyNote>
	<skos:prefLabel xml:lang="en">CGI Metamorphic Facies Categories</skos:prefLabel>
</rdf:Description>

<rdf:Description rdf:about="http://resource.geosciml.org/vocabulary/cgi/201211/metamorphicfacies">
	<rdf:type rdf:resource="http://rdfs.org/ns/void#Dataset"/>
	<rdfs:label rdf:datatype="http://www.w3.org/2001/XMLSchema#string">Metamorphic facies vocabulary</rdfs:label>
</rdf:Description>

<rdf:Description rdf:about="http://www.w3.org/2004/02/skos/core#ConceptScheme">
	<rdf:type rdf:resource="http://www.w3.org/2002/07/owl#Class"/>
</rdf:Description>

</rdf:RDF>