# baseURI: http://resource.geosciml.org/classifierscheme/cgi/201211/metamorphicgrade
# imports: http://rdfs.org/ns/void
# imports: http://www.w3.org/2004/02/skos/core

@prefix :        <http://resource.geosciml.org/classifierscheme/cgi/201211/metamorphicgrade#> .
@prefix cgi:     <http://resource.geosciml.org/classifierscheme/cgi/201211/> .
@prefix dc:      <http://purl.org/dc/elements/1.1/> .
@prefix metagrade:  <http://resource.geosciml.org/classifier/cgi/metamorphicgrade/> .
@prefix owl:     <http://www.w3.org/2002/07/owl#> .
@prefix owl2xml:  <http://www.w3.org/2006/12/owl2-xml#> .
@prefix rdf:     <http://www.w3.org/1999/02/22-rdf-syntax-ns#> .
@prefix rdfs:    <http://www.w3.org/2000/01/rdf-schema#> .
@prefix skos:    <http://www.w3.org/2004/02/skos/core#> .
@prefix void:    <http://rdfs.org/ns/void#> .
@prefix xsd:     <http://www.w3.org/2001/XMLSchema#> .

metagrade:
      rdf:type skos:Collection ;
      rdfs:label "metamorphic grade concepts"@en ;
      skos:definition "This resource defines the concept space for metamorphic grade concepts by extension; it includes all concepts in this conceptScheme, as well as concepts in previous versions of the scheme."@en ;
      skos:member metagrade:very_high_metamorphic_grade , metagrade:not_metamorphosed , metagrade:very_low_metamorphic_grade , metagrade:high_metamorphic_grade , metagrade:metamorphic_grade_unknown , metagrade:metamorphic_grade_not_specified , metagrade:low_metamorphic_grade , metagrade:medium_metamorphic_grade , metagrade:metamorphosed_grade_not_specified ;
      skos:prefLabel "CGI Metamorphic Grade"@en .

<http://resource.geosciml.org/classifier/cgi/metamorphicgrade/0001>
      rdf:type owl:NamedIndividual .

<http://resource.geosciml.org/classifier/cgi/metamorphicgrade/0002>
      rdf:type owl:NamedIndividual .

<http://resource.geosciml.org/classifier/cgi/metamorphicgrade/0003>
      rdf:type owl:NamedIndividual .

<http://resource.geosciml.org/classifier/cgi/metamorphicgrade/0004>
      rdf:type owl:NamedIndividual .

<http://resource.geosciml.org/classifier/cgi/metamorphicgrade/0005>
      rdf:type owl:NamedIndividual .

<http://resource.geosciml.org/classifier/cgi/metamorphicgrade/0006>
      rdf:type owl:NamedIndividual .

<http://resource.geosciml.org/classifier/cgi/metamorphicgrade/0007>
      rdf:type owl:NamedIndividual .

<http://resource.geosciml.org/classifier/cgi/metamorphicgrade/0008>
      rdf:type owl:NamedIndividual .

<http://resource.geosciml.org/classifier/cgi/metamorphicgrade/0009>
      rdf:type owl:NamedIndividual .

metagrade:high_metamorphic_grade
      rdf:type skos:Concept ;
      dc:creator "Concept Definition Task Group of IUGS CGI Interoperability Working Group (http://www.cgi-iugs.org/tech_collaboration/interoperability_working_group.html)"@en ;
      dc:source "Smulikowski et al, 2003; Fry, 1984" ;
      skos:broader metagrade:metamorphosed_grade_not_specified ;
      skos:definition "Protolith structures almost always obliterated, evidence of partial melting common. Includes rocks metamorphosed in high-temperature amphibolite, pyroxene hornfels, and medium to high-temperature eclogite facies. Mineral assemblages according to Fry (1984) Table 10-1: ultramafic-olivine, anthophyllite, cummingtonite, enstatite; mafic-hornblende, (diopside, garnet); calc-aluminous basic-plagioclase; pelite, semi-pelite -- K-feldspar, biotite, quartz, Al-minerals (garnet), migmatite."@en ;
      skos:exactMatch <http://resource.geosciml.org/classifier/cgi/metamorphicgrade/0001> ;
      skos:inScheme cgi:metamorphicgrade ;
      skos:prefLabel "high metamorphic grade"@en .

metagrade:low_metamorphic_grade
      rdf:type skos:Concept ;
      dc:creator "Concept Definition Task Group of IUGS CGI Interoperability Working Group (http://www.cgi-iugs.org/tech_collaboration/interoperability_working_group.html)"@en ;
      dc:source "Smulikowski et al, 2003; Fry, 1984" ;
      skos:broader metagrade:metamorphosed_grade_not_specified ;
      skos:definition "Metamorphic effects clearly visible, protolith structures typically still observable, includes rocks metamorphosed in greenschist, high-temperature blueschist, very low temperature eclogite facies. Mineral assemblages according to Fry (1984) Table 10-1: ultramafic-serpentine (talc, magnesite); mafic-chlorite, actinolite (garnet); calc-aluminous basic-albite, epidote; pelite, semi-pelite -- white mica, chlorite, quartz, biotite (garnet, Al-minerals)."@en ;
      skos:exactMatch <http://resource.geosciml.org/classifier/cgi/metamorphicgrade/0002> ;
      skos:inScheme cgi:metamorphicgrade ;
      skos:prefLabel "low metamorphic grade"@en .

metagrade:medium_metamorphic_grade
      rdf:type skos:Concept ;
      dc:creator "Concept Definition Task Group of IUGS CGI Interoperability Working Group (http://www.cgi-iugs.org/tech_collaboration/interoperability_working_group.html)"@en ;
      dc:source "Smulikowski et al, 2003; Fry, 1984" ;
      skos:broader metagrade:metamorphosed_grade_not_specified ;
      skos:definition "Protolith structure typically obliterated. Includes rocks metamorphosed in high-temperature epidote-amphibolite, low-temperature amphibolite, and low temperature eclogite facies. Mineral assemblages according to Fry (1984) Table 10-1: ultramafic-olivine, talc (magnesite, anthophyllite); mafic-hornblende, (diopside, garnet); calc-aluminous basic-plagioclase; pelite, semi-pelite -- white mica, biotite, quartz (garnet, Al-minerals)."@en ;
      skos:exactMatch <http://resource.geosciml.org/classifier/cgi/metamorphicgrade/0003> ;
      skos:inScheme cgi:metamorphicgrade ;
      skos:prefLabel "medium metamorphic grade"@en .

metagrade:metamorphic_grade_not_specified
      rdf:type skos:Concept ;
      dc:creator "Concept Definition Task Group of IUGS CGI Interoperability Working Group (http://www.cgi-iugs.org/tech_collaboration/interoperability_working_group.html)"@en ;
      dc:source "This Vocabulary" ;
      skos:definition "for use in normative descriptions to explicitly indicate that any metamorphic condition is allowed (including non-metamorphosed)."@en ;
      skos:exactMatch <http://resource.geosciml.org/classifier/cgi/metamorphicgrade/0004> ;
      skos:inScheme cgi:metamorphicgrade ;
      skos:narrower metagrade:metamorphosed_grade_not_specified , metagrade:not_metamorphosed ;
      skos:prefLabel "metamorphic grade not specified"@en ;
      skos:topConceptOf cgi:metamorphicgrade .

metagrade:metamorphic_grade_unknown
      rdf:type skos:Concept ;
      dc:creator "Concept Definition Task Group of IUGS CGI Interoperability Working Group (http://www.cgi-iugs.org/tech_collaboration/interoperability_working_group.html)"@en ;
      dc:source "This Vocabulary" ;
      skos:definition "For use in instance descriptions to indicate that no information is available on metamorphic grade"@en ;
      skos:exactMatch <http://resource.geosciml.org/classifier/cgi/metamorphicgrade/0005> ;
      skos:inScheme cgi:metamorphicgrade ;
      skos:prefLabel "metamorphic grade unknown"@en ;
      skos:topConceptOf cgi:metamorphicgrade .

metagrade:metamorphosed_grade_not_specified
      rdf:type skos:Concept ;
      dc:creator "Concept Definition Task Group of IUGS CGI Interoperability Working Group (http://www.cgi-iugs.org/tech_collaboration/interoperability_working_group.html)"@en ;
      dc:source "This Vocabulary" ;
      skos:broader metagrade:metamorphic_grade_not_specified ;
      skos:definition "Rock is metamorphosed, may have any value for metamorphic grade."@en ;
      skos:exactMatch <http://resource.geosciml.org/classifier/cgi/metamorphicgrade/0006> ;
      skos:inScheme cgi:metamorphicgrade ;
      skos:narrower metagrade:high_metamorphic_grade , metagrade:medium_metamorphic_grade , metagrade:very_high_metamorphic_grade , metagrade:low_metamorphic_grade , metagrade:very_low_metamorphic_grade ;
      skos:prefLabel "metamorphosed grade not specified"@en .

metagrade:not_metamorphosed
      rdf:type skos:Concept ;
      dc:creator "Concept Definition Task Group of IUGS CGI Interoperability Working Group (http://www.cgi-iugs.org/tech_collaboration/interoperability_working_group.html)"@en ;
      dc:source "This Vocabulary" ;
      skos:broader metagrade:metamorphic_grade_not_specified ;
      skos:definition "Rock or sediment not metamorphosed."@en ;
      skos:exactMatch <http://resource.geosciml.org/classifier/cgi/metamorphicgrade/0007> ;
      skos:inScheme cgi:metamorphicgrade ;
      skos:prefLabel "not metamorphosed"@en .

metagrade:very_high_metamorphic_grade
      rdf:type skos:Concept ;
      dc:creator "Concept Definition Task Group of IUGS CGI Interoperability Working Group (http://www.cgi-iugs.org/tech_collaboration/interoperability_working_group.html)"@en ;
      dc:source "Smulikowski et al, 2003; Fry, 1984" ;
      skos:broader metagrade:metamorphosed_grade_not_specified ;
      skos:definition "Protolith structures almost always obliterated. Includes rocks metamorphosed in granulite (or sanidinite), and high-temperature eclogite facies. Mineral assemblages according to Fry (1984) Table 10-1: ultramafic-olivine, enstatite; mafic-hypersthene, diopside (hornblende); calc-aluminous basic-plagioclase; pelite, semi-pelite -- hypersthene + Al-minerals (K-feldspar, quartz), or sapphirine."@en ;
      skos:exactMatch <http://resource.geosciml.org/classifier/cgi/metamorphicgrade/0008> ;
      skos:inScheme cgi:metamorphicgrade ;
      skos:prefLabel "very high metamorphic grade"@en .

metagrade:very_low_metamorphic_grade
      rdf:type skos:Concept ;
      dc:creator "Concept Definition Task Group of IUGS CGI Interoperability Working Group (http://www.cgi-iugs.org/tech_collaboration/interoperability_working_group.html)"@en ;
      dc:source "Smulikowski et al, 2003; Fry, 1984" ;
      skos:broader metagrade:metamorphosed_grade_not_specified ;
      skos:definition "Rock very slightly metamorphosed, protolith structure ubiquitous; mineral assemblage of zeolite facies, subgreenschist facies, or low temperature part of blueschist facies. Mineral assemblages according to Fry (1984) Table 10-1: ultramafic-serpentine (quartz, magnesite); mafic-clay, chlorite, relict igneous minerals; calc-aluminous basic-zeolite, pumpellite, epidote, albite; pelite, semi-pelite -- clays, chlorite, sericite, quartz."@en ;
      skos:exactMatch <http://resource.geosciml.org/classifier/cgi/metamorphicgrade/0009> ;
      skos:inScheme cgi:metamorphicgrade ;
      skos:prefLabel "very low metamorphic grade"@en .

cgi:metamorphicgrade
      rdf:type skos:ConceptScheme , owl:Ontology ;
      dc:creator "Concept Definition Task Group of IUGS CGI Interoperability Working Group (http://www.cgi-iugs.org/tech_collaboration/interoperability_working_group.html)"@en ;
      dc:format "application/rdf+xml" ;
      dc:identifier "http://resource.geosciml.org/classifierscheme/cgi/201211/metamorphicgrade" ;
      dc:language "en" ;
      dc:publisher "Concept Definition Task Group of IUGS CGI Interoperability Working Group (http://www.cgi-iugs.org/tech_collaboration/interoperability_working_group.html)"@en ;
      dc:title "CGI Metamorphic Grade Categories"@en ;
      owl:imports <http://www.w3.org/2004/02/skos/core> , <http://rdfs.org/ns/void> ;
      owl:versionInfo "201211" ;
      skos:definition "This file contains the CGI Metamorphic Grade vocabulary. Vocabulary for populating Metamorphic grade property in GeoSciML metamorphicDescription elements. Derived from Fettes and Desmons, 2007"@en ;
      skos:historyNote "2012-02-27 SMR add skos:exactMatch triples relating URI in this vocabulary to URI with number tokens in 201012 vocabulary"@en , "2010-02-11 Add narrower relationship links by adding skos:narrower link in Protege, defining skos:narrower as inverse of skos:broader, calculating with Pellet reasoner to add inferred axioms, and using 'file/Export inferred axioms as ontology' in Protege."@en , "2012-02-07 SMR update URI to replace numeric final token with English-language string as in original URN scheme."@en , "2012-11-24 SMR Update to 201211 version; add collection entity, check all pref labels are lower case, remove owl:NamedIndividual and Owl:Thing rdf:types."@en , "2010-11-28 SMR replace URN identifiers with http URI identifiers according to CGI URI scheme (see https://www.seegrid.csiro.au/wiki/bin/view/CGIModel/PersistentIdentifiersInGeoSciMLServices)"@en ;
      skos:prefLabel "CGI Metamorphic Grade Categories"@en .

<http://resource.geosciml.org/vocabulary/cgi/201211/metamorphicgrade>
      rdf:type void:Dataset ;
      rdfs:label "Metamorphic grade vocabulary"^^xsd:string .
