# baseURI: http://resource.geosciml.org/classifierscheme/cgi/201211/metamorphicfacies
# imports: http://rdfs.org/ns/void
# imports: http://www.w3.org/2004/02/skos/core

@prefix :        <http://resource.geosciml.org/classifierscheme/cgi/201211/metamorphicfacies#> .
@prefix cgi:     <http://resource.geosciml.org/classifierscheme/cgi/201211/> .
@prefix dc:      <http://purl.org/dc/elements/1.1/> .
@prefix metafac:  <http://resource.geosciml.org/classifier/cgi/metamorphicfacies/> .
@prefix owl:     <http://www.w3.org/2002/07/owl#> .
@prefix owl2xml:  <http://www.w3.org/2006/12/owl2-xml#> .
@prefix rdf:     <http://www.w3.org/1999/02/22-rdf-syntax-ns#> .
@prefix rdfs:    <http://www.w3.org/2000/01/rdf-schema#> .
@prefix skos:    <http://www.w3.org/2004/02/skos/core#> .
@prefix void:    <http://rdfs.org/ns/void#> .
@prefix xsd:     <http://www.w3.org/2001/XMLSchema#> .

metafac:
      rdf:type skos:Collection ;
      rdfs:label "metamorphic facies concepts"@en ;
      skos:definition "This resource defines the concept space for metamorphic facies concepts by extension; it includes all concepts in this conceptScheme, as well as concepts in previous versions of the scheme."@en ;
      skos:member metafac:no_metamorphic_minerals , metafac:epidote_amphibolite_metamorphic_facies , metafac:glaucophane_schist_facies , metafac:zeolite_metamorphic_facies , metafac:sanidinite_metamorphic_facies , metafac:amphibolite_metamorphic_facies , metafac:greenschist_metamorphic_facies , metafac:granulite_facies , metafac:metamorphic_facies_unknown , metafac:pyroxene_hornfels_metamorphic_facies , metafac:metamorphic_facies_not_specified , metafac:eclogite_metamorphic_facies , metafac:subgreenschist_metamorphic_facies ;
      skos:prefLabel "CGI Metamorphic Facies"@en .

<http://resource.geosciml.org/classifier/cgi/metamorphicfacies/0001>
      rdf:type owl:NamedIndividual .

<http://resource.geosciml.org/classifier/cgi/metamorphicfacies/0002>
      rdf:type owl:NamedIndividual .

<http://resource.geosciml.org/classifier/cgi/metamorphicfacies/0003>
      rdf:type owl:NamedIndividual .

<http://resource.geosciml.org/classifier/cgi/metamorphicfacies/0004>
      rdf:type owl:NamedIndividual .

<http://resource.geosciml.org/classifier/cgi/metamorphicfacies/0005>
      rdf:type owl:NamedIndividual .

<http://resource.geosciml.org/classifier/cgi/metamorphicfacies/0006>
      rdf:type owl:NamedIndividual .

<http://resource.geosciml.org/classifier/cgi/metamorphicfacies/0007>
      rdf:type owl:NamedIndividual .

<http://resource.geosciml.org/classifier/cgi/metamorphicfacies/0008>
      rdf:type owl:NamedIndividual .

<http://resource.geosciml.org/classifier/cgi/metamorphicfacies/0009>
      rdf:type owl:NamedIndividual .

<http://resource.geosciml.org/classifier/cgi/metamorphicfacies/0010>
      rdf:type owl:NamedIndividual .

<http://resource.geosciml.org/classifier/cgi/metamorphicfacies/0011>
      rdf:type owl:NamedIndividual .

<http://resource.geosciml.org/classifier/cgi/metamorphicfacies/0012>
      rdf:type owl:NamedIndividual .

<http://resource.geosciml.org/classifier/cgi/metamorphicfacies/0013>
      rdf:type owl:NamedIndividual .

metafac:amphibolite_metamorphic_facies
      rdf:type skos:Concept ;
      dc:creator "Concept Definition Task Group of IUGS CGI Interoperability Working Group (http://www.cgi-iugs.org/tech_collaboration/interoperability_working_group.html)"@en ;
      dc:source "Smulikowski et al. 2003; Fettes and Desmons 2007" ;
      skos:broader metafac:metamorphic_facies_not_specified ;
      skos:definition "Metamorphic facies characterized in rocks of basaltic composition by hornblende-plagioclase (plagioclase more calcic than An17)."@en ;
      skos:exactMatch <http://resource.geosciml.org/classifier/cgi/metamorphicfacies/0001> ;
      skos:inScheme cgi:metamorphicfacies ;
      skos:prefLabel "amphibolite metamorphic facies"@en .

metafac:eclogite_metamorphic_facies
      rdf:type skos:Concept ;
      dc:creator "Concept Definition Task Group of IUGS CGI Interoperability Working Group (http://www.cgi-iugs.org/tech_collaboration/interoperability_working_group.html)"@en ;
      dc:source "Fettes and Desmons 2007"@en ;
      skos:broader metafac:metamorphic_facies_not_specified ;
      skos:definition "omphacite-garnet-quartz (no plagioclase, olivine stable with garnet); assemblage for rocks of basaltic composition"@en ;
      skos:exactMatch <http://resource.geosciml.org/classifier/cgi/metamorphicfacies/0002> ;
      skos:inScheme cgi:metamorphicfacies ;
      skos:prefLabel "eclogite metamorphic facies"@en .

metafac:epidote_amphibolite_metamorphic_facies
      rdf:type skos:Concept ;
      dc:creator "Concept Definition Task Group of IUGS CGI Interoperability Working Group (http://www.cgi-iugs.org/tech_collaboration/interoperability_working_group.html)"@en ;
      dc:source "Fettes and Desmons 2007"@en ;
      skos:broader metafac:metamorphic_facies_not_specified ;
      skos:definition "hornblende-albite-epidote(-chlorite); assemblage for rocks of basaltic composition"@en ;
      skos:exactMatch <http://resource.geosciml.org/classifier/cgi/metamorphicfacies/0003> ;
      skos:inScheme cgi:metamorphicfacies ;
      skos:prefLabel "epidote amphibolite metamorphic facies"@en .

metafac:glaucophane_schist_facies
      rdf:type skos:Concept ;
      dc:creator "Concept Definition Task Group of IUGS CGI Interoperability Working Group (http://www.cgi-iugs.org/tech_collaboration/interoperability_working_group.html)"@en ;
      dc:source "Smulikowski et al., 2003; Fettes and Desmons 2007"@en ;
      skos:broader metafac:metamorphic_facies_not_specified ;
      skos:definition "Metamorphic facies characterized in rocks of basaltic composition by glaucophane-epidote (-garnet), glaucophane-lawsonite, or glaucophane-lawsonite-jadeite."@en ;
      skos:exactMatch <http://resource.geosciml.org/classifier/cgi/metamorphicfacies/0004> ;
      skos:inScheme cgi:metamorphicfacies ;
      skos:prefLabel "glaucophane schist facies"@en .

metafac:granulite_facies
      rdf:type skos:Concept ;
      dc:creator "Concept Definition Task Group of IUGS CGI Interoperability Working Group (http://www.cgi-iugs.org/tech_collaboration/interoperability_working_group.html)"@en ;
      dc:source "Smulikowski et al., 2003; Fettes and Desmons 2007"@en ;
      skos:broader metafac:metamorphic_facies_not_specified ;
      skos:definition "Metamorphic facies characterized in rocks of basaltic composition by the mineral assemblage clinopyroxene-orthopyroxene-plagioclase (olivine not stable with plagioclase or with garnet), or especially high-temperature varieties or polymorphs of minerals (e"@en ;
      skos:exactMatch <http://resource.geosciml.org/classifier/cgi/metamorphicfacies/0005> ;
      skos:inScheme cgi:metamorphicfacies ;
      skos:prefLabel "granulite facies"@en .

metafac:greenschist_metamorphic_facies
      rdf:type skos:Concept ;
      dc:creator "Concept Definition Task Group of IUGS CGI Interoperability Working Group (http://www.cgi-iugs.org/tech_collaboration/interoperability_working_group.html)"@en ;
      dc:source "Smulikowski et al., 2003; Fettes and Desmons 2007"@en ;
      skos:broader metafac:metamorphic_facies_not_specified ;
      skos:definition "Metamorphic facies characterized in rocks of basaltic composition by actinolite-albite-epidote-chlorite (an epidote group mineral is the diagnostic Ca-Al silicate rather than prehnite or pumpellyite)."@en ;
      skos:exactMatch <http://resource.geosciml.org/classifier/cgi/metamorphicfacies/0006> ;
      skos:inScheme cgi:metamorphicfacies ;
      skos:prefLabel "greenschist metamorphic facies"@en .

metafac:metamorphic_facies_not_specified
      rdf:type skos:Concept ;
      dc:creator "Concept Definition Task Group of IUGS CGI Interoperability Working Group (http://www.cgi-iugs.org/tech_collaboration/interoperability_working_group.html)"@en ;
      dc:source "this vocabulary"@en ;
      skos:definition "Metamorphosed, but facies not specified in more detail. For use in normative description to indicate that any metamorphic facies value is valid."@en ;
      skos:exactMatch <http://resource.geosciml.org/classifier/cgi/metamorphicfacies/0007> ;
      skos:inScheme cgi:metamorphicfacies ;
      skos:narrower metafac:eclogite_metamorphic_facies , metafac:zeolite_metamorphic_facies , metafac:epidote_amphibolite_metamorphic_facies , metafac:glaucophane_schist_facies , metafac:greenschist_metamorphic_facies , metafac:granulite_facies , metafac:sanidinite_metamorphic_facies , metafac:pyroxene_hornfels_metamorphic_facies , metafac:subgreenschist_metamorphic_facies , metafac:amphibolite_metamorphic_facies ;
      skos:prefLabel "metamorphic facies not specified"@en ;
      skos:topConceptOf cgi:metamorphicfacies .

metafac:metamorphic_facies_unknown
      rdf:type skos:Concept ;
      dc:creator "Concept Definition Task Group of IUGS CGI Interoperability Working Group (http://www.cgi-iugs.org/tech_collaboration/interoperability_working_group.html)"@en ;
      dc:source "this vocabulary"@en ;
      skos:definition "For use in instance descriptions to indicate that no data are available to constrain metamorphic facies.  May be metamorphosed or non-metamorphosed."@en ;
      skos:exactMatch <http://resource.geosciml.org/classifier/cgi/metamorphicfacies/0008> ;
      skos:inScheme cgi:metamorphicfacies ;
      skos:prefLabel "metamorphic facies unknown"@en ;
      skos:topConceptOf cgi:metamorphicfacies .

metafac:no_metamorphic_minerals
      rdf:type skos:Concept ;
      dc:creator "Concept Definition Task Group of IUGS CGI Interoperability Working Group (http://www.cgi-iugs.org/tech_collaboration/interoperability_working_group.html)"@en ;
      dc:source "this vocabulary"@en ;
      skos:definition "Corresponds to non-metamorphosed condition; since metamorphic facies classification is based on mineral assemblages, absence of metamorphic minerals means that the classification does not apply."@en ;
      skos:exactMatch <http://resource.geosciml.org/classifier/cgi/metamorphicfacies/0009> ;
      skos:inScheme cgi:metamorphicfacies ;
      skos:prefLabel "no metamorphic minerals"@en ;
      skos:topConceptOf cgi:metamorphicfacies .

metafac:pyroxene_hornfels_metamorphic_facies
      rdf:type skos:Concept ;
      dc:creator "Concept Definition Task Group of IUGS CGI Interoperability Working Group (http://www.cgi-iugs.org/tech_collaboration/interoperability_working_group.html)"@en ;
      dc:source "Smulikowski et al. 2003;Fettes and Desmons 2007"@en ;
      skos:broader metafac:metamorphic_facies_not_specified ;
      skos:definition "Metamorphic facies characterized in rocks of basaltic composition by clinopyroxene-orthopyroxene-plagioclase (olivine stable with plagioclase)."@en ;
      skos:exactMatch <http://resource.geosciml.org/classifier/cgi/metamorphicfacies/0010> ;
      skos:inScheme cgi:metamorphicfacies ;
      skos:prefLabel "pyroxene hornfels metamorphic facies"@en .

metafac:sanidinite_metamorphic_facies
      rdf:type skos:Concept ;
      dc:creator "Concept Definition Task Group of IUGS CGI Interoperability Working Group (http://www.cgi-iugs.org/tech_collaboration/interoperability_working_group.html)"@en ;
      dc:source "Fettes and Desmons 2007"@en ;
      skos:broader metafac:metamorphic_facies_not_specified ;
      skos:definition "distinguished from the pyroxene hornfels facies by the occurrence of especially high-temperature varieties and polymorphs of minerals (eg. pigeonite, K-rich labradorite); assemblage for rocks of basaltic composition"@en ;
      skos:exactMatch <http://resource.geosciml.org/classifier/cgi/metamorphicfacies/0011> ;
      skos:inScheme cgi:metamorphicfacies ;
      skos:prefLabel "sanidinite metamorphic facies"@en .

metafac:subgreenschist_metamorphic_facies
      rdf:type skos:Concept ;
      dc:creator "Concept Definition Task Group of IUGS CGI Interoperability Working Group (http://www.cgi-iugs.org/tech_collaboration/interoperability_working_group.html)"@en ;
      dc:source "Smulikowski et al. 2003; Fettes and Desmons 2007"@en ;
      skos:broader metafac:metamorphic_facies_not_specified ;
      skos:definition "Metamorphic facies characterized in rocks of basaltic composition by prehnite-pumpellyite, pumpellyite-actinolite, prehnite-actinolite (prehnite and pumpellyite are the diagnostic Ca-Al silicates rather than minerals of the epidote or zeolite groups)."@en ;
      skos:exactMatch <http://resource.geosciml.org/classifier/cgi/metamorphicfacies/0012> ;
      skos:inScheme cgi:metamorphicfacies ;
      skos:prefLabel "subgreenschist metamorphic facies"@en .

metafac:zeolite_metamorphic_facies
      rdf:type skos:Concept ;
      dc:creator "Concept Definition Task Group of IUGS CGI Interoperability Working Group (http://www.cgi-iugs.org/tech_collaboration/interoperability_working_group.html)"@en ;
      dc:source "Smulikowski et al. 2003; Fettes and Desmons 2007"@en ;
      skos:broader metafac:metamorphic_facies_not_specified ;
      skos:definition "Metamorphic facies characterized in rocks of basaltic composition by zeolite minerals such as laumontite and heulandites (in place of other Ca-Al silicates such as prehnite, pumpellyite and epidote)."@en ;
      skos:exactMatch <http://resource.geosciml.org/classifier/cgi/metamorphicfacies/0013> ;
      skos:inScheme cgi:metamorphicfacies ;
      skos:prefLabel "zeolite metamorphic facies"@en .

cgi:metamorphicfacies
      rdf:type owl:Ontology , skos:ConceptScheme ;
      dc:creator "Concept Definition Task Group of IUGS CGI Interoperability Working Group (http://www.cgi-iugs.org/tech_collaboration/interoperability_working_group.html)"@en ;
      dc:format "application/rdf+xml"^^xsd:string ;
      dc:identifier "http://resource.geosciml.org/classifierscheme/cgi/201211/metamorphicfacies" ;
      dc:language "en" ;
      dc:publisher "Concept Definition Task Group of IUGS CGI Interoperability Working Group (http://www.cgi-iugs.org/tech_collaboration/interoperability_working_group.html)"@en ;
      dc:title "CGI Metamorphic Facies Categories"@en ;
      owl:imports <http://rdfs.org/ns/void> , <http://www.w3.org/2004/02/skos/core> ;
      owl:versionInfo "201211" ;
      skos:definition "This file contains the CGI metamorphic facies vocabulary; vocabulary is based on Fettes and Desmons, 2007. Use to populate metamorphic facies property in metamorphic description"@en ;
      skos:historyNote "2012-02-27 SMR add skos:exactMatch triples associating URIs with number token URI in 201012 version."@en , "2012-11-24 SMR Update to 201211 version; add collection entity, check all pref labels are lower case, remove owl:NamedIndividual and Owl:Thing rdf:types."@en , "2012-02-07 SMR update URI to replace numeric final token with English-language string as in original URN scheme."@en , "2010-02-11 Add narrower relationship links by adding skos:narrower link in Protege, defining skos:narrower as inverse of skos:broader, calculating with Pellet reasoner to add inferred axioms, and using 'file/Export inferred axioms as ontology' in Protege."@en , "2010-11-28 SMR Replace URN identifiers with http URI identifiers according to CGI URI scheme (see https://www.seegrid.csiro.au/wiki/bin/view/CGIModel/PersistentIdentifiersInGeoSciMLServices)"@en ;
      skos:prefLabel "CGI Metamorphic Facies Categories"@en .

<http://resource.geosciml.org/vocabulary/cgi/201211/metamorphicfacies>
      rdf:type void:Dataset ;
      rdfs:label "Metamorphic facies vocabulary"^^xsd:string .

skos:ConceptScheme
      rdf:type owl:Class .
