<?xml version="1.0" encoding="UTF-8"?>
<rdf:RDF
	xmlns="http://resource.geosciml.org/classifierscheme/cgi/201211/metamorphicgrade#"
	xmlns:cgi="http://resource.geosciml.org/classifierscheme/cgi/201211/"
	xmlns:dc="http://purl.org/dc/elements/1.1/"
	xmlns:metagrade="http://resource.geosciml.org/classifier/cgi/metamorphicgrade/"
	xmlns:owl="http://www.w3.org/2002/07/owl#"
	xmlns:owl2xml="http://www.w3.org/2006/12/owl2-xml#"
	xmlns:rdf="http://www.w3.org/1999/02/22-rdf-syntax-ns#"
	xmlns:rdfs="http://www.w3.org/2000/01/rdf-schema#"
	xmlns:skos="http://www.w3.org/2004/02/skos/core#"
	xmlns:void="http://rdfs.org/ns/void#"
	xmlns:xsd="http://www.w3.org/2001/XMLSchema#">

<rdf:Description rdf:about="http://resource.geosciml.org/classifier/cgi/metamorphicgrade/">
	<rdf:type rdf:resource="http://www.w3.org/2004/02/skos/core#Collection"/>
	<rdfs:label xml:lang="en">metamorphic grade concepts</rdfs:label>
	<skos:definition xml:lang="en">This resource defines the concept space for metamorphic grade concepts by extension; it includes all concepts in this conceptScheme, as well as concepts in previous versions of the scheme.</skos:definition>
	<skos:member rdf:resource="http://resource.geosciml.org/classifier/cgi/metamorphicgrade/very_high_metamorphic_grade"/>
	<skos:member rdf:resource="http://resource.geosciml.org/classifier/cgi/metamorphicgrade/not_metamorphosed"/>
	<skos:member rdf:resource="http://resource.geosciml.org/classifier/cgi/metamorphicgrade/very_low_metamorphic_grade"/>
	<skos:member rdf:resource="http://resource.geosciml.org/classifier/cgi/metamorphicgrade/high_metamorphic_grade"/>
	<skos:member rdf:resource="http://resource.geosciml.org/classifier/cgi/metamorphicgrade/metamorphic_grade_unknown"/>
	<skos:member rdf:resource="http://resource.geosciml.org/classifier/cgi/metamorphicgrade/metamorphic_grade_not_specified"/>
	<skos:member rdf:resource="http://resource.geosciml.org/classifier/cgi/metamorphicgrade/low_metamorphic_grade"/>
	<skos:member rdf:resource="http://resource.geosciml.org/classifier/cgi/metamorphicgrade/medium_metamorphic_grade"/>
	<skos:member rdf:resource="http://resource.geosciml.org/classifier/cgi/metamorphicgrade/metamorphosed_grade_not_specified"/>
	<skos:prefLabel xml:lang="en">CGI Metamorphic Grade</skos:prefLabel>
</rdf:Description>

<rdf:Description rdf:about="http://resource.geosciml.org/classifier/cgi/metamorphicgrade/0001">
	<rdf:type rdf:resource="http://www.w3.org/2002/07/owl#NamedIndividual"/>
</rdf:Description>

<rdf:Description rdf:about="http://resource.geosciml.org/classifier/cgi/metamorphicgrade/0002">
	<rdf:type rdf:resource="http://www.w3.org/2002/07/owl#NamedIndividual"/>
</rdf:Description>

<rdf:Description rdf:about="http://resource.geosciml.org/classifier/cgi/metamorphicgrade/0003">
	<rdf:type rdf:resource="http://www.w3.org/2002/07/owl#NamedIndividual"/>
</rdf:Description>

<rdf:Description rdf:about="http://resource.geosciml.org/classifier/cgi/metamorphicgrade/0004">
	<rdf:type rdf:resource="http://www.w3.org/2002/07/owl#NamedIndividual"/>
</rdf:Description>

<rdf:Description rdf:about="http://resource.geosciml.org/classifier/cgi/metamorphicgrade/0005">
	<rdf:type rdf:resource="http://www.w3.org/2002/07/owl#NamedIndividual"/>
</rdf:Description>

<rdf:Description rdf:about="http://resource.geosciml.org/classifier/cgi/metamorphicgrade/0006">
	<rdf:type rdf:resource="http://www.w3.org/2002/07/owl#NamedIndividual"/>
</rdf:Description>

<rdf:Description rdf:about="http://resource.geosciml.org/classifier/cgi/metamorphicgrade/0007">
	<rdf:type rdf:resource="http://www.w3.org/2002/07/owl#NamedIndividual"/>
</rdf:Description>

<rdf:Description rdf:about="http://resource.geosciml.org/classifier/cgi/metamorphicgrade/0008">
	<rdf:type rdf:resource="http://www.w3.org/2002/07/owl#NamedIndividual"/>
</rdf:Description>

<rdf:Description rdf:about="http://resource.geosciml.org/classifier/cgi/metamorphicgrade/0009">
	<rdf:type rdf:resource="http://www.w3.org/2002/07/owl#NamedIndividual"/>
</rdf:Description>

<rdf:Description rdf:about="http://resource.geosciml.org/classifier/cgi/metamorphicgrade/high_metamorphic_grade">
	<rdf:type rdf:resource="http://www.w3.org/2004/02/skos/core#Concept"/>
	<dc:creator xml:lang="en">Concept Definition Task Group of IUGS CGI Interoperability Working Group (http://www.cgi-iugs.org/tech_collaboration/interoperability_working_group.html)</dc:creator>
	<dc:source>Smulikowski et al, 2003; Fry, 1984</dc:source>
	<skos:broader rdf:resource="http://resource.geosciml.org/classifier/cgi/metamorphicgrade/metamorphosed_grade_not_specified"/>
	<skos:definition xml:lang="en">Protolith structures almost always obliterated, evidence of partial melting common. Includes rocks metamorphosed in high-temperature amphibolite, pyroxene hornfels, and medium to high-temperature eclogite facies. Mineral assemblages according to Fry (1984) Table 10-1: ultramafic-olivine, anthophyllite, cummingtonite, enstatite; mafic-hornblende, (diopside, garnet); calc-aluminous basic-plagioclase; pelite, semi-pelite -- K-feldspar, biotite, quartz, Al-minerals (garnet), migmatite.</skos:definition>
	<skos:exactMatch rdf:resource="http://resource.geosciml.org/classifier/cgi/metamorphicgrade/0001"/>
	<skos:inScheme rdf:resource="http://resource.geosciml.org/classifierscheme/cgi/201211/metamorphicgrade"/>
	<skos:prefLabel xml:lang="en">high metamorphic grade</skos:prefLabel>
</rdf:Description>

<rdf:Description rdf:about="http://resource.geosciml.org/classifier/cgi/metamorphicgrade/low_metamorphic_grade">
	<rdf:type rdf:resource="http://www.w3.org/2004/02/skos/core#Concept"/>
	<dc:creator xml:lang="en">Concept Definition Task Group of IUGS CGI Interoperability Working Group (http://www.cgi-iugs.org/tech_collaboration/interoperability_working_group.html)</dc:creator>
	<dc:source>Smulikowski et al, 2003; Fry, 1984</dc:source>
	<skos:broader rdf:resource="http://resource.geosciml.org/classifier/cgi/metamorphicgrade/metamorphosed_grade_not_specified"/>
	<skos:definition xml:lang="en">Metamorphic effects clearly visible, protolith structures typically still observable, includes rocks metamorphosed in greenschist, high-temperature blueschist, very low temperature eclogite facies. Mineral assemblages according to Fry (1984) Table 10-1: ultramafic-serpentine (talc, magnesite); mafic-chlorite, actinolite (garnet); calc-aluminous basic-albite, epidote; pelite, semi-pelite -- white mica, chlorite, quartz, biotite (garnet, Al-minerals).</skos:definition>
	<skos:exactMatch rdf:resource="http://resource.geosciml.org/classifier/cgi/metamorphicgrade/0002"/>
	<skos:inScheme rdf:resource="http://resource.geosciml.org/classifierscheme/cgi/201211/metamorphicgrade"/>
	<skos:prefLabel xml:lang="en">low metamorphic grade</skos:prefLabel>
</rdf:Description>

<rdf:Description rdf:about="http://resource.geosciml.org/classifier/cgi/metamorphicgrade/medium_metamorphic_grade">
	<rdf:type rdf:resource="http://www.w3.org/2004/02/skos/core#Concept"/>
	<dc:creator xml:lang="en">Concept Definition Task Group of IUGS CGI Interoperability Working Group (http://www.cgi-iugs.org/tech_collaboration/interoperability_working_group.html)</dc:creator>
	<dc:source>Smulikowski et al, 2003; Fry, 1984</dc:source>
	<skos:broader rdf:resource="http://resource.geosciml.org/classifier/cgi/metamorphicgrade/metamorphosed_grade_not_specified"/>
	<skos:definition xml:lang="en">Protolith structure typically obliterated. Includes rocks metamorphosed in high-temperature epidote-amphibolite, low-temperature amphibolite, and low temperature eclogite facies. Mineral assemblages according to Fry (1984) Table 10-1: ultramafic-olivine, talc (magnesite, anthophyllite); mafic-hornblende, (diopside, garnet); calc-aluminous basic-plagioclase; pelite, semi-pelite -- white mica, biotite, quartz (garnet, Al-minerals).</skos:definition>
	<skos:exactMatch rdf:resource="http://resource.geosciml.org/classifier/cgi/metamorphicgrade/0003"/>
	<skos:inScheme rdf:resource="http://resource.geosciml.org/classifierscheme/cgi/201211/metamorphicgrade"/>
	<skos:prefLabel xml:lang="en">medium metamorphic grade</skos:prefLabel>
</rdf:Description>

<rdf:Description rdf:about="http://resource.geosciml.org/classifier/cgi/metamorphicgrade/metamorphic_grade_not_specified">
	<rdf:type rdf:resource="http://www.w3.org/2004/02/skos/core#Concept"/>
	<dc:creator xml:lang="en">Concept Definition Task Group of IUGS CGI Interoperability Working Group (http://www.cgi-iugs.org/tech_collaboration/interoperability_working_group.html)</dc:creator>
	<dc:source>This Vocabulary</dc:source>
	<skos:definition xml:lang="en">for use in normative descriptions to explicitly indicate that any metamorphic condition is allowed (including non-metamorphosed).</skos:definition>
	<skos:exactMatch rdf:resource="http://resource.geosciml.org/classifier/cgi/metamorphicgrade/0004"/>
	<skos:inScheme rdf:resource="http://resource.geosciml.org/classifierscheme/cgi/201211/metamorphicgrade"/>
	<skos:narrower rdf:resource="http://resource.geosciml.org/classifier/cgi/metamorphicgrade/metamorphosed_grade_not_specified"/>
	<skos:narrower rdf:resource="http://resource.geosciml.org/classifier/cgi/metamorphicgrade/not_metamorphosed"/>
	<skos:prefLabel xml:lang="en">metamorphic grade not specified</skos:prefLabel>
	<skos:topConceptOf rdf:resource="http://resource.geosciml.org/classifierscheme/cgi/201211/metamorphicgrade"/>
</rdf:Description>

<rdf:Description rdf:about="http://resource.geosciml.org/classifier/cgi/metamorphicgrade/metamorphic_grade_unknown">
	<rdf:type rdf:resource="http://www.w3.org/2004/02/skos/core#Concept"/>
	<dc:creator xml:lang="en">Concept Definition Task Group of IUGS CGI Interoperability Working Group (http://www.cgi-iugs.org/tech_collaboration/interoperability_working_group.html)</dc:creator>
	<dc:source>This Vocabulary</dc:source>
	<skos:definition xml:lang="en">For use in instance descriptions to indicate that no information is available on metamorphic grade</skos:definition>
	<skos:exactMatch rdf:resource="http://resource.geosciml.org/classifier/cgi/metamorphicgrade/0005"/>
	<skos:inScheme rdf:resource="http://resource.geosciml.org/classifierscheme/cgi/201211/metamorphicgrade"/>
	<skos:prefLabel xml:lang="en">metamorphic grade unknown</skos:prefLabel>
	<skos:topConceptOf rdf:resource="http://resource.geosciml.org/classifierscheme/cgi/201211/metamorphicgrade"/>
</rdf:Description>

<rdf:Description rdf:about="http://resource.geosciml.org/classifier/cgi/metamorphicgrade/metamorphosed_grade_not_specified">
	<rdf:type rdf:resource="http://www.w3.org/2004/02/skos/core#Concept"/>
	<dc:creator xml:lang="en">Concept Definition Task Group of IUGS CGI Interoperability Working Group (http://www.cgi-iugs.org/tech_collaboration/interoperability_working_group.html)</dc:creator>
	<dc:source>This Vocabulary</dc:source>
	<skos:broader rdf:resource="http://resource.geosciml.org/classifier/cgi/metamorphicgrade/metamorphic_grade_not_specified"/>
	<skos:definition xml:lang="en">Rock is metamorphosed, may have any value for metamorphic grade.</skos:definition>
	<skos:exactMatch rdf:resource="http://resource.geosciml.org/classifier/cgi/metamorphicgrade/0006"/>
	<skos:inScheme rdf:resource="http://resource.geosciml.org/classifierscheme/cgi/201211/metamorphicgrade"/>
	<skos:narrower rdf:resource="http://resource.geosciml.org/classifier/cgi/metamorphicgrade/high_metamorphic_grade"/>
	<skos:narrower rdf:resource="http://resource.geosciml.org/classifier/cgi/metamorphicgrade/medium_metamorphic_grade"/>
	<skos:narrower rdf:resource="http://resource.geosciml.org/classifier/cgi/metamorphicgrade/very_high_metamorphic_grade"/>
	<skos:narrower rdf:resource="http://resource.geosciml.org/classifier/cgi/metamorphicgrade/low_metamorphic_grade"/>
	<skos:narrower rdf:resource="http://resource.geosciml.org/classifier/cgi/metamorphicgrade/very_low_metamorphic_grade"/>
	<skos:prefLabel xml:lang="en">metamorphosed grade not specified</skos:prefLabel>
</rdf:Description>

<rdf:Description rdf:about="http://resource.geosciml.org/classifier/cgi/metamorphicgrade/not_metamorphosed">
	<rdf:type rdf:resource="http://www.w3.org/2004/02/skos/core#Concept"/>
	<dc:creator xml:lang="en">Concept Definition Task Group of IUGS CGI Interoperability Working Group (http://www.cgi-iugs.org/tech_collaboration/interoperability_working_group.html)</dc:creator>
	<dc:source>This Vocabulary</dc:source>
	<skos:broader rdf:resource="http://resource.geosciml.org/classifier/cgi/metamorphicgrade/metamorphic_grade_not_specified"/>
	<skos:definition xml:lang="en">Rock or sediment not metamorphosed.</skos:definition>
	<skos:exactMatch rdf:resource="http://resource.geosciml.org/classifier/cgi/metamorphicgrade/0007"/>
	<skos:inScheme rdf:resource="http://resource.geosciml.org/classifierscheme/cgi/201211/metamorphicgrade"/>
	<skos:prefLabel xml:lang="en">not metamorphosed</skos:prefLabel>
</rdf:Description>

<rdf:Description rdf:about="http://resource.geosciml.org/classifier/cgi/metamorphicgrade/very_high_metamorphic_grade">
	<rdf:type rdf:resource="http://www.w3.org/2004/02/skos/core#Concept"/>
	<dc:creator xml:lang="en">Concept Definition Task Group of IUGS CGI Interoperability Working Group (http://www.cgi-iugs.org/tech_collaboration/interoperability_working_group.html)</dc:creator>
	<dc:source>Smulikowski et al, 2003; Fry, 1984</dc:source>
	<skos:broader rdf:resource="http://resource.geosciml.org/classifier/cgi/metamorphicgrade/metamorphosed_grade_not_specified"/>
	<skos:definition xml:lang="en">Protolith structures almost always obliterated. Includes rocks metamorphosed in granulite (or sanidinite), and high-temperature eclogite facies. Mineral assemblages according to Fry (1984) Table 10-1: ultramafic-olivine, enstatite; mafic-hypersthene, diopside (hornblende); calc-aluminous basic-plagioclase; pelite, semi-pelite -- hypersthene + Al-minerals (K-feldspar, quartz), or sapphirine.</skos:definition>
	<skos:exactMatch rdf:resource="http://resource.geosciml.org/classifier/cgi/metamorphicgrade/0008"/>
	<skos:inScheme rdf:resource="http://resource.geosciml.org/classifierscheme/cgi/201211/metamorphicgrade"/>
	<skos:prefLabel xml:lang="en">very high metamorphic grade</skos:prefLabel>
</rdf:Description>

<rdf:Description rdf:about="http://resource.geosciml.org/classifier/cgi/metamorphicgrade/very_low_metamorphic_grade">
	<rdf:type rdf:resource="http://www.w3.org/2004/02/skos/core#Concept"/>
	<dc:creator xml:lang="en">Concept Definition Task Group of IUGS CGI Interoperability Working Group (http://www.cgi-iugs.org/tech_collaboration/interoperability_working_group.html)</dc:creator>
	<dc:source>Smulikowski et al, 2003; Fry, 1984</dc:source>
	<skos:broader rdf:resource="http://resource.geosciml.org/classifier/cgi/metamorphicgrade/metamorphosed_grade_not_specified"/>
	<skos:definition xml:lang="en">Rock very slightly metamorphosed, protolith structure ubiquitous; mineral assemblage of zeolite facies, subgreenschist facies, or low temperature part of blueschist facies. Mineral assemblages according to Fry (1984) Table 10-1: ultramafic-serpentine (quartz, magnesite); mafic-clay, chlorite, relict igneous minerals; calc-aluminous basic-zeolite, pumpellite, epidote, albite; pelite, semi-pelite -- clays, chlorite, sericite, quartz.</skos:definition>
	<skos:exactMatch rdf:resource="http://resource.geosciml.org/classifier/cgi/metamorphicgrade/0009"/>
	<skos:inScheme rdf:resource="http://resource.geosciml.org/classifierscheme/cgi/201211/metamorphicgrade"/>
	<skos:prefLabel xml:lang="en">very low metamorphic grade</skos:prefLabel>
</rdf:Description>

<rdf:Description rdf:about="http://resource.geosciml.org/classifierscheme/cgi/201211/metamorphicgrade">
	<rdf:type rdf:resource="http://www.w3.org/2004/02/skos/core#ConceptScheme"/>
	<rdf:type rdf:resource="http://www.w3.org/2002/07/owl#Ontology"/>
	<dc:creator xml:lang="en">Concept Definition Task Group of IUGS CGI Interoperability Working Group (http://www.cgi-iugs.org/tech_collaboration/interoperability_working_group.html)</dc:creator>
	<dc:format>application/rdf+xml</dc:format>
	<dc:identifier>http://resource.geosciml.org/classifierscheme/cgi/201211/metamorphicgrade</dc:identifier>
	<dc:language>en</dc:language>
	<dc:publisher xml:lang="en">Concept Definition Task Group of IUGS CGI Interoperability Working Group (http://www.cgi-iugs.org/tech_collaboration/interoperability_working_group.html)</dc:publisher>
	<dc:title xml:lang="en">CGI Metamorphic Grade Categories</dc:title>
	<owl:imports rdf:resource="http://www.w3.org/2004/02/skos/core"/>
	<owl:imports rdf:resource="http://rdfs.org/ns/void"/>
	<owl:versionInfo>201211</owl:versionInfo>
	<skos:definition xml:lang="en">This file contains the CGI Metamorphic Grade vocabulary. Vocabulary for populating Metamorphic grade property in GeoSciML metamorphicDescription elements. Derived from Fettes and Desmons, 2007</skos:definition>
	<skos:historyNote xml:lang="en">2012-02-27 SMR add skos:exactMatch triples relating URI in this vocabulary to URI with number tokens in 201012 vocabulary</skos:historyNote>
	<skos:historyNote xml:lang="en">2010-02-11 Add narrower relationship links by adding skos:narrower link in Protege, defining skos:narrower as inverse of skos:broader, calculating with Pellet reasoner to add inferred axioms, and using 'file/Export inferred axioms as ontology' in Protege.</skos:historyNote>
	<skos:historyNote xml:lang="en">2012-02-07 SMR update URI to replace numeric final token with English-language string as in original URN scheme.</skos:historyNote>
	<skos:historyNote xml:lang="en">2012-11-24 SMR Update to 201211 version; add collection entity, check all pref labels are lower case, remove owl:NamedIndividual and Owl:Thing rdf:types.</skos:historyNote>
	<skos:historyNote xml:lang="en">2010-11-28 SMR replace URN identifiers with http URI identifiers according to CGI URI scheme (see https://www.seegrid.csiro.au/wiki/bin/view/CGIModel/PersistentIdentifiersInGeoSciMLServices)</skos:historyNote>
	<skos:prefLabel xml:lang="en">CGI Metamorphic Grade Categories</skos:prefLabel>
</rdf:Description>

<rdf:Description rdf:about="http://resource.geosciml.org/vocabulary/cgi/201211/metamorphicgrade">
	<rdf:type rdf:resource="http://rdfs.org/ns/void#Dataset"/>
	<rdfs:label rdf:datatype="http://www.w3.org/2001/XMLSchema#string">Metamorphic grade vocabulary</rdfs:label>
</rdf:Description>

</rdf:RDF>