<?xml version="1.0" encoding="UTF-8"?>
<rdf:RDF
	xmlns="http://resource.geosciml.org/classifierscheme/cgi/201211/particleshape#"
	xmlns:cgi="http://resource.geosciml.org/classifierscheme/cgi/201211/"
	xmlns:dc="http://purl.org/dc/elements/1.1/"
	xmlns:owl="http://www.w3.org/2002/07/owl#"
	xmlns:owl2xml="http://www.w3.org/2006/12/owl2-xml#"
	xmlns:partshp="http://resource.geosciml.org/classifier/cgi/particleshape/"
	xmlns:rdf="http://www.w3.org/1999/02/22-rdf-syntax-ns#"
	xmlns:rdfs="http://www.w3.org/2000/01/rdf-schema#"
	xmlns:skos="http://www.w3.org/2004/02/skos/core#"
	xmlns:void="http://rdfs.org/ns/void#"
	xmlns:xsd="http://www.w3.org/2001/XMLSchema#">

<rdf:Description rdf:about="http://resource.geosciml.org/classifier/cgi/particleshape/">
	<rdf:type rdf:resource="http://www.w3.org/2004/02/skos/core#Collection"/>
	<rdfs:label xml:lang="en">particle shape concepts</rdfs:label>
	<skos:member rdf:resource="http://resource.geosciml.org/classifier/cgi/particleshape/shape_not_specified"/>
	<skos:member rdf:resource="http://resource.geosciml.org/classifier/cgi/particleshape/subhedral"/>
	<skos:member rdf:resource="http://resource.geosciml.org/classifier/cgi/particleshape/sub_rounded"/>
	<skos:member rdf:resource="http://resource.geosciml.org/classifier/cgi/particleshape/euhedral"/>
	<skos:member rdf:resource="http://resource.geosciml.org/classifier/cgi/particleshape/rounded"/>
	<skos:member rdf:resource="http://resource.geosciml.org/classifier/cgi/particleshape/angular"/>
	<skos:member rdf:resource="http://resource.geosciml.org/classifier/cgi/particleshape/anhedral"/>
	<skos:member rdf:resource="http://resource.geosciml.org/classifier/cgi/particleshape/resorbed"/>
	<skos:member rdf:resource="http://resource.geosciml.org/classifier/cgi/particleshape/well_rounded"/>
	<skos:member rdf:resource="http://resource.geosciml.org/classifier/cgi/particleshape/very_angular"/>
	<skos:member rdf:resource="http://resource.geosciml.org/classifier/cgi/particleshape/diffuse"/>
	<skos:member rdf:resource="http://resource.geosciml.org/classifier/cgi/particleshape/sub_angular"/>
	<skos:prefLabel xml:lang="en">CGI Particle Shape Concepts</skos:prefLabel>
</rdf:Description>

<rdf:Description rdf:about="http://resource.geosciml.org/classifier/cgi/particleshape/0001">
	<rdf:type rdf:resource="http://www.w3.org/2002/07/owl#NamedIndividual"/>
</rdf:Description>

<rdf:Description rdf:about="http://resource.geosciml.org/classifier/cgi/particleshape/0002">
	<rdf:type rdf:resource="http://www.w3.org/2002/07/owl#NamedIndividual"/>
</rdf:Description>

<rdf:Description rdf:about="http://resource.geosciml.org/classifier/cgi/particleshape/0003">
	<rdf:type rdf:resource="http://www.w3.org/2002/07/owl#NamedIndividual"/>
</rdf:Description>

<rdf:Description rdf:about="http://resource.geosciml.org/classifier/cgi/particleshape/0004">
	<rdf:type rdf:resource="http://www.w3.org/2002/07/owl#NamedIndividual"/>
</rdf:Description>

<rdf:Description rdf:about="http://resource.geosciml.org/classifier/cgi/particleshape/0005">
	<rdf:type rdf:resource="http://www.w3.org/2002/07/owl#NamedIndividual"/>
</rdf:Description>

<rdf:Description rdf:about="http://resource.geosciml.org/classifier/cgi/particleshape/0006">
	<rdf:type rdf:resource="http://www.w3.org/2002/07/owl#NamedIndividual"/>
</rdf:Description>

<rdf:Description rdf:about="http://resource.geosciml.org/classifier/cgi/particleshape/0007">
	<rdf:type rdf:resource="http://www.w3.org/2002/07/owl#NamedIndividual"/>
</rdf:Description>

<rdf:Description rdf:about="http://resource.geosciml.org/classifier/cgi/particleshape/0008">
	<rdf:type rdf:resource="http://www.w3.org/2002/07/owl#NamedIndividual"/>
</rdf:Description>

<rdf:Description rdf:about="http://resource.geosciml.org/classifier/cgi/particleshape/0009">
	<rdf:type rdf:resource="http://www.w3.org/2002/07/owl#NamedIndividual"/>
</rdf:Description>

<rdf:Description rdf:about="http://resource.geosciml.org/classifier/cgi/particleshape/0010">
	<rdf:type rdf:resource="http://www.w3.org/2002/07/owl#NamedIndividual"/>
</rdf:Description>

<rdf:Description rdf:about="http://resource.geosciml.org/classifier/cgi/particleshape/0011">
	<rdf:type rdf:resource="http://www.w3.org/2002/07/owl#NamedIndividual"/>
</rdf:Description>

<rdf:Description rdf:about="http://resource.geosciml.org/classifier/cgi/particleshape/0012">
	<rdf:type rdf:resource="http://www.w3.org/2002/07/owl#NamedIndividual"/>
</rdf:Description>

<rdf:Description rdf:about="http://resource.geosciml.org/classifier/cgi/particleshape/angular">
	<rdf:type rdf:resource="http://www.w3.org/2004/02/skos/core#Concept"/>
	<dc:source>Powers, M. C., 1953 A new roundness scale for sedimentary particles. Journal of Sedimentary Petrology, v. 23, p. 117-119</dc:source>
	<skos:definition xml:lang="en">A clastic sedimentary particle showing very little or no evidence of abrasion, with all of its edges and corners sharp, such as blocks with numerous (15-30) secondary corners and a roundness value between 0.17 and 0.25 (midpoint at 0.21).</skos:definition>
	<skos:exactMatch rdf:resource="http://resource.geosciml.org/classifier/cgi/particleshape/0001"/>
	<skos:inScheme rdf:resource="http://resource.geosciml.org/classifierscheme/cgi/201211/particleshape"/>
	<skos:prefLabel xml:lang="en">angular</skos:prefLabel>
</rdf:Description>

<rdf:Description rdf:about="http://resource.geosciml.org/classifier/cgi/particleshape/anhedral">
	<rdf:type rdf:resource="http://www.w3.org/2004/02/skos/core#Concept"/>
	<dc:source>MacKenzie, W.S., Donaldson, C.H. &amp; Guilford, C., 1982. Atlas of igneous rocks and their textures. John Wiley &amp; Sons, New York</dc:source>
	<skos:definition xml:lang="en">Crystalline particles in a rock lack well-developed crystal faces; usually referring to igneous or metamorphic grains</skos:definition>
	<skos:exactMatch rdf:resource="http://resource.geosciml.org/classifier/cgi/particleshape/0002"/>
	<skos:inScheme rdf:resource="http://resource.geosciml.org/classifierscheme/cgi/201211/particleshape"/>
	<skos:prefLabel xml:lang="en">anhedral</skos:prefLabel>
</rdf:Description>

<rdf:Description rdf:about="http://resource.geosciml.org/classifier/cgi/particleshape/diffuse">
	<rdf:type rdf:resource="http://www.w3.org/2004/02/skos/core#Concept"/>
	<dc:source xml:lang="en">SLTTs 2004</dc:source>
	<skos:definition xml:lang="en">Particles in aggregate have diffuse, ill-defined boundaries</skos:definition>
	<skos:exactMatch rdf:resource="http://resource.geosciml.org/classifier/cgi/particleshape/0003"/>
	<skos:inScheme rdf:resource="http://resource.geosciml.org/classifierscheme/cgi/201211/particleshape"/>
	<skos:prefLabel xml:lang="en">diffuse</skos:prefLabel>
</rdf:Description>

<rdf:Description rdf:about="http://resource.geosciml.org/classifier/cgi/particleshape/euhedral">
	<rdf:type rdf:resource="http://www.w3.org/2004/02/skos/core#Concept"/>
	<dc:source>MacKenzie, W.S., Donaldson, C.H. &amp; Guilford, C., 1982. Atlas of igneous rocks and their textures. John Wiley &amp; Sons, New York</dc:source>
	<skos:definition xml:lang="en">Crystalline particles in a rock are mostly bounded by perfect crystal faces; usually referring to igneous or metamorphoc grains</skos:definition>
	<skos:exactMatch rdf:resource="http://resource.geosciml.org/classifier/cgi/particleshape/0004"/>
	<skos:inScheme rdf:resource="http://resource.geosciml.org/classifierscheme/cgi/201211/particleshape"/>
	<skos:prefLabel xml:lang="en">euhedral</skos:prefLabel>
</rdf:Description>

<rdf:Description rdf:about="http://resource.geosciml.org/classifier/cgi/particleshape/resorbed">
	<rdf:type rdf:resource="http://www.w3.org/2004/02/skos/core#Concept"/>
	<dc:source>Neuendorf, K.K.E, Mehl, J.P. &amp; Jackson, J.A. (eds), 2005. Glossary of geology, 5th Edition. American Geological Institute, Alexandria, 779 p.</dc:source>
	<skos:definition xml:lang="en">Particles have with smooth, embayed boundaries caused by resorption by the host magma</skos:definition>
	<skos:exactMatch rdf:resource="http://resource.geosciml.org/classifier/cgi/particleshape/0005"/>
	<skos:inScheme rdf:resource="http://resource.geosciml.org/classifierscheme/cgi/201211/particleshape"/>
	<skos:prefLabel xml:lang="en">resorbed</skos:prefLabel>
</rdf:Description>

<rdf:Description rdf:about="http://resource.geosciml.org/classifier/cgi/particleshape/rounded">
	<rdf:type rdf:resource="http://www.w3.org/2004/02/skos/core#Concept"/>
	<dc:source>Powers, M. C., 1953 A new roundness scale for sedimentary particles. Journal of Sedimentary Petrology, v. 23, p. 117-119</dc:source>
	<skos:definition xml:lang="en">A clastic sedimentary particle whose original edges and corners have been smoothed off to rather broad curves and whose original faces are almost completely removed by abrasion (although some comparatively flat surfaces may be present), such as a pebble with a roundness value between 0.49 and 0.70 (midpoint at 0.59) and few (0-5) and greatly subdued secondary corners. The original shape is still readily apparent.</skos:definition>
	<skos:exactMatch rdf:resource="http://resource.geosciml.org/classifier/cgi/particleshape/0006"/>
	<skos:inScheme rdf:resource="http://resource.geosciml.org/classifierscheme/cgi/201211/particleshape"/>
	<skos:prefLabel xml:lang="en">rounded</skos:prefLabel>
</rdf:Description>

<rdf:Description rdf:about="http://resource.geosciml.org/classifier/cgi/particleshape/shape_not_specified">
	<rdf:type rdf:resource="http://www.w3.org/2004/02/skos/core#Concept"/>
	<dc:source xml:lang="en">this vocabulary</dc:source>
	<skos:definition xml:lang="en">Shape property may have any value. Use in normative definitions where shape may take any value.</skos:definition>
	<skos:exactMatch rdf:resource="http://resource.geosciml.org/classifier/cgi/particleshape/0007"/>
	<skos:inScheme rdf:resource="http://resource.geosciml.org/classifierscheme/cgi/201211/particleshape"/>
	<skos:prefLabel xml:lang="en">any shape</skos:prefLabel>
</rdf:Description>

<rdf:Description rdf:about="http://resource.geosciml.org/classifier/cgi/particleshape/sub_angular">
	<rdf:type rdf:resource="http://www.w3.org/2004/02/skos/core#Concept"/>
	<dc:source>Powers, M. C., 1953 A new roundness scale for sedimentary particles. Journal of Sedimentary Petrology, v. 23, p. 117-119</dc:source>
	<skos:definition xml:lang="en">A clastic sedimentary particle showing definite effects of slight abrasion, retaining its original general form, and having faces that are virtually untouched and edges and corners that are rounded off to some extent, such as a glacial boulder with numerous (10-20) secondary corners and a roundness value between 0.25 and 0.35 (midpoint at 0.300).</skos:definition>
	<skos:exactMatch rdf:resource="http://resource.geosciml.org/classifier/cgi/particleshape/0008"/>
	<skos:inScheme rdf:resource="http://resource.geosciml.org/classifierscheme/cgi/201211/particleshape"/>
	<skos:prefLabel xml:lang="en">sub angular</skos:prefLabel>
</rdf:Description>

<rdf:Description rdf:about="http://resource.geosciml.org/classifier/cgi/particleshape/sub_rounded">
	<rdf:type rdf:resource="http://www.w3.org/2004/02/skos/core#Concept"/>
	<dc:source>Powers, M. C., 1953 A new roundness scale for sedimentary particles. Journal of Sedimentary Petrology, v. 23, p. 117-119</dc:source>
	<skos:definition xml:lang="en">A clastic sedimentary particle showing considerable but incomplete abrasion and an original general form that is still discernible, and having many of its edges and corners noticeably rounded off to smooth curves, such as a cobble with a reduced number (5-10) of secondary corners, a considerably reduced area of the original faces, and a roundness value between 0.35 and 0.49 (midpoint at 0.41).</skos:definition>
	<skos:exactMatch rdf:resource="http://resource.geosciml.org/classifier/cgi/particleshape/0009"/>
	<skos:inScheme rdf:resource="http://resource.geosciml.org/classifierscheme/cgi/201211/particleshape"/>
	<skos:prefLabel xml:lang="en">sub rounded</skos:prefLabel>
</rdf:Description>

<rdf:Description rdf:about="http://resource.geosciml.org/classifier/cgi/particleshape/subhedral">
	<rdf:type rdf:resource="http://www.w3.org/2004/02/skos/core#Concept"/>
	<dc:source>MacKenzie, W.S., Donaldson, C.H. &amp; Guilford, C., 1982. Atlas of igneous rocks and their textures. John Wiley &amp; Sons, New York</dc:source>
	<skos:definition xml:lang="en">Crystalline particles in a rock are partly bounded by crystal faces; usually referring to igneous or metamorphic grains</skos:definition>
	<skos:exactMatch rdf:resource="http://resource.geosciml.org/classifier/cgi/particleshape/0010"/>
	<skos:inScheme rdf:resource="http://resource.geosciml.org/classifierscheme/cgi/201211/particleshape"/>
	<skos:prefLabel xml:lang="en">subhedral</skos:prefLabel>
</rdf:Description>

<rdf:Description rdf:about="http://resource.geosciml.org/classifier/cgi/particleshape/very_angular">
	<rdf:type rdf:resource="http://www.w3.org/2004/02/skos/core#Concept"/>
	<dc:source>Powers, M. C., 1953 A new roundness scale for sedimentary particles. Journal of Sedimentary Petrology, v. 23, p. 117-119</dc:source>
	<skos:definition xml:lang="en">A clastic sedimentary particle with a roundness value between 0.12 and 0.17 (midpoint at 0.14).</skos:definition>
	<skos:exactMatch rdf:resource="http://resource.geosciml.org/classifier/cgi/particleshape/0011"/>
	<skos:inScheme rdf:resource="http://resource.geosciml.org/classifierscheme/cgi/201211/particleshape"/>
	<skos:prefLabel xml:lang="en">very angular</skos:prefLabel>
</rdf:Description>

<rdf:Description rdf:about="http://resource.geosciml.org/classifier/cgi/particleshape/well_rounded">
	<rdf:type rdf:resource="http://www.w3.org/2004/02/skos/core#Concept"/>
	<dc:source>Powers, M. C., 1953 A new roundness scale for sedimentary particles. Journal of Sedimentary Petrology, v. 23, p. 117-119</dc:source>
	<skos:definition xml:lang="en">A clastic sedimentary particle whose original faces, edges, and corners have been destroyed by abrasion and whose entire surface consists of broad curves without any flat areas; specif. said of a particle with no secondary corners and a roundness value between 0.70 and 1.00 (midpoint at 0.84). The original shape may be suggested by the present form of the particle.</skos:definition>
	<skos:exactMatch rdf:resource="http://resource.geosciml.org/classifier/cgi/particleshape/0012"/>
	<skos:inScheme rdf:resource="http://resource.geosciml.org/classifierscheme/cgi/201211/particleshape"/>
	<skos:prefLabel xml:lang="en">well rounded</skos:prefLabel>
</rdf:Description>

<rdf:Description rdf:about="http://resource.geosciml.org/classifierscheme/cgi/201211/particleshape">
	<rdf:type rdf:resource="http://www.w3.org/2002/07/owl#Ontology"/>
	<rdf:type rdf:resource="http://www.w3.org/2004/02/skos/core#ConceptScheme"/>
	<dc:creator>Concept Definition Task Group of IUGS CGI Interoperability Working Group (http://www.cgi-iugs.org/tech_collaboration/interoperability_working_group.html)</dc:creator>
	<dc:format rdf:datatype="http://www.w3.org/2001/XMLSchema#string">application/rdf+xml</dc:format>
	<dc:identifier>http://resource.geosciml.org/classifierscheme/cgi/201211/particleshape</dc:identifier>
	<dc:language>en</dc:language>
	<dc:publisher>Concept Definition Task Group of IUGS CGI Interoperability Working Group (http://www.cgi-iugs.org/tech_collaboration/interoperability_working_group.html)</dc:publisher>
	<dc:title xml:lang="en">CGI Particle Shape Term Vocabulary</dc:title>
	<owl:imports rdf:resource="http://rdfs.org/ns/void"/>
	<owl:imports rdf:resource="http://www.w3.org/2004/02/skos/core"/>
	<owl:versionInfo>201211</owl:versionInfo>
	<skos:changeNote xml:lang="en">2009-12-07 SMR Update metadata properties for version, creator, title, and format.  Change skos:HistoryNote to dc:source for information on origin of terms and definitions.</skos:changeNote>
	<skos:definition xml:lang="en">This file contains the CGI Particle Shape vocabulary. The Shape attribute describes, a) the development of crystal faces bounding particles in crystalline compond materials, and b) surface rounding of grains in sedimentary rocks. Roundness is a measure of the sharpness of the edges between surfaces bounding a particle (see Jackson, 1997; Wadell, 1932) and is an indication of the degree of abrasion of a clastic particle. Expressed by Wadell (1932) as the ratio of the average radius of curvature of the several edges or corners of the particle to the radius of curvature of the maximum inscribed sphere (or to one-half the nominal diameter of the particle). The value is more conveniently computed from a plane figure (a projection or cross section); thus, roundness may be defined as the ratio of the average radius of curvature of the corners of the particle image to the radius of the maximum inscribed circle. A perfectly rounded particle (such as a sphere) has a roundness value of 1.0; less-rounded particles have values less than 1.0. The corresponding concept in aggregates with crystalline as opposed to clastic grains is here referred to as crystallinity, and is the degree to which a mineral grain is bounded by crystal faces. Terms should be appropriate for the kind of compound material (eg: for crystalline rocks- euhedral, ideoblastic, subhedral, anhedral, xenoblastic; for sedimentary rocks - angular, rounded)</skos:definition>
	<skos:historyNote xml:lang="en">2012-11-24 SMR Update to 201211 version; add collection entity, check all pref labels are lower case, remove owl:NamedIndividual and Owl:Thing rdf:types.</skos:historyNote>
	<skos:historyNote xml:lang="en">2009-07-14. Generate SKOS encoding of vocabulary from Excel spreadsheet.</skos:historyNote>
	<skos:historyNote xml:lang="en">2010-11-28 SMR Replace URN with htt URI identifiers according to CGI URI scheme (see https://www.seegrid.csiro.au/wiki/bin/view/CGIModel/PersistentIdentifiersInGeoSciMLServices)</skos:historyNote>
	<skos:historyNote xml:lang="en">2012-02-07 SMR update URI to replace numeric final token with English-language string as in original URN scheme.</skos:historyNote>
	<skos:historyNote xml:lang="en">2012-02-27 SMR add skos:exactMatch triples to map URIs for concepts in this vocabulary to number-token URIs in 201012 version of same concepts.</skos:historyNote>
	<skos:prefLabel xml:lang="en">CGI Particle Shape Term Vocabulary</skos:prefLabel>
</rdf:Description>

<rdf:Description rdf:about="http://resource.geosciml.org/vocabulary/cgi/201211/particleshape">
	<rdf:type rdf:resource="http://rdfs.org/ns/void#Dataset"/>
	<rdfs:label rdf:datatype="http://www.w3.org/2001/XMLSchema#string">Particle shape vocabulary</rdfs:label>
</rdf:Description>

<rdf:Description rdf:about="http://www.w3.org/2004/02/skos/core#ConceptScheme">
	<rdf:type rdf:resource="http://www.w3.org/2002/07/owl#Class"/>
</rdf:Description>

</rdf:RDF>