<?xml version="1.0" encoding="UTF-8"?>
<rdf:RDF
	xmlns:cgi="http://resource.geosciml.org/classifierscheme/cgi/201211/"
	xmlns:dc="http://purl.org/dc/elements/1.1/"
	xmlns:owl="http://www.w3.org/2002/07/owl#"
	xmlns:owl2xml="http://www.w3.org/2006/12/owl2-xml#"
	xmlns:partaspectrat2="http://resource.geosciml.org/classifier/cgi/particleaspectratio/"
	xmlns:partasprat="http://resource.geosciml.org/classifierscheme/cgi/201211/particleaspectratio#"
	xmlns:rdf="http://www.w3.org/1999/02/22-rdf-syntax-ns#"
	xmlns:rdfs="http://www.w3.org/2000/01/rdf-schema#"
	xmlns:skos="http://www.w3.org/2004/02/skos/core#"
	xmlns:void="http://rdfs.org/ns/void#"
	xmlns:xsd="http://www.w3.org/2001/XMLSchema#">

<rdf:Description rdf:about="http://resource.geosciml.org/classifier/cgi/particleaspectratio/">
	<rdf:type rdf:resource="http://www.w3.org/2004/02/skos/core#Collection"/>
	<rdfs:label xml:lang="en">particle aspect ratio concepts</rdfs:label>
	<skos:definition xml:lang="en">This resource defines the concept space for particle aspect ratio concepts by extension; it includes all concepts in this conceptScheme, as well as concepts in previous versions of the scheme.</skos:definition>
	<skos:member rdf:resource="http://resource.geosciml.org/classifier/cgi/particleaspectratio/bladed"/>
	<skos:member rdf:resource="http://resource.geosciml.org/classifier/cgi/particleaspectratio/strongly_prolate"/>
	<skos:member rdf:resource="http://resource.geosciml.org/classifier/cgi/particleaspectratio/slightly_flattened"/>
	<skos:member rdf:resource="http://resource.geosciml.org/classifier/cgi/particleaspectratio/any_form"/>
	<skos:member rdf:resource="http://resource.geosciml.org/classifier/cgi/particleaspectratio/prolate"/>
	<skos:member rdf:resource="http://resource.geosciml.org/classifier/cgi/particleaspectratio/equant"/>
	<skos:member rdf:resource="http://resource.geosciml.org/classifier/cgi/particleaspectratio/oblate"/>
	<skos:member rdf:resource="http://resource.geosciml.org/classifier/cgi/particleaspectratio/bladed_medium"/>
	<skos:member rdf:resource="http://resource.geosciml.org/classifier/cgi/particleaspectratio/compact_bladed"/>
	<skos:member rdf:resource="http://resource.geosciml.org/classifier/cgi/particleaspectratio/form_not_specified"/>
	<skos:member rdf:resource="http://resource.geosciml.org/classifier/cgi/particleaspectratio/slightly_prolate"/>
	<skos:member rdf:resource="http://resource.geosciml.org/classifier/cgi/particleaspectratio/oblate_medium"/>
	<skos:member rdf:resource="http://resource.geosciml.org/classifier/cgi/particleaspectratio/strongly_flattened"/>
	<skos:member rdf:resource="http://resource.geosciml.org/classifier/cgi/particleaspectratio/prolate_medium"/>
	<skos:member rdf:resource="http://resource.geosciml.org/classifier/cgi/particleaspectratio/very_bladed"/>
	<skos:member rdf:resource="http://resource.geosciml.org/classifier/cgi/particleaspectratio/fibrous"/>
	<skos:member rdf:resource="http://resource.geosciml.org/classifier/cgi/particleaspectratio/particle_geometry_uncertain"/>
	<skos:prefLabel xml:lang="en">CGI Particle Aspect Ratio</skos:prefLabel>
</rdf:Description>

<rdf:Description rdf:about="http://resource.geosciml.org/classifier/cgi/particleaspectratio/0001">
	<rdf:type rdf:resource="http://www.w3.org/2002/07/owl#NamedIndividual"/>
</rdf:Description>

<rdf:Description rdf:about="http://resource.geosciml.org/classifier/cgi/particleaspectratio/0002">
	<rdf:type rdf:resource="http://www.w3.org/2002/07/owl#NamedIndividual"/>
</rdf:Description>

<rdf:Description rdf:about="http://resource.geosciml.org/classifier/cgi/particleaspectratio/0003">
	<rdf:type rdf:resource="http://www.w3.org/2002/07/owl#NamedIndividual"/>
</rdf:Description>

<rdf:Description rdf:about="http://resource.geosciml.org/classifier/cgi/particleaspectratio/0004">
	<rdf:type rdf:resource="http://www.w3.org/2002/07/owl#NamedIndividual"/>
</rdf:Description>

<rdf:Description rdf:about="http://resource.geosciml.org/classifier/cgi/particleaspectratio/0005">
	<rdf:type rdf:resource="http://www.w3.org/2002/07/owl#NamedIndividual"/>
</rdf:Description>

<rdf:Description rdf:about="http://resource.geosciml.org/classifier/cgi/particleaspectratio/0006">
	<rdf:type rdf:resource="http://www.w3.org/2002/07/owl#NamedIndividual"/>
</rdf:Description>

<rdf:Description rdf:about="http://resource.geosciml.org/classifier/cgi/particleaspectratio/0007">
	<rdf:type rdf:resource="http://www.w3.org/2002/07/owl#NamedIndividual"/>
</rdf:Description>

<rdf:Description rdf:about="http://resource.geosciml.org/classifier/cgi/particleaspectratio/0008">
	<rdf:type rdf:resource="http://www.w3.org/2002/07/owl#NamedIndividual"/>
</rdf:Description>

<rdf:Description rdf:about="http://resource.geosciml.org/classifier/cgi/particleaspectratio/0009">
	<rdf:type rdf:resource="http://www.w3.org/2002/07/owl#NamedIndividual"/>
</rdf:Description>

<rdf:Description rdf:about="http://resource.geosciml.org/classifier/cgi/particleaspectratio/0010">
	<rdf:type rdf:resource="http://www.w3.org/2002/07/owl#NamedIndividual"/>
</rdf:Description>

<rdf:Description rdf:about="http://resource.geosciml.org/classifier/cgi/particleaspectratio/0011">
	<rdf:type rdf:resource="http://www.w3.org/2002/07/owl#NamedIndividual"/>
</rdf:Description>

<rdf:Description rdf:about="http://resource.geosciml.org/classifier/cgi/particleaspectratio/0012">
	<rdf:type rdf:resource="http://www.w3.org/2002/07/owl#NamedIndividual"/>
</rdf:Description>

<rdf:Description rdf:about="http://resource.geosciml.org/classifier/cgi/particleaspectratio/0013">
	<rdf:type rdf:resource="http://www.w3.org/2002/07/owl#NamedIndividual"/>
</rdf:Description>

<rdf:Description rdf:about="http://resource.geosciml.org/classifier/cgi/particleaspectratio/0014">
	<rdf:type rdf:resource="http://www.w3.org/2002/07/owl#NamedIndividual"/>
</rdf:Description>

<rdf:Description rdf:about="http://resource.geosciml.org/classifier/cgi/particleaspectratio/0015">
	<rdf:type rdf:resource="http://www.w3.org/2002/07/owl#NamedIndividual"/>
</rdf:Description>

<rdf:Description rdf:about="http://resource.geosciml.org/classifier/cgi/particleaspectratio/0016">
	<rdf:type rdf:resource="http://www.w3.org/2002/07/owl#NamedIndividual"/>
</rdf:Description>

<rdf:Description rdf:about="http://resource.geosciml.org/classifier/cgi/particleaspectratio/0017">
	<rdf:type rdf:resource="http://www.w3.org/2002/07/owl#NamedIndividual"/>
</rdf:Description>

<rdf:Description rdf:about="http://resource.geosciml.org/classifier/cgi/particleaspectratio/any_form">
	<rdf:type rdf:resource="http://www.w3.org/2004/02/skos/core#Concept"/>
	<skos:broader rdf:resource="http://resource.geosciml.org/classifier/cgi/particleaspectratio/form_not_specified"/>
	<skos:definition xml:lang="en">Particle has some form, but it is not specified.</skos:definition>
	<skos:exactMatch rdf:resource="http://resource.geosciml.org/classifier/cgi/particleaspectratio/0017"/>
	<skos:inScheme rdf:resource="http://resource.geosciml.org/classifierscheme/cgi/201211/particleaspectratio"/>
	<skos:narrower rdf:resource="http://resource.geosciml.org/classifier/cgi/particleaspectratio/prolate"/>
	<skos:narrower rdf:resource="http://resource.geosciml.org/classifier/cgi/particleaspectratio/oblate"/>
	<skos:narrower rdf:resource="http://resource.geosciml.org/classifier/cgi/particleaspectratio/bladed"/>
	<skos:narrower rdf:resource="http://resource.geosciml.org/classifier/cgi/particleaspectratio/equant"/>
	<skos:prefLabel xml:lang="en">any form</skos:prefLabel>
</rdf:Description>

<rdf:Description rdf:about="http://resource.geosciml.org/classifier/cgi/particleaspectratio/bladed">
	<rdf:type rdf:resource="http://www.w3.org/2004/02/skos/core#Concept"/>
	<dc:source>Sneed and Folk, 1958; Pettijohn et al., 1972; NADM SLTTs, 2004</dc:source>
	<skos:broader rdf:resource="http://resource.geosciml.org/classifier/cgi/particleaspectratio/any_form"/>
	<skos:definition xml:lang="en">Bladed group in Sneed&amp;Folk, (1958); S/L is less than 0.7 and (L-I)/(L-S) is between 0.33 and 0.66.</skos:definition>
	<skos:exactMatch rdf:resource="http://resource.geosciml.org/classifier/cgi/particleaspectratio/0001"/>
	<skos:inScheme rdf:resource="http://resource.geosciml.org/classifierscheme/cgi/201211/particleaspectratio"/>
	<skos:narrower rdf:resource="http://resource.geosciml.org/classifier/cgi/particleaspectratio/compact_bladed"/>
	<skos:narrower rdf:resource="http://resource.geosciml.org/classifier/cgi/particleaspectratio/bladed_medium"/>
	<skos:narrower rdf:resource="http://resource.geosciml.org/classifier/cgi/particleaspectratio/very_bladed"/>
	<skos:prefLabel xml:lang="en">bladed</skos:prefLabel>
</rdf:Description>

<rdf:Description rdf:about="http://resource.geosciml.org/classifier/cgi/particleaspectratio/bladed_medium">
	<rdf:type rdf:resource="http://www.w3.org/2004/02/skos/core#Concept"/>
	<dc:source>Sneed and Folk, 1958; Pettijohn et al., 1972; NADM SLTTs, 2004</dc:source>
	<skos:broader rdf:resource="http://resource.geosciml.org/classifier/cgi/particleaspectratio/bladed"/>
	<skos:definition xml:lang="en">S/L is between 0.3 and 0.5 and (L-I)/(L-S) is between 0.33 and 0.66 Sneed&amp;Folk, (1958).</skos:definition>
	<skos:exactMatch rdf:resource="http://resource.geosciml.org/classifier/cgi/particleaspectratio/0002"/>
	<skos:inScheme rdf:resource="http://resource.geosciml.org/classifierscheme/cgi/201211/particleaspectratio"/>
	<skos:prefLabel xml:lang="en">bladed medium</skos:prefLabel>
</rdf:Description>

<rdf:Description rdf:about="http://resource.geosciml.org/classifier/cgi/particleaspectratio/compact_bladed">
	<rdf:type rdf:resource="http://www.w3.org/2004/02/skos/core#Concept"/>
	<dc:source>Sneed and Folk, 1958; Pettijohn et al., 1972; NADM SLTTs, 2004</dc:source>
	<skos:broader rdf:resource="http://resource.geosciml.org/classifier/cgi/particleaspectratio/bladed"/>
	<skos:definition xml:lang="en">S/L is between 0.5 and 0.7 and (L-I)/(L-S) is between 0.33 and 0.66 Sneed&amp;Folk, (1958).</skos:definition>
	<skos:exactMatch rdf:resource="http://resource.geosciml.org/classifier/cgi/particleaspectratio/0003"/>
	<skos:inScheme rdf:resource="http://resource.geosciml.org/classifierscheme/cgi/201211/particleaspectratio"/>
	<skos:prefLabel xml:lang="en">compact bladed</skos:prefLabel>
</rdf:Description>

<rdf:Description rdf:about="http://resource.geosciml.org/classifier/cgi/particleaspectratio/equant">
	<rdf:type rdf:resource="http://www.w3.org/2004/02/skos/core#Concept"/>
	<dc:source>Sneed and Folk, 1958; Pettijohn et al., 1972; NADM SLTTs, 2004</dc:source>
	<skos:broader rdf:resource="http://resource.geosciml.org/classifier/cgi/particleaspectratio/any_form"/>
	<skos:definition xml:lang="en">Particles are compact in Sneed &amp; Folk (1958); ratio of S/L is greater than 0.7.</skos:definition>
	<skos:exactMatch rdf:resource="http://resource.geosciml.org/classifier/cgi/particleaspectratio/0004"/>
	<skos:inScheme rdf:resource="http://resource.geosciml.org/classifierscheme/cgi/201211/particleaspectratio"/>
	<skos:prefLabel xml:lang="en">equant</skos:prefLabel>
</rdf:Description>

<rdf:Description rdf:about="http://resource.geosciml.org/classifier/cgi/particleaspectratio/fibrous">
	<rdf:type rdf:resource="http://www.w3.org/2004/02/skos/core#Concept"/>
	<dc:source>Sneed and Folk, 1958; Pettijohn et al., 1972; NADM SLTTs, 2004</dc:source>
	<skos:broader rdf:resource="http://resource.geosciml.org/classifier/cgi/particleaspectratio/strongly_prolate"/>
	<skos:definition xml:lang="en">Particles are so elongate they are fibrous.</skos:definition>
	<skos:exactMatch rdf:resource="http://resource.geosciml.org/classifier/cgi/particleaspectratio/0005"/>
	<skos:inScheme rdf:resource="http://resource.geosciml.org/classifierscheme/cgi/201211/particleaspectratio"/>
	<skos:prefLabel>fibrous</skos:prefLabel>
</rdf:Description>

<rdf:Description rdf:about="http://resource.geosciml.org/classifier/cgi/particleaspectratio/form_not_specified">
	<rdf:type rdf:resource="http://www.w3.org/2004/02/skos/core#Concept"/>
	<dc:source xml:lang="en">this vocabulary</dc:source>
	<skos:definition xml:lang="en">Particle form may take any or no value. For use in normative descriptions.</skos:definition>
	<skos:exactMatch rdf:resource="http://resource.geosciml.org/classifier/cgi/particleaspectratio/0006"/>
	<skos:inScheme rdf:resource="http://resource.geosciml.org/classifierscheme/cgi/201211/particleaspectratio"/>
	<skos:narrower rdf:resource="http://resource.geosciml.org/classifier/cgi/particleaspectratio/particle_geometry_uncertain"/>
	<skos:narrower rdf:resource="http://resource.geosciml.org/classifier/cgi/particleaspectratio/any_form"/>
	<skos:prefLabel>form not specified</skos:prefLabel>
	<skos:topConceptOf rdf:resource="http://resource.geosciml.org/classifierscheme/cgi/201211/particleaspectratio"/>
</rdf:Description>

<rdf:Description rdf:about="http://resource.geosciml.org/classifier/cgi/particleaspectratio/oblate">
	<rdf:type rdf:resource="http://www.w3.org/2004/02/skos/core#Concept"/>
	<dc:source>Sneed and Folk, 1958; Pettijohn et al., 1972; NADM SLTTs, 2004</dc:source>
	<skos:broader rdf:resource="http://resource.geosciml.org/classifier/cgi/particleaspectratio/any_form"/>
	<skos:definition xml:lang="en">Particles are in 'platy group' in Sneed&amp;Folk, (1958); S/L is less than 0.7 and (L-I)/(L-S) is less than 0.33.</skos:definition>
	<skos:exactMatch rdf:resource="http://resource.geosciml.org/classifier/cgi/particleaspectratio/0007"/>
	<skos:inScheme rdf:resource="http://resource.geosciml.org/classifierscheme/cgi/201211/particleaspectratio"/>
	<skos:narrower rdf:resource="http://resource.geosciml.org/classifier/cgi/particleaspectratio/strongly_flattened"/>
	<skos:narrower rdf:resource="http://resource.geosciml.org/classifier/cgi/particleaspectratio/slightly_flattened"/>
	<skos:narrower rdf:resource="http://resource.geosciml.org/classifier/cgi/particleaspectratio/oblate_medium"/>
	<skos:prefLabel>oblate</skos:prefLabel>
</rdf:Description>

<rdf:Description rdf:about="http://resource.geosciml.org/classifier/cgi/particleaspectratio/oblate_medium">
	<rdf:type rdf:resource="http://www.w3.org/2004/02/skos/core#Concept"/>
	<dc:source>Sneed and Folk, 1958; Pettijohn et al., 1972; NADM SLTTs, 2004</dc:source>
	<skos:broader rdf:resource="http://resource.geosciml.org/classifier/cgi/particleaspectratio/oblate"/>
	<skos:definition xml:lang="en">Particles are 'just platy' in Sneed&amp;Folk, (1958); S/L is between 0.3 and 0.5 and (L-I)/(L-S) is less than 0.33.</skos:definition>
	<skos:exactMatch rdf:resource="http://resource.geosciml.org/classifier/cgi/particleaspectratio/0008"/>
	<skos:inScheme rdf:resource="http://resource.geosciml.org/classifierscheme/cgi/201211/particleaspectratio"/>
	<skos:notation rdf:datatype="http://resource.geosciml.org/classifierscheme/cgi/201211/particleaspectratio">oblate_medium</skos:notation>
	<skos:prefLabel>oblate medium</skos:prefLabel>
</rdf:Description>

<rdf:Description rdf:about="http://resource.geosciml.org/classifier/cgi/particleaspectratio/particle_geometry_uncertain">
	<rdf:type rdf:resource="http://www.w3.org/2004/02/skos/core#Concept"/>
	<dc:source xml:lang="en">this vocabulary</dc:source>
	<skos:broader rdf:resource="http://resource.geosciml.org/classifier/cgi/particleaspectratio/form_not_specified"/>
	<skos:definition xml:lang="en">Particle form is uncertain or not categorizable, generally obscured by overprinting deformation, metamorphism, or alteration, but reason is not specified.</skos:definition>
	<skos:exactMatch rdf:resource="http://resource.geosciml.org/classifier/cgi/particleaspectratio/0009"/>
	<skos:inScheme rdf:resource="http://resource.geosciml.org/classifierscheme/cgi/201211/particleaspectratio"/>
	<skos:prefLabel>particle form indeterminate</skos:prefLabel>
</rdf:Description>

<rdf:Description rdf:about="http://resource.geosciml.org/classifier/cgi/particleaspectratio/prolate">
	<rdf:type rdf:resource="http://www.w3.org/2004/02/skos/core#Concept"/>
	<dc:source>Sneed and Folk, 1958; Pettijohn et al., 1972; NADM SLTTs, 2004</dc:source>
	<skos:broader rdf:resource="http://resource.geosciml.org/classifier/cgi/particleaspectratio/any_form"/>
	<skos:definition xml:lang="en">Particles are in 'elongated group' in Sneed &amp; Folk, (1958); S/L is less than 0.7 and (L-I)/(L-S) is greater than 0.66.</skos:definition>
	<skos:exactMatch rdf:resource="http://resource.geosciml.org/classifier/cgi/particleaspectratio/0010"/>
	<skos:inScheme rdf:resource="http://resource.geosciml.org/classifierscheme/cgi/201211/particleaspectratio"/>
	<skos:narrower rdf:resource="http://resource.geosciml.org/classifier/cgi/particleaspectratio/slightly_prolate"/>
	<skos:narrower rdf:resource="http://resource.geosciml.org/classifier/cgi/particleaspectratio/strongly_prolate"/>
	<skos:narrower rdf:resource="http://resource.geosciml.org/classifier/cgi/particleaspectratio/prolate_medium"/>
	<skos:notation rdf:datatype="http://resource.geosciml.org/classifierscheme/cgi/201211/particleaspectratio">prolate</skos:notation>
	<skos:prefLabel>prolate</skos:prefLabel>
</rdf:Description>

<rdf:Description rdf:about="http://resource.geosciml.org/classifier/cgi/particleaspectratio/prolate_medium">
	<rdf:type rdf:resource="http://www.w3.org/2004/02/skos/core#Concept"/>
	<dc:source>Sneed and Folk, 1958; Pettijohn et al., 1972; NADM SLTTs, 2004</dc:source>
	<skos:broader rdf:resource="http://resource.geosciml.org/classifier/cgi/particleaspectratio/prolate"/>
	<skos:definition xml:lang="en">Particle are 'just elongated' in Sneed&amp;Folk, (1958); S/L is between 0.3 and 0.5 and (L-I)/(L-S) is greater than 0.66.</skos:definition>
	<skos:exactMatch rdf:resource="http://resource.geosciml.org/classifier/cgi/particleaspectratio/0011"/>
	<skos:inScheme rdf:resource="http://resource.geosciml.org/classifierscheme/cgi/201211/particleaspectratio"/>
	<skos:prefLabel>prolate medium</skos:prefLabel>
</rdf:Description>

<rdf:Description rdf:about="http://resource.geosciml.org/classifier/cgi/particleaspectratio/slightly_flattened">
	<rdf:type rdf:resource="http://www.w3.org/2004/02/skos/core#Concept"/>
	<dc:source>Sneed and Folk, 1958; Pettijohn et al., 1972; NADM SLTTs, 2004</dc:source>
	<skos:broader rdf:resource="http://resource.geosciml.org/classifier/cgi/particleaspectratio/oblate"/>
	<skos:definition xml:lang="en">Particles are 'compact-platy' in Sneed&amp;Folk, (1958); S/L is between 0.5 and 0.7 and (L-I)/(L-S) is less than 0.33.</skos:definition>
	<skos:exactMatch rdf:resource="http://resource.geosciml.org/classifier/cgi/particleaspectratio/0012"/>
	<skos:inScheme rdf:resource="http://resource.geosciml.org/classifierscheme/cgi/201211/particleaspectratio"/>
	<skos:prefLabel>slightly flattened</skos:prefLabel>
</rdf:Description>

<rdf:Description rdf:about="http://resource.geosciml.org/classifier/cgi/particleaspectratio/slightly_prolate">
	<rdf:type rdf:resource="http://www.w3.org/2004/02/skos/core#Concept"/>
	<dc:source>Sneed and Folk, 1958; Pettijohn et al., 1972; NADM SLTTs, 2004</dc:source>
	<skos:broader rdf:resource="http://resource.geosciml.org/classifier/cgi/particleaspectratio/prolate"/>
	<skos:definition xml:lang="en">Particles are compact-elongated in Sneed&amp;Folk, (1958); S/L is between 0.5 and 0.7 and (L-I)/(L-S) is greater than 0.66.</skos:definition>
	<skos:exactMatch rdf:resource="http://resource.geosciml.org/classifier/cgi/particleaspectratio/0013"/>
	<skos:inScheme rdf:resource="http://resource.geosciml.org/classifierscheme/cgi/201211/particleaspectratio"/>
	<skos:prefLabel>slightly prolate</skos:prefLabel>
</rdf:Description>

<rdf:Description rdf:about="http://resource.geosciml.org/classifier/cgi/particleaspectratio/strongly_flattened">
	<rdf:type rdf:resource="http://www.w3.org/2004/02/skos/core#Concept"/>
	<dc:source>Sneed and Folk, 1958; Pettijohn et al., 1972; NADM SLTTs, 2004</dc:source>
	<skos:broader rdf:resource="http://resource.geosciml.org/classifier/cgi/particleaspectratio/oblate"/>
	<skos:definition xml:lang="en">Particles are 'very platy' in Sneed&amp;Folk, (1958); S/L is less than 0.3 and (L-I)/(L-S) is less than 0.33.</skos:definition>
	<skos:exactMatch rdf:resource="http://resource.geosciml.org/classifier/cgi/particleaspectratio/0014"/>
	<skos:inScheme rdf:resource="http://resource.geosciml.org/classifierscheme/cgi/201211/particleaspectratio"/>
	<skos:prefLabel>strongly flattened</skos:prefLabel>
</rdf:Description>

<rdf:Description rdf:about="http://resource.geosciml.org/classifier/cgi/particleaspectratio/strongly_prolate">
	<rdf:type rdf:resource="http://www.w3.org/2004/02/skos/core#Concept"/>
	<dc:source>Sneed and Folk, 1958; Pettijohn et al., 1972; NADM SLTTs, 2004</dc:source>
	<skos:broader rdf:resource="http://resource.geosciml.org/classifier/cgi/particleaspectratio/prolate"/>
	<skos:definition xml:lang="en">Particles are very elongated in Sneed&amp;Folk, (1958); S/L is less than 0.3 and (L-I)/(L-S) is greater than 0.66.</skos:definition>
	<skos:exactMatch rdf:resource="http://resource.geosciml.org/classifier/cgi/particleaspectratio/0015"/>
	<skos:inScheme rdf:resource="http://resource.geosciml.org/classifierscheme/cgi/201211/particleaspectratio"/>
	<skos:narrower rdf:resource="http://resource.geosciml.org/classifier/cgi/particleaspectratio/fibrous"/>
	<skos:prefLabel>strongly prolate</skos:prefLabel>
</rdf:Description>

<rdf:Description rdf:about="http://resource.geosciml.org/classifier/cgi/particleaspectratio/very_bladed">
	<rdf:type rdf:resource="http://www.w3.org/2004/02/skos/core#Concept"/>
	<dc:source>Sneed and Folk, 1958; Pettijohn et al., 1972; NADM SLTTs, 2004</dc:source>
	<skos:broader rdf:resource="http://resource.geosciml.org/classifier/cgi/particleaspectratio/bladed"/>
	<skos:definition xml:lang="en">S/L is less than 0.3 and (L-I)/(L-S) is between 0.33 and 0.66 Sneed&amp;Folk, (1958).</skos:definition>
	<skos:exactMatch rdf:resource="http://resource.geosciml.org/classifier/cgi/particleaspectratio/0016"/>
	<skos:inScheme rdf:resource="http://resource.geosciml.org/classifierscheme/cgi/201211/particleaspectratio"/>
	<skos:prefLabel>very bladed</skos:prefLabel>
</rdf:Description>

<rdf:Description rdf:about="http://resource.geosciml.org/classifierscheme/cgi/201211/particleaspectratio">
	<rdf:type rdf:resource="http://www.w3.org/2004/02/skos/core#ConceptScheme"/>
	<rdf:type rdf:resource="http://www.w3.org/2002/07/owl#Ontology"/>
	<dc:creator>Concept Definition Task Group of IUGS CGI Interoperability Working Group (http://www.cgi-iugs.org/tech_collaboration/interoperability_working_group.html)</dc:creator>
	<dc:format rdf:datatype="http://www.w3.org/2001/XMLSchema#string">application/rdf+xml</dc:format>
	<dc:identifier>http://resource.geosciml.org/classifierscheme/cgi/201211/particleaspectratio</dc:identifier>
	<dc:language>en</dc:language>
	<dc:publisher>Concept Definition Task Group of IUGS CGI Interoperability Working Group (http://www.cgi-iugs.org/tech_collaboration/interoperability_working_group.html)</dc:publisher>
	<dc:title xml:lang="en">CGI Particle Aspect Ratio Term Vocabulary</dc:title>
	<owl:imports rdf:resource="http://www.w3.org/2004/02/skos/core"/>
	<owl:imports rdf:resource="http://rdfs.org/ns/void"/>
	<owl:versionInfo>201211</owl:versionInfo>
	<skos:definition xml:lang="en">This file contains the CGI Particle Aspect Ratio vocabulary. AspectRatio describes the geometry of particles based on the ratios of lengths of long, intermediate and short axes of grains. Equates to sphericity in sedimentary rocks (ie: the degree to which the shape of a particle approximates a sphere). A quantitative specification is based on the ratio of lengths of long, intermediate and short axes of grain shape (Sneed and Folk, 1958; Zingg, 1935). This vocabulary includes terms for specifying average shape of some collection of particles.(eg: prolate, slightly flattened, very bladed, equant, acicular, tabular). Numeric shape values from Sneed and Folk (1958) are best understood by looking at the pictures of particles with the different shapes there and in Pettijohn et al. (1972).</skos:definition>
	<skos:historyNote xml:lang="en">2009-07-14. Generate SKOS encoding of vocabulary from Excel spreadsheet.</skos:historyNote>
	<skos:historyNote xml:lang="en">2012-11-24 SMR Update to 201211 version; add collection entity, check all pref labels are lower case, remove owl:NamedIndividual and Owl:Thing rdf:types.</skos:historyNote>
	<skos:historyNote xml:lang="en">2009-12-07. SMR add collections for mineralogical and sedimentary petrographic categories, improve annotation and notes on vocabulary.</skos:historyNote>
	<skos:historyNote xml:lang="en">2012-02-07 SMR update URI to replace numeric final token with English-language string as in original URN scheme.</skos:historyNote>
	<skos:historyNote xml:lang="en">2010-02-13 Add narrower relationship links by adding skos:narrower link in Protege, defining skos:narrower as inverse of skos:broader, calculating with Pellet reasoner to add inferred axioms, and using 'file/Export inferred axioms as ontology' in Protege.</skos:historyNote>
	<skos:historyNote xml:lang="en">2009-12-07 SMR Update metadata properties for version, creator, title, and format.  Change skos:HistoryNote to dc:source for information on origin of terms and definitions.</skos:historyNote>
	<skos:historyNote xml:lang="en">2012-02-27 SMR add skos:exactMatch triples to map URIs for concepts in this vocabulary to number-token URIs in 201012 version of same concepts.</skos:historyNote>
	<skos:historyNote xml:lang="en">2010-11-28 SMR Replace URN identifiers with http URI identifiers according to CGI URI scheme (see https://www.seegrid.csiro.au/wiki/bin/view/CGIModel/PersistentIdentifiersInGeoSciMLServices)</skos:historyNote>
	<skos:prefLabel xml:lang="en">CGI Particle Aspect Ratio Term Vocabulary</skos:prefLabel>
</rdf:Description>

<rdf:Description rdf:about="http://resource.geosciml.org/vocabulary/cgi/201211/particleaspectratio">
	<rdf:type rdf:resource="http://rdfs.org/ns/void#Dataset"/>
	<rdfs:label rdf:datatype="http://www.w3.org/2001/XMLSchema#string">Particle aspect ratio vocabulary</rdfs:label>
</rdf:Description>

</rdf:RDF>