# baseURI: http://resource.geosciml.org/classifierscheme/cgi/201211/stratigraphicrank
# imports: http://rdfs.org/ns/void
# imports: http://www.w3.org/2004/02/skos/core

@prefix :        <http://resource.geosciml.org/classifierscheme/cgi/201211/stratigraphicrank#> .
@prefix cgi:     <http://resource.geosciml.org/classifierscheme/cgi/201211/> .
@prefix dc:      <http://purl.org/dc/elements/1.1/> .
@prefix owl:     <http://www.w3.org/2002/07/owl#> .
@prefix owl2xml:  <http://www.w3.org/2006/12/owl2-xml#> .
@prefix rdf:     <http://www.w3.org/1999/02/22-rdf-syntax-ns#> .
@prefix rdfs:    <http://www.w3.org/2000/01/rdf-schema#> .
@prefix skos:    <http://www.w3.org/2004/02/skos/core#> .
@prefix stratrank:  <http://resource.geosciml.org/classifier/cgi/stratigraphicrank/> .
@prefix void:    <http://rdfs.org/ns/void#> .
@prefix xsd:     <http://www.w3.org/2001/XMLSchema#> .

stratrank:
      rdf:type skos:Collection ;
      rdfs:label "stratigraphic rank concepts"@en ;
      skos:definition "This resource defines the concept space for stratigraphic rank concepts by extension; it includes all concepts in this conceptScheme, as well as concepts in previous versions of the scheme."@en ;
      skos:member stratrank:supersequence , stratrank:supergroup , stratrank:member , stratrank:subgroup , stratrank:formation , stratrank:lithodeme , stratrank:rank_not_specified , stratrank:suite , stratrank:complex , stratrank:sequence , stratrank:group , stratrank:supersuite , stratrank:bed , stratrank:megasequence ;
      skos:prefLabel "CGI Stratigraphic Rank"@en .

<http://resource.geosciml.org/classifier/cgi/stratigraphicrank/0001>
      rdf:type owl:NamedIndividual .

<http://resource.geosciml.org/classifier/cgi/stratigraphicrank/0002>
      rdf:type owl:NamedIndividual .

<http://resource.geosciml.org/classifier/cgi/stratigraphicrank/0003>
      rdf:type owl:NamedIndividual .

<http://resource.geosciml.org/classifier/cgi/stratigraphicrank/0004>
      rdf:type owl:NamedIndividual .

<http://resource.geosciml.org/classifier/cgi/stratigraphicrank/0005>
      rdf:type owl:NamedIndividual .

<http://resource.geosciml.org/classifier/cgi/stratigraphicrank/0006>
      rdf:type owl:NamedIndividual .

<http://resource.geosciml.org/classifier/cgi/stratigraphicrank/0007>
      rdf:type owl:NamedIndividual .

<http://resource.geosciml.org/classifier/cgi/stratigraphicrank/0008>
      rdf:type owl:NamedIndividual .

<http://resource.geosciml.org/classifier/cgi/stratigraphicrank/0009>
      rdf:type owl:NamedIndividual .

<http://resource.geosciml.org/classifier/cgi/stratigraphicrank/0010>
      rdf:type owl:NamedIndividual .

<http://resource.geosciml.org/classifier/cgi/stratigraphicrank/0011>
      rdf:type owl:NamedIndividual .

<http://resource.geosciml.org/classifier/cgi/stratigraphicrank/0012>
      rdf:type owl:NamedIndividual .

<http://resource.geosciml.org/classifier/cgi/stratigraphicrank/0013>
      rdf:type owl:NamedIndividual .

<http://resource.geosciml.org/classifier/cgi/stratigraphicrank/0014>
      rdf:type owl:NamedIndividual .

<http://resource.geosciml.org/classifier/cgi/stratigraphicrank/0015>
      rdf:type owl:NamedIndividual .

stratrank:bed
      rdf:type skos:Concept ;
      dc:source "North American commission on Stratigraphic Nomenclature, 2005; Salvador, 1994" ;
      skos:broader stratrank:member ;
      skos:broaderTransitive
              stratrank:formation ;
      skos:definition "The smallest formal lithostratigraphic unit, usually a distinctive lithic entity which can be distinguished from adjacent rocks by one or more physical characteristics."@en ;
      skos:exactMatch <http://resource.geosciml.org/classifier/cgi/stratigraphicrank/0001> ;
      skos:inScheme cgi:stratigraphicrank ;
      skos:prefLabel "bed"@en .

stratrank:complex
      rdf:type skos:Concept ;
      dc:source "Salvador, A., ed. 1994. International Stratigraphic Guide: International Union of Geological Sciences, Trondheim, NO, 214 p." ;
      skos:definition "A lithostratigraphic unit composed of diverse types of any class or classes of rock (sedimentary, igneous, metamorphic), and characterized by irregularly mixed lithology or by hightly complicated structure relations to the extent that the original sequence of the component rocks may be obscured and the individual rocks or rock sequence cannot be readily mapped."@en ;
      skos:exactMatch <http://resource.geosciml.org/classifier/cgi/stratigraphicrank/0015> ;
      skos:inScheme cgi:stratigraphicrank ;
      skos:prefLabel "complex"@en ;
      skos:related stratrank:lithodeme ;
      skos:topConceptOf cgi:stratigraphicrank .

stratrank:formation
      rdf:type skos:Concept ;
      dc:source "North American commission on Stratigraphic Nomenclature, 2005; Salvador, 1994" ;
      skos:broader stratrank:group , stratrank:subgroup ;
      skos:broaderTransitive
              stratrank:supergroup ;
      skos:definition "A body of rock identified by lithic characteristics and stratigraphic position; it is usually but not necessarily tabular and is mappable at the Earth's surface or traceable in the subsurface."@en ;
      skos:exactMatch <http://resource.geosciml.org/classifier/cgi/stratigraphicrank/0003> ;
      skos:inScheme cgi:stratigraphicrank ;
      skos:narrower stratrank:member ;
      skos:narrowerTransitive
              stratrank:bed ;
      skos:prefLabel "formation"@en ;
      skos:related stratrank:lithodeme .

stratrank:group
      rdf:type skos:Concept ;
      dc:source "North American commission on Stratigraphic Nomenclature, 2005;  Salvador, 1994" ;
      skos:broader stratrank:supergroup ;
      skos:definition "A group is the lithostratigraphic unit next higher in rank to either subgroup or formation. A groups may consist of two or more subgroups or two or more formations or a combination of both."@en ;
      skos:exactMatch <http://resource.geosciml.org/classifier/cgi/stratigraphicrank/0004> ;
      skos:inScheme cgi:stratigraphicrank ;
      skos:narrower stratrank:formation , stratrank:subgroup ;
      skos:prefLabel "group"@en ;
      skos:related stratrank:suite .

stratrank:lithodeme
      rdf:type skos:Concept ;
      dc:source "North American commission on Stratigraphic Nomenclature, 2005" ;
      skos:broader stratrank:suite ;
      skos:broaderTransitive
              stratrank:supersuite ;
      skos:definition "A body of predominantly intrusive, highly deformed and/or highly metamorphosed rock, distinguished and delimited on the basis of rock characteristics."@en ;
      skos:exactMatch <http://resource.geosciml.org/classifier/cgi/stratigraphicrank/0005> ;
      skos:inScheme cgi:stratigraphicrank ;
      skos:prefLabel "lithodeme"@en ;
      skos:related stratrank:complex , stratrank:sequence , stratrank:formation .

stratrank:megasequence
      rdf:type skos:Concept ;
      rdfs:seeAlso """http://www.sepmstrata.org/terminology/seq-strat.html; http://sepmstrata.org/terminology/second-order-cyc.html;
Heward, A.P., 1978, Alluvial fan sequence and megasequence models: With examples from Westphalian D-Stephanian B coal-fields, northern Spain, in A.D. Miall, ed., fluvial sedimentation: Canadian Society of Petroleum Geologists Memoir 5, p. 59-76.""" ;
      dc:source """Haq, B.U., Hardenbol, J., and Vail, P.R., 1988, Mesozoic and Cenozoic chronostratigraphy an dcycles of sea-level changes, in Wilgus, C.K., et al., eds, Sea-level Changes: an Integrated Approach: Society of Sedimentary Geology Special Publication 42, p. 71-108.
Peel, F., Cole, Gary A, Apps, Gillian M., and Moore, M. G., 2002, Implications of Megasequence Stratigraphy for the Petroleum System of the Ultra Deep Water Gulf of Mexico [abstract], Gulf Coast Association of Geological Societies Meeting October 30 - November 1, 2002, Austin, Texas, accessed at http://www.searchanddiscovery.net/documents/abstracts/gcags/images/peel01.htm, 2011-02-17"""@en ;
      skos:definition "A succession of strata comprising two or more supersequences. A large-scale sequence-stratigraphic unit deposited during one distinct phase of basin evolution, separated by major unconformities that mark a change in fundamental basin-controlling processes."@en ;
      skos:exactMatch <http://resource.geosciml.org/classifier/cgi/stratigraphicrank/0006> ;
      skos:inScheme cgi:stratigraphicrank ;
      skos:narrower stratrank:supersequence ;
      skos:narrowerTransitive
              stratrank:sequence ;
      skos:prefLabel "megasequence"@en ;
      skos:related stratrank:supersuite ;
      skos:topConceptOf cgi:stratigraphicrank .

stratrank:member
      rdf:type skos:Concept ;
      dc:source "North American commission on Stratigraphic Nomenclature, 2005; Salvador, 1994" ;
      skos:broader stratrank:formation ;
      skos:definition "A formal lithostratigraphic unit next in rank below a formation, and always part of a formation. It is a named entity within a formation because it possesses characteristics distinguishing it from adjacent parts of the formation."@en ;
      skos:exactMatch <http://resource.geosciml.org/classifier/cgi/stratigraphicrank/0007> ;
      skos:inScheme cgi:stratigraphicrank ;
      skos:narrower stratrank:bed ;
      skos:prefLabel "member"@en .

stratrank:rank_not_specified
      rdf:type skos:Concept ;
      dc:source "this vocabulary"@en ;
      skos:definition "unit is not part of a defined stratigraphic hierarchy."@en ;
      skos:exactMatch <http://resource.geosciml.org/classifier/cgi/stratigraphicrank/0008> ;
      skos:inScheme cgi:stratigraphicrank ;
      skos:prefLabel "not specified"@en ;
      skos:topConceptOf cgi:stratigraphicrank .

stratrank:sequence
      rdf:type skos:Concept ;
      rdfs:seeAlso "http://www.sepmstrata.org/terminology/seq-strat.html" ;
      dc:source "Van Wagoner, J.C., Posamentier, H.W., Mitchum, R.M., Vail, P.R., Sarg, J.F., Loutit, T.S., Hardenbol, J., 1988, An overview of sequence stratigraphy and key definitions. In: Wilgus, C.K., Hastings, B.S., Kendall, C.G.St.C., Posamentier, H.W., Ross, C.A., Van Wagoner, J.C. (Eds.), Sea Level Changes––An Integrated Approach, vol. 42. SEPM Special Publication, pp. 39–45."@en ;
      skos:broader stratrank:supersequence ;
      skos:broaderTransitive
              stratrank:megasequence ;
      skos:definition "A genetically related succession of strata bounded by unconformites or their correlative conformable contacts, and typically having a thickness of 10-100 metres."@en ;
      skos:exactMatch <http://resource.geosciml.org/classifier/cgi/stratigraphicrank/0009> ;
      skos:inScheme cgi:stratigraphicrank ;
      skos:notation "sequence"^^cgi:stratigraphicrank ;
      skos:prefLabel "sequence"@en ;
      skos:related stratrank:lithodeme .

stratrank:subgroup
      rdf:type skos:Concept ;
      dc:source "Salvador, 1994"@en ;
      skos:broader stratrank:group ;
      skos:broaderTransitive
              stratrank:supergroup ;
      skos:definition "A subgroup is the lithostratigraphic unit next higher in rank to formation. A subgroup usually consists of several formations."@en ;
      skos:exactMatch <http://resource.geosciml.org/classifier/cgi/stratigraphicrank/0010> ;
      skos:inScheme cgi:stratigraphicrank ;
      skos:narrower stratrank:formation ;
      skos:prefLabel "subgroup"@en .

stratrank:suite
      rdf:type skos:Concept ;
      dc:source "North American commission on Stratigraphic Nomenclature, 2005" ;
      skos:broader stratrank:supersuite ;
      skos:definition "A formal lithodemic unit next higher in rank to lithodeme. It comprises two or more associated lithodemes of the same class (e.g., plutonic, metamorphic)."@en ;
      skos:exactMatch <http://resource.geosciml.org/classifier/cgi/stratigraphicrank/0011> ;
      skos:inScheme cgi:stratigraphicrank ;
      skos:narrower stratrank:lithodeme ;
      skos:prefLabel "suite"@en ;
      skos:related stratrank:group , stratrank:supersequence .

stratrank:supergroup
      rdf:type skos:Concept ;
      dc:source "North American commission on Stratigraphic Nomenclature, 2005; Salvador, 1994" ;
      skos:definition "A supergroup is a formal assemblage of related or superposed groups or of groups and formations"@en ;
      skos:exactMatch <http://resource.geosciml.org/classifier/cgi/stratigraphicrank/0012> ;
      skos:inScheme cgi:stratigraphicrank ;
      skos:narrower stratrank:group ;
      skos:narrowerTransitive
              stratrank:formation , stratrank:subgroup ;
      skos:prefLabel "supergroup"@en ;
      skos:related stratrank:supersuite ;
      skos:topConceptOf cgi:stratigraphicrank .

stratrank:supersequence
      rdf:type skos:Concept ;
      rdfs:seeAlso "http://www.sepmstrata.org/terminology/seq-strat.html" ;
      dc:source "Haq, B.U., Hardenbol, J., and Vail, P.R., 1988, Mesozoic and Cenozoic chronostratigraphy an dcycles of sea-level changes, in Wilgus, C.K., et al., eds, Sea-level Changes: an Integrated Approach: Society of Sedimentary Geology Special Publication 42, p. 71-108." ;
      skos:broader stratrank:megasequence ;
      skos:definition "A succession of strata comprising two or more sequences"@en ;
      skos:exactMatch <http://resource.geosciml.org/classifier/cgi/stratigraphicrank/0013> ;
      skos:inScheme cgi:stratigraphicrank ;
      skos:narrower stratrank:sequence ;
      skos:prefLabel "supersequence"@en ;
      skos:related stratrank:suite .

stratrank:supersuite
      rdf:type skos:Concept ;
      dc:source "North American commission on Stratigraphic Nomenclature, 2005" ;
      skos:definition "A formal lithodemic unit next higher in rank to suite. It comprises two or more suites having a degree of natural relationship to one another"@en ;
      skos:exactMatch <http://resource.geosciml.org/classifier/cgi/stratigraphicrank/0014> ;
      skos:inScheme cgi:stratigraphicrank ;
      skos:narrower stratrank:suite ;
      skos:narrowerTransitive
              stratrank:lithodeme ;
      skos:prefLabel "supersuite"@en ;
      skos:related stratrank:megasequence , stratrank:supergroup ;
      skos:topConceptOf cgi:stratigraphicrank .

cgi:stratigraphicrank
      rdf:type owl:Ontology , skos:ConceptScheme ;
      dc:creator "Concept Definition Task Group of IUGS CGI Interoperability Working Group (http://www.cgi-iugs.org/tech_collaboration/interoperability_working_group.html)" ;
      dc:format "application/rdf+xml"^^xsd:string ;
      dc:identifier "http://resource.geosciml.org/classifierscheme/cgi/201211/stratigraphicrank" ;
      dc:language "en" ;
      dc:publisher "Concept Definition Task Group of IUGS CGI Interoperability Working Group (http://www.cgi-iugs.org/tech_collaboration/interoperability_working_group.html)" ;
      dc:title "CGI Stratigraphic Rank Term Vocabulary"@en ;
      owl:imports <http://www.w3.org/2004/02/skos/core> , <http://rdfs.org/ns/void> ;
      owl:versionInfo "201211" ;
      skos:changeNote "2009-12-07 SMR Update metadata properties for version, creator, title, and format.  Change skos:HistoryNote to dc:source for information on origin of terms and definitions."@en ;
      skos:definition "This file contains the CGI StratigraphicRank vocabulary. This vocabulary contains categories used to classify geologic units in a generalization hierarchy from most local/smallest volume to most regional. Examples: group, subgroup, formation, member. No parent links because relation between e.g. formation and group is not 'is a' it is 'part of'. All formations are not groups, and a formation is not necessarily part of a group, therefore group is not a broader term than formation."@en ;
      skos:hasTopConcept stratrank:megasequence , stratrank:complex , stratrank:supergroup , stratrank:rank_not_specified , stratrank:supersuite ;
      skos:historyNote "2012-11-24 SMR Update to 201211 version; add collection entity, check all pref labels are lower case, remove owl:NamedIndividual and Owl:Thing rdf:types."@en , "2011-02-16 SMR Add broader/narrower relations according to stratigraphic code. These are not meant to be formal isA or PartOf relations, rather should be read something like 'broader in local intention' or 'may be part of'. Add term 'complex' to vocabulary"@en , "2010-02-08. SMR Clean up namespace declarations so concept URI's follow CGI URN scheme; concepts have URN, are not document fragments."@en , "2009-07-14. Generate SKOS encoding of vocabulary from Excel spreadsheet."@en , "2010-11-28 SMR replace URN with http URI constructed according to CGI URI scheme (see https://www.seegrid.csiro.au/wiki/bin/view/CGIModel/PersistentIdentifiersInGeoSciMLServices)"@en , "2012-02-07 SMR update URI to replace numeric final token with English-language string as in original URN scheme."@en , "2012-02-27 SMR add skos:exactMatch triples to map URIs for concepts in this vocabulary to number-token URIs in 201012 version of same concepts."@en ;
      skos:prefLabel "CGI Stratigraphic Rank Term Vocabulary"@en .

<http://resource.geosciml.org/vocabulary/cgi/201211/stratigraphicrank>
      rdf:type void:Dataset ;
      rdfs:label "Stratigraphic rank vocabulary"^^xsd:string .

skos:ConceptScheme
      rdf:type owl:Class .
