<?xml version="1.0"?>


<!DOCTYPE rdf:RDF [
    <!ENTITY p1 "#" >
    <!ENTITY owl "http://www.w3.org/2002/07/owl#" >
    <!ENTITY dc "http://purl.org/dc/elements/1.1/" >
    <!ENTITY xsd "http://www.w3.org/2001/XMLSchema#" >
    <!ENTITY owl2xml "http://www.w3.org/2006/12/owl2-xml#" >
    <!ENTITY xml "http://www.w3.org/XML/1998/namespace" >
    <!ENTITY skos "http://www.w3.org/2004/02/skos/core#" >
    <!ENTITY rdfs "http://www.w3.org/2000/01/rdf-schema#" >
    <!ENTITY rdf "http://www.w3.org/1999/02/22-rdf-syntax-ns#" >
    <!ENTITY cgi "http://resource.geosciml.org/classifierscheme/cgi/201202/" >
    <!ENTITY proportionterm "http://resource.geosciml.org/classifier/cgi/proportionterm/" >
]>


<rdf:RDF xmlns="&cgi;proportionterm#"
     xml:base="&cgi;proportionterm"
     xmlns:owl2xml="http://www.w3.org/2006/12/owl2-xml#"
     xmlns:cgi="http://resource.geosciml.org/classifierscheme/cgi/201202/"
     xmlns:p1="#"
     xmlns:proportionterm="http://resource.geosciml.org/classifier/cgi/proportionterm/"
     xmlns:xsd="http://www.w3.org/2001/XMLSchema#"
     xmlns:xml="http://www.w3.org/XML/1998/namespace"
     xmlns:rdfs="http://www.w3.org/2000/01/rdf-schema#"
     xmlns:owl="http://www.w3.org/2002/07/owl#"
     xmlns:skos="http://www.w3.org/2004/02/skos/core#"
     xmlns:dc="http://purl.org/dc/elements/1.1/"
     xmlns:rdf="http://www.w3.org/1999/02/22-rdf-syntax-ns#">
    <owl:Ontology rdf:about="&cgi;proportionterm">
        <dc:identifier>http://resource.geosciml.org/classifierscheme/cgi/201202/proportionterm</dc:identifier>
        <dc:language>en</dc:language>
        <skos:historyNote xml:lang="en">2010-02-11 Add narrower relationship links by adding skos:narrower link in Protege, defining skos:narrower as inverse of skos:broader, calculating with Pellet reasoner to add inferred axioms, and using &#39;file/Export inferred axioms as ontology&#39; in Protege.</skos:historyNote>
        <skos:historyNote xml:lang="en">2010-09-26 SMR work on rearranging hierarchy to recognize that the top concept is &#39;present&#39;, all others are entailed by this property. Also recognize inconsistent labeling of major-minor and dominant-subordinate. Proposal in this is &#39;more than half&#39;, &#39;less than half&#39;, and change &#39;dominant&#39; label to &#39;major&#39; to parallel usage of &#39;minor&#39;. Awaiting comment...</skos:historyNote>
        <skos:historyNote xml:lang="en">2011-07-07. GD Clean up remaining namespace declarations so no URN is present in the ontology. Removed empty concepts with genid.</skos:historyNote>
        <skos:historyNote xml:lang="en">2012-02-07 SMR update URI to replace numeric final token with English-language string as in original URN scheme.</skos:historyNote>
        <owl:versionInfo>201202</owl:versionInfo>
        <skos:historyNote xml:lang="en">2010-11-28 SMR replace URN with http URI according to CGI URI scheme (see https://www.seegrid.csiro.au/wiki/bin/view/CGIModel/PersistentIdentifiersInGeoSciMLServices)</skos:historyNote>
        <dc:publisher>Concept Definition Task Group of IUGS CGI Interoperability Working Group (http://www.cgi-iugs.org/tech_collaboration/interoperability_working_group.html)</dc:publisher>
        <skos:historyNote xml:lang="en">2012-02-27 SMR add skos:exactMatch relating URI in this vocabulary to URI in 201012 version using numeric tokens.  Update the vocabulary definition text.</skos:historyNote>
        <dc:title xml:lang="en">CGI Proportion Term Vocabulary</dc:title>
        <dc:creator xml:lang="en">Concept Definition Task Group of IUGS CGI Interoperability Working Group (http://www.cgi-iugs.org/tech_collaboration/interoperability_working_group.html)</dc:creator>
        <dc:format>application/rdf-xml</dc:format>
    </owl:Ontology>
    


    <!-- 
    ///////////////////////////////////////////////////////////////////////////////////////
    //
    // Annotation properties
    //
    ///////////////////////////////////////////////////////////////////////////////////////
     -->

    <owl:AnnotationProperty rdf:about="&dc;identifier"/>
    <owl:AnnotationProperty rdf:about="&dc;language"/>
    <owl:AnnotationProperty rdf:about="&dc;title"/>
    <owl:AnnotationProperty rdf:about="&dc;source"/>
    <owl:AnnotationProperty rdf:about="&dc;publisher"/>
    <owl:AnnotationProperty rdf:about="&dc;creator"/>
    <owl:AnnotationProperty rdf:about="&dc;format"/>
    <owl:AnnotationProperty rdf:about="&skos;historyNote"/>
    


    <!-- 
    ///////////////////////////////////////////////////////////////////////////////////////
    //
    // Datatypes
    //
    ///////////////////////////////////////////////////////////////////////////////////////
     -->

    


    <!-- 
    ///////////////////////////////////////////////////////////////////////////////////////
    //
    // Object Properties
    //
    ///////////////////////////////////////////////////////////////////////////////////////
     -->

    


    <!-- http://www.w3.org/2002/07/owl#topObjectProperty -->

    <owl:ObjectProperty rdf:about="&owl;topObjectProperty"/>
    


    <!-- http://www.w3.org/2004/02/skos/core#broadMatch -->

    <owl:ObjectProperty rdf:about="&skos;broadMatch">
        <rdfs:label xml:lang="en">broader match</rdfs:label>
        <rdfs:isDefinedBy rdf:datatype="&xsd;anyURI">http://www.w3.org/2004/02/skos/core</rdfs:isDefinedBy>
        <rdfs:subPropertyOf rdf:resource="&skos;broader"/>
        <rdfs:subPropertyOf rdf:resource="&skos;mappingRelation"/>
    </owl:ObjectProperty>
    


    <!-- http://www.w3.org/2004/02/skos/core#broader -->

    <owl:ObjectProperty rdf:about="&skos;broader">
        <rdfs:label xml:lang="en">has broader</rdfs:label>
        <rdfs:isDefinedBy rdf:datatype="&xsd;anyURI">http://www.w3.org/2004/02/skos/core</rdfs:isDefinedBy>
        <rdfs:comment xml:lang="en">Broader concepts are typically rendered as parents in a concept
      hierarchy (tree).</rdfs:comment>
        <rdfs:comment xml:lang="en">By convention, skos:broader is only used to assert an immediate
      (i.e. direct) hierarchical link between two conceptual resources.</rdfs:comment>
        <rdfs:subPropertyOf rdf:resource="&skos;broaderTransitive"/>
        <owl:inverseOf rdf:resource="&skos;narrower"/>
    </owl:ObjectProperty>
    


    <!-- http://www.w3.org/2004/02/skos/core#broaderTransitive -->

    <owl:ObjectProperty rdf:about="&skos;broaderTransitive">
        <rdf:type rdf:resource="&owl;TransitiveProperty"/>
        <rdfs:label xml:lang="en">broader transitive</rdfs:label>
        <rdfs:isDefinedBy rdf:datatype="&xsd;anyURI">http://www.w3.org/2004/02/skos/core</rdfs:isDefinedBy>
        <rdfs:comment xml:lang="en">By convention, skos:broaderTransitive is not used to make
      assertions. Rather, the properties can be used to draw inferences about the transitive closure
      of the hierarchical relation, which is useful e.g. when implementing a simple query expansion
      algorithm in a search application.</rdfs:comment>
        <owl:inverseOf rdf:resource="&skos;narrowerTransitive"/>
        <rdfs:subPropertyOf rdf:resource="&skos;semanticRelation"/>
    </owl:ObjectProperty>
    


    <!-- http://www.w3.org/2004/02/skos/core#changeNote -->

    <owl:ObjectProperty rdf:about="&skos;changeNote">
        <rdfs:subPropertyOf rdf:resource="&owl;topObjectProperty"/>
    </owl:ObjectProperty>
    


    <!-- http://www.w3.org/2004/02/skos/core#closeMatch -->

    <owl:ObjectProperty rdf:about="&skos;closeMatch">
        <rdf:type rdf:resource="&owl;SymmetricProperty"/>
        <rdfs:label xml:lang="en">close match</rdfs:label>
        <rdfs:isDefinedBy rdf:datatype="&xsd;anyURI">http://www.w3.org/2004/02/skos/core</rdfs:isDefinedBy>
        <owl:inverseOf rdf:resource="&skos;closeMatch"/>
        <rdfs:subPropertyOf rdf:resource="&skos;mappingRelation"/>
    </owl:ObjectProperty>
    


    <!-- http://www.w3.org/2004/02/skos/core#exactMatch -->

    <owl:ObjectProperty rdf:about="&skos;exactMatch">
        <rdf:type rdf:resource="&owl;SymmetricProperty"/>
        <rdf:type rdf:resource="&owl;TransitiveProperty"/>
        <rdfs:label xml:lang="en">exact match</rdfs:label>
        <rdfs:isDefinedBy rdf:datatype="&xsd;anyURI">http://www.w3.org/2004/02/skos/core</rdfs:isDefinedBy>
        <rdfs:comment xml:lang="en">skos:exactMatch is disjoint with each of the properties
      skos:broadMatch and skos:relatedMatch.</rdfs:comment>
        <rdfs:subPropertyOf rdf:resource="&skos;closeMatch"/>
        <owl:inverseOf rdf:resource="&skos;exactMatch"/>
    </owl:ObjectProperty>
    


    <!-- http://www.w3.org/2004/02/skos/core#hasTopConcept -->

    <owl:ObjectProperty rdf:about="&skos;hasTopConcept">
        <rdf:type rdf:resource="&owl;AsymmetricProperty"/>
        <rdf:type rdf:resource="&owl;IrreflexiveProperty"/>
        <rdf:type rdf:resource="&owl;TransitiveProperty"/>
        <rdfs:label xml:lang="en">has top concept</rdfs:label>
        <rdfs:isDefinedBy rdf:datatype="&xsd;anyURI">http://www.w3.org/2004/02/skos/core</rdfs:isDefinedBy>
        <rdfs:range rdf:resource="&skos;Concept"/>
        <rdfs:domain rdf:resource="&skos;ConceptScheme"/>
    </owl:ObjectProperty>
    


    <!-- http://www.w3.org/2004/02/skos/core#inScheme -->

    <owl:ObjectProperty rdf:about="&skos;inScheme">
        <rdfs:label xml:lang="en">in scheme</rdfs:label>
        <rdfs:isDefinedBy rdf:datatype="&xsd;anyURI">http://www.w3.org/2004/02/skos/core</rdfs:isDefinedBy>
        <rdfs:comment xml:lang="en">A concept may be a member of more than one concept scheme.</rdfs:comment>
        <rdfs:subPropertyOf rdf:resource="&owl;topObjectProperty"/>
        <rdfs:range rdf:resource="&skos;ConceptScheme"/>
    </owl:ObjectProperty>
    


    <!-- http://www.w3.org/2004/02/skos/core#mappingRelation -->

    <owl:ObjectProperty rdf:about="&skos;mappingRelation">
        <rdfs:label xml:lang="en">mapping relation</rdfs:label>
        <rdfs:isDefinedBy rdf:datatype="&xsd;anyURI">http://www.w3.org/2004/02/skos/core</rdfs:isDefinedBy>
        <rdfs:comment xml:lang="en">These concept mapping relations mirror semantic relations, and the
      data model defined below is similar (with the exception of skos:exactMatch) to the data model
      defined for semantic relations. A distinct vocabulary is provided for concept mapping
      relations, to provide a convenient way to differentiate links within a concept scheme from
      links between concept schemes. However, this pattern of usage is not a formal requirement of
      the SKOS data model, and relies on informal definitions of best practice.</rdfs:comment>
        <rdfs:subPropertyOf rdf:resource="&skos;semanticRelation"/>
    </owl:ObjectProperty>
    


    <!-- http://www.w3.org/2004/02/skos/core#member -->

    <owl:ObjectProperty rdf:about="&skos;member">
        <rdfs:label xml:lang="en">member</rdfs:label>
        <rdfs:isDefinedBy rdf:datatype="&xsd;anyURI">http://www.w3.org/2004/02/skos/core</rdfs:isDefinedBy>
        <rdfs:subPropertyOf rdf:resource="&owl;topObjectProperty"/>
        <rdfs:domain rdf:resource="&skos;Collection"/>
        <rdfs:range>
            <owl:Class>
                <owl:unionOf rdf:parseType="Collection">
                    <rdf:Description rdf:about="&skos;Collection"/>
                    <rdf:Description rdf:about="&skos;Concept"/>
                </owl:unionOf>
            </owl:Class>
        </rdfs:range>
    </owl:ObjectProperty>
    


    <!-- http://www.w3.org/2004/02/skos/core#memberList -->

    <owl:ObjectProperty rdf:about="&skos;memberList">
        <rdf:type rdf:resource="&owl;FunctionalProperty"/>
        <rdfs:label xml:lang="en">member list</rdfs:label>
        <rdfs:isDefinedBy rdf:datatype="&xsd;anyURI">http://www.w3.org/2004/02/skos/core</rdfs:isDefinedBy>
        <rdfs:comment xml:lang="en">For any resource, every item in the list given as the value of the
      skos:memberList property is also a value of the skos:member property.</rdfs:comment>
        <rdfs:subPropertyOf rdf:resource="&owl;topObjectProperty"/>
        <rdfs:domain rdf:resource="&skos;OrderedCollection"/>
    </owl:ObjectProperty>
    


    <!-- http://www.w3.org/2004/02/skos/core#narrowMatch -->

    <owl:ObjectProperty rdf:about="&skos;narrowMatch">
        <rdfs:label xml:lang="en">narrower match</rdfs:label>
        <rdfs:isDefinedBy rdf:datatype="&xsd;anyURI">http://www.w3.org/2004/02/skos/core</rdfs:isDefinedBy>
        <owl:inverseOf rdf:resource="&skos;broadMatch"/>
        <rdfs:subPropertyOf rdf:resource="&skos;mappingRelation"/>
        <rdfs:subPropertyOf rdf:resource="&skos;narrower"/>
    </owl:ObjectProperty>
    


    <!-- http://www.w3.org/2004/02/skos/core#narrower -->

    <owl:ObjectProperty rdf:about="&skos;narrower">
        <rdfs:label xml:lang="en">has narrower</rdfs:label>
        <rdfs:isDefinedBy rdf:datatype="&xsd;anyURI">http://www.w3.org/2004/02/skos/core</rdfs:isDefinedBy>
        <rdfs:comment xml:lang="en">By convention, skos:broader is only used to assert an immediate
      (i.e. direct) hierarchical link between two conceptual resources.</rdfs:comment>
        <rdfs:comment xml:lang="en">Narrower concepts are typically rendered as children in a concept
      hierarchy (tree).</rdfs:comment>
        <rdfs:subPropertyOf rdf:resource="&skos;narrowerTransitive"/>
    </owl:ObjectProperty>
    


    <!-- http://www.w3.org/2004/02/skos/core#narrowerTransitive -->

    <owl:ObjectProperty rdf:about="&skos;narrowerTransitive">
        <rdf:type rdf:resource="&owl;TransitiveProperty"/>
        <rdfs:label xml:lang="en">narrower transitive</rdfs:label>
        <rdfs:isDefinedBy rdf:datatype="&xsd;anyURI">http://www.w3.org/2004/02/skos/core</rdfs:isDefinedBy>
        <rdfs:comment xml:lang="en">By convention, skos:narrowerTransitive is not used to make
      assertions. Rather, the properties can be used to draw inferences about the transitive closure
      of the hierarchical relation, which is useful e.g. when implementing a simple query expansion
      algorithm in a search application.</rdfs:comment>
        <rdfs:subPropertyOf rdf:resource="&skos;semanticRelation"/>
    </owl:ObjectProperty>
    


    <!-- http://www.w3.org/2004/02/skos/core#related -->

    <owl:ObjectProperty rdf:about="&skos;related">
        <rdf:type rdf:resource="&owl;SymmetricProperty"/>
        <rdfs:label xml:lang="en">related to</rdfs:label>
        <rdfs:isDefinedBy rdf:datatype="&xsd;anyURI">http://www.w3.org/2004/02/skos/core</rdfs:isDefinedBy>
        <rdfs:comment xml:lang="en">skos:related is disjoint with skos:broaderTransitive</rdfs:comment>
        <owl:inverseOf rdf:resource="&skos;related"/>
        <rdfs:subPropertyOf rdf:resource="&skos;semanticRelation"/>
    </owl:ObjectProperty>
    


    <!-- http://www.w3.org/2004/02/skos/core#relatedMatch -->

    <owl:ObjectProperty rdf:about="&skos;relatedMatch">
        <rdf:type rdf:resource="&owl;SymmetricProperty"/>
        <rdfs:label xml:lang="en">related match</rdfs:label>
        <rdfs:isDefinedBy rdf:datatype="&xsd;anyURI">http://www.w3.org/2004/02/skos/core</rdfs:isDefinedBy>
        <rdfs:subPropertyOf rdf:resource="&skos;mappingRelation"/>
        <rdfs:subPropertyOf rdf:resource="&skos;related"/>
        <owl:inverseOf rdf:resource="&skos;relatedMatch"/>
    </owl:ObjectProperty>
    


    <!-- http://www.w3.org/2004/02/skos/core#semanticRelation -->

    <owl:ObjectProperty rdf:about="&skos;semanticRelation">
        <rdfs:label xml:lang="en">semantic relation</rdfs:label>
        <rdfs:isDefinedBy rdf:datatype="&xsd;anyURI">http://www.w3.org/2004/02/skos/core</rdfs:isDefinedBy>
        <rdfs:comment xml:lang="en">This property should not be used directly, but as a super-property
      for all properties denoting a relationship of meaning between concepts.</rdfs:comment>
        <rdfs:subPropertyOf rdf:resource="&owl;topObjectProperty"/>
        <rdfs:domain rdf:resource="&skos;Concept"/>
        <rdfs:range rdf:resource="&skos;Concept"/>
    </owl:ObjectProperty>
    


    <!-- http://www.w3.org/2004/02/skos/core#topConceptOf -->

    <owl:ObjectProperty rdf:about="&skos;topConceptOf">
        <rdfs:label xml:lang="en">top concept in scheme</rdfs:label>
        <rdfs:isDefinedBy rdf:datatype="&xsd;anyURI">http://www.w3.org/2004/02/skos/core</rdfs:isDefinedBy>
        <owl:inverseOf rdf:resource="&skos;hasTopConcept"/>
        <rdfs:subPropertyOf rdf:resource="&skos;inScheme"/>
    </owl:ObjectProperty>
    


    <!-- 
    ///////////////////////////////////////////////////////////////////////////////////////
    //
    // Data properties
    //
    ///////////////////////////////////////////////////////////////////////////////////////
     -->

    


    <!-- http://www.w3.org/1999/02/22-rdf-syntax-ns#value -->

    <owl:DatatypeProperty rdf:about="&rdf;value">
        <rdfs:subPropertyOf rdf:resource="&owl;topDataProperty"/>
    </owl:DatatypeProperty>
    


    <!-- http://www.w3.org/2002/07/owl#topDataProperty -->

    <owl:DatatypeProperty rdf:about="&owl;topDataProperty"/>
    


    <!-- http://www.w3.org/2004/02/skos/core#changeNote -->

    <owl:DatatypeProperty rdf:about="&skos;changeNote"/>
    


    <!-- http://www.w3.org/2004/02/skos/core#definition -->

    <owl:DatatypeProperty rdf:about="&skos;definition">
        <rdfs:label xml:lang="en">definition</rdfs:label>
        <rdfs:isDefinedBy rdf:datatype="&xsd;anyURI">http://www.w3.org/2004/02/skos/core</rdfs:isDefinedBy>
        <rdfs:subPropertyOf rdf:resource="&owl;topDataProperty"/>
    </owl:DatatypeProperty>
    


    <!-- http://www.w3.org/2004/02/skos/core#historyNote -->

    <owl:DatatypeProperty rdf:about="&skos;historyNote">
        <rdfs:subPropertyOf rdf:resource="&owl;topDataProperty"/>
    </owl:DatatypeProperty>
    


    <!-- http://www.w3.org/2004/02/skos/core#notation -->

    <owl:DatatypeProperty rdf:about="&skos;notation">
        <rdfs:label xml:lang="en">notation</rdfs:label>
        <rdfs:isDefinedBy rdf:datatype="&xsd;anyURI">http://www.w3.org/2004/02/skos/core</rdfs:isDefinedBy>
        <rdfs:comment xml:lang="en">By convention, skos:notation is used with a typed literal in the
      object position of the triple.</rdfs:comment>
        <rdfs:subPropertyOf rdf:resource="&owl;topDataProperty"/>
    </owl:DatatypeProperty>
    


    <!-- http://www.w3.org/2004/02/skos/core#prefLabel -->

    <owl:DatatypeProperty rdf:about="&skos;prefLabel">
        <rdfs:subPropertyOf rdf:resource="&owl;topDataProperty"/>
    </owl:DatatypeProperty>
    


    <!-- 
    ///////////////////////////////////////////////////////////////////////////////////////
    //
    // Classes
    //
    ///////////////////////////////////////////////////////////////////////////////////////
     -->

    


    <!-- http://www.w3.org/2002/07/owl#Thing -->

    <owl:Class rdf:about="&owl;Thing"/>
    


    <!-- http://www.w3.org/2004/02/skos/core#Collection -->

    <owl:Class rdf:about="&skos;Collection">
        <rdfs:label xml:lang="en">Collection</rdfs:label>
        <rdfs:subClassOf rdf:resource="&owl;Thing"/>
        <owl:disjointWith rdf:resource="&skos;Concept"/>
        <owl:disjointWith rdf:resource="&skos;ConceptScheme"/>
        <rdfs:isDefinedBy rdf:datatype="&xsd;anyURI">http://www.w3.org/2004/02/skos/core</rdfs:isDefinedBy>
        <rdfs:comment xml:lang="en">Labelled collections can be used with collectable semantic relation
      properties e.g. skos:narrower, where you would like a set of concepts to be displayed under a
      &#39;node label&#39; in the hierarchy.</rdfs:comment>
    </owl:Class>
    


    <!-- http://www.w3.org/2004/02/skos/core#Concept -->

    <owl:Class rdf:about="&skos;Concept">
        <rdfs:label xml:lang="en">Concept</rdfs:label>
        <rdfs:subClassOf rdf:resource="&owl;Thing"/>
        <owl:disjointWith rdf:resource="&skos;ConceptScheme"/>
        <owl:disjointWith rdf:resource="&skos;OrderedCollection"/>
        <rdfs:isDefinedBy rdf:datatype="&xsd;anyURI">http://www.w3.org/2004/02/skos/core</rdfs:isDefinedBy>
    </owl:Class>
    


    <!-- http://www.w3.org/2004/02/skos/core#ConceptScheme -->

    <owl:Class rdf:about="&skos;ConceptScheme">
        <rdfs:label xml:lang="en">Concept Scheme</rdfs:label>
        <rdfs:subClassOf rdf:resource="&owl;Thing"/>
        <owl:disjointWith rdf:resource="&skos;OrderedCollection"/>
        <rdfs:isDefinedBy rdf:datatype="&xsd;anyURI">http://www.w3.org/2004/02/skos/core</rdfs:isDefinedBy>
        <rdfs:comment xml:lang="en">A concept scheme may be defined to include concepts from different
      sources.</rdfs:comment>
        <rdfs:comment xml:lang="en">Thesauri, classification schemes, subject heading lists, taxonomies,
      &#39;folksonomies&#39;, and other types of controlled vocabulary are all examples of concept schemes.
      Concept schemes are also embedded in glossaries and terminologies.</rdfs:comment>
    </owl:Class>
    


    <!-- http://www.w3.org/2004/02/skos/core#OrderedCollection -->

    <owl:Class rdf:about="&skos;OrderedCollection">
        <rdfs:label xml:lang="en">Ordered Collection</rdfs:label>
        <rdfs:subClassOf rdf:resource="&skos;Collection"/>
        <rdfs:isDefinedBy rdf:datatype="&xsd;anyURI">http://www.w3.org/2004/02/skos/core</rdfs:isDefinedBy>
        <rdfs:comment xml:lang="en">Ordered collections can be used where you would like a set of concepts to be displayed in a specific order, and optionally under a &#39;node label&#39;.</rdfs:comment>
    </owl:Class>
    


    <!-- 
    ///////////////////////////////////////////////////////////////////////////////////////
    //
    // Individuals
    //
    ///////////////////////////////////////////////////////////////////////////////////////
     -->

    


    <!-- http://resource.geosciml.org/classifier/cgi/proportionterm/0001 -->

    <owl:NamedIndividual rdf:about="&proportionterm;0001"/>
    


    <!-- http://resource.geosciml.org/classifier/cgi/proportionterm/0002 -->

    <owl:NamedIndividual rdf:about="&proportionterm;0002"/>
    


    <!-- http://resource.geosciml.org/classifier/cgi/proportionterm/0003 -->

    <owl:NamedIndividual rdf:about="&proportionterm;0003"/>
    


    <!-- http://resource.geosciml.org/classifier/cgi/proportionterm/0004 -->

    <owl:NamedIndividual rdf:about="&proportionterm;0004"/>
    


    <!-- http://resource.geosciml.org/classifier/cgi/proportionterm/0005 -->

    <owl:NamedIndividual rdf:about="&proportionterm;0005"/>
    


    <!-- http://resource.geosciml.org/classifier/cgi/proportionterm/0006 -->

    <owl:NamedIndividual rdf:about="&proportionterm;0006"/>
    


    <!-- http://resource.geosciml.org/classifier/cgi/proportionterm/0007 -->

    <owl:NamedIndividual rdf:about="&proportionterm;0007"/>
    


    <!-- http://resource.geosciml.org/classifier/cgi/proportionterm/0008 -->

    <owl:NamedIndividual rdf:about="&proportionterm;0008"/>
    


    <!-- http://resource.geosciml.org/classifier/cgi/proportionterm/0009 -->

    <owl:NamedIndividual rdf:about="&proportionterm;0009"/>
    


    <!-- http://resource.geosciml.org/classifier/cgi/proportionterm/0010 -->

    <owl:NamedIndividual rdf:about="&proportionterm;0010"/>
    


    <!-- http://resource.geosciml.org/classifier/cgi/proportionterm/all -->

    <skos:Concept rdf:about="&proportionterm;all">
        <rdf:type rdf:resource="&owl;NamedIndividual"/>
        <rdf:type rdf:resource="&owl;Thing"/>
        <skos:definition xml:lang="en">Component constitutes effectively 100 percent of the volume of the described entity.</skos:definition>
        <skos:prefLabel xml:lang="en">all</skos:prefLabel>
        <dc:source xml:lang="en">this vocabulary</dc:source>
        <skos:exactMatch rdf:resource="&proportionterm;0001"/>
        <skos:broader rdf:resource="&proportionterm;dominant"/>
        <skos:broaderTransitive rdf:resource="&proportionterm;major"/>
        <skos:broaderTransitive rdf:resource="&proportionterm;present"/>
        <skos:inScheme rdf:resource="&cgi;proportionterm"/>
    </skos:Concept>
    


    <!-- http://resource.geosciml.org/classifier/cgi/proportionterm/dominant -->

    <skos:Concept rdf:about="&proportionterm;dominant">
        <rdf:type rdf:resource="&owl;NamedIndividual"/>
        <rdf:type rdf:resource="&owl;Thing"/>
        <skos:definition xml:lang="en">Component constitutes greater than 75 percent of the volume of the described entity.</skos:definition>
        <skos:prefLabel xml:lang="en">major</skos:prefLabel>
        <dc:source xml:lang="en">this vocabulary</dc:source>
        <skos:exactMatch rdf:resource="&proportionterm;0002"/>
        <skos:narrower rdf:resource="&proportionterm;all"/>
        <skos:broader rdf:resource="&proportionterm;major"/>
        <skos:broaderTransitive rdf:resource="&proportionterm;present"/>
        <skos:inScheme rdf:resource="&cgi;proportionterm"/>
    </skos:Concept>
    


    <!-- http://resource.geosciml.org/classifier/cgi/proportionterm/major -->

    <skos:Concept rdf:about="&proportionterm;major">
        <rdf:type rdf:resource="&owl;NamedIndividual"/>
        <rdf:type rdf:resource="&owl;Thing"/>
        <skos:definition xml:lang="en">Component constitutes greater than 50 percent of the volume of the described entity.</skos:definition>
        <skos:prefLabel xml:lang="en">more than half</skos:prefLabel>
        <dc:source xml:lang="en">this vocabulary</dc:source>
        <skos:exactMatch rdf:resource="&proportionterm;0003"/>
        <skos:narrowerTransitive rdf:resource="&proportionterm;all"/>
        <skos:narrower rdf:resource="&proportionterm;dominant"/>
        <skos:broader rdf:resource="&proportionterm;present"/>
        <skos:inScheme rdf:resource="&cgi;proportionterm"/>
    </skos:Concept>
    


    <!-- http://resource.geosciml.org/classifier/cgi/proportionterm/minor -->

    <skos:Concept rdf:about="&proportionterm;minor">
        <rdf:type rdf:resource="&owl;NamedIndividual"/>
        <rdf:type rdf:resource="&owl;Thing"/>
        <skos:definition xml:lang="en">component constitutes less than 25 percent of the volume of the described entity.</skos:definition>
        <skos:prefLabel xml:lang="en">minor</skos:prefLabel>
        <dc:source xml:lang="en">this vocabulary</dc:source>
        <skos:exactMatch rdf:resource="&proportionterm;0004"/>
        <skos:broaderTransitive rdf:resource="&proportionterm;present"/>
        <skos:narrower rdf:resource="&proportionterm;rare"/>
        <skos:broader rdf:resource="&proportionterm;subordinate"/>
        <skos:narrowerTransitive rdf:resource="&proportionterm;trace"/>
        <skos:inScheme rdf:resource="&cgi;proportionterm"/>
    </skos:Concept>
    


    <!-- http://resource.geosciml.org/classifier/cgi/proportionterm/predominant -->

    <skos:Concept rdf:about="&proportionterm;predominant">
        <rdf:type rdf:resource="&owl;NamedIndividual"/>
        <rdf:type rdf:resource="&owl;Thing"/>
        <dc:source xml:lang="en">17-12-2009 Added based on reviews for OneGeology Europe</dc:source>
        <skos:definition xml:lang="en">Constituent forms more of the described entity than any other constituent.</skos:definition>
        <skos:prefLabel xml:lang="en">most abundant</skos:prefLabel>
        <skos:exactMatch rdf:resource="&proportionterm;0005"/>
        <skos:broader rdf:resource="&proportionterm;present"/>
        <skos:inScheme rdf:resource="&cgi;proportionterm"/>
    </skos:Concept>
    


    <!-- http://resource.geosciml.org/classifier/cgi/proportionterm/present -->

    <skos:Concept rdf:about="&proportionterm;present">
        <rdf:type rdf:resource="&owl;NamedIndividual"/>
        <rdf:type rdf:resource="&owl;Thing"/>
        <skos:definition xml:lang="en">Component is present, but proportion is unknown</skos:definition>
        <skos:prefLabel xml:lang="en">present</skos:prefLabel>
        <dc:source xml:lang="en">this vocabulary</dc:source>
        <skos:exactMatch rdf:resource="&proportionterm;0006"/>
        <skos:narrowerTransitive rdf:resource="&proportionterm;all"/>
        <skos:narrowerTransitive rdf:resource="&proportionterm;dominant"/>
        <skos:narrowerTransitive rdf:resource="&proportionterm;major"/>
        <skos:narrower rdf:resource="&proportionterm;major"/>
        <skos:narrowerTransitive rdf:resource="&proportionterm;minor"/>
        <skos:narrower rdf:resource="&proportionterm;predominant"/>
        <skos:narrowerTransitive rdf:resource="&proportionterm;rare"/>
        <skos:narrower rdf:resource="&proportionterm;subordinate"/>
        <skos:narrowerTransitive rdf:resource="&proportionterm;trace"/>
        <skos:narrower rdf:resource="&proportionterm;variable"/>
        <skos:inScheme rdf:resource="&cgi;proportionterm"/>
        <skos:topConceptOf rdf:resource="&cgi;proportionterm"/>
    </skos:Concept>
    


    <!-- http://resource.geosciml.org/classifier/cgi/proportionterm/rare -->

    <skos:Concept rdf:about="&proportionterm;rare">
        <rdf:type rdf:resource="&owl;NamedIndividual"/>
        <rdf:type rdf:resource="&owl;Thing"/>
        <skos:definition xml:lang="en">Component constitutes less than 5 percent of the volume of the described entity.</skos:definition>
        <skos:prefLabel xml:lang="en">rare</skos:prefLabel>
        <dc:source xml:lang="en">this vocabulary; follows Neuendorf et al 2005 usage scoped to coal description</dc:source>
        <skos:exactMatch rdf:resource="&proportionterm;0007"/>
        <skos:broader rdf:resource="&proportionterm;minor"/>
        <skos:semanticRelation rdf:resource="&proportionterm;minor"/>
        <skos:broaderTransitive rdf:resource="&proportionterm;minor"/>
        <skos:semanticRelation rdf:resource="&proportionterm;present"/>
        <skos:broaderTransitive rdf:resource="&proportionterm;present"/>
        <skos:broaderTransitive rdf:resource="&proportionterm;subordinate"/>
        <skos:semanticRelation rdf:resource="&proportionterm;subordinate"/>
        <skos:narrowerTransitive rdf:resource="&proportionterm;trace"/>
        <skos:narrower rdf:resource="&proportionterm;trace"/>
        <skos:semanticRelation rdf:resource="&proportionterm;trace"/>
        <skos:inScheme rdf:resource="&cgi;proportionterm"/>
    </skos:Concept>
    


    <!-- http://resource.geosciml.org/classifier/cgi/proportionterm/subordinate -->

    <skos:Concept rdf:about="&proportionterm;subordinate">
        <rdf:type rdf:resource="&owl;NamedIndividual"/>
        <rdf:type rdf:resource="&owl;Thing"/>
        <skos:definition xml:lang="en">Component constitutes less than 50 percent of the volume of the described entity.</skos:definition>
        <skos:prefLabel xml:lang="en">less than half</skos:prefLabel>
        <dc:source xml:lang="en">this vocabulary</dc:source>
        <skos:exactMatch rdf:resource="&proportionterm;0008"/>
        <skos:narrower rdf:resource="&proportionterm;minor"/>
        <skos:broader rdf:resource="&proportionterm;present"/>
        <skos:narrowerTransitive rdf:resource="&proportionterm;rare"/>
        <skos:narrowerTransitive rdf:resource="&proportionterm;trace"/>
        <skos:inScheme rdf:resource="&cgi;proportionterm"/>
    </skos:Concept>
    


    <!-- http://resource.geosciml.org/classifier/cgi/proportionterm/trace -->

    <skos:Concept rdf:about="&proportionterm;trace">
        <rdf:type rdf:resource="&owl;NamedIndividual"/>
        <rdf:type rdf:resource="&owl;Thing"/>
        <skos:definition xml:lang="en">Component constitutes less than approximately 1 percent of the volume of the described entity. Presence is detectable but too small for accurate determination.</skos:definition>
        <dc:source xml:lang="en">this vocabulary; Neuendorf et al 2005</dc:source>
        <skos:prefLabel xml:lang="en">trace</skos:prefLabel>
        <skos:exactMatch rdf:resource="&proportionterm;0009"/>
        <skos:broaderTransitive rdf:resource="&proportionterm;minor"/>
        <skos:broaderTransitive rdf:resource="&proportionterm;present"/>
        <skos:broader rdf:resource="&proportionterm;rare"/>
        <skos:broaderTransitive rdf:resource="&proportionterm;subordinate"/>
        <skos:inScheme rdf:resource="&cgi;proportionterm"/>
    </skos:Concept>
    


    <!-- http://resource.geosciml.org/classifier/cgi/proportionterm/variable -->

    <skos:Concept rdf:about="&proportionterm;variable">
        <rdf:type rdf:resource="&owl;NamedIndividual"/>
        <rdf:type rdf:resource="&owl;Thing"/>
        <skos:definition xml:lang="en">Component varies in proportion throughout the described entity.</skos:definition>
        <dc:source xml:lang="en">this vocabulary</dc:source>
        <skos:prefLabel xml:lang="en">variable</skos:prefLabel>
        <skos:exactMatch rdf:resource="&proportionterm;0010"/>
        <skos:broader rdf:resource="&proportionterm;present"/>
        <skos:inScheme rdf:resource="&cgi;proportionterm"/>
    </skos:Concept>
    


    <!-- http://resource.geosciml.org/classifierscheme/cgi/201202/proportionterm -->

    <skos:ConceptScheme rdf:about="&cgi;proportionterm">
        <rdf:type rdf:resource="&owl;NamedIndividual"/>
        <rdf:type rdf:resource="&owl;Thing"/>
        <skos:changeNote xml:lang="en">2009-12-07 SMR Update metadata properties for version, creator, title, and format.  Change skos:HistoryNote to dc:source for information on origin of terms and definitions.</skos:changeNote>
        <skos:prefLabel xml:lang="en">CGI Proportion Term Vocabulary</skos:prefLabel>
        <skos:definition xml:lang="en">This file contains the CGI Proportion term vocabulary. This vocabulary provides terms that may be used to qualitatively express abundance of composition parts in a geologic unit or earth material description. Quantity that specifies the fraction of the geologic unit composed of the compound material. This vocabulary is used for GeologicUnit.GeologicUnitPart.proportion, GeologicUnit.CompositionPart.proportion, and for CompoundMaterial.ConsituentPart.proportion.</skos:definition>
        <skos:hasTopConcept rdf:resource="&proportionterm;present"/>
    </skos:ConceptScheme>
    


    <!-- http://www.w3.org/2004/02/skos/core#Collection -->

    <owl:Thing rdf:about="&skos;Collection">
        <rdf:type rdf:resource="&owl;NamedIndividual"/>
        <rdfs:label xml:lang="en">Collection</rdfs:label>
        <rdfs:isDefinedBy rdf:datatype="&xsd;anyURI">http://www.w3.org/2004/02/skos/core</rdfs:isDefinedBy>
        <skos:definition xml:lang="en">A meaningful collection of concepts.</skos:definition>
        <rdfs:comment xml:lang="en">Labelled collections can be used with collectable semantic relation
      properties e.g. skos:narrower, where you would like a set of concepts to be displayed under a
      &#39;node label&#39; in the hierarchy.</rdfs:comment>
    </owl:Thing>
    


    <!-- http://www.w3.org/2004/02/skos/core#Concept -->

    <owl:Thing rdf:about="&skos;Concept">
        <rdf:type rdf:resource="&owl;NamedIndividual"/>
        <rdfs:label xml:lang="en">Concept</rdfs:label>
        <rdfs:isDefinedBy rdf:datatype="&xsd;anyURI">http://www.w3.org/2004/02/skos/core</rdfs:isDefinedBy>
        <skos:definition xml:lang="en">An abstract idea or notion; a unit of thought.</skos:definition>
    </owl:Thing>
    


    <!-- http://www.w3.org/2004/02/skos/core#ConceptScheme -->

    <owl:Thing rdf:about="&skos;ConceptScheme">
        <rdf:type rdf:resource="&owl;NamedIndividual"/>
        <rdfs:label xml:lang="en">Concept Scheme</rdfs:label>
        <rdfs:isDefinedBy rdf:datatype="&xsd;anyURI">http://www.w3.org/2004/02/skos/core</rdfs:isDefinedBy>
        <rdfs:comment xml:lang="en">A concept scheme may be defined to include concepts from different
      sources.</rdfs:comment>
        <skos:definition xml:lang="en">A set of concepts, optionally including statements about semantic
      relationships between those concepts.</skos:definition>
        <skos:definition xml:lang="en">A set of concepts, optionally including statements about semanticn      relationships between those concepts.</skos:definition>
        <rdfs:comment xml:lang="en">Thesauri, classification schemes, subject heading lists, taxonomies,
      &#39;folksonomies&#39;, and other types of controlled vocabulary are all examples of concept schemes.
      Concept schemes are also embedded in glossaries and terminologies.</rdfs:comment>
    </owl:Thing>
    


    <!-- http://www.w3.org/2004/02/skos/core#OrderedCollection -->

    <owl:Thing rdf:about="&skos;OrderedCollection">
        <rdf:type rdf:resource="&owl;NamedIndividual"/>
        <rdfs:label xml:lang="en">Ordered Collection</rdfs:label>
        <rdfs:isDefinedBy rdf:datatype="&xsd;anyURI">http://www.w3.org/2004/02/skos/core</rdfs:isDefinedBy>
        <skos:definition xml:lang="en">An ordered collection of concepts, where both the grouping and
      the ordering are meaningful.</skos:definition>
        <skos:definition xml:lang="en">An ordered collection of concepts, where both the grouping andn      the ordering are meaningful.</skos:definition>
        <rdfs:comment xml:lang="en">Ordered collections can be used where you would like a set of concepts to be displayed in a specific order, and optionally under a &#39;node label&#39;.</rdfs:comment>
    </owl:Thing>
    


    <!-- http://www.w3.org/2004/02/skos/core#altLabel -->

    <owl:Thing rdf:about="&skos;altLabel">
        <rdf:type rdf:resource="&owl;NamedIndividual"/>
        <skos:definition xml:lang="en">An alternative lexical label for a resource.</skos:definition>
    </owl:Thing>
    


    <!-- http://www.w3.org/2004/02/skos/core#broadMatch -->

    <owl:Thing rdf:about="&skos;broadMatch">
        <rdf:type rdf:resource="&owl;NamedIndividual"/>
        <rdfs:label xml:lang="en">broader match</rdfs:label>
        <rdfs:isDefinedBy rdf:datatype="&xsd;anyURI">http://www.w3.org/2004/02/skos/core</rdfs:isDefinedBy>
        <skos:definition xml:lang="en">skos:broadMatch is used to state a hierarchical mapping link
      between two conceptual resources in different concept schemes.</skos:definition>
        <skos:definition xml:lang="en">skos:broadMatch is used to state a hierarchical mapping linkn      between two conceptual resources in different concept schemes.</skos:definition>
    </owl:Thing>
    


    <!-- http://www.w3.org/2004/02/skos/core#broader -->

    <owl:Thing rdf:about="&skos;broader">
        <rdf:type rdf:resource="&owl;NamedIndividual"/>
        <rdfs:label xml:lang="en">has broader</rdfs:label>
        <rdfs:isDefinedBy rdf:datatype="&xsd;anyURI">http://www.w3.org/2004/02/skos/core</rdfs:isDefinedBy>
        <skos:definition xml:lang="en">A concept that is more general in meaning.</skos:definition>
        <rdfs:comment xml:lang="en">Broader concepts are typically rendered as parents in a concept
      hierarchy (tree).</rdfs:comment>
        <rdfs:comment xml:lang="en">By convention, skos:broader is only used to assert an immediate
      (i.e. direct) hierarchical link between two conceptual resources.</rdfs:comment>
    </owl:Thing>
    


    <!-- http://www.w3.org/2004/02/skos/core#broaderTransitive -->

    <owl:Thing rdf:about="&skos;broaderTransitive">
        <rdf:type rdf:resource="&owl;NamedIndividual"/>
        <rdfs:label xml:lang="en">broader transitive</rdfs:label>
        <rdfs:isDefinedBy rdf:datatype="&xsd;anyURI">http://www.w3.org/2004/02/skos/core</rdfs:isDefinedBy>
        <skos:definition>skos:broaderTransitive is a transitive superproperty of skos:broader.</skos:definition>
        <rdfs:comment xml:lang="en">By convention, skos:broaderTransitive is not used to make
      assertions. Rather, the properties can be used to draw inferences about the transitive closure
      of the hierarchical relation, which is useful e.g. when implementing a simple query expansion
      algorithm in a search application.</rdfs:comment>
    </owl:Thing>
    


    <!-- http://www.w3.org/2004/02/skos/core#changeNote -->

    <owl:Thing rdf:about="&skos;changeNote">
        <rdf:type rdf:resource="&owl;NamedIndividual"/>
        <skos:definition xml:lang="en">A note about a modification to a concept.</skos:definition>
    </owl:Thing>
    


    <!-- http://www.w3.org/2004/02/skos/core#closeMatch -->

    <owl:Thing rdf:about="&skos;closeMatch">
        <rdf:type rdf:resource="&owl;NamedIndividual"/>
        <rdfs:label xml:lang="en">close match</rdfs:label>
        <rdfs:isDefinedBy rdf:datatype="&xsd;anyURI">http://www.w3.org/2004/02/skos/core</rdfs:isDefinedBy>
        <skos:definition xml:lang="en">skos:closeMatch is used to link two concepts that are
      sufficiently similar that they can be used interchangeably in some information retrieval
      applications. In order to avoid the possibility of &quot;compound errors&quot; when combining mappings
      across more than two concept schemes, skos:closeMatch is not declared to be a transitive
      property.</skos:definition>
        <skos:definition xml:lang="en">skos:closeMatch is used to link two concepts that aren      sufficiently similar that they can be used interchangeably in some information retrievaln      applications. In order to avoid the possibility of \&quot;compound errors\&quot; when combining mappingsn      across more than two concept schemes, skos:closeMatch is not declared to be a transitiven      property.</skos:definition>
    </owl:Thing>
    


    <!-- http://www.w3.org/2004/02/skos/core#definition -->

    <owl:Thing rdf:about="&skos;definition">
        <rdf:type rdf:resource="&owl;NamedIndividual"/>
        <rdfs:label xml:lang="en">definition</rdfs:label>
        <rdfs:isDefinedBy rdf:datatype="&xsd;anyURI">http://www.w3.org/2004/02/skos/core</rdfs:isDefinedBy>
        <skos:definition xml:lang="en">A statement or formal explanation of the meaning of a concept.</skos:definition>
    </owl:Thing>
    


    <!-- http://www.w3.org/2004/02/skos/core#editorialNote -->

    <owl:Thing rdf:about="&skos;editorialNote">
        <rdf:type rdf:resource="&owl;NamedIndividual"/>
        <skos:definition xml:lang="en">A note for an editor, translator or maintainer of the vocabulary.</skos:definition>
    </owl:Thing>
    


    <!-- http://www.w3.org/2004/02/skos/core#exactMatch -->

    <owl:Thing rdf:about="&skos;exactMatch">
        <rdf:type rdf:resource="&owl;NamedIndividual"/>
        <rdfs:label xml:lang="en">exact match</rdfs:label>
        <rdfs:isDefinedBy rdf:datatype="&xsd;anyURI">http://www.w3.org/2004/02/skos/core</rdfs:isDefinedBy>
        <rdfs:comment xml:lang="en">skos:exactMatch is disjoint with each of the properties
      skos:broadMatch and skos:relatedMatch.</rdfs:comment>
        <skos:definition xml:lang="en">skos:exactMatch is used to link two concepts, indicating a high
      degree of confidence that the concepts can be used interchangeably across a wide range of
      information retrieval applications. skos:exactMatch is a transitive property, and is a
      sub-property of skos:closeMatch.</skos:definition>
        <skos:definition xml:lang="en">skos:exactMatch is used to link two concepts, indicating a highn      degree of confidence that the concepts can be used interchangeably across a wide range ofn      information retrieval applications. skos:exactMatch is a transitive property, and is an      sub-property of skos:closeMatch.</skos:definition>
    </owl:Thing>
    


    <!-- http://www.w3.org/2004/02/skos/core#example -->

    <owl:Thing rdf:about="&skos;example">
        <rdf:type rdf:resource="&owl;NamedIndividual"/>
        <skos:definition xml:lang="en">An example of the use of a concept.</skos:definition>
    </owl:Thing>
    


    <!-- http://www.w3.org/2004/02/skos/core#hasTopConcept -->

    <owl:Thing rdf:about="&skos;hasTopConcept">
        <rdf:type rdf:resource="&owl;NamedIndividual"/>
        <rdfs:label xml:lang="en">has top concept</rdfs:label>
        <rdfs:isDefinedBy rdf:datatype="&xsd;anyURI">http://www.w3.org/2004/02/skos/core</rdfs:isDefinedBy>
        <skos:definition xml:lang="en">A top level concept in the concept scheme.</skos:definition>
    </owl:Thing>
    


    <!-- http://www.w3.org/2004/02/skos/core#hiddenLabel -->

    <owl:Thing rdf:about="&skos;hiddenLabel">
        <rdf:type rdf:resource="&owl;NamedIndividual"/>
        <skos:definition xml:lang="en">A lexical label for a resource that should be hidden when
      generating visual displays of the resource, but should still be accessible to free text search
      operations.</skos:definition>
        <skos:definition xml:lang="en">A lexical label for a resource that should be hidden whenn      generating visual displays of the resource, but should still be accessible to free text searchn      operations.</skos:definition>
    </owl:Thing>
    


    <!-- http://www.w3.org/2004/02/skos/core#historyNote -->

    <owl:Thing rdf:about="&skos;historyNote">
        <rdf:type rdf:resource="&owl;NamedIndividual"/>
        <skos:definition xml:lang="en">A note about the past state/use/meaning of a concept.</skos:definition>
    </owl:Thing>
    


    <!-- http://www.w3.org/2004/02/skos/core#inScheme -->

    <owl:Thing rdf:about="&skos;inScheme">
        <rdf:type rdf:resource="&owl;NamedIndividual"/>
        <rdfs:label xml:lang="en">in scheme</rdfs:label>
        <rdfs:isDefinedBy rdf:datatype="&xsd;anyURI">http://www.w3.org/2004/02/skos/core</rdfs:isDefinedBy>
        <rdfs:comment xml:lang="en">A concept may be a member of more than one concept scheme.</rdfs:comment>
        <skos:definition xml:lang="en">A concept scheme in which the concept is included.</skos:definition>
    </owl:Thing>
    


    <!-- http://www.w3.org/2004/02/skos/core#mappingRelation -->

    <owl:Thing rdf:about="&skos;mappingRelation">
        <rdf:type rdf:resource="&owl;NamedIndividual"/>
        <rdfs:label xml:lang="en">mapping relation</rdfs:label>
        <rdfs:isDefinedBy rdf:datatype="&xsd;anyURI">http://www.w3.org/2004/02/skos/core</rdfs:isDefinedBy>
        <skos:definition xml:lang="en">Definition</skos:definition>
        <rdfs:comment xml:lang="en">These concept mapping relations mirror semantic relations, and the
      data model defined below is similar (with the exception of skos:exactMatch) to the data model
      defined for semantic relations. A distinct vocabulary is provided for concept mapping
      relations, to provide a convenient way to differentiate links within a concept scheme from
      links between concept schemes. However, this pattern of usage is not a formal requirement of
      the SKOS data model, and relies on informal definitions of best practice.</rdfs:comment>
    </owl:Thing>
    


    <!-- http://www.w3.org/2004/02/skos/core#member -->

    <owl:Thing rdf:about="&skos;member">
        <rdf:type rdf:resource="&owl;NamedIndividual"/>
        <rdfs:label xml:lang="en">member</rdfs:label>
        <rdfs:isDefinedBy rdf:datatype="&xsd;anyURI">http://www.w3.org/2004/02/skos/core</rdfs:isDefinedBy>
        <skos:definition xml:lang="en">A member of a collection.</skos:definition>
    </owl:Thing>
    


    <!-- http://www.w3.org/2004/02/skos/core#memberList -->

    <owl:Thing rdf:about="&skos;memberList">
        <rdf:type rdf:resource="&owl;NamedIndividual"/>
        <rdfs:label xml:lang="en">member list</rdfs:label>
        <rdfs:isDefinedBy rdf:datatype="&xsd;anyURI">http://www.w3.org/2004/02/skos/core</rdfs:isDefinedBy>
        <skos:definition xml:lang="en">An RDF list containing the members of an ordered collection.</skos:definition>
        <rdfs:comment xml:lang="en">For any resource, every item in the list given as the value of the
      skos:memberList property is also a value of the skos:member property.</rdfs:comment>
    </owl:Thing>
    


    <!-- http://www.w3.org/2004/02/skos/core#narrowMatch -->

    <owl:Thing rdf:about="&skos;narrowMatch">
        <rdf:type rdf:resource="&owl;NamedIndividual"/>
        <rdfs:label xml:lang="en">narrower match</rdfs:label>
        <rdfs:isDefinedBy rdf:datatype="&xsd;anyURI">http://www.w3.org/2004/02/skos/core</rdfs:isDefinedBy>
        <skos:definition xml:lang="en">skos:narrowMatch is used to state a hierarchical mapping link
      between two conceptual resources in different concept schemes.</skos:definition>
        <skos:definition xml:lang="en">skos:narrowMatch is used to state a hierarchical mapping linkn      between two conceptual resources in different concept schemes.</skos:definition>
    </owl:Thing>
    


    <!-- http://www.w3.org/2004/02/skos/core#narrower -->

    <owl:Thing rdf:about="&skos;narrower">
        <rdf:type rdf:resource="&owl;NamedIndividual"/>
        <rdfs:label xml:lang="en">has narrower</rdfs:label>
        <rdfs:isDefinedBy rdf:datatype="&xsd;anyURI">http://www.w3.org/2004/02/skos/core</rdfs:isDefinedBy>
        <skos:definition xml:lang="en">A concept that is more specific in meaning.</skos:definition>
        <rdfs:comment xml:lang="en">By convention, skos:broader is only used to assert an immediate
      (i.e. direct) hierarchical link between two conceptual resources.</rdfs:comment>
        <rdfs:comment xml:lang="en">Narrower concepts are typically rendered as children in a concept
      hierarchy (tree).</rdfs:comment>
    </owl:Thing>
    


    <!-- http://www.w3.org/2004/02/skos/core#narrowerTransitive -->

    <owl:Thing rdf:about="&skos;narrowerTransitive">
        <rdf:type rdf:resource="&owl;NamedIndividual"/>
        <rdfs:label xml:lang="en">narrower transitive</rdfs:label>
        <rdfs:isDefinedBy rdf:datatype="&xsd;anyURI">http://www.w3.org/2004/02/skos/core</rdfs:isDefinedBy>
        <rdfs:comment xml:lang="en">By convention, skos:narrowerTransitive is not used to make
      assertions. Rather, the properties can be used to draw inferences about the transitive closure
      of the hierarchical relation, which is useful e.g. when implementing a simple query expansion
      algorithm in a search application.</rdfs:comment>
        <skos:definition>skos:narrowerTransitive is a transitive superproperty of skos:broader. By
      convention, skos:narrowerTransitive is not intended to be used in assertions, but provides a
      mechanism whereby the transitive closure of skos:narrower can be queried.</skos:definition>
        <skos:definition>skos:narrowerTransitive is a transitive superproperty of skos:broader. Byn      convention, skos:narrowerTransitive is not intended to be used in assertions, but provides an      mechanism whereby the transitive closure of skos:narrower can be queried.</skos:definition>
    </owl:Thing>
    


    <!-- http://www.w3.org/2004/02/skos/core#notation -->

    <owl:Thing rdf:about="&skos;notation">
        <rdf:type rdf:resource="&owl;NamedIndividual"/>
        <rdfs:label xml:lang="en">notation</rdfs:label>
        <rdfs:isDefinedBy rdf:datatype="&xsd;anyURI">http://www.w3.org/2004/02/skos/core</rdfs:isDefinedBy>
        <skos:definition xml:lang="en">A notation, also known as classification code, is a string of
      characters such as &quot;T58.5&quot; or &quot;303.4833&quot; used to uniquely identify a concept within the scope
      of a given concept scheme.</skos:definition>
        <skos:definition xml:lang="en">A notation, also known as classification code, is a string ofn      characters such as \&quot;T58.5\&quot; or \&quot;303.4833\&quot; used to uniquely identify a concept within the scopen      of a given concept scheme.</skos:definition>
        <rdfs:comment xml:lang="en">By convention, skos:notation is used with a typed literal in the
      object position of the triple.</rdfs:comment>
    </owl:Thing>
    


    <!-- http://www.w3.org/2004/02/skos/core#note -->

    <owl:Thing rdf:about="&skos;note">
        <rdf:type rdf:resource="&owl;NamedIndividual"/>
        <skos:definition xml:lang="en">A general note, for any purpose.</skos:definition>
    </owl:Thing>
    


    <!-- http://www.w3.org/2004/02/skos/core#prefLabel -->

    <owl:Thing rdf:about="&skos;prefLabel">
        <rdf:type rdf:resource="&owl;NamedIndividual"/>
        <skos:definition xml:lang="en">The preferred lexical label for a resource, in a given language.</skos:definition>
    </owl:Thing>
    


    <!-- http://www.w3.org/2004/02/skos/core#related -->

    <owl:Thing rdf:about="&skos;related">
        <rdf:type rdf:resource="&owl;NamedIndividual"/>
        <rdfs:label xml:lang="en">related to</rdfs:label>
        <rdfs:isDefinedBy rdf:datatype="&xsd;anyURI">http://www.w3.org/2004/02/skos/core</rdfs:isDefinedBy>
        <skos:definition xml:lang="en">A concept with which there is an associative semantic
      relationship.</skos:definition>
        <skos:definition xml:lang="en">A concept with which there is an associative semanticn      relationship.</skos:definition>
        <rdfs:comment xml:lang="en">skos:related is disjoint with skos:broaderTransitive</rdfs:comment>
    </owl:Thing>
    


    <!-- http://www.w3.org/2004/02/skos/core#relatedMatch -->

    <owl:Thing rdf:about="&skos;relatedMatch">
        <rdf:type rdf:resource="&owl;NamedIndividual"/>
        <rdfs:label xml:lang="en">related match</rdfs:label>
        <rdfs:isDefinedBy rdf:datatype="&xsd;anyURI">http://www.w3.org/2004/02/skos/core</rdfs:isDefinedBy>
        <skos:definition xml:lang="en">skos:relatedMatch is used to state an associative mapping link
      between two conceptual resources in different concept schemes.</skos:definition>
        <skos:definition xml:lang="en">skos:relatedMatch is used to state an associative mapping linkn      between two conceptual resources in different concept schemes.</skos:definition>
    </owl:Thing>
    


    <!-- http://www.w3.org/2004/02/skos/core#scopeNote -->

    <owl:Thing rdf:about="&skos;scopeNote">
        <rdf:type rdf:resource="&owl;NamedIndividual"/>
        <skos:definition xml:lang="en">A note that helps to clarify the meaning of a concept.</skos:definition>
    </owl:Thing>
    


    <!-- http://www.w3.org/2004/02/skos/core#semanticRelation -->

    <owl:Thing rdf:about="&skos;semanticRelation">
        <rdf:type rdf:resource="&owl;NamedIndividual"/>
        <rdfs:label xml:lang="en">semantic relation</rdfs:label>
        <rdfs:isDefinedBy rdf:datatype="&xsd;anyURI">http://www.w3.org/2004/02/skos/core</rdfs:isDefinedBy>
        <skos:definition xml:lang="en">A concept related by meaning.</skos:definition>
        <rdfs:comment xml:lang="en">This property should not be used directly, but as a super-property
      for all properties denoting a relationship of meaning between concepts.</rdfs:comment>
    </owl:Thing>
    


    <!-- http://www.w3.org/2004/02/skos/core#topConceptOf -->

    <owl:Thing rdf:about="&skos;topConceptOf">
        <rdf:type rdf:resource="&owl;NamedIndividual"/>
        <rdfs:label xml:lang="en">top concept in scheme</rdfs:label>
        <rdfs:isDefinedBy rdf:datatype="&xsd;anyURI">http://www.w3.org/2004/02/skos/core</rdfs:isDefinedBy>
        <skos:definition xml:lang="en">Relates a concept to the concept scheme that it is a top level
      concept of.</skos:definition>
        <skos:definition xml:lang="en">Relates a concept to the concept scheme that it is a top leveln      concept of.</skos:definition>
    </owl:Thing>
</rdf:RDF>



<!-- Generated by the OWL API (version 3.2.3.1824) http://owlapi.sourceforge.net -->

