@prefix cgi: <http://resource.geosciml.org/classifierscheme/cgi/201202/> .
@prefix xsd: <http://www.w3.org/2001/XMLSchema#> .
@prefix owl2xml: <http://www.w3.org/2006/12/owl2-xml#> .
@prefix owl: <http://www.w3.org/2002/07/owl#> .
@prefix : <http://resource.geosciml.org/classifierscheme/cgi/201202/stratigraphicrank#> .
@prefix xml: <http://www.w3.org/XML/1998/namespace> .
@prefix rdf: <http://www.w3.org/1999/02/22-rdf-syntax-ns#> .
@prefix dc: <http://purl.org/dc/elements/1.1/> .
@prefix rdfs: <http://www.w3.org/2000/01/rdf-schema#> .
@prefix skos: <http://www.w3.org/2004/02/skos/core#> .
@base <http://resource.geosciml.org/classifierscheme/cgi/201202/stratigraphicrank> .

<http://resource.geosciml.org/classifierscheme/cgi/201202/stratigraphicrank> rdf:type owl:Ontology ;
                                                                             
                                                                             skos:historyNote "2010-02-08. SMR Clean up namespace declarations so concept URI's follow CGI URN scheme; concepts have URN, are not document fragments."@en ;
                                                                             
                                                                             dc:language "en" ;
                                                                             
                                                                             skos:historyNote "2009-07-14. Generate SKOS encoding of vocabulary from Excel spreadsheet."@en ,
                                                                                              "2011-02-16 SMR Add broader/narrower relations according to stratigraphic code. These are not meant to be formal isA or PartOf relations, rather should be read something like 'broader in local intention' or 'may be part of'. Add term 'Complex' to vocabulary"@en ;
                                                                             
                                                                             dc:publisher "Concept Definition Task Group of IUGS CGI Interoperability Working Group (http://www.cgi-iugs.org/tech_collaboration/interoperability_working_group.html)" ;
                                                                             
                                                                             owl:versionInfo "201202" ;
                                                                             
                                                                             dc:format "text/turtle" ;
                                                                             
                                                                             dc:identifier "http://resource.geosciml.org/classifierscheme/cgi/201202/stratigraphicrank" ;
                                                                             
                                                                             dc:creator "Concept Definition Task Group of IUGS CGI Interoperability Working Group (http://www.cgi-iugs.org/tech_collaboration/interoperability_working_group.html)" ;
                                                                             
                                                                             skos:historyNote "2010-11-28 SMR replace URN with http URI constructed according to CGI URI scheme (see https://www.seegrid.csiro.au/wiki/bin/view/CGIModel/PersistentIdentifiersInGeoSciMLServices)"@en ,
                                                                                              "2012-02-07 SMR update URI to replace numeric final token with English-language string as in original URN scheme."@en ;
                                                                             
                                                                             dc:title "CGI Stratigraphic Rank Term Vocabulary"@en .


#################################################################
#
#    Annotation properties
#
#################################################################


dc:creator rdf:type owl:AnnotationProperty .



dc:publisher rdf:type owl:AnnotationProperty .



skos:historyNote rdf:type owl:AnnotationProperty .



dc:language rdf:type owl:AnnotationProperty .



dc:identifier rdf:type owl:AnnotationProperty .



dc:source rdf:type owl:AnnotationProperty .



dc:format rdf:type owl:AnnotationProperty .



dc:title rdf:type owl:AnnotationProperty .





#################################################################
#
#    Datatypes
#
#################################################################


###  http://resource.geosciml.org/classifierscheme/cgi/201202/stratigraphicrank

<http://resource.geosciml.org/classifierscheme/cgi/201202/stratigraphicrank> rdf:type rdfs:Datatype .





#################################################################
#
#    Object Properties
#
#################################################################


###  http://www.w3.org/1999/02/22-rdf-syntax-ns#value

rdf:value rdf:type owl:ObjectProperty ;
          
          rdfs:subPropertyOf owl:topDataProperty .



###  http://www.w3.org/2002/07/owl#topDataProperty

owl:topDataProperty rdf:type owl:ObjectProperty .



###  http://www.w3.org/2002/07/owl#topObjectProperty

owl:topObjectProperty rdf:type owl:ObjectProperty .



###  http://www.w3.org/2004/02/skos/core#broadMatch

skos:broadMatch rdf:type owl:ObjectProperty ;
                
                rdfs:label "broader match"@en ;
                
                rdfs:isDefinedBy "http://www.w3.org/2004/02/skos/core"^^xsd:anyURI ;
                
                rdfs:subPropertyOf skos:broader ,
                                   skos:mappingRelation .



###  http://www.w3.org/2004/02/skos/core#broader

skos:broader rdf:type owl:ObjectProperty ;
             
             rdfs:label "has broader"@en ;
             
             rdfs:isDefinedBy "http://www.w3.org/2004/02/skos/core"^^xsd:anyURI ;
             
             rdfs:comment """Broader concepts are typically rendered as parents in a concept
      hierarchy (tree)."""@en ,
                          """By convention, skos:broader is only used to assert an immediate
      (i.e. direct) hierarchical link between two conceptual resources."""@en ;
             
             rdfs:subPropertyOf skos:broaderTransitive .



###  http://www.w3.org/2004/02/skos/core#broaderTransitive

skos:broaderTransitive rdf:type owl:ObjectProperty ,
                                owl:TransitiveProperty ;
                       
                       rdfs:label "broader transitive"@en ;
                       
                       rdfs:isDefinedBy "http://www.w3.org/2004/02/skos/core"^^xsd:anyURI ;
                       
                       rdfs:comment """By convention, skos:broaderTransitive is not used to make
      assertions. Rather, the properties can be used to draw inferences about the transitive closure
      of the hierarchical relation, which is useful e.g. when implementing a simple query expansion
      algorithm in a search application."""@en ;
                       
                       owl:inverseOf skos:narrowerTransitive ;
                       
                       rdfs:subPropertyOf skos:semanticRelation .



###  http://www.w3.org/2004/02/skos/core#changeNote

skos:changeNote rdf:type owl:ObjectProperty ;
                
                rdfs:subPropertyOf owl:topDataProperty .



###  http://www.w3.org/2004/02/skos/core#closeMatch

skos:closeMatch rdf:type owl:ObjectProperty ,
                         owl:SymmetricProperty ;
                
                rdfs:label "close match"@en ;
                
                rdfs:isDefinedBy "http://www.w3.org/2004/02/skos/core"^^xsd:anyURI ;
                
                owl:inverseOf skos:closeMatch ;
                
                rdfs:subPropertyOf skos:mappingRelation .



###  http://www.w3.org/2004/02/skos/core#definition

skos:definition rdf:type owl:ObjectProperty ;
                
                rdfs:label "definition"@en ;
                
                rdfs:isDefinedBy "http://www.w3.org/2004/02/skos/core"^^xsd:anyURI ;
                
                rdfs:subPropertyOf owl:topDataProperty .



###  http://www.w3.org/2004/02/skos/core#exactMatch

skos:exactMatch rdf:type owl:ObjectProperty ,
                         owl:SymmetricProperty ,
                         owl:TransitiveProperty ;
                
                rdfs:label "exact match"@en ;
                
                rdfs:isDefinedBy "http://www.w3.org/2004/02/skos/core"^^xsd:anyURI ;
                
                rdfs:comment """skos:exactMatch is disjoint with each of the properties
      skos:broadMatch and skos:relatedMatch."""@en ;
                
                rdfs:subPropertyOf skos:closeMatch ;
                
                owl:inverseOf skos:exactMatch .



###  http://www.w3.org/2004/02/skos/core#hasTopConcept

skos:hasTopConcept rdf:type owl:AsymmetricProperty ,
                            owl:IrreflexiveProperty ,
                            owl:ObjectProperty ;
                   
                   rdfs:label "has top concept"@en ;
                   
                   rdfs:isDefinedBy "http://www.w3.org/2004/02/skos/core"^^xsd:anyURI ;
                   
                   rdfs:range skos:Concept ;
                   
                   rdfs:domain skos:ConceptScheme .



###  http://www.w3.org/2004/02/skos/core#historyNote

skos:historyNote rdf:type owl:ObjectProperty ;
                 
                 rdfs:subPropertyOf owl:topDataProperty .



###  http://www.w3.org/2004/02/skos/core#inScheme

skos:inScheme rdf:type owl:ObjectProperty ;
              
              rdfs:label "in scheme"@en ;
              
              rdfs:isDefinedBy "http://www.w3.org/2004/02/skos/core"^^xsd:anyURI ;
              
              rdfs:comment "A concept may be a member of more than one concept scheme."@en ;
              
              rdfs:subPropertyOf owl:topObjectProperty ;
              
              rdfs:range skos:ConceptScheme .



###  http://www.w3.org/2004/02/skos/core#mappingRelation

skos:mappingRelation rdf:type owl:ObjectProperty ;
                     
                     rdfs:label "mapping relation"@en ;
                     
                     rdfs:isDefinedBy "http://www.w3.org/2004/02/skos/core"^^xsd:anyURI ;
                     
                     rdfs:comment """These concept mapping relations mirror semantic relations, and the
      data model defined below is similar (with the exception of skos:exactMatch) to the data model
      defined for semantic relations. A distinct vocabulary is provided for concept mapping
      relations, to provide a convenient way to differentiate links within a concept scheme from
      links between concept schemes. However, this pattern of usage is not a formal requirement of
      the SKOS data model, and relies on informal definitions of best practice."""@en ;
                     
                     rdfs:subPropertyOf skos:semanticRelation .



###  http://www.w3.org/2004/02/skos/core#member

skos:member rdf:type owl:ObjectProperty ;
            
            rdfs:label "member"@en ;
            
            rdfs:isDefinedBy "http://www.w3.org/2004/02/skos/core"^^xsd:anyURI ;
            
            rdfs:subPropertyOf owl:topObjectProperty ;
            
            rdfs:domain skos:Collection ;
            
            rdfs:range [ rdf:type owl:Class ;
                         owl:unionOf ( skos:Collection
                                       skos:Concept
                                     )
                       ] .



###  http://www.w3.org/2004/02/skos/core#memberList

skos:memberList rdf:type owl:FunctionalProperty ,
                         owl:ObjectProperty ;
                
                rdfs:label "member list"@en ;
                
                rdfs:isDefinedBy "http://www.w3.org/2004/02/skos/core"^^xsd:anyURI ;
                
                rdfs:comment """For any resource, every item in the list given as the value of the
      skos:memberList property is also a value of the skos:member property."""@en ;
                
                rdfs:subPropertyOf owl:topObjectProperty ;
                
                rdfs:domain skos:OrderedCollection .



###  http://www.w3.org/2004/02/skos/core#narrowMatch

skos:narrowMatch rdf:type owl:ObjectProperty ;
                 
                 rdfs:label "narrower match"@en ;
                 
                 rdfs:isDefinedBy "http://www.w3.org/2004/02/skos/core"^^xsd:anyURI ;
                 
                 owl:inverseOf skos:broadMatch ;
                 
                 rdfs:subPropertyOf skos:mappingRelation ,
                                    skos:narrower .



###  http://www.w3.org/2004/02/skos/core#narrower

skos:narrower rdf:type owl:ObjectProperty ;
              
              rdfs:label "has narrower"@en ;
              
              rdfs:isDefinedBy "http://www.w3.org/2004/02/skos/core"^^xsd:anyURI ;
              
              rdfs:comment """By convention, skos:broader is only used to assert an immediate
      (i.e. direct) hierarchical link between two conceptual resources."""@en ,
                           """Narrower concepts are typically rendered as children in a concept
      hierarchy (tree)."""@en ;
              
              owl:inverseOf skos:broader ;
              
              rdfs:subPropertyOf skos:narrowerTransitive .



###  http://www.w3.org/2004/02/skos/core#narrowerTransitive

skos:narrowerTransitive rdf:type owl:ObjectProperty ,
                                 owl:TransitiveProperty ;
                        
                        rdfs:label "narrower transitive"@en ;
                        
                        rdfs:isDefinedBy "http://www.w3.org/2004/02/skos/core"^^xsd:anyURI ;
                        
                        rdfs:comment """By convention, skos:narrowerTransitive is not used to make
      assertions. Rather, the properties can be used to draw inferences about the transitive closure
      of the hierarchical relation, which is useful e.g. when implementing a simple query expansion
      algorithm in a search application."""@en ;
                        
                        rdfs:subPropertyOf skos:semanticRelation .



###  http://www.w3.org/2004/02/skos/core#notation

skos:notation rdf:type owl:ObjectProperty ;
              
              rdfs:label "notation"@en ;
              
              rdfs:isDefinedBy "http://www.w3.org/2004/02/skos/core"^^xsd:anyURI ;
              
              rdfs:comment """By convention, skos:notation is used with a typed literal in the
      object position of the triple."""@en ;
              
              rdfs:subPropertyOf owl:topDataProperty .



###  http://www.w3.org/2004/02/skos/core#prefLabel

skos:prefLabel rdf:type owl:ObjectProperty ;
               
               rdfs:subPropertyOf owl:topDataProperty .



###  http://www.w3.org/2004/02/skos/core#related

skos:related rdf:type owl:ObjectProperty ,
                      owl:SymmetricProperty ;
             
             rdfs:label "related to"@en ;
             
             rdfs:isDefinedBy "http://www.w3.org/2004/02/skos/core"^^xsd:anyURI ;
             
             rdfs:comment "skos:related is disjoint with skos:broaderTransitive"@en ;
             
             owl:inverseOf skos:related ;
             
             rdfs:subPropertyOf skos:semanticRelation .



###  http://www.w3.org/2004/02/skos/core#relatedMatch

skos:relatedMatch rdf:type owl:ObjectProperty ,
                           owl:SymmetricProperty ;
                  
                  rdfs:label "related match"@en ;
                  
                  rdfs:isDefinedBy "http://www.w3.org/2004/02/skos/core"^^xsd:anyURI ;
                  
                  rdfs:subPropertyOf skos:mappingRelation ,
                                     skos:related ;
                  
                  owl:inverseOf skos:relatedMatch .



###  http://www.w3.org/2004/02/skos/core#semanticRelation

skos:semanticRelation rdf:type owl:ObjectProperty ;
                      
                      rdfs:label "semantic relation"@en ;
                      
                      rdfs:isDefinedBy "http://www.w3.org/2004/02/skos/core"^^xsd:anyURI ;
                      
                      rdfs:comment """This property should not be used directly, but as a super-property
      for all properties denoting a relationship of meaning between concepts."""@en ;
                      
                      rdfs:subPropertyOf owl:topObjectProperty ;
                      
                      rdfs:domain skos:Concept ;
                      
                      rdfs:range skos:Concept .



###  http://www.w3.org/2004/02/skos/core#topConceptOf

skos:topConceptOf rdf:type owl:AsymmetricProperty ,
                           owl:IrreflexiveProperty ,
                           owl:ObjectProperty ;
                  
                  rdfs:label "top concept in scheme"@en ;
                  
                  rdfs:isDefinedBy "http://www.w3.org/2004/02/skos/core"^^xsd:anyURI ;
                  
                  owl:inverseOf skos:hasTopConcept ;
                  
                  rdfs:subPropertyOf skos:inScheme .





#################################################################
#
#    Data properties
#
#################################################################


###  http://www.w3.org/1999/02/22-rdf-syntax-ns#value

rdf:value rdf:type owl:DatatypeProperty .



###  http://www.w3.org/2002/07/owl#topDataProperty

owl:topDataProperty rdf:type owl:DatatypeProperty .



###  http://www.w3.org/2004/02/skos/core#changeNote

skos:changeNote rdf:type owl:DatatypeProperty .



###  http://www.w3.org/2004/02/skos/core#definition

skos:definition rdf:type owl:DatatypeProperty ;
                
                rdfs:label "definition"@en ;
                
                rdfs:isDefinedBy "http://www.w3.org/2004/02/skos/core"^^xsd:anyURI .



###  http://www.w3.org/2004/02/skos/core#historyNote

skos:historyNote rdf:type owl:DatatypeProperty .



###  http://www.w3.org/2004/02/skos/core#notation

skos:notation rdf:type owl:DatatypeProperty ;
              
              rdfs:label "notation"@en ;
              
              rdfs:isDefinedBy "http://www.w3.org/2004/02/skos/core"^^xsd:anyURI ;
              
              rdfs:comment """By convention, skos:notation is used with a typed literal in the
      object position of the triple."""@en .



###  http://www.w3.org/2004/02/skos/core#prefLabel

skos:prefLabel rdf:type owl:DatatypeProperty .





#################################################################
#
#    Classes
#
#################################################################


###  http://www.w3.org/2002/07/owl#Thing

owl:Thing rdf:type owl:Class .



###  http://www.w3.org/2004/02/skos/core#Collection

skos:Collection rdf:type owl:Class ;
                
                rdfs:label "Collection"@en ;
                
                rdfs:subClassOf owl:Thing ;
                
                owl:disjointWith skos:Concept ,
                                 skos:ConceptScheme ;
                
                rdfs:isDefinedBy "http://www.w3.org/2004/02/skos/core"^^xsd:anyURI ;
                
                rdfs:comment """Labelled collections can be used with collectable semantic relation
      properties e.g. skos:narrower, where you would like a set of concepts to be displayed under a
      'node label' in the hierarchy."""@en .



###  http://www.w3.org/2004/02/skos/core#Concept

skos:Concept rdf:type owl:Class ;
             
             rdfs:label "Concept"@en ;
             
             rdfs:subClassOf owl:Thing ;
             
             owl:disjointWith skos:ConceptScheme ,
                              skos:OrderedCollection ;
             
             rdfs:isDefinedBy "http://www.w3.org/2004/02/skos/core"^^xsd:anyURI .



###  http://www.w3.org/2004/02/skos/core#ConceptScheme

skos:ConceptScheme rdf:type owl:Class ;
                   
                   rdfs:label "Concept Scheme"@en ;
                   
                   rdfs:subClassOf owl:Thing ;
                   
                   owl:disjointWith skos:OrderedCollection ;
                   
                   rdfs:isDefinedBy "http://www.w3.org/2004/02/skos/core"^^xsd:anyURI ;
                   
                   rdfs:comment """A concept scheme may be defined to include concepts from different
      sources."""@en ,
                                """Thesauri, classification schemes, subject heading lists, taxonomies,
      'folksonomies', and other types of controlled vocabulary are all examples of concept schemes.
      Concept schemes are also embedded in glossaries and terminologies."""@en .



###  http://www.w3.org/2004/02/skos/core#OrderedCollection

skos:OrderedCollection rdf:type owl:Class ;
                       
                       rdfs:label "Ordered Collection"@en ;
                       
                       rdfs:subClassOf skos:Collection ;
                       
                       rdfs:isDefinedBy "http://www.w3.org/2004/02/skos/core"^^xsd:anyURI ;
                       
                       rdfs:comment "Ordered collections can be used where you would like a set of concepts to be displayed in a specific order, and optionally under a 'node label'."@en .





#################################################################
#
#    Individuals
#
#################################################################


###  http://resource.geosciml.org/classifier/cgi/stratigraphicrank/0001

<http://resource.geosciml.org/classifier/cgi/stratigraphicrank/0001> rdf:type owl:NamedIndividual .



###  http://resource.geosciml.org/classifier/cgi/stratigraphicrank/0002

<http://resource.geosciml.org/classifier/cgi/stratigraphicrank/0002> rdf:type owl:NamedIndividual .



###  http://resource.geosciml.org/classifier/cgi/stratigraphicrank/0003

<http://resource.geosciml.org/classifier/cgi/stratigraphicrank/0003> rdf:type owl:NamedIndividual .



###  http://resource.geosciml.org/classifier/cgi/stratigraphicrank/0004

<http://resource.geosciml.org/classifier/cgi/stratigraphicrank/0004> rdf:type owl:NamedIndividual .



###  http://resource.geosciml.org/classifier/cgi/stratigraphicrank/0005

<http://resource.geosciml.org/classifier/cgi/stratigraphicrank/0005> rdf:type owl:NamedIndividual .



###  http://resource.geosciml.org/classifier/cgi/stratigraphicrank/0006

<http://resource.geosciml.org/classifier/cgi/stratigraphicrank/0006> rdf:type owl:NamedIndividual .



###  http://resource.geosciml.org/classifier/cgi/stratigraphicrank/0007

<http://resource.geosciml.org/classifier/cgi/stratigraphicrank/0007> rdf:type owl:NamedIndividual .



###  http://resource.geosciml.org/classifier/cgi/stratigraphicrank/0008

<http://resource.geosciml.org/classifier/cgi/stratigraphicrank/0008> rdf:type owl:NamedIndividual .



###  http://resource.geosciml.org/classifier/cgi/stratigraphicrank/0009

<http://resource.geosciml.org/classifier/cgi/stratigraphicrank/0009> rdf:type owl:NamedIndividual .



###  http://resource.geosciml.org/classifier/cgi/stratigraphicrank/0010

<http://resource.geosciml.org/classifier/cgi/stratigraphicrank/0010> rdf:type owl:NamedIndividual .



###  http://resource.geosciml.org/classifier/cgi/stratigraphicrank/0011

<http://resource.geosciml.org/classifier/cgi/stratigraphicrank/0011> rdf:type owl:NamedIndividual .



###  http://resource.geosciml.org/classifier/cgi/stratigraphicrank/0012

<http://resource.geosciml.org/classifier/cgi/stratigraphicrank/0012> rdf:type owl:NamedIndividual .



###  http://resource.geosciml.org/classifier/cgi/stratigraphicrank/0013

<http://resource.geosciml.org/classifier/cgi/stratigraphicrank/0013> rdf:type owl:NamedIndividual .



###  http://resource.geosciml.org/classifier/cgi/stratigraphicrank/0014

<http://resource.geosciml.org/classifier/cgi/stratigraphicrank/0014> rdf:type owl:NamedIndividual .



###  http://resource.geosciml.org/classifier/cgi/stratigraphicrank/0015

<http://resource.geosciml.org/classifier/cgi/stratigraphicrank/0015> rdf:type owl:NamedIndividual .



###  http://resource.geosciml.org/classifier/cgi/stratigraphicrank/bed

<http://resource.geosciml.org/classifier/cgi/stratigraphicrank/bed> rdf:type owl:NamedIndividual ,
                                                                             owl:Thing ,
                                                                             skos:Concept ;
                                                                    
                                                                    dc:source "North American Commission on Stratigraphic Nomenclature, 2005; Salvador, 1994" ;
                                                                    
                                                                    skos:definition "The smallest formal lithostratigraphic unit, usually a distinctive lithic entity which can be distinguished from adjacent rocks by one or more physical characteristics." ;
                                                                    
                                                                    skos:prefLabel "Bed"@en ;
                                                                    
                                                                    skos:exactMatch <http://resource.geosciml.org/classifier/cgi/stratigraphicrank/0001> ;
                                                                    
                                                                    skos:broaderTransitive <http://resource.geosciml.org/classifier/cgi/stratigraphicrank/formation> ;
                                                                    
                                                                    skos:broader <http://resource.geosciml.org/classifier/cgi/stratigraphicrank/member> ;
                                                                    
                                                                    skos:inScheme <http://resource.geosciml.org/classifierscheme/cgi/201202/stratigraphicrank> .



###  http://resource.geosciml.org/classifier/cgi/stratigraphicrank/beds

<http://resource.geosciml.org/classifier/cgi/stratigraphicrank/beds> rdf:type owl:NamedIndividual ;
                                                                     
                                                                     skos:exactMatch <http://resource.geosciml.org/classifier/cgi/stratigraphicrank/0002> .



###  http://resource.geosciml.org/classifier/cgi/stratigraphicrank/complex

<http://resource.geosciml.org/classifier/cgi/stratigraphicrank/complex> rdf:type owl:NamedIndividual ,
                                                                                 owl:Thing ,
                                                                                 skos:Concept ;
                                                                        
                                                                        dc:source "Salvador, A., ed. 1994. International Stratigraphic Guide: International Union of Geological Sciences, Trondheim, NO, 214 p." ;
                                                                        
                                                                        skos:definition "A lithostratigraphic unit composed of diverse types of any class or classes of rock (sedimentary, igneous, metamorphic), and characterized by irregularly mixed lithology or by hightly complicated structure relations to the extent that the original sequence of the component rocks may be obscured and the individual rocks or rock sequence cannot be readily mapped."@en ;
                                                                        
                                                                        skos:prefLabel "Complex"@en ;
                                                                        
                                                                        skos:exactMatch <http://resource.geosciml.org/classifier/cgi/stratigraphicrank/0015> ;
                                                                        
                                                                        skos:related <http://resource.geosciml.org/classifier/cgi/stratigraphicrank/lithodeme> ;
                                                                        
                                                                        skos:inScheme <http://resource.geosciml.org/classifierscheme/cgi/201202/stratigraphicrank> ;
                                                                        
                                                                        skos:topConceptOf <http://resource.geosciml.org/classifierscheme/cgi/201202/stratigraphicrank> .



###  http://resource.geosciml.org/classifier/cgi/stratigraphicrank/formation

<http://resource.geosciml.org/classifier/cgi/stratigraphicrank/formation> rdf:type owl:NamedIndividual ,
                                                                                   owl:Thing ,
                                                                                   skos:Concept ;
                                                                          
                                                                          skos:definition "A body of rock identified by lithic characteristics and stratigraphic position; it is usually but not necessarily tabular and is mappable at the Earth's surface or traceable in the subsurface." ;
                                                                          
                                                                          skos:prefLabel "Formation"@en ;
                                                                          
                                                                          dc:source "North American Commission on Stratigraphic Nomenclature, 2005; Salvador, 1994" ;
                                                                          
                                                                          skos:exactMatch <http://resource.geosciml.org/classifier/cgi/stratigraphicrank/0003> ;
                                                                          
                                                                          skos:narrowerTransitive <http://resource.geosciml.org/classifier/cgi/stratigraphicrank/bed> ;
                                                                          
                                                                          skos:broader <http://resource.geosciml.org/classifier/cgi/stratigraphicrank/group> ;
                                                                          
                                                                          skos:related <http://resource.geosciml.org/classifier/cgi/stratigraphicrank/lithodeme> ;
                                                                          
                                                                          skos:narrower <http://resource.geosciml.org/classifier/cgi/stratigraphicrank/member> ;
                                                                          
                                                                          skos:broader <http://resource.geosciml.org/classifier/cgi/stratigraphicrank/subgroup> ;
                                                                          
                                                                          skos:broaderTransitive <http://resource.geosciml.org/classifier/cgi/stratigraphicrank/supergroup> ;
                                                                          
                                                                          skos:inScheme <http://resource.geosciml.org/classifierscheme/cgi/201202/stratigraphicrank> .



###  http://resource.geosciml.org/classifier/cgi/stratigraphicrank/group

<http://resource.geosciml.org/classifier/cgi/stratigraphicrank/group> rdf:type owl:NamedIndividual ,
                                                                               owl:Thing ,
                                                                               skos:Concept ;
                                                                      
                                                                      dc:source "North American Commission on Stratigraphic Nomenclature, 2005;  Salvador, 1994" ;
                                                                      
                                                                      skos:definition "A group is the lithostratigraphic unit next higher in rank to either subgroup or formation. A groups may consist of two or more subgroups or two or more formations or a combination of both." ;
                                                                      
                                                                      skos:prefLabel "Group"@en ;
                                                                      
                                                                      skos:exactMatch <http://resource.geosciml.org/classifier/cgi/stratigraphicrank/0004> ;
                                                                      
                                                                      skos:narrower <http://resource.geosciml.org/classifier/cgi/stratigraphicrank/formation> ,
                                                                                    <http://resource.geosciml.org/classifier/cgi/stratigraphicrank/subgroup> ;
                                                                      
                                                                      skos:related <http://resource.geosciml.org/classifier/cgi/stratigraphicrank/suite> ;
                                                                      
                                                                      skos:broader <http://resource.geosciml.org/classifier/cgi/stratigraphicrank/supergroup> ;
                                                                      
                                                                      skos:inScheme <http://resource.geosciml.org/classifierscheme/cgi/201202/stratigraphicrank> .



###  http://resource.geosciml.org/classifier/cgi/stratigraphicrank/lithodeme

<http://resource.geosciml.org/classifier/cgi/stratigraphicrank/lithodeme> rdf:type owl:NamedIndividual ,
                                                                                   owl:Thing ,
                                                                                   skos:Concept ;
                                                                          
                                                                          skos:definition "A body of predominantly intrusive, highly deformed and/or highly metamorphosed rock, distinguished and delimited on the basis of rock characteristics." ;
                                                                          
                                                                          skos:prefLabel "Lithodeme"@en ;
                                                                          
                                                                          dc:source "North American Commission on Stratigraphic Nomenclature, 2005" ;
                                                                          
                                                                          skos:exactMatch <http://resource.geosciml.org/classifier/cgi/stratigraphicrank/0005> ;
                                                                          
                                                                          skos:related <http://resource.geosciml.org/classifier/cgi/stratigraphicrank/complex> ,
                                                                                       <http://resource.geosciml.org/classifier/cgi/stratigraphicrank/formation> ,
                                                                                       <http://resource.geosciml.org/classifier/cgi/stratigraphicrank/sequence> ;
                                                                          
                                                                          skos:broader <http://resource.geosciml.org/classifier/cgi/stratigraphicrank/suite> ;
                                                                          
                                                                          skos:broaderTransitive <http://resource.geosciml.org/classifier/cgi/stratigraphicrank/supersuite> ;
                                                                          
                                                                          skos:inScheme <http://resource.geosciml.org/classifierscheme/cgi/201202/stratigraphicrank> .



###  http://resource.geosciml.org/classifier/cgi/stratigraphicrank/megasequence

<http://resource.geosciml.org/classifier/cgi/stratigraphicrank/megasequence> rdf:type owl:NamedIndividual ,
                                                                                      owl:Thing ,
                                                                                      skos:Concept ;
                                                                             
                                                                             dc:source """Haq, B.U., Hardenbol, J., and Vail, P.R., 1988, Mesozoic and Cenozoic chronostratigraphy an dcycles of sea-level changes, in Wilgus, C.K., et al., eds, Sea-level Changes: an Integrated Approach: Society of Sedimentary Geology Special Publication 42, p. 71-108.
Peel, F., Cole, Gary A, Apps, Gillian M., and Moore, M. G., 2002, Implications of Megasequence Stratigraphy for the Petroleum System of the Ultra Deep Water Gulf of Mexico [abstract], Gulf Coast Association of Geological Societies Meeting October 30 - November 1, 2002, Austin, Texas, accessed at http://www.searchanddiscovery.net/documents/abstracts/gcags/images/peel01.htm, 2011-02-17"""@en ;
                                                                             
                                                                             skos:prefLabel "Megasequence"@en ;
                                                                             
                                                                             rdfs:seeAlso """http://www.sepmstrata.org/terminology/seq-strat.html; http://sepmstrata.org/terminology/second-order-cyc.html;
Heward, A.P., 1978, Alluvial fan sequence and megasequence models: With examples from Westphalian D-Stephanian B coal-fields, northern Spain, in A.D. Miall, ed., fluvial sedimentation: Canadian Society of Petroleum Geologists Memoir 5, p. 59-76.""" ;
                                                                             
                                                                             skos:definition "A succession of strata comprising two or more supersequences. A large-scale sequence-stratigraphic unit deposited during one distinct phase of basin evolution, separated by major unconformities that mark a change in fundamental basin-controlling processes."@en ;
                                                                             
                                                                             skos:exactMatch <http://resource.geosciml.org/classifier/cgi/stratigraphicrank/0006> ;
                                                                             
                                                                             skos:narrowerTransitive <http://resource.geosciml.org/classifier/cgi/stratigraphicrank/sequence> ;
                                                                             
                                                                             skos:narrower <http://resource.geosciml.org/classifier/cgi/stratigraphicrank/supersequence> ;
                                                                             
                                                                             skos:related <http://resource.geosciml.org/classifier/cgi/stratigraphicrank/supersuite> ;
                                                                             
                                                                             skos:topConceptOf <http://resource.geosciml.org/classifierscheme/cgi/201202/stratigraphicrank> ;
                                                                             
                                                                             skos:inScheme <http://resource.geosciml.org/classifierscheme/cgi/201202/stratigraphicrank> .



###  http://resource.geosciml.org/classifier/cgi/stratigraphicrank/member

<http://resource.geosciml.org/classifier/cgi/stratigraphicrank/member> rdf:type owl:NamedIndividual ,
                                                                                owl:Thing ,
                                                                                skos:Concept ;
                                                                       
                                                                       dc:source "North American Commission on Stratigraphic Nomenclature, 2005; Salvador, 1994" ;
                                                                       
                                                                       skos:definition "A formal lithostratigraphic unit next in rank below a formation, and always part of a formation. It is a named entity within a formation because it possesses characteristics distinguishing it from adjacent parts of the formation." ;
                                                                       
                                                                       skos:prefLabel "Member"@en ;
                                                                       
                                                                       skos:exactMatch <http://resource.geosciml.org/classifier/cgi/stratigraphicrank/0007> ;
                                                                       
                                                                       skos:narrower <http://resource.geosciml.org/classifier/cgi/stratigraphicrank/bed> ;
                                                                       
                                                                       skos:broader <http://resource.geosciml.org/classifier/cgi/stratigraphicrank/formation> ;
                                                                       
                                                                       skos:inScheme <http://resource.geosciml.org/classifierscheme/cgi/201202/stratigraphicrank> .



###  http://resource.geosciml.org/classifier/cgi/stratigraphicrank/rank_not_specified

<http://resource.geosciml.org/classifier/cgi/stratigraphicrank/rank_not_specified> rdf:type owl:NamedIndividual ,
                                                                                            owl:Thing ,
                                                                                            skos:Concept ;
                                                                                   
                                                                                   skos:definition "unit is not part of a defined stratigraphic hierarchy." ;
                                                                                   
                                                                                   skos:prefLabel "Not specified"@en ;
                                                                                   
                                                                                   dc:source "this vocabulary"@en ;
                                                                                   
                                                                                   skos:exactMatch <http://resource.geosciml.org/classifier/cgi/stratigraphicrank/0008> ;
                                                                                   
                                                                                   skos:inScheme <http://resource.geosciml.org/classifierscheme/cgi/201202/stratigraphicrank> ;
                                                                                   
                                                                                   skos:topConceptOf <http://resource.geosciml.org/classifierscheme/cgi/201202/stratigraphicrank> .



###  http://resource.geosciml.org/classifier/cgi/stratigraphicrank/sequence

<http://resource.geosciml.org/classifier/cgi/stratigraphicrank/sequence> rdf:type owl:NamedIndividual ,
                                                                                  owl:Thing ,
                                                                                  skos:Concept ;
                                                                         
                                                                         skos:notation "sequence"^^<http://resource.geosciml.org/classifierscheme/cgi/201202/stratigraphicrank> ;
                                                                         
                                                                         skos:definition "A genetically related succession of strata bounded by unconformites or their correlative conformable contacts, and typically having a thickness of 10-100 metres."@en ;
                                                                         
                                                                         rdfs:seeAlso "http://www.sepmstrata.org/terminology/seq-strat.html" ;
                                                                         
                                                                         skos:prefLabel "Sequence"@en ;
                                                                         
                                                                         dc:source "Van Wagoner, J.C., Posamentier, H.W., Mitchum, R.M., Vail, P.R., Sarg, J.F., Loutit, T.S., Hardenbol, J., 1988, An overview of sequence stratigraphy and key definitions. In: Wilgus, C.K., Hastings, B.S., Kendall, C.G.St.C., Posamentier, H.W., Ross, C.A., Van Wagoner, J.C. (Eds.), Sea Level Changes––An Integrated Approach, vol. 42. SEPM Special Publication, pp. 39–45."@en ;
                                                                         
                                                                         skos:exactMatch <http://resource.geosciml.org/classifier/cgi/stratigraphicrank/0009> ;
                                                                         
                                                                         skos:related <http://resource.geosciml.org/classifier/cgi/stratigraphicrank/lithodeme> ;
                                                                         
                                                                         skos:broaderTransitive <http://resource.geosciml.org/classifier/cgi/stratigraphicrank/megasequence> ;
                                                                         
                                                                         skos:broader <http://resource.geosciml.org/classifier/cgi/stratigraphicrank/supersequence> ;
                                                                         
                                                                         skos:inScheme <http://resource.geosciml.org/classifierscheme/cgi/201202/stratigraphicrank> .



###  http://resource.geosciml.org/classifier/cgi/stratigraphicrank/subgroup

<http://resource.geosciml.org/classifier/cgi/stratigraphicrank/subgroup> rdf:type owl:NamedIndividual ,
                                                                                  owl:Thing ,
                                                                                  skos:Concept ;
                                                                         
                                                                         skos:definition "A subgroup is the lithostratigraphic unit next higher in rank to formation. A subgroup usually consists of several formations." ;
                                                                         
                                                                         dc:source "Salvador, 1994"@en ;
                                                                         
                                                                         skos:prefLabel "Subgroup"@en ;
                                                                         
                                                                         skos:exactMatch <http://resource.geosciml.org/classifier/cgi/stratigraphicrank/0010> ;
                                                                         
                                                                         skos:narrower <http://resource.geosciml.org/classifier/cgi/stratigraphicrank/formation> ;
                                                                         
                                                                         skos:broader <http://resource.geosciml.org/classifier/cgi/stratigraphicrank/group> ;
                                                                         
                                                                         skos:broaderTransitive <http://resource.geosciml.org/classifier/cgi/stratigraphicrank/supergroup> ;
                                                                         
                                                                         skos:inScheme <http://resource.geosciml.org/classifierscheme/cgi/201202/stratigraphicrank> .



###  http://resource.geosciml.org/classifier/cgi/stratigraphicrank/suite

<http://resource.geosciml.org/classifier/cgi/stratigraphicrank/suite> rdf:type owl:NamedIndividual ,
                                                                               owl:Thing ,
                                                                               skos:Concept ;
                                                                      
                                                                      dc:source "North American Commission on Stratigraphic Nomenclature, 2005" ;
                                                                      
                                                                      skos:definition "A formal lithodemic unit next higher in rank to lithodeme. It comprises two or more associated lithodemes of the same class (e.g., plutonic, metamorphic)." ;
                                                                      
                                                                      skos:prefLabel "Suite"@en ;
                                                                      
                                                                      skos:exactMatch <http://resource.geosciml.org/classifier/cgi/stratigraphicrank/0011> ;
                                                                      
                                                                      skos:related <http://resource.geosciml.org/classifier/cgi/stratigraphicrank/group> ;
                                                                      
                                                                      skos:narrower <http://resource.geosciml.org/classifier/cgi/stratigraphicrank/lithodeme> ;
                                                                      
                                                                      skos:related <http://resource.geosciml.org/classifier/cgi/stratigraphicrank/supersequence> ;
                                                                      
                                                                      skos:broader <http://resource.geosciml.org/classifier/cgi/stratigraphicrank/supersuite> ;
                                                                      
                                                                      skos:inScheme <http://resource.geosciml.org/classifierscheme/cgi/201202/stratigraphicrank> .



###  http://resource.geosciml.org/classifier/cgi/stratigraphicrank/supergroup

<http://resource.geosciml.org/classifier/cgi/stratigraphicrank/supergroup> rdf:type owl:NamedIndividual ,
                                                                                    owl:Thing ,
                                                                                    skos:Concept ;
                                                                           
                                                                           dc:source "North American Commission on Stratigraphic Nomenclature, 2005; Salvador, 1994" ;
                                                                           
                                                                           skos:definition "A supergroup is a formal assemblage of related or superposed groups or of groups and formations" ;
                                                                           
                                                                           skos:prefLabel "Supergroup"@en ;
                                                                           
                                                                           skos:exactMatch <http://resource.geosciml.org/classifier/cgi/stratigraphicrank/0012> ;
                                                                           
                                                                           skos:narrowerTransitive <http://resource.geosciml.org/classifier/cgi/stratigraphicrank/formation> ;
                                                                           
                                                                           skos:narrower <http://resource.geosciml.org/classifier/cgi/stratigraphicrank/group> ;
                                                                           
                                                                           skos:narrowerTransitive <http://resource.geosciml.org/classifier/cgi/stratigraphicrank/subgroup> ;
                                                                           
                                                                           skos:related <http://resource.geosciml.org/classifier/cgi/stratigraphicrank/supersuite> ;
                                                                           
                                                                           skos:topConceptOf <http://resource.geosciml.org/classifierscheme/cgi/201202/stratigraphicrank> ;
                                                                           
                                                                           skos:inScheme <http://resource.geosciml.org/classifierscheme/cgi/201202/stratigraphicrank> .



###  http://resource.geosciml.org/classifier/cgi/stratigraphicrank/supersequence

<http://resource.geosciml.org/classifier/cgi/stratigraphicrank/supersequence> rdf:type owl:NamedIndividual ,
                                                                                       owl:Thing ,
                                                                                       skos:Concept ;
                                                                              
                                                                              dc:source "Haq, B.U., Hardenbol, J., and Vail, P.R., 1988, Mesozoic and Cenozoic chronostratigraphy an dcycles of sea-level changes, in Wilgus, C.K., et al., eds, Sea-level Changes: an Integrated Approach: Society of Sedimentary Geology Special Publication 42, p. 71-108." ;
                                                                              
                                                                              skos:definition "A succession of strata comprising two or more sequences" ;
                                                                              
                                                                              skos:prefLabel "Supersequence"@en ;
                                                                              
                                                                              rdfs:seeAlso "http://www.sepmstrata.org/terminology/seq-strat.html" ;
                                                                              
                                                                              skos:exactMatch <http://resource.geosciml.org/classifier/cgi/stratigraphicrank/0013> ;
                                                                              
                                                                              skos:broader <http://resource.geosciml.org/classifier/cgi/stratigraphicrank/megasequence> ;
                                                                              
                                                                              skos:narrower <http://resource.geosciml.org/classifier/cgi/stratigraphicrank/sequence> ;
                                                                              
                                                                              skos:related <http://resource.geosciml.org/classifier/cgi/stratigraphicrank/suite> ;
                                                                              
                                                                              skos:inScheme <http://resource.geosciml.org/classifierscheme/cgi/201202/stratigraphicrank> .



###  http://resource.geosciml.org/classifier/cgi/stratigraphicrank/supersuite

<http://resource.geosciml.org/classifier/cgi/stratigraphicrank/supersuite> rdf:type owl:NamedIndividual ,
                                                                                    owl:Thing ,
                                                                                    skos:Concept ;
                                                                           
                                                                           dc:source "North American Commission on Stratigraphic Nomenclature, 2005" ;
                                                                           
                                                                           skos:definition "A formal lithodemic unit next higher in rank to suite. It comprises two or more suites having a degree of natural relationship to one another" ;
                                                                           
                                                                           skos:prefLabel "Supersuite"@en ;
                                                                           
                                                                           skos:exactMatch <http://resource.geosciml.org/classifier/cgi/stratigraphicrank/0014> ;
                                                                           
                                                                           skos:narrowerTransitive <http://resource.geosciml.org/classifier/cgi/stratigraphicrank/lithodeme> ;
                                                                           
                                                                           skos:related <http://resource.geosciml.org/classifier/cgi/stratigraphicrank/megasequence> ;
                                                                           
                                                                           skos:narrower <http://resource.geosciml.org/classifier/cgi/stratigraphicrank/suite> ;
                                                                           
                                                                           skos:related <http://resource.geosciml.org/classifier/cgi/stratigraphicrank/supergroup> ;
                                                                           
                                                                           skos:topConceptOf <http://resource.geosciml.org/classifierscheme/cgi/201202/stratigraphicrank> ;
                                                                           
                                                                           skos:inScheme <http://resource.geosciml.org/classifierscheme/cgi/201202/stratigraphicrank> .



###  http://resource.geosciml.org/classifierscheme/cgi/201202/stratigraphicrank

<http://resource.geosciml.org/classifierscheme/cgi/201202/stratigraphicrank> rdf:type owl:NamedIndividual ,
                                                                                      owl:Thing ,
                                                                                      skos:ConceptScheme ;
                                                                             
                                                                             skos:changeNote "2009-12-07 SMR Update metadata properties for version, creator, title, and format.  Change skos:HistoryNote to dc:source for information on origin of terms and definitions."@en ;
                                                                             
                                                                             skos:historyNote "2012-02-27 SMR add skos:exactMatch triples to map URIs for concepts in this vocabulary to number-token URIs in 201012 version of same concepts."@en ;
                                                                             
                                                                             skos:prefLabel "CGI Stratigraphic Rank Term Vocabulary"@en ;
                                                                             
                                                                             skos:definition "This file contains the CGI StratigraphicRank vocabulary. This vocabulary contains categories used to classify geologic units in a generalization hierarchy from most local/smallest volume to most regional. Examples: group, subgroup, formation, member. No parent links because relation between e.g. formation and group is not 'is a' it is 'part of'. All formations are not groups, and a formation is not necessarily part of a group, therefore group is not a broader term than formation."@en ;
                                                                             
                                                                             skos:hasTopConcept <http://resource.geosciml.org/classifier/cgi/stratigraphicrank/complex> ,
                                                                                                <http://resource.geosciml.org/classifier/cgi/stratigraphicrank/megasequence> ,
                                                                                                <http://resource.geosciml.org/classifier/cgi/stratigraphicrank/rank_not_specified> ,
                                                                                                <http://resource.geosciml.org/classifier/cgi/stratigraphicrank/supergroup> ,
                                                                                                <http://resource.geosciml.org/classifier/cgi/stratigraphicrank/supersuite> .



###  http://www.w3.org/2004/02/skos/core#Collection

skos:Collection rdf:type owl:NamedIndividual ,
                         owl:Thing ;
                
                rdfs:label "Collection"@en ;
                
                rdfs:isDefinedBy "http://www.w3.org/2004/02/skos/core"^^xsd:anyURI ;
                
                skos:definition "A meaningful collection of concepts."@en ;
                
                rdfs:comment """Labelled collections can be used with collectable semantic relation
      properties e.g. skos:narrower, where you would like a set of concepts to be displayed under a
      'node label' in the hierarchy."""@en .



###  http://www.w3.org/2004/02/skos/core#Concept

skos:Concept rdf:type owl:NamedIndividual ,
                      owl:Thing ;
             
             rdfs:label "Concept"@en ;
             
             rdfs:isDefinedBy "http://www.w3.org/2004/02/skos/core"^^xsd:anyURI ;
             
             skos:definition "An abstract idea or notion; a unit of thought."@en .



###  http://www.w3.org/2004/02/skos/core#ConceptScheme

skos:ConceptScheme rdf:type owl:NamedIndividual ,
                            owl:Thing ;
                   
                   rdfs:label "Concept Scheme"@en ;
                   
                   rdfs:isDefinedBy "http://www.w3.org/2004/02/skos/core"^^xsd:anyURI ;
                   
                   rdfs:comment """A concept scheme may be defined to include concepts from different
      sources."""@en ;
                   
                   skos:definition """A set of concepts, optionally including statements about semantic
      relationships between those concepts."""@en ,
                                   "A set of concepts, optionally including statements about semanticn      relationships between those concepts."@en ;
                   
                   rdfs:comment """Thesauri, classification schemes, subject heading lists, taxonomies,
      'folksonomies', and other types of controlled vocabulary are all examples of concept schemes.
      Concept schemes are also embedded in glossaries and terminologies."""@en .



###  http://www.w3.org/2004/02/skos/core#OrderedCollection

skos:OrderedCollection rdf:type owl:NamedIndividual ,
                                owl:Thing ;
                       
                       rdfs:label "Ordered Collection"@en ;
                       
                       rdfs:isDefinedBy "http://www.w3.org/2004/02/skos/core"^^xsd:anyURI ;
                       
                       skos:definition """An ordered collection of concepts, where both the grouping and
      the ordering are meaningful."""@en ,
                                       "An ordered collection of concepts, where both the grouping andn      the ordering are meaningful."@en ;
                       
                       rdfs:comment "Ordered collections can be used where you would like a set of concepts to be displayed in a specific order, and optionally under a 'node label'."@en .



###  http://www.w3.org/2004/02/skos/core#altLabel

skos:altLabel rdf:type owl:NamedIndividual ,
                       owl:Thing ;
              
              skos:definition "An alternative lexical label for a resource."@en .



###  http://www.w3.org/2004/02/skos/core#broadMatch

skos:broadMatch rdf:type owl:NamedIndividual ,
                         owl:Thing ;
                
                rdfs:label "broader match"@en ;
                
                rdfs:isDefinedBy "http://www.w3.org/2004/02/skos/core"^^xsd:anyURI ;
                
                skos:definition """skos:broadMatch is used to state a hierarchical mapping link
      between two conceptual resources in different concept schemes."""@en ,
                                "skos:broadMatch is used to state a hierarchical mapping linkn      between two conceptual resources in different concept schemes."@en .



###  http://www.w3.org/2004/02/skos/core#broader

skos:broader rdf:type owl:NamedIndividual ,
                      owl:Thing ;
             
             rdfs:label "has broader"@en ;
             
             rdfs:isDefinedBy "http://www.w3.org/2004/02/skos/core"^^xsd:anyURI ;
             
             skos:definition "A concept that is more general in meaning."@en ;
             
             rdfs:comment """Broader concepts are typically rendered as parents in a concept
      hierarchy (tree)."""@en ,
                          """By convention, skos:broader is only used to assert an immediate
      (i.e. direct) hierarchical link between two conceptual resources."""@en .



###  http://www.w3.org/2004/02/skos/core#broaderTransitive

skos:broaderTransitive rdf:type owl:NamedIndividual ,
                                owl:Thing ;
                       
                       rdfs:label "broader transitive"@en ;
                       
                       rdfs:isDefinedBy "http://www.w3.org/2004/02/skos/core"^^xsd:anyURI ;
                       
                       rdfs:comment """By convention, skos:broaderTransitive is not used to make
      assertions. Rather, the properties can be used to draw inferences about the transitive closure
      of the hierarchical relation, which is useful e.g. when implementing a simple query expansion
      algorithm in a search application."""@en ;
                       
                       skos:definition "skos:broaderTransitive is a transitive superproperty of skos:broader." .



###  http://www.w3.org/2004/02/skos/core#changeNote

skos:changeNote rdf:type owl:NamedIndividual ,
                         owl:Thing ;
                
                skos:definition "A note about a modification to a concept."@en .



###  http://www.w3.org/2004/02/skos/core#closeMatch

skos:closeMatch rdf:type owl:NamedIndividual ,
                         owl:Thing ;
                
                rdfs:label "close match"@en ;
                
                rdfs:isDefinedBy "http://www.w3.org/2004/02/skos/core"^^xsd:anyURI ;
                
                skos:definition """skos:closeMatch is used to link two concepts that are
      sufficiently similar that they can be used interchangeably in some information retrieval
      applications. In order to avoid the possibility of \"compound errors\" when combining mappings
      across more than two concept schemes, skos:closeMatch is not declared to be a transitive
      property."""@en.


###  http://www.w3.org/2004/02/skos/core#definition

skos:definition rdf:type owl:NamedIndividual ,
                         owl:Thing ;
                
                rdfs:label "definition"@en ;
                
                rdfs:isDefinedBy "http://www.w3.org/2004/02/skos/core"^^xsd:anyURI ;
                
                skos:definition "A statement or formal explanation of the meaning of a concept."@en .



###  http://www.w3.org/2004/02/skos/core#editorialNote

skos:editorialNote rdf:type owl:NamedIndividual ,
                            owl:Thing ;
                   
                   skos:definition "A note for an editor, translator or maintainer of the vocabulary."@en .



###  http://www.w3.org/2004/02/skos/core#exactMatch

skos:exactMatch rdf:type owl:NamedIndividual ,
                         owl:Thing ;
                
                rdfs:label "exact match"@en ;
                
                rdfs:isDefinedBy "http://www.w3.org/2004/02/skos/core"^^xsd:anyURI ;
                
                rdfs:comment """skos:exactMatch is disjoint with each of the properties
      skos:broadMatch and skos:relatedMatch."""@en ;
                
                skos:definition """skos:exactMatch is used to link two concepts, indicating a high
      degree of confidence that the concepts can be used interchangeably across a wide range of
      information retrieval applications. skos:exactMatch is a transitive property, and is a
      sub-property of skos:closeMatch."""@en .



###  http://www.w3.org/2004/02/skos/core#example

skos:example rdf:type owl:NamedIndividual ,
                      owl:Thing ;
             
             skos:definition "An example of the use of a concept."@en .



###  http://www.w3.org/2004/02/skos/core#hasTopConcept

skos:hasTopConcept rdf:type owl:NamedIndividual ,
                            owl:Thing ;
                   
                   rdfs:label "has top concept"@en ;
                   
                   rdfs:isDefinedBy "http://www.w3.org/2004/02/skos/core"^^xsd:anyURI ;
                   
                   skos:definition "A top level concept in the concept scheme."@en .



###  http://www.w3.org/2004/02/skos/core#hiddenLabel

skos:hiddenLabel rdf:type owl:NamedIndividual ,
                          owl:Thing ;
                 
                 skos:definition """A lexical label for a resource that should be hidden when
      generating visual displays of the resource, but should still be accessible to free text search
      operations."""@en .



###  http://www.w3.org/2004/02/skos/core#historyNote

skos:historyNote rdf:type owl:NamedIndividual ,
                          owl:Thing ;
                 
                 skos:definition "A note about the past state/use/meaning of a concept."@en .



###  http://www.w3.org/2004/02/skos/core#inScheme

skos:inScheme rdf:type owl:NamedIndividual ,
                       owl:Thing ;
              
              rdfs:label "in scheme"@en ;
              
              rdfs:isDefinedBy "http://www.w3.org/2004/02/skos/core"^^xsd:anyURI ;
              
              rdfs:comment "A concept may be a member of more than one concept scheme."@en ;
              
              skos:definition "A concept scheme in which the concept is included."@en .



###  http://www.w3.org/2004/02/skos/core#mappingRelation

skos:mappingRelation rdf:type owl:NamedIndividual ,
                              owl:Thing ;
                     
                     rdfs:label "mapping relation"@en ;
                     
                     rdfs:isDefinedBy "http://www.w3.org/2004/02/skos/core"^^xsd:anyURI ;
                     
                     skos:definition "Definition"@en ;
                     
                     rdfs:comment """These concept mapping relations mirror semantic relations, and the
      data model defined below is similar (with the exception of skos:exactMatch) to the data model
      defined for semantic relations. A distinct vocabulary is provided for concept mapping
      relations, to provide a convenient way to differentiate links within a concept scheme from
      links between concept schemes. However, this pattern of usage is not a formal requirement of
      the SKOS data model, and relies on informal definitions of best practice."""@en .



###  http://www.w3.org/2004/02/skos/core#member

skos:member rdf:type owl:NamedIndividual ,
                     owl:Thing ;
            
            rdfs:label "member"@en ;
            
            rdfs:isDefinedBy "http://www.w3.org/2004/02/skos/core"^^xsd:anyURI ;
            
            skos:definition "A member of a collection."@en .



###  http://www.w3.org/2004/02/skos/core#memberList

skos:memberList rdf:type owl:NamedIndividual ,
                         owl:Thing ;
                
                rdfs:label "member list"@en ;
                
                rdfs:isDefinedBy "http://www.w3.org/2004/02/skos/core"^^xsd:anyURI ;
                
                skos:definition "An RDF list containing the members of an ordered collection."@en ;
                
                rdfs:comment """For any resource, every item in the list given as the value of the
      skos:memberList property is also a value of the skos:member property."""@en .



###  http://www.w3.org/2004/02/skos/core#narrowMatch

skos:narrowMatch rdf:type owl:NamedIndividual ,
                          owl:Thing ;
                 
                 rdfs:label "narrower match"@en ;
                 
                 rdfs:isDefinedBy "http://www.w3.org/2004/02/skos/core"^^xsd:anyURI ;
                 
                 skos:definition """skos:narrowMatch is used to state a hierarchical mapping link
      between two conceptual resources in different concept schemes."""@en .


###  http://www.w3.org/2004/02/skos/core#narrower

skos:narrower rdf:type owl:NamedIndividual ,
                       owl:Thing ;
              
              rdfs:label "has narrower"@en ;
              
              rdfs:isDefinedBy "http://www.w3.org/2004/02/skos/core"^^xsd:anyURI ;
              
              skos:definition "A concept that is more specific in meaning."@en ;
              
              rdfs:comment """By convention, skos:broader is only used to assert an immediate
      (i.e. direct) hierarchical link between two conceptual resources."""@en ,
                           """Narrower concepts are typically rendered as children in a concept
      hierarchy (tree)."""@en .



###  http://www.w3.org/2004/02/skos/core#narrowerTransitive

skos:narrowerTransitive rdf:type owl:NamedIndividual ,
                                 owl:Thing ;
                        
                        rdfs:label "narrower transitive"@en ;
                        
                        rdfs:isDefinedBy "http://www.w3.org/2004/02/skos/core"^^xsd:anyURI ;
                        
                        rdfs:comment """By convention, skos:narrowerTransitive is not used to make
      assertions. Rather, the properties can be used to draw inferences about the transitive closure
      of the hierarchical relation, which is useful e.g. when implementing a simple query expansion
      algorithm in a search application."""@en ;
                        
                        skos:definition """skos:narrowerTransitive is a transitive superproperty of skos:broader. By
      convention, skos:narrowerTransitive is not intended to be used in assertions, but provides a
      mechanism whereby the transitive closure of skos:narrower can be queried."""@en .



###  http://www.w3.org/2004/02/skos/core#notation

skos:notation rdf:type owl:NamedIndividual ,
                       owl:Thing ;
              
              rdfs:label "notation"@en ;
              
              rdfs:isDefinedBy "http://www.w3.org/2004/02/skos/core"^^xsd:anyURI ;
              
              skos:definition """A notation, also known as classification code, is a string of
      characters such as \"T58.5\" or \"303.4833\" used to uniquely identify a concept within the scope
      of a given concept scheme."""@en ;
              rdfs:comment """By convention, skos:notation is used with a typed literal in the
      object position of the triple."""@en .



###  http://www.w3.org/2004/02/skos/core#note

skos:note rdf:type owl:NamedIndividual ,
                   owl:Thing ;
          
          skos:definition "A general note, for any purpose."@en .



###  http://www.w3.org/2004/02/skos/core#prefLabel

skos:prefLabel rdf:type owl:NamedIndividual ,
                        owl:Thing ;
               
               skos:definition "The preferred lexical label for a resource, in a given language."@en .



###  http://www.w3.org/2004/02/skos/core#related

skos:related rdf:type owl:NamedIndividual ,
                      owl:Thing ;
             
             rdfs:label "related to"@en ;
             
             rdfs:isDefinedBy "http://www.w3.org/2004/02/skos/core"^^xsd:anyURI ;
             
             skos:definition """A concept with which there is an associative semantic
      relationship."""@en ;
             
             rdfs:comment "skos:related is disjoint with skos:broaderTransitive"@en .



###  http://www.w3.org/2004/02/skos/core#relatedMatch

skos:relatedMatch rdf:type owl:NamedIndividual ,
                           owl:Thing ;
                  
                  rdfs:label "related match"@en ;
                  
                  rdfs:isDefinedBy "http://www.w3.org/2004/02/skos/core"^^xsd:anyURI ;
                  
                  skos:definition """skos:relatedMatch is used to state an associative mapping link
      between two conceptual resources in different concept schemes."""@en ,
                                  "skos:relatedMatch is used to state an associative mapping linkn      between two conceptual resources in different concept schemes."@en .



###  http://www.w3.org/2004/02/skos/core#scopeNote

skos:scopeNote rdf:type owl:NamedIndividual ,
                        owl:Thing ;
               
               skos:definition "A note that helps to clarify the meaning of a concept."@en .



###  http://www.w3.org/2004/02/skos/core#semanticRelation

skos:semanticRelation rdf:type owl:NamedIndividual ,
                               owl:Thing ;
                      
                      rdfs:label "semantic relation"@en ;
                      
                      rdfs:isDefinedBy "http://www.w3.org/2004/02/skos/core"^^xsd:anyURI ;
                      
                      skos:definition "A concept related by meaning."@en ;
                      
                      rdfs:comment """This property should not be used directly, but as a super-property
      for all properties denoting a relationship of meaning between concepts."""@en .



###  http://www.w3.org/2004/02/skos/core#topConceptOf

skos:topConceptOf rdf:type owl:NamedIndividual ,
                           owl:Thing ;
                  
                  rdfs:label "top concept in scheme"@en ;
                  
                  rdfs:isDefinedBy "http://www.w3.org/2004/02/skos/core"^^xsd:anyURI ;
                  
                  skos:definition "Relates a concept to the concept scheme in which it is a top level concept."@en .




###  Generated by the OWL API (version 3.2.3.1824) http://owlapi.sourceforge.net

